# baseURI: http://pi.pauwel.be/voc/distributionelement
# prefix: mep

@prefix : <http://pi.pauwel.be/voc/distributionelement#> .
@prefix cc: <http://creativecommons.org/ns#> .
@prefix contax: <https://w3id.org/con-tax#> .
@prefix dbr: <http://dbpedia.org/resource/> .
@prefix dcterms: <http://purl.org/dc/terms/> .
@prefix foaf: <http://xmlns.com/foaf/0.1/> .
@prefix furn: <http://pi.pauwel.be/voc/furniture#> .
@prefix gr: <http://purl.org/goodrelations/v1#> .
@prefix ifc: <https://standards.buildingsmart.org/IFC/DEV/IFC4/ADD2/OWL#> .
@prefix mep: <http://pi.pauwel.be/voc/distributionelement#> .
@prefix owl: <http://www.w3.org/2002/07/owl#> .
@prefix rdf: <http://www.w3.org/1999/02/22-rdf-syntax-ns#> .
@prefix rdfs: <http://www.w3.org/2000/01/rdf-schema#> .
@prefix schema: <https://schema.org/> .
@prefix vann: <http://purl.org/vocab/vann/> .
@prefix vcard: <http://www.w3.org/2006/vcard/ns#> .
@prefix voaf: <http://purl.org/vocommons/voaf#> .
@prefix vs: <http://www.w3.org/2003/06/sw-vocab-status/ns#> .
@prefix xml: <http://www.w3.org/XML/1998/namespace> .
@prefix xsd: <http://www.w3.org/2001/XMLSchema#> .

<http://pi.pauwel.be/voc/distributionelement>
  rdf:type voaf:Vocabulary ;
  rdf:type owl:Ontology ;
  cc:license <https://creativecommons.org/licenses/by/1.0/> ;
  dcterms:contributor [
      rdf:type vcard:Individual ;
      vcard:family-name "Bonduel" ;
      vcard:fn "Mathias Bonduel" ;
      vcard:given-name "Mathias" ;
      vcard:hasOrganizationName [
          rdf:type vcard:Organization ;
          owl:sameAs dbr:Katholieke_Universiteit_Leuven ;
          vcard:hasURL <https://www.kuleuven.be> ;
          vcard:organization-name "KU Leuven" ;
        ] ;
      vcard:hasURL <https://orcid.org/0000-0002-3313-924X> ;
      vcard:hasURL <https://www.kuleuven.be/wieiswie/nl/person/00110827> ;
      vcard:hasURL <https://www.researchgate.net/profile/Mathias_Bonduel> ;
    ] ;
  dcterms:creator [
      rdf:type foaf:Person ;
      foaf:name "Pieter Pauwels" ;
    ] ;
  dcterms:description "The Distribution Element Ontology (MEP) provides an ontology based on the IfcDistributionElement subtree in the IFC specification, containing a taxonomy of classes that allow to define common distribution elements (actuators, flowterminals, ...)."@en ;
  dcterms:issued "2019-01-28"^^xsd:date ;
  dcterms:modified "2020-07-29"^^xsd:date ;
  dcterms:title "MEP: Distribution Element Ontology"@en ;
  vann:preferredNamespacePrefix "mep" ;
  vann:preferredNamespaceUri "http://pi.pauwel.be/voc/distributionelement#" ;
  rdfs:comment """
- Version 0.3.0: changed ccc:ConstructionComponent into contax:ConstructionComponent. Added rdfs:isDefinedBy
- Version 0.2.0: changed all subclasses of schema:Product and gr:SomeItems into a subclass of ccc:ConstructionComponent
- Version 0.1.1: small changes and corrections (completed onto metadata; changed labels containing a bSDD URL to URIs connected via rdfs:seeAlso; updated ifcOWL URI; replace erroneous language tags (remove @ifc-2x4); added missing language tags to strings; )
- Version 0.1.0: initial version"""@en ;
  owl:versionInfo "0.3.0" ;
.
mep:Actuator
  rdf:type owl:Class ;
  rdfs:comment "A mechanical device for moving or controlling a mechanism or system. An actuator takes energy, usually created by air, electricity, or liquid, and converts that into some kind of motion."@en ;
  rdfs:comment "An artefact intended to convert energy (electric, pneumatic, hydraulic) from an external source to kinetic energy in response to a signal..                "@en ;
  rdfs:isDefinedBy <http://pi.pauwel.be/voc/distributionelement> ;
  rdfs:label "Actuator"@en ;
  rdfs:label "actionneur"@fr-fr ;
  rdfs:label "aktor"@de-de ;
  rdfs:label "aktuator"@nb-no ;
  rdfs:label "antrieb"@de-de ;
  rdfs:label "appareillage de commande"@fr-fr ;
  rdfs:label "utløser"@nb-no ;
  rdfs:seeAlso <http://bsdd.buildingsmart.org/#concept/details/14RHCzJ6j6MOcOYy1uRfnX> ;
  rdfs:seeAlso ifc:IfcActuator ;
  rdfs:subClassOf mep:DistributionControlElement ;
.
mep:Actuator-ELECTRICACTUATOR
  rdf:type owl:Class ;
  rdfs:comment "a device that electrically actuates a control element"@en ;
  rdfs:isDefinedBy <http://pi.pauwel.be/voc/distributionelement> ;
  rdfs:label "Electric Actuator"@en ;
  rdfs:label "elektrisk aktuator"@nb-no ;
  rdfs:seeAlso <http://bsdd.buildingsmart.org/#concept/details/0_R289D0r6oPsUChqMMWr1> ;
  rdfs:seeAlso ifc:IfcActuatorEnumType ;
  rdfs:subClassOf mep:Actuator ;
.
mep:Actuator-HANDOPERATEDACTUATOR
  rdf:type owl:Class ;
  rdfs:isDefinedBy <http://pi.pauwel.be/voc/distributionelement> ;
  rdfs:label "Hand-Operated Actuator"@en ;
  rdfs:seeAlso <http://bsdd.buildingsmart.org/#concept/details/0FuSpPYcbBcAKNNq77IEUN> ;
  rdfs:seeAlso ifc:IfcActuatorEnumType ;
  rdfs:subClassOf mep:Actuator ;
.
mep:Actuator-HYDRAULICACTUATOR
  rdf:type owl:Class ;
  rdfs:isDefinedBy <http://pi.pauwel.be/voc/distributionelement> ;
  rdfs:label "Hydraulic Actuator"@en ;
  rdfs:seeAlso <http://bsdd.buildingsmart.org/#concept/details/23inrfSJTEjPmdb42m6RPS> ;
  rdfs:seeAlso ifc:IfcActuatorEnumType ;
  rdfs:subClassOf mep:Actuator ;
.
mep:Actuator-PNEUMATICACTUATOR
  rdf:type owl:Class ;
  rdfs:isDefinedBy <http://pi.pauwel.be/voc/distributionelement> ;
  rdfs:label "Pneumatic Actuator"@en ;
  rdfs:seeAlso <http://bsdd.buildingsmart.org/#concept/details/1An85fZE5EZuDCIYomL2WH> ;
  rdfs:seeAlso ifc:IfcActuatorEnumType ;
  rdfs:subClassOf mep:Actuator ;
.
mep:Actuator-THERMOSTATICACTUATOR
  rdf:type owl:Class ;
  rdfs:isDefinedBy <http://pi.pauwel.be/voc/distributionelement> ;
  rdfs:label "Thermostatic Actuator"@en ;
  rdfs:seeAlso <http://bsdd.buildingsmart.org/#concept/details/3dkx9QS9HB_emzU3ErhfqY> ;
  rdfs:seeAlso ifc:IfcActuatorEnumType ;
  rdfs:subClassOf mep:Actuator ;
.
mep:AirTerminal
  rdf:type owl:Class ;
  rdfs:comment "A terminal terminating or origination point for the transfer of air between distribution system(s) and one or more spaces. It can also be used for the transfer of air between adjacent spaces."@en ;
  rdfs:isDefinedBy <http://pi.pauwel.be/voc/distributionelement> ;
  rdfs:label "Air Terminal"@en ;
  rdfs:label "Luftauslass"@de-de ;
  rdfs:label "entrée ou sortie d'air"@fr-fr ;
  rdfs:label "ventilasjonsterminal"@nb-no ;
  rdfs:seeAlso <http://bsdd.buildingsmart.org/#concept/details/3ydOg0qRuHuO00025QrE$V> ;
  rdfs:seeAlso ifc:IfcAirTerminal ;
  rdfs:subClassOf mep:FlowTerminal ;
.
mep:AirTerminal-DIFFUSER
  rdf:type owl:Class ;
  rdfs:isDefinedBy <http://pi.pauwel.be/voc/distributionelement> ;
  rdfs:label "Diffuser"@en ;
  rdfs:label "luftterminal - diffusor"@nb-no ;
  rdfs:seeAlso <http://bsdd.buildingsmart.org/#concept/details/1FTT5hVkDA$QvjrFJNJEnI> ;
  rdfs:seeAlso ifc:IfcAirTerminalEnumType ;
  rdfs:subClassOf mep:AirTerminal ;
.
mep:AirTerminal-GRILLE
  rdf:type owl:Class ;
  rdfs:comment "a covering for any area through which air passes."@en ;
  rdfs:isDefinedBy <http://pi.pauwel.be/voc/distributionelement> ;
  rdfs:label "Grille"@en ;
  rdfs:label "gitter"@nb-no ;
  rdfs:label "grille"@fr-fr ;
  rdfs:seeAlso <http://bsdd.buildingsmart.org/#concept/details/2hjaxvDcLE49ehxXYke964> ;
  rdfs:seeAlso ifc:IfcAirTerminalEnumType ;
  rdfs:subClassOf mep:AirTerminal ;
.
mep:AirTerminal-LOUVRE
  rdf:type owl:Class ;
  rdfs:comment "a rectilinear louvre."@en ;
  rdfs:isDefinedBy <http://pi.pauwel.be/voc/distributionelement> ;
  rdfs:label "Louvre"@en ;
  rdfs:label "rist"@nb-no ;
  rdfs:seeAlso <http://bsdd.buildingsmart.org/#concept/details/0cCEo7qnfDSgG93nJsd3eQ> ;
  rdfs:seeAlso ifc:IfcAirTerminalEnumType ;
  rdfs:subClassOf mep:AirTerminal ;
.
mep:AirTerminal-REGISTER
  rdf:type owl:Class ;
  rdfs:comment "a grille typically equipped with a damper or control valve."@en ;
  rdfs:isDefinedBy <http://pi.pauwel.be/voc/distributionelement> ;
  rdfs:label "Register"@en ;
  rdfs:label "register"@nb-no ;
  rdfs:seeAlso <http://bsdd.buildingsmart.org/#concept/details/3PWMnCjqP5peD0PtO2aiy5> ;
  rdfs:seeAlso ifc:IfcAirTerminalEnumType ;
  rdfs:subClassOf mep:AirTerminal ;
.
mep:AirTerminalBox
  rdf:type owl:Class ;
  rdfs:comment "A terminal box in an HVAC duct distribution system and is used to control or modulate the amount of air delivered to its downstream ductwork. Often referred to as an 'air flow regulator'."@en ;
  rdfs:isDefinedBy <http://pi.pauwel.be/voc/distributionelement> ;
  rdfs:label "Air Terminal Box"@en ;
  rdfs:label "Diffuseur d'air"@fr-fr ;
  rdfs:label "Volumenstromregler"@de-de ;
  rdfs:label "plenumskammer"@nb-no ;
  rdfs:seeAlso <http://bsdd.buildingsmart.org/#concept/details/0zPqWPJST5LRtUuSJBlWpM> ;
  rdfs:seeAlso ifc:IfcAirTerminalBox ;
  rdfs:subClassOf mep:FlowController ;
.
mep:AirTerminalBox-CONSTANTFLOW
  rdf:type owl:Class ;
  rdfs:isDefinedBy <http://pi.pauwel.be/voc/distributionelement> ;
  rdfs:label "Constant Flow Air Terminal Box"@en ;
  rdfs:seeAlso <http://bsdd.buildingsmart.org/#concept/details/0dsGGCiP10ouwdibwvCd4F> ;
  rdfs:seeAlso ifc:IfcAirTerminalBoxEnumType ;
  rdfs:subClassOf mep:AirTerminalBox ;
.
mep:AirTerminalBox-VARIABLEFLOWPRESSUREDEPENDANT
  rdf:type owl:Class ;
  rdfs:isDefinedBy <http://pi.pauwel.be/voc/distributionelement> ;
  rdfs:label "Variable Flow Pressure Dependent Air Terminal Box"@en ;
  rdfs:seeAlso <http://bsdd.buildingsmart.org/#concept/details/2EJZMcPDLDIvG04WI9UZaC> ;
  rdfs:seeAlso ifc:IfcAirTerminalBoxEnumType ;
  rdfs:subClassOf mep:AirTerminalBox ;
.
mep:AirTerminalBox-VARIABLEFLOWPRESSUREINDEPENDANT
  rdf:type owl:Class ;
  rdfs:isDefinedBy <http://pi.pauwel.be/voc/distributionelement> ;
  rdfs:label "Variable Flow Pressure Independent Air Terminal Box"@en ;
  rdfs:seeAlso <http://bsdd.buildingsmart.org/#concept/details/2zgc7TxXP2igAw6tyDqxcB> ;
  rdfs:seeAlso ifc:IfcAirTerminalBoxEnumType ;
  rdfs:subClassOf mep:AirTerminalBox ;
.
mep:AirToAirHeatRecovery
  rdf:type owl:Class ;
  rdfs:comment "A counter-flow heat exchanger between inbound and outbound air flow. Typically used to transfer heat from warmer air in one chamber to cooler air in the second chamber (i.e., typically used to recover heat from the conditioned air being exhausted and the outside air being supplied to a building), resulting in energy savings from reduced heating (or cooling) requirements."@en ;
  rdfs:isDefinedBy <http://pi.pauwel.be/voc/distributionelement> ;
  rdfs:label "Air-to-Air Heat Recovery"@en ;
  rdfs:label "Echangeur air-air"@fr-fr ;
  rdfs:label "Wärmerückgewinner"@de-de ;
  rdfs:label "luft/luft-varmegjenvinningsanlegg"@nb-no ;
  rdfs:seeAlso <http://bsdd.buildingsmart.org/#concept/details/2NT_DsArH7_Q5msK_YfU$N> ;
  rdfs:seeAlso ifc:IfcAirToAirHeatRecovery ;
  rdfs:subClassOf mep:EnergyConversionDevice ;
.
mep:AirToAirHeatRecovery-FIXEDPLATECOUNTERFLOWEXCHANGER
  rdf:type owl:Class ;
  rdfs:comment "heat exchanger with moving parts and alternate layers of plates, separated and sealed from the exhaust and supply air stream passages with primary air entering at secondary air outlet location and exiting at secondary air inlet location"@en ;
  rdfs:comment "heat exchanger with moving parts and alternate layers of plates, separated and sealed from the exhaust and supply air stream passages with primary air entering at secondary air outlet location and exiting at secondary air inlet location"@en-gb ;
  rdfs:isDefinedBy <http://pi.pauwel.be/voc/distributionelement> ;
  rdfs:label "Fixed-Plate Counter-Flow Exchanger"@en ;
  rdfs:label "fast plate motstrømsveksler"@nb-no ;
  rdfs:seeAlso <http://bsdd.buildingsmart.org/#concept/details/32kk64JBbDDPM$6p$uBj_5> ;
  rdfs:seeAlso ifc:IfcAirToAirHeatRecoveryEnumType ;
  rdfs:subClassOf mep:AirToAirHeatRecovery ;
.
mep:AirToAirHeatRecovery-FIXEDPLATECROSSFLOWEXCHANGER
  rdf:type owl:Class ;
  rdfs:comment "not available"@en ;
  rdfs:isDefinedBy <http://pi.pauwel.be/voc/distributionelement> ;
  rdfs:label "Fixed-Plate Cross-Flow Exchanger"@en ;
  rdfs:seeAlso <http://bsdd.buildingsmart.org/#concept/details/2LTpG80kz5Oh41Z0r9nlld> ;
  rdfs:seeAlso ifc:IfcAirToAirHeatRecoveryEnumType ;
  rdfs:subClassOf mep:AirToAirHeatRecovery ;
.
mep:AirToAirHeatRecovery-FIXEDPLATEPARALLELFLOWEXCHANGER
  rdf:type owl:Class ;
  rdfs:isDefinedBy <http://pi.pauwel.be/voc/distributionelement> ;
  rdfs:label "Fixed-Plate Parallel-Flow Exchanger"@en ;
  rdfs:seeAlso <http://bsdd.buildingsmart.org/#concept/details/2miQYyrOfDkQ3LRDmm98s2> ;
  rdfs:seeAlso ifc:IfcAirToAirHeatRecoveryEnumType ;
  rdfs:subClassOf mep:AirToAirHeatRecovery ;
.
mep:AirToAirHeatRecovery-HEATPIPE
  rdf:type owl:Class ;
  rdfs:comment "a passive energy recovery device with a heat pipe divided into evaporator and condenser sections"@en ;
  rdfs:comment "a passive energy recovery device with a heat pipe divided into evaporator and condenser sections"@en-gb ;
  rdfs:isDefinedBy <http://pi.pauwel.be/voc/distributionelement> ;
  rdfs:label "Heat Pipe"@en ;
  rdfs:label "varmerør"@nb-no ;
  rdfs:seeAlso <http://bsdd.buildingsmart.org/#concept/details/3g4XqNsbDCXxINl9l4yi1C> ;
  rdfs:seeAlso ifc:IfcAirToAirHeatRecoveryEnumType ;
  rdfs:subClassOf mep:AirToAirHeatRecovery ;
.
mep:AirToAirHeatRecovery-ROTARYWHEEL
  rdf:type owl:Class ;
  rdfs:comment "a heat wheel with a revolving cylinder filled with an air-permeable medium having a large internal surface area"@en ;
  rdfs:comment "a heat wheel with a revolving cylinder filled with an air-permeable medium having a large internal surface area"@en-gb ;
  rdfs:isDefinedBy <http://pi.pauwel.be/voc/distributionelement> ;
  rdfs:label "Rotary Wheel"@en ;
  rdfs:label "dreiehjul"@nb-no ;
  rdfs:seeAlso <http://bsdd.buildingsmart.org/#concept/details/1jrV4bYDD3JfDdNo49vivZ> ;
  rdfs:seeAlso ifc:IfcAirToAirHeatRecoveryEnumType ;
  rdfs:subClassOf mep:AirToAirHeatRecovery ;
.
mep:AirToAirHeatRecovery-RUNAROUNDCOILLOOP
  rdf:type owl:Class ;
  rdfs:isDefinedBy <http://pi.pauwel.be/voc/distributionelement> ;
  rdfs:label "Run-Around Coil Loop"@en ;
  rdfs:seeAlso <http://bsdd.buildingsmart.org/#concept/details/2cqFu4yIn4g8zaq7Ari71H> ;
  rdfs:seeAlso ifc:IfcAirToAirHeatRecoveryEnumType ;
  rdfs:subClassOf mep:AirToAirHeatRecovery ;
.
mep:AirToAirHeatRecovery-THERMOSIPHONCOILTYPEHEATEXCHANGERS
  rdf:type owl:Class ;
  rdfs:isDefinedBy <http://pi.pauwel.be/voc/distributionelement> ;
  rdfs:label "Thermosiphon Coil-Type Heat Exchangers"@en ;
  rdfs:seeAlso <http://bsdd.buildingsmart.org/#concept/details/1tRIVmPDzFEwR3BpMALcZq> ;
  rdfs:seeAlso ifc:IfcAirToAirHeatRecoveryEnumType ;
  rdfs:subClassOf mep:AirToAirHeatRecovery ;
.
mep:AirToAirHeatRecovery-THERMOSIPHONSEALEDTUBEHEATEXCHANGERS
  rdf:type owl:Class ;
  rdfs:isDefinedBy <http://pi.pauwel.be/voc/distributionelement> ;
  rdfs:label "Thermosiphon Sealed-Tube Heat Exchanger"@en ;
  rdfs:seeAlso <http://bsdd.buildingsmart.org/#concept/details/3sRN7JNafC$OyVXS$9WPxV> ;
  rdfs:seeAlso ifc:IfcAirToAirHeatRecoveryEnumType ;
  rdfs:subClassOf mep:AirToAirHeatRecovery ;
.
mep:AirToAirHeatRecovery-TWINTOWERENTHALPYRECOVERYLOOPS
  rdf:type owl:Class ;
  rdfs:isDefinedBy <http://pi.pauwel.be/voc/distributionelement> ;
  rdfs:label "Twin Tower Enthalpy Recovery Loop"@en ;
  rdfs:seeAlso <http://bsdd.buildingsmart.org/#concept/details/0LF0EN7b17KRgoO5lIZDTY> ;
  rdfs:seeAlso ifc:IfcAirToAirHeatRecoveryEnumType ;
  rdfs:subClassOf mep:AirToAirHeatRecovery ;
.
mep:Alarm
  rdf:type owl:Class ;
  rdfs:comment "device, which may be connected into a transmission path of a fire detection and fire alarm system, to limit the consequences of low parallel resistance faults between the lines of this transmission path"@en ;
  rdfs:isDefinedBy <http://pi.pauwel.be/voc/distributionelement> ;
  rdfs:label "Alarm"@en ;
  rdfs:label "brannalarm - kortslutningsisolator"@nb-no ;
  rdfs:seeAlso <http://bsdd.buildingsmart.org/#concept/details/1lb9XO$N58HxZ1Bunuwfkb> ;
  rdfs:seeAlso ifc:IfcAlarm ;
  rdfs:subClassOf mep:DistributionControlElement ;
.
mep:Alarm-BELL
  rdf:type owl:Class ;
  rdfs:comment "an audible alarm"@en ;
  rdfs:isDefinedBy <http://pi.pauwel.be/voc/distributionelement> ;
  rdfs:label "Bell"@en ;
  rdfs:label "bjelle"@nb-no ;
  rdfs:seeAlso <http://bsdd.buildingsmart.org/#concept/details/2iAce1_ub4pRT_gbGydGqi> ;
  rdfs:seeAlso ifc:IfcAlarmEnumType ;
  rdfs:subClassOf mep:Alarm ;
.
mep:Alarm-BREAKGLASSBUTTON
  rdf:type owl:Class ;
  rdfs:comment "an alarm activation mechanism in which a protective glass has to be broken to enable a button to be pressed"@en ;
  rdfs:comment "an alarm activation mechanism in which a protective glass has to be broken to enable a button to be pressed"@en-gb ;
  rdfs:isDefinedBy <http://pi.pauwel.be/voc/distributionelement> ;
  rdfs:label "Break Glass Button"@en ;
  rdfs:label "brannvarslingsknapp"@nb-no ;
  rdfs:seeAlso <http://bsdd.buildingsmart.org/#concept/details/1PccK35QXEef9_Kn79zIxl> ;
  rdfs:seeAlso ifc:IfcAlarmEnumType ;
  rdfs:subClassOf mep:Alarm ;
.
mep:Alarm-LIGHT
  rdf:type owl:Class ;
  rdfs:comment "a visual alarm"@en ;
  rdfs:isDefinedBy <http://pi.pauwel.be/voc/distributionelement> ;
  rdfs:label "Licht"@de-de ;
  rdfs:label "Light"@en ;
  rdfs:label "lys"@nb-no ;
  rdfs:seeAlso <http://bsdd.buildingsmart.org/#concept/details/3S8_P1o2L01Ozx8doI6nGk> ;
  rdfs:seeAlso ifc:IfcAlarmEnumType ;
  rdfs:subClassOf mep:Alarm ;
.
mep:Alarm-MANUALPULLBOX
  rdf:type owl:Class ;
  rdfs:isDefinedBy <http://pi.pauwel.be/voc/distributionelement> ;
  rdfs:label "Manual Pullbox"@en ;
  rdfs:label "manuell trekkeboks"@nb-no ;
  rdfs:seeAlso <http://bsdd.buildingsmart.org/#concept/details/3zt85EwTXD_QTso9MWvKcg> ;
  rdfs:seeAlso ifc:IfcAlarmEnumType ;
  rdfs:subClassOf mep:Alarm ;
.
mep:Alarm-SIREN
  rdf:type owl:Class ;
  rdfs:comment "an audible alarm"@en ;
  rdfs:isDefinedBy <http://pi.pauwel.be/voc/distributionelement> ;
  rdfs:label "Siren"@en ;
  rdfs:label "sirene"@nb-no ;
  rdfs:seeAlso <http://bsdd.buildingsmart.org/#concept/details/1UTy6cbg964OXOMBBCXymq> ;
  rdfs:seeAlso ifc:IfcAlarmEnumType ;
  rdfs:subClassOf mep:Alarm ;
.
mep:Alarm-WHISTLE
  rdf:type owl:Class ;
  rdfs:comment "an audible alarm"@en ;
  rdfs:isDefinedBy <http://pi.pauwel.be/voc/distributionelement> ;
  rdfs:label "Whistle"@en ;
  rdfs:label "fløyte"@nb-no ;
  rdfs:seeAlso <http://bsdd.buildingsmart.org/#concept/details/2AoyxzFcb3MB1ULS_ZzZZX> ;
  rdfs:seeAlso ifc:IfcAlarmEnumType ;
  rdfs:subClassOf mep:Alarm ;
.
mep:AudioVisualAppliance
  rdf:type owl:Class ;
  rdfs:comment """A device that displays, captures, transmits, or receives audio or video.
Audio-visual appliances may be fixed in place or may be able to be moved from one space to another. They may require an electrical supply that may be supplied either by an electrical circuit or provided from a local battery source. Audio-visual appliances may be connected to data circuits including specialist circuits for audio visual purposes only."""@en ;
  rdfs:isDefinedBy <http://pi.pauwel.be/voc/distributionelement> ;
  rdfs:label "Audio Visual Appliance"@en ;
  rdfs:label "appareil audiovisuel"@fr-fr ;
  rdfs:label "audiovisuell enheten"@nb-no ;
  rdfs:label "audiovisuelles Gerät"@de-de ;
  rdfs:seeAlso <http://bsdd.buildingsmart.org/#concept/details/2ZaJrCZM56p8CnFEqtkRj5> ;
  rdfs:seeAlso ifc:IfcAudioVisualAppliance ;
  rdfs:subClassOf mep:FlowTerminal ;
.
mep:AudioVisualAppliance-AMPLIFIER
  rdf:type owl:Class ;
  rdfs:comment "device for boosting audio signal power by means of auxiliary power"@en ;
  rdfs:comment "device for boosting audio signal power by means of auxiliary power"@en-gb ;
  rdfs:isDefinedBy <http://pi.pauwel.be/voc/distributionelement> ;
  rdfs:label "Amplifier"@en ;
  rdfs:label "forsterker"@nb-no ;
  rdfs:seeAlso <http://bsdd.buildingsmart.org/#concept/details/3wRrr4McP2IPDX2xDHWMb5> ;
  rdfs:seeAlso ifc:IfcAudioVisualApplianceEnumType ;
  rdfs:subClassOf mep:AudioVisualAppliance ;
.
mep:AudioVisualAppliance-CAMERA
  rdf:type owl:Class ;
  rdfs:comment "a device that records images, either as a still photograph or as moving images known as videos or movies. Note that a camera may operate with light from the visible spectrum or from other parts of the electromagnetic spectrum such as infrared or ultraviolet."@en ;
  rdfs:comment "a device that records images, either as a still photograph or as moving images known as videos or movies. Note that a camera may operate with light from the visible spectrum or from other parts of the electromagnetic spectrum such as infrared or ultraviolet."@en-gb ;
  rdfs:isDefinedBy <http://pi.pauwel.be/voc/distributionelement> ;
  rdfs:label "Camera"@en ;
  rdfs:label "Camera"@nl-nl ;
  rdfs:label "kamera"@nb-no ;
  rdfs:seeAlso <http://bsdd.buildingsmart.org/#concept/details/0Iits$HO92OhljjIcBPane> ;
  rdfs:seeAlso ifc:IfcAudioVisualApplianceEnumType ;
  rdfs:subClassOf mep:AudioVisualAppliance ;
.
mep:AudioVisualAppliance-DISPLAY
  rdf:type owl:Class ;
  rdfs:comment "an electronic device that represents information in visual form such as a flat-panel display or television."@en ;
  rdfs:isDefinedBy <http://pi.pauwel.be/voc/distributionelement> ;
  rdfs:label "Display"@en ;
  rdfs:label "viser"@nb-no ;
  rdfs:seeAlso <http://bsdd.buildingsmart.org/#concept/details/3zbk7NQJzCte2YLviWyYiT> ;
  rdfs:seeAlso ifc:IfcAudioVisualApplianceEnumType ;
  rdfs:subClassOf mep:AudioVisualAppliance ;
.
mep:AudioVisualAppliance-MICROPHONE
  rdf:type owl:Class ;
  rdfs:comment "an instrument for converting sound waves into electrical energy variations which may then be amplified, transmitted, or recorded"@en ;
  rdfs:comment "an instrument for converting sound waves into electrical energy variations which may then be amplified, transmitted, or recorded"@en-gb ;
  rdfs:isDefinedBy <http://pi.pauwel.be/voc/distributionelement> ;
  rdfs:label "Microfoon"@nl-nl ;
  rdfs:label "Microphone"@en ;
  rdfs:label "mikrofon"@nb-no ;
  rdfs:seeAlso <http://bsdd.buildingsmart.org/#concept/details/2L42aAWJmHu000025QrE$V> ;
  rdfs:seeAlso ifc:IfcAudioVisualApplianceEnumType ;
  rdfs:subClassOf mep:AudioVisualAppliance ;
.
mep:AudioVisualAppliance-PLAYER
  rdf:type owl:Class ;
  rdfs:comment "a device for playing recorded music"@en ;
  rdfs:comment "a device for playing recorded music"@en-gb ;
  rdfs:isDefinedBy <http://pi.pauwel.be/voc/distributionelement> ;
  rdfs:label "Player"@en ;
  rdfs:label "avspiller"@nb-no ;
  rdfs:seeAlso <http://bsdd.buildingsmart.org/#concept/details/3eOLloUdbACBmRDqUZRsWN> ;
  rdfs:seeAlso ifc:IfcAudioVisualApplianceEnumType ;
  rdfs:subClassOf mep:AudioVisualAppliance ;
.
mep:AudioVisualAppliance-PROJECTOR
  rdf:type owl:Class ;
  rdfs:comment "a device that is used to project rays of light, especially an apparatus with a system of lenses for projecting slides or film on to a screen"@en ;
  rdfs:comment "a device that is used to project rays of light, especially an apparatus with a system of lenses for projecting slides or film on to a screen"@en-gb ;
  rdfs:isDefinedBy <http://pi.pauwel.be/voc/distributionelement> ;
  rdfs:label "Projector"@en ;
  rdfs:label "prosjektor"@nb-no ;
  rdfs:seeAlso <http://bsdd.buildingsmart.org/#concept/details/3PFxyF66H6Awpa8qVklE0D> ;
  rdfs:seeAlso ifc:IfcAudioVisualApplianceEnumType ;
  rdfs:subClassOf mep:AudioVisualAppliance ;
.
mep:AudioVisualAppliance-RECEIVER
  rdf:type owl:Class ;
  rdfs:comment "the part of a telephone apparatus contained in the earpiece, in which electrical signals are converted into sounds"@en ;
  rdfs:comment "the part of a telephone apparatus contained in the earpiece, in which electrical signals are converted into sounds"@en-gb ;
  rdfs:isDefinedBy <http://pi.pauwel.be/voc/distributionelement> ;
  rdfs:label "Receiver"@en ;
  rdfs:label "mottaker"@nb-no ;
  rdfs:seeAlso <http://bsdd.buildingsmart.org/#concept/details/0f5ylhxBD1hxZPMi642Cwa> ;
  rdfs:seeAlso ifc:IfcAudioVisualApplianceEnumType ;
  rdfs:subClassOf mep:AudioVisualAppliance ;
.
mep:AudioVisualAppliance-SPEAKER
  rdf:type owl:Class ;
  rdfs:comment "an apparatus that converts electrical impulses into sound, typically as part of a public address system"@en ;
  rdfs:comment "an apparatus that converts electrical impulses into sound, typically as part of a public address system"@en-gb ;
  rdfs:isDefinedBy <http://pi.pauwel.be/voc/distributionelement> ;
  rdfs:label "Speaker"@en ;
  rdfs:label "haut-parleur"@fr-fr ;
  rdfs:label "høytaler"@nb-no ;
  rdfs:label "høyttaler"@nb-no ;
  rdfs:seeAlso <http://bsdd.buildingsmart.org/#concept/details/3VXQt2hgT5iRydKNBGNLUm> ;
  rdfs:seeAlso ifc:IfcAudioVisualApplianceEnumType ;
  rdfs:subClassOf mep:AudioVisualAppliance ;
.
mep:AudioVisualAppliance-SWITCHER
  rdf:type owl:Class ;
  rdfs:comment "a piece of electronic equipment used to select or combine different video and audio signals"@en ;
  rdfs:comment "a piece of electronic equipment used to select or combine different video and audio signals"@en-gb ;
  rdfs:isDefinedBy <http://pi.pauwel.be/voc/distributionelement> ;
  rdfs:label "Switcher"@en ;
  rdfs:label "bryter"@nb-no ;
  rdfs:seeAlso <http://bsdd.buildingsmart.org/#concept/details/15RfXB4Cf9VOzccs$seVij> ;
  rdfs:seeAlso ifc:IfcAudioVisualApplianceEnumType ;
  rdfs:subClassOf mep:AudioVisualAppliance ;
.
mep:AudioVisualAppliance-TELEPHONE
  rdf:type owl:Class ;
  rdfs:isDefinedBy <http://pi.pauwel.be/voc/distributionelement> ;
  rdfs:label "Telephone"@en ;
  rdfs:label "telefon"@nb-no ;
  rdfs:seeAlso <http://bsdd.buildingsmart.org/#concept/details/3LvBfsxh5A9OLMJxpzp_5P> ;
  rdfs:seeAlso ifc:IfcAudioVisualApplianceEnumType ;
  rdfs:subClassOf mep:AudioVisualAppliance ;
.
mep:AudioVisualAppliance-TUNER
  rdf:type owl:Class ;
  rdfs:comment "an electronic device for varying the frequency to which a radio or television is tuned"@en ;
  rdfs:comment "an electronic device for varying the frequency to which a radio or television is tuned"@en-gb ;
  rdfs:isDefinedBy <http://pi.pauwel.be/voc/distributionelement> ;
  rdfs:label "Tuner"@en ;
  rdfs:label "tuner"@nb-no ;
  rdfs:seeAlso <http://bsdd.buildingsmart.org/#concept/details/0sGM9efvTEy8OclWcCNG6k> ;
  rdfs:seeAlso ifc:IfcAudioVisualApplianceEnumType ;
  rdfs:subClassOf mep:AudioVisualAppliance ;
.
mep:Boiler
  rdf:type owl:Class ;
  rdfs:comment "A closed, pressure-rated vessel in which water or other fluid is heated using an energy source such as natural gas, heating oil, or electricity. "@en ;
  rdfs:isDefinedBy <http://pi.pauwel.be/voc/distributionelement> ;
  rdfs:label "Boiler"@en ;
  rdfs:label "Boiler"@nl-nl ;
  rdfs:label "Chaudière"@fr-fr ;
  rdfs:label "Heizkessel"@de-de ;
  rdfs:label "Warmwater voorraadtoestel"@nl-nl ;
  rdfs:label "Warmwatertoestel"@nl-nl ;
  rdfs:label "kjel"@nb-no ;
  rdfs:label "water boiler"@en ;
  rdfs:seeAlso <http://bsdd.buildingsmart.org/#concept/details/2n42GxcQv3ZeE_LK7_FaP7> ;
  rdfs:seeAlso ifc:IfcBoiler ;
  rdfs:subClassOf mep:EnergyConversionDevice ;
.
mep:Boiler-STEAM
  rdf:type owl:Class ;
  rdfs:comment "The amount of steam consumed during the period specified in the time series."@en ;
  rdfs:isDefinedBy <http://pi.pauwel.be/voc/distributionelement> ;
  rdfs:label "Steam Boiler"@en ;
  rdfs:label "dampkjel"@nb-no ;
  rdfs:seeAlso <http://bsdd.buildingsmart.org/#concept/details/3r3yMQaETCj9yTgeFnY6eO> ;
  rdfs:seeAlso ifc:IfcBoilerEnumType ;
  rdfs:subClassOf mep:Boiler ;
.
mep:Boiler-WATER
  rdf:type owl:Class ;
  rdfs:isDefinedBy <http://pi.pauwel.be/voc/distributionelement> ;
  rdfs:label "Water Boiler"@en ;
  rdfs:seeAlso <http://bsdd.buildingsmart.org/#concept/details/3vHZlaoT0Hsm00051Mm008> ;
  rdfs:seeAlso ifc:IfcBoilerEnumType ;
  rdfs:subClassOf mep:Boiler ;
.
mep:Burner
  rdf:type owl:Class ;
  rdfs:comment "A device that converts fuel into heat through combustion."@en ;
  rdfs:isDefinedBy <http://pi.pauwel.be/voc/distributionelement> ;
  rdfs:label "Brenner"@de-de ;
  rdfs:label "Brûleur"@fr-fr ;
  rdfs:label "Burner"@en ;
  rdfs:label "brenner"@nb-no ;
  rdfs:seeAlso <http://bsdd.buildingsmart.org/#concept/details/3eaWqihr5FfBQB2Eu0SSfd> ;
  rdfs:seeAlso ifc:IfcBurner ;
  rdfs:subClassOf mep:EnergyConversionDevice ;
.
mep:CableCarrierFitting
  rdf:type owl:Class ;
  rdfs:comment "A fitting that is placed at junction or transition in a cable carrier system."@en ;
  rdfs:isDefinedBy <http://pi.pauwel.be/voc/distributionelement> ;
  rdfs:label "Cable Carrier Fitting"@en ;
  rdfs:label "Kabelträger Passstück"@de-de ;
  rdfs:label "Raccord de chemin de cable"@fr-fr ;
  rdfs:label "kabelføringskobling"@nb-no ;
  rdfs:seeAlso <http://bsdd.buildingsmart.org/#concept/details/1UxFU0Z7L3wgssm2xurkpg> ;
  rdfs:seeAlso ifc:IfcCableCarrierFitting ;
  rdfs:subClassOf mep:FlowFitting ;
.
mep:CableCarrierFitting-BEND
  rdf:type owl:Class ;
  rdfs:comment "a fitting that changes the route of the cable carrier."@en ;
  rdfs:comment "a fitting that changes the route of the cable carrier."@en-gb ;
  rdfs:isDefinedBy <http://pi.pauwel.be/voc/distributionelement> ;
  rdfs:label "Bend"@en ;
  rdfs:label "bend"@nb-no ;
  rdfs:seeAlso <http://bsdd.buildingsmart.org/#concept/details/02T1S3SGrDMBMfyCIF7X4E> ;
  rdfs:seeAlso ifc:IfcCableCarrierFittingEnumType ;
  rdfs:subClassOf mep:CableCarrierFitting ;
.
mep:CableCarrierFitting-CROSS
  rdf:type owl:Class ;
  rdfs:comment "a fitting at which two branches are taken from the main route of the cable carrier simultaneously."@en ;
  rdfs:isDefinedBy <http://pi.pauwel.be/voc/distributionelement> ;
  rdfs:label "Cross"@en ;
  rdfs:label "kryss"@nb-no ;
  rdfs:seeAlso <http://bsdd.buildingsmart.org/#concept/details/0Nz$21cnn4VwLtD25_Kdcr> ;
  rdfs:seeAlso ifc:IfcCableCarrierFittingEnumType ;
  rdfs:subClassOf mep:CableCarrierFitting ;
.
mep:CableCarrierFitting-REDUCER
  rdf:type owl:Class ;
  rdfs:isDefinedBy <http://pi.pauwel.be/voc/distributionelement> ;
  rdfs:label "Reducer"@en ;
  rdfs:label "reduksjon"@nb-no ;
  rdfs:seeAlso <http://bsdd.buildingsmart.org/#concept/details/3$DOQ8x9jEFehexpevTRMs> ;
  rdfs:seeAlso ifc:IfcCableCarrierFittingEnumType ;
  rdfs:subClassOf mep:CableCarrierFitting ;
.
mep:CableCarrierFitting-TEE
  rdf:type owl:Class ;
  rdfs:comment "a fitting at which a branch is taken from the main route of the cable carrier."@en ;
  rdfs:isDefinedBy <http://pi.pauwel.be/voc/distributionelement> ;
  rdfs:label "T-rør"@nb-no ;
  rdfs:label "Tee"@en ;
  rdfs:seeAlso <http://bsdd.buildingsmart.org/#concept/details/2qYrhIwZ1BQgGx_wwRrFAA> ;
  rdfs:seeAlso ifc:IfcCableCarrierFittingEnumType ;
  rdfs:subClassOf mep:CableCarrierFitting ;
.
mep:CableCarrierSegment
  rdf:type owl:Class ;
  rdfs:comment "A flow segment that is specifically used to carry and support cabling."@en ;
  rdfs:isDefinedBy <http://pi.pauwel.be/voc/distributionelement> ;
  rdfs:label "Cable Carrier Segment"@en ;
  rdfs:label "Kabelträgersegment"@de-de ;
  rdfs:label "Segment de chemin de cable"@fr-fr ;
  rdfs:label "kabelføringssegment"@nb-no ;
  rdfs:seeAlso <http://bsdd.buildingsmart.org/#concept/details/0wEcZCe1zEsO4LVirAd0ZF> ;
  rdfs:seeAlso ifc:IfcCableCarrierSegment ;
  rdfs:subClassOf mep:FlowSegment ;
.
mep:CableCarrierSegment-CABLELADDERSEGMENT
  rdf:type owl:Class ;
  rdfs:isDefinedBy <http://pi.pauwel.be/voc/distributionelement> ;
  rdfs:label "Cable Ladder Segment"@en ;
  rdfs:seeAlso <http://bsdd.buildingsmart.org/#concept/details/0FImfTYGb48ursCbLXsTCr> ;
  rdfs:seeAlso ifc:IfcCableCarrierSegmentEnumType ;
  rdfs:subClassOf mep:CableCarrierSegment ;
.
mep:CableCarrierSegment-CABLETRAYSEGMENT
  rdf:type owl:Class ;
  rdfs:isDefinedBy <http://pi.pauwel.be/voc/distributionelement> ;
  rdfs:label "Cable Tray Segment"@en ;
  rdfs:seeAlso <http://bsdd.buildingsmart.org/#concept/details/3t8hY0ZCvEj8gC2KrGLxGu> ;
  rdfs:seeAlso ifc:IfcCableCarrierSegmentEnumType ;
  rdfs:subClassOf mep:CableCarrierSegment ;
.
mep:CableCarrierSegment-CABLETRUNKINGSEGMENT
  rdf:type owl:Class ;
  rdfs:isDefinedBy <http://pi.pauwel.be/voc/distributionelement> ;
  rdfs:label "Cable Trunk Segment"@en ;
  rdfs:seeAlso <http://bsdd.buildingsmart.org/#concept/details/0bkSD8Eh1ByuLzjMf5xfTq> ;
  rdfs:seeAlso ifc:IfcCableCarrierSegmentEnumType ;
  rdfs:subClassOf mep:CableCarrierSegment ;
.
mep:CableCarrierSegment-CONDUITSEGMENT
  rdf:type owl:Class ;
  rdfs:isDefinedBy <http://pi.pauwel.be/voc/distributionelement> ;
  rdfs:label "Conduit Segment"@en ;
  rdfs:seeAlso <http://bsdd.buildingsmart.org/#concept/details/3MuSnBn2PFkfAY3gBeVAlk> ;
  rdfs:seeAlso ifc:IfcCableCarrierSegmentEnumType ;
  rdfs:subClassOf mep:CableCarrierSegment ;
.
mep:CableFitting
  rdf:type owl:Class ;
  rdfs:comment "A fitting that is placed at a junction, transition or termination in a cable system."@en ;
  rdfs:isDefinedBy <http://pi.pauwel.be/voc/distributionelement> ;
  rdfs:label "Cable Fitting"@en ;
  rdfs:label "Kabelverbinder - Typ"@de-de ;
  rdfs:label "Kabelverbinder"@de-de ;
  rdfs:seeAlso <http://bsdd.buildingsmart.org/#concept/details/27LUFoJu97RuNCAIoglvnW> ;
  rdfs:seeAlso ifc:IfcCableFitting ;
  rdfs:subClassOf mep:FlowFitting ;
.
mep:CableFitting-CONNECTOR
  rdf:type owl:Class ;
  rdfs:comment "a device for keeping two parts of an electric circuit in contact"@en ;
  rdfs:comment "a device for keeping two parts of an electric circuit in contact"@en-gb ;
  rdfs:isDefinedBy <http://pi.pauwel.be/voc/distributionelement> ;
  rdfs:label "Connector"@en ;
  rdfs:label "connecteur"@fr-fr ;
  rdfs:label "forbindelse"@nb-no ;
  rdfs:seeAlso <http://bsdd.buildingsmart.org/#concept/details/1xjOGZ4kX1g8pvaS5Bd5bG> ;
  rdfs:seeAlso ifc:IfcCableFittingEnumType ;
  rdfs:subClassOf mep:CableFitting ;
.
mep:CableFitting-ENTRY
  rdf:type owl:Class ;
  rdfs:comment "a fitting that begins a cable segment at a non-electrical element such as a grounding clamp attached to a pipe"@en ;
  rdfs:isDefinedBy <http://pi.pauwel.be/voc/distributionelement> ;
  rdfs:label "Entry"@en ;
  rdfs:label "inngang"@nb-no ;
  rdfs:seeAlso <http://bsdd.buildingsmart.org/#concept/details/07gAPw_U1EguTzO5UilotA> ;
  rdfs:seeAlso ifc:IfcCableFittingEnumType ;
  rdfs:subClassOf mep:CableFitting ;
.
mep:CableFitting-EXIT
  rdf:type owl:Class ;
  rdfs:isDefinedBy <http://pi.pauwel.be/voc/distributionelement> ;
  rdfs:label "Exit"@en ;
  rdfs:label "utgang"@nb-no ;
  rdfs:seeAlso <http://bsdd.buildingsmart.org/#concept/details/1_YaBIQW905QZ9AjtoPTNy> ;
  rdfs:seeAlso ifc:IfcCableFittingEnumType ;
  rdfs:subClassOf mep:CableFitting ;
.
mep:CableFitting-JUNCTION
  rdf:type owl:Class ;
  rdfs:comment "a fitting that joins three or more segments of arbitrary connector types for signal splitting or multiplexing."@en ;
  rdfs:comment "a fitting that joins three or more segments of arbitrary connector types for signal splitting or multiplexing."@en-gb ;
  rdfs:isDefinedBy <http://pi.pauwel.be/voc/distributionelement> ;
  rdfs:label "Junction"@en ;
  rdfs:label "gren"@nb-no ;
  rdfs:seeAlso <http://bsdd.buildingsmart.org/#concept/details/1RPq5LwjT7VwBv_u4OjJrf> ;
  rdfs:seeAlso ifc:IfcCableFittingEnumType ;
  rdfs:subClassOf mep:CableFitting ;
.
mep:CableFitting-TRANSITION
  rdf:type owl:Class ;
  rdfs:isDefinedBy <http://pi.pauwel.be/voc/distributionelement> ;
  rdfs:label "Transition"@en ;
  rdfs:label "overgang"@nb-no ;
  rdfs:seeAlso <http://bsdd.buildingsmart.org/#concept/details/2H3YKfRzn2u9Nog81SAl8k> ;
  rdfs:seeAlso ifc:IfcCableFittingEnumType ;
  rdfs:subClassOf mep:CableFitting ;
.
mep:CableSegment
  rdf:type owl:Class ;
  rdfs:comment "A flow segment used to carry electrical power, data, or telecommunications signals."@en ;
  rdfs:isDefinedBy <http://pi.pauwel.be/voc/distributionelement> ;
  rdfs:label "Cable Segment"@en ;
  rdfs:label "Kabelsegment"@de-de ;
  rdfs:label "Segment de câble"@fr-fr ;
  rdfs:seeAlso <http://bsdd.buildingsmart.org/#concept/details/26thIKCK1FhfE8oeEPRbVn> ;
  rdfs:seeAlso ifc:IfcCableSegment ;
  rdfs:subClassOf mep:FlowSegment ;
.
mep:CableSegment-BUSBARSEGMENT
  rdf:type owl:Class ;
  rdfs:isDefinedBy <http://pi.pauwel.be/voc/distributionelement> ;
  rdfs:label "Busbar Segment"@en ;
  rdfs:seeAlso <http://bsdd.buildingsmart.org/#concept/details/0uFCFVhl53Re8TGtNoQbaU> ;
  rdfs:seeAlso ifc:IfcCableSegmentEnumType ;
  rdfs:subClassOf mep:CableSegment ;
.
mep:CableSegment-CONDUCTORSEGMENT
  rdf:type owl:Class ;
  rdfs:isDefinedBy <http://pi.pauwel.be/voc/distributionelement> ;
  rdfs:label "Conductor Segment"@en ;
  rdfs:seeAlso <http://bsdd.buildingsmart.org/#concept/details/2dlPSgGMHCnu9mfLG8gZtL> ;
  rdfs:seeAlso ifc:IfcCableSegmentEnumType ;
  rdfs:subClassOf mep:CableSegment ;
.
mep:CableSegment-CORESEGMENT
  rdf:type owl:Class ;
  rdfs:isDefinedBy <http://pi.pauwel.be/voc/distributionelement> ;
  rdfs:label "Core Segment"@en ;
  rdfs:seeAlso <http://bsdd.buildingsmart.org/#concept/details/2AYnQG0vTDUwn_LR9znomO> ;
  rdfs:seeAlso ifc:IfcCableSegmentEnumType ;
  rdfs:subClassOf mep:CableSegment ;
.
mep:Chiller
  rdf:type owl:Class ;
  rdfs:comment "A device used to remove heat from a liquid via a vapor-compression or absorption refrigeration cycle to cool a fluid, typically water or a mixture of water and glycol."@en ;
  rdfs:isDefinedBy <http://pi.pauwel.be/voc/distributionelement> ;
  rdfs:label "Chiller"@en ;
  rdfs:label "Kältemaschine"@de-de ;
  rdfs:label "Refroidisseur"@fr-fr ;
  rdfs:label "kjøler"@nb-no ;
  rdfs:label "kylare"@sv-se ;
  rdfs:label "refrigeratore"@it-it ;
  rdfs:seeAlso <http://bsdd.buildingsmart.org/#concept/details/1Zpzuw4lf8p9CkbZR8gJou> ;
  rdfs:seeAlso ifc:IfcChiller ;
  rdfs:subClassOf mep:EnergyConversionDevice ;
.
mep:Chiller-AIRCOOLED
  rdf:type owl:Class ;
  rdfs:comment "air cooled chiller"@en ;
  rdfs:comment "air cooled chiller"@en-gb ;
  rdfs:isDefinedBy <http://pi.pauwel.be/voc/distributionelement> ;
  rdfs:label "Air-Cooled Chiller"@en ;
  rdfs:label "luftkjølt kjøler"@nb-no ;
  rdfs:seeAlso <http://bsdd.buildingsmart.org/#concept/details/0Tmp5umYX80uDxxCJQrW$a> ;
  rdfs:seeAlso ifc:IfcChillerEnumType ;
  rdfs:subClassOf mep:Chiller ;
.
mep:Chiller-HEATRECOVERY
  rdf:type owl:Class ;
  rdfs:comment "heat recovery chiller."@en ;
  rdfs:isDefinedBy <http://pi.pauwel.be/voc/distributionelement> ;
  rdfs:label "Heat Recovery Chiller"@en ;
  rdfs:label "varmegjenvinning"@nb-no ;
  rdfs:seeAlso <http://bsdd.buildingsmart.org/#concept/details/30ALQiOHn5LetyiGCdujt6> ;
  rdfs:seeAlso ifc:IfcChillerEnumType ;
  rdfs:subClassOf mep:Chiller ;
.
mep:Chiller-WATERCOOLED
  rdf:type owl:Class ;
  rdfs:comment "water cooled chiller"@en ;
  rdfs:comment "water cooled chiller"@en-gb ;
  rdfs:isDefinedBy <http://pi.pauwel.be/voc/distributionelement> ;
  rdfs:label "Water-Cooled Chiller"@en ;
  rdfs:label "vannkjølt"@nb-no ;
  rdfs:seeAlso <http://bsdd.buildingsmart.org/#concept/details/1$b15itWrEVeOmpk8LNP3I> ;
  rdfs:seeAlso ifc:IfcChillerEnumType ;
  rdfs:subClassOf mep:Chiller ;
.
mep:Coil
  rdf:type owl:Class ;
  rdfs:comment "A device used to provide heat transfer between non-mixing media."@en ;
  rdfs:isDefinedBy <http://pi.pauwel.be/voc/distributionelement> ;
  rdfs:label "Bobine"@fr-fr ;
  rdfs:label "Coil"@en ;
  rdfs:label "Flade"@da ;
  rdfs:label "Heiz-Kühlelemente"@de-de ;
  rdfs:label "spoletype"@nb-no ;
  rdfs:seeAlso <http://bsdd.buildingsmart.org/#concept/details/1reT_0qSaHuO00025QrE$V> ;
  rdfs:seeAlso ifc:IfcCoil ;
  rdfs:subClassOf mep:EnergyConversionDevice ;
.
mep:Coil-DXCOOLINGCOIL
  rdf:type owl:Class ;
  rdfs:comment "cooling coil using a refrigerant to cool the air stream directly."@en ;
  rdfs:isDefinedBy <http://pi.pauwel.be/voc/distributionelement> ;
  rdfs:label "DXCoolingCoil"@en ;
  rdfs:label "dx kjølecoil"@nb-no ;
  rdfs:seeAlso <http://bsdd.buildingsmart.org/#concept/details/1exlqEQr96eATeS6qcQeE3> ;
  rdfs:seeAlso ifc:IfcCoilEnumType ;
  rdfs:subClassOf mep:Coil ;
.
mep:Coil-ELECTRICHEATINGCOIL
  rdf:type owl:Class ;
  rdfs:comment "heating coil using electricity as a heating source."@en ;
  rdfs:isDefinedBy <http://pi.pauwel.be/voc/distributionelement> ;
  rdfs:label "Electric Heating Coil"@en ;
  rdfs:label "varmecoil"@nb-no ;
  rdfs:seeAlso <http://bsdd.buildingsmart.org/#concept/details/1sKDt$czD8mQchRqMMNYlB> ;
  rdfs:seeAlso ifc:IfcCoilEnumType ;
  rdfs:subClassOf mep:Coil ;
.
mep:Coil-GASHEATINGCOIL
  rdf:type owl:Class ;
  rdfs:comment "heating coil using gas as a heating source."@en ;
  rdfs:isDefinedBy <http://pi.pauwel.be/voc/distributionelement> ;
  rdfs:label "Gas Heating Coil"@en ;
  rdfs:label "gassfyring coil"@nb-no ;
  rdfs:seeAlso <http://bsdd.buildingsmart.org/#concept/details/2Y2dXDycvEJe30WIRF8tsM> ;
  rdfs:seeAlso ifc:IfcCoilEnumType ;
  rdfs:subClassOf mep:Coil ;
.
mep:Coil-HYDRONICCOIL
  rdf:type owl:Class ;
  rdfs:comment "cooling or Heating coil that uses a hydronic fluid as a cooling or heating source."@en ;
  rdfs:isDefinedBy <http://pi.pauwel.be/voc/distributionelement> ;
  rdfs:label "Hydronic Coil"@en ;
  rdfs:label "vann/luft spole"@nb-no ;
  rdfs:seeAlso <http://bsdd.buildingsmart.org/#concept/details/0KqvZFKzH5SQiVr$vKoSfk> ;
  rdfs:seeAlso ifc:IfcCoilEnumType ;
  rdfs:subClassOf mep:Coil ;
.
mep:Coil-STEAMHEATINGCOIL
  rdf:type owl:Class ;
  rdfs:comment "heating coil using steam as heating source."@en ;
  rdfs:isDefinedBy <http://pi.pauwel.be/voc/distributionelement> ;
  rdfs:label "Steam Heating Coil"@en ;
  rdfs:seeAlso <http://bsdd.buildingsmart.org/#concept/details/2rXlQ3zHz1IwGGCAc5t50T> ;
  rdfs:seeAlso ifc:IfcCoilEnumType ;
  rdfs:subClassOf mep:Coil ;
.
mep:Coil-WATERCOOLINGCOIL
  rdf:type owl:Class ;
  rdfs:comment "cooling coil using chilled water. HYDRONICCOIL supercedes this enumerator."@en ;
  rdfs:isDefinedBy <http://pi.pauwel.be/voc/distributionelement> ;
  rdfs:label "Water Cooling Coil"@en ;
  rdfs:label "vannkjøler - coil"@nb-no ;
  rdfs:seeAlso <http://bsdd.buildingsmart.org/#concept/details/3AbyMrisP4ehArYy89RfYX> ;
  rdfs:seeAlso ifc:IfcCoilEnumType ;
  rdfs:subClassOf mep:Coil ;
.
mep:Coil-WATERHEATINGCOIL
  rdf:type owl:Class ;
  rdfs:comment "heating coil using hot water as a heating source. HYDRONICCOIL supercedes this enumerator."@en ;
  rdfs:isDefinedBy <http://pi.pauwel.be/voc/distributionelement> ;
  rdfs:label "Water Heating Coil"@en ;
  rdfs:label "vannvarme - coil"@nb-no ;
  rdfs:seeAlso <http://bsdd.buildingsmart.org/#concept/details/0ZF$5RRJPDkPP$6rdC$LOy> ;
  rdfs:seeAlso ifc:IfcCoilEnumType ;
  rdfs:subClassOf mep:Coil ;
.
mep:CommunicationsAppliance
  rdf:type owl:Class ;
  rdfs:comment "A communications device transmits and receives electronic or digital information as data or sound."@en ;
  rdfs:isDefinedBy <http://pi.pauwel.be/voc/distributionelement> ;
  rdfs:label "Appareil de communications"@fr-fr ;
  rdfs:label "Communications Appliance"@en ;
  rdfs:label "Kommunikationsgerät"@de-de ;
  rdfs:label "kommunikasjonsapparat"@nb-no ;
  rdfs:seeAlso <http://bsdd.buildingsmart.org/#concept/details/3dS_KvJn16dgqG0Y8M0_8M> ;
  rdfs:seeAlso ifc:IfcCommunicationsAppliance ;
  rdfs:subClassOf mep:FlowTerminal ;
.
mep:CommunicationsAppliance-ANTENNA
  rdf:type owl:Class ;
  rdfs:comment "a transducer designed to transmit or receive electromagnetic waves."@en ;
  rdfs:isDefinedBy <http://pi.pauwel.be/voc/distributionelement> ;
  rdfs:label "Antenna"@en ;
  rdfs:label "antenne"@nb-no ;
  rdfs:seeAlso <http://bsdd.buildingsmart.org/#concept/details/0C2VVYeDP29xB3DZDSeUl0> ;
  rdfs:seeAlso ifc:IfcCommunicationsApplianceEnumType ;
  rdfs:subClassOf mep:CommunicationsAppliance ;
.
mep:CommunicationsAppliance-COMPUTER
  rdf:type owl:Class ;
  rdfs:comment "an electronic device which is capable of receiving information (data) in a particular form and of performing a sequence of operations in accordance with a predetermined but variable set of procedural instructions (program) to produce a result in the form of information or signals"@en ;
  rdfs:comment "an electronic device which is capable of receiving information (data) in a particular form and of performing a sequence of operations in accordance with a predetermined but variable set of procedural instructions (program) to produce a result in the form of information or signals"@en-gb ;
  rdfs:isDefinedBy <http://pi.pauwel.be/voc/distributionelement> ;
  rdfs:label "Computer"@en ;
  rdfs:label "computer"@nb-no ;
  rdfs:label "datagolv"@nb-no ;
  rdfs:label "datagulv"@nb-no ;
  rdfs:label "datamaskin"@nb-no ;
  rdfs:label "gulvsystem datagulv"@nb-no ;
  rdfs:seeAlso <http://bsdd.buildingsmart.org/#concept/details/3YJ0SHSxL2Se6$_7rNWY_P> ;
  rdfs:seeAlso ifc:IfcCommunicationsApplianceEnumType ;
  rdfs:subClassOf mep:CommunicationsAppliance ;
.
mep:CommunicationsAppliance-FAX
  rdf:type owl:Class ;
  rdfs:comment "a machine for transmitting and receiving faxes"@en ;
  rdfs:comment "a machine for transmitting and receiving faxes"@en-gb ;
  rdfs:isDefinedBy <http://pi.pauwel.be/voc/distributionelement> ;
  rdfs:label "Fax"@en ;
  rdfs:label "fax"@nb-no ;
  rdfs:seeAlso <http://bsdd.buildingsmart.org/#concept/details/0rZr4shW90zOb$tqxFAwq_> ;
  rdfs:seeAlso ifc:IfcCommunicationsApplianceEnumType ;
  rdfs:subClassOf mep:CommunicationsAppliance ;
.
mep:CommunicationsAppliance-GATEWAY
  rdf:type owl:Class ;
  rdfs:comment "a gateway connects multiple network segments with different protocols at all layers (layers 1-7) of the Open Systems Interconnection (OSI) model."@en ;
  rdfs:isDefinedBy <http://pi.pauwel.be/voc/distributionelement> ;
  rdfs:label "Gateway"@en ;
  rdfs:label "gateway"@nb-no ;
  rdfs:label "nettgrense - gateway"@nb-no ;
  rdfs:seeAlso <http://bsdd.buildingsmart.org/#concept/details/32NV4lWbbC8fXXlHfMs1EJ> ;
  rdfs:seeAlso ifc:IfcCommunicationsApplianceEnumType ;
  rdfs:subClassOf mep:CommunicationsAppliance ;
.
mep:CommunicationsAppliance-MODEM
  rdf:type owl:Class ;
  rdfs:comment "a combined device for modulation and demodulation, for example, between the digital data of a computer and the analogue signal of a telephone line"@en ;
  rdfs:comment "a combined device for modulation and demodulation, for example, between the digital data of a computer and the analogue signal of a telephone line"@en-gb ;
  rdfs:isDefinedBy <http://pi.pauwel.be/voc/distributionelement> ;
  rdfs:label "Modem"@en ;
  rdfs:label "modem"@nb-no ;
  rdfs:seeAlso <http://bsdd.buildingsmart.org/#concept/details/0KFUxRBVf7AAcbfoB6t3UZ> ;
  rdfs:seeAlso ifc:IfcCommunicationsApplianceEnumType ;
  rdfs:subClassOf mep:CommunicationsAppliance ;
.
mep:CommunicationsAppliance-NETWORKAPPLIANCE
  rdf:type owl:Class ;
  rdfs:isDefinedBy <http://pi.pauwel.be/voc/distributionelement> ;
  rdfs:label "Network Appliance"@en ;
  rdfs:seeAlso <http://bsdd.buildingsmart.org/#concept/details/2WnZ6tZHfC7gNz8mylrfCG> ;
  rdfs:seeAlso ifc:IfcCommunicationsApplianceEnumType ;
  rdfs:subClassOf mep:CommunicationsAppliance ;
.
mep:CommunicationsAppliance-NETWORKBRIDGE
  rdf:type owl:Class ;
  rdfs:isDefinedBy <http://pi.pauwel.be/voc/distributionelement> ;
  rdfs:label "Network Bridge"@en ;
  rdfs:seeAlso <http://bsdd.buildingsmart.org/#concept/details/2BwyUI_XTBHhVWLVNXjmP1> ;
  rdfs:seeAlso ifc:IfcCommunicationsApplianceEnumType ;
  rdfs:subClassOf mep:CommunicationsAppliance ;
.
mep:CommunicationsAppliance-NETWORKHUB
  rdf:type owl:Class ;
  rdfs:isDefinedBy <http://pi.pauwel.be/voc/distributionelement> ;
  rdfs:label "Network Hub"@en ;
  rdfs:seeAlso <http://bsdd.buildingsmart.org/#concept/details/2isi2CWT5C8hpM6didtFuS> ;
  rdfs:seeAlso ifc:IfcCommunicationsApplianceEnumType ;
  rdfs:subClassOf mep:CommunicationsAppliance ;
.
mep:CommunicationsAppliance-PRINTER
  rdf:type owl:Class ;
  rdfs:comment "a machine for printing text or pictures, especially one linked to a computer"@en ;
  rdfs:comment "a machine for printing text or pictures, especially one linked to a computer"@en-gb ;
  rdfs:isDefinedBy <http://pi.pauwel.be/voc/distributionelement> ;
  rdfs:label "Printer"@en ;
  rdfs:label "printer"@nb-no ;
  rdfs:seeAlso <http://bsdd.buildingsmart.org/#concept/details/2gEEth5ArE5hgXWDZ2HEeu> ;
  rdfs:seeAlso ifc:IfcCommunicationsApplianceEnumType ;
  rdfs:subClassOf mep:CommunicationsAppliance ;
.
mep:CommunicationsAppliance-REPEATER
  rdf:type owl:Class ;
  rdfs:comment "a device for the automatic retransmission or amplification of an electrically transmitted message"@en ;
  rdfs:comment "a device for the automatic retransmission or amplification of an electrically transmitted message"@en-gb ;
  rdfs:isDefinedBy <http://pi.pauwel.be/voc/distributionelement> ;
  rdfs:label "Repeater"@en ;
  rdfs:label "repeater"@nb-no ;
  rdfs:seeAlso <http://bsdd.buildingsmart.org/#concept/details/0kMGElI9XD5x0JqYWcVH5G> ;
  rdfs:seeAlso ifc:IfcCommunicationsApplianceEnumType ;
  rdfs:subClassOf mep:CommunicationsAppliance ;
.
mep:CommunicationsAppliance-ROUTER
  rdf:type owl:Class ;
  rdfs:comment "A router is a networking device whose software and hardware are usually tailored to the tasks of routing and forwarding information. For example, on the Internet, information is directed to various paths by routers."@en ;
  rdfs:comment "A router is a networking device whose software and hardware are usually tailored to the tasks of routing and forwarding information. For example, on the Internet, information is directed to various paths by routers."@en-gb ;
  rdfs:isDefinedBy <http://pi.pauwel.be/voc/distributionelement> ;
  rdfs:label "Router"@en ;
  rdfs:label "nettverksruter"@nb-no ;
  rdfs:seeAlso <http://bsdd.buildingsmart.org/#concept/details/3iPUFOOkn9CR_oYn1_vIJe> ;
  rdfs:seeAlso ifc:IfcCommunicationsApplianceEnumType ;
  rdfs:subClassOf mep:CommunicationsAppliance ;
.
mep:CommunicationsAppliance-SCANNER
  rdf:type owl:Class ;
  rdfs:comment "a device that scans documents and converts them into digital data"@en ;
  rdfs:comment "a device that scans documents and converts them into digital data"@en-gb ;
  rdfs:isDefinedBy <http://pi.pauwel.be/voc/distributionelement> ;
  rdfs:label "Scanner"@en ;
  rdfs:label "scanner"@nb-no ;
  rdfs:seeAlso <http://bsdd.buildingsmart.org/#concept/details/3Zb4cC11TBmAB3gBWRepr4> ;
  rdfs:seeAlso ifc:IfcCommunicationsApplianceEnumType ;
  rdfs:subClassOf mep:CommunicationsAppliance ;
.
mep:Compressor
  rdf:type owl:Class ;
  rdfs:comment "A device that compresses a fluid typically used in a refrigeration circuit."@en ;
  rdfs:isDefinedBy <http://pi.pauwel.be/voc/distributionelement> ;
  rdfs:label "Compresseur"@fr-fr ;
  rdfs:label "Compressor"@en ;
  rdfs:label "Kompressor"@de-de ;
  rdfs:seeAlso <http://bsdd.buildingsmart.org/#concept/details/1Qp4AN19X6Huz0qWsWQk2Q> ;
  rdfs:seeAlso ifc:IfcCompressor ;
  rdfs:subClassOf mep:FlowMovingDevice ;
.
mep:Compressor-BOOSTER
  rdf:type owl:Class ;
  rdfs:comment "positive-displacement reciprocating compressor where pressure is increased by a booster."@en ;
  rdfs:isDefinedBy <http://pi.pauwel.be/voc/distributionelement> ;
  rdfs:label "Booster"@en ;
  rdfs:label "forsterker"@nb-no ;
  rdfs:seeAlso <http://bsdd.buildingsmart.org/#concept/details/0KvKrF8Vv38QKJC3iDOsZR> ;
  rdfs:seeAlso ifc:IfcCompressorEnumType ;
  rdfs:subClassOf mep:Compressor ;
.
mep:Compressor-DYNAMIC
  rdf:type owl:Class ;
  rdfs:comment "the pressure of refrigerant vapor is increased by a continuous transfer of angular momentum from a rotating member to the vapor followed by conversion of this momentum into static pressure."@en ;
  rdfs:isDefinedBy <http://pi.pauwel.be/voc/distributionelement> ;
  rdfs:label "Dynamic Compressor"@en ;
  rdfs:label "dynamisk"@nb-no ;
  rdfs:seeAlso <http://bsdd.buildingsmart.org/#concept/details/0bjNJRb7f3bOrNnlEVDx$V> ;
  rdfs:seeAlso ifc:IfcCompressorEnumType ;
  rdfs:subClassOf mep:Compressor ;
.
mep:Compressor-HERMETIC
  rdf:type owl:Class ;
  rdfs:comment "positive-displacement reciprocating compressor where the motor and compressor are contained within the same housing, with the motor shaft integral with the compressor crankshaft and the motor in contact with refrigerant."@en ;
  rdfs:isDefinedBy <http://pi.pauwel.be/voc/distributionelement> ;
  rdfs:label "Hermetic Compressor"@en ;
  rdfs:label "lukket"@nb-no ;
  rdfs:seeAlso <http://bsdd.buildingsmart.org/#concept/details/1QxsNyRLjDEfER9sd9a4nA> ;
  rdfs:seeAlso ifc:IfcCompressorEnumType ;
  rdfs:subClassOf mep:Compressor ;
.
mep:Compressor-OPENTYPE
  rdf:type owl:Class ;
  rdfs:comment "positive-displacement reciprocating compressor where the shaft extends through a seal in the crankcase for an external drive."@en ;
  rdfs:isDefinedBy <http://pi.pauwel.be/voc/distributionelement> ;
  rdfs:label "Open Type Compressor"@en ;
  rdfs:label "kompressor - åpen"@nb-no ;
  rdfs:seeAlso <http://bsdd.buildingsmart.org/#concept/details/35$2VQ6Vf3yAbaBgoiZ_Qy> ;
  rdfs:seeAlso ifc:IfcCompressorEnumType ;
  rdfs:subClassOf mep:Compressor ;
.
mep:Compressor-RECIPROCATING
  rdf:type owl:Class ;
  rdfs:comment "positive-displacement compressor using a piston driven by a connecting rod from a crankshaft."@en ;
  rdfs:isDefinedBy <http://pi.pauwel.be/voc/distributionelement> ;
  rdfs:label "Reciprocating Compressor"@en ;
  rdfs:label "stempel"@nb-no ;
  rdfs:seeAlso <http://bsdd.buildingsmart.org/#concept/details/1rD1BDTTnA4Opl9hEUzc3J> ;
  rdfs:seeAlso ifc:IfcCompressorEnumType ;
  rdfs:subClassOf mep:Compressor ;
.
mep:Compressor-ROLLINGPISTON
  rdf:type owl:Class ;
  rdfs:comment "positive-displacement rotary compressor using a roller mounted on the eccentric of a shaft with a single vane in the nonrotating cylindrical housing."@en ;
  rdfs:isDefinedBy <http://pi.pauwel.be/voc/distributionelement> ;
  rdfs:label "Rolling Piston Compressor"@en ;
  rdfs:label "rullestempel"@nb-no ;
  rdfs:seeAlso <http://bsdd.buildingsmart.org/#concept/details/25ip$MycH3CApiL8P1Zfua> ;
  rdfs:seeAlso ifc:IfcCompressorEnumType ;
  rdfs:subClassOf mep:Compressor ;
.
mep:Compressor-ROTARY
  rdf:type owl:Class ;
  rdfs:comment "positive-displacement compressor using a roller or rotor device."@en ;
  rdfs:isDefinedBy <http://pi.pauwel.be/voc/distributionelement> ;
  rdfs:label "Rotary Compressor"@en ;
  rdfs:label "kompressor - roterende"@nb-no ;
  rdfs:seeAlso <http://bsdd.buildingsmart.org/#concept/details/34DscBiG12O81W_KaUsgZs> ;
  rdfs:seeAlso ifc:IfcCompressorEnumType ;
  rdfs:subClassOf mep:Compressor ;
.
mep:Compressor-ROTARYVANE
  rdf:type owl:Class ;
  rdfs:comment "positive-displacement rotary compressor using a roller mounted on the eccentric of a shaft with multiple vanes in the nontotating cylindrical housing."@en ;
  rdfs:isDefinedBy <http://pi.pauwel.be/voc/distributionelement> ;
  rdfs:label "Rotary Vane Compressor"@en ;
  rdfs:label "kompressor - roterende vinge"@nb-no ;
  rdfs:seeAlso <http://bsdd.buildingsmart.org/#concept/details/3Fnn56$If0Ywd7AMXubW5r> ;
  rdfs:seeAlso ifc:IfcCompressorEnumType ;
  rdfs:subClassOf mep:Compressor ;
.
mep:Compressor-SCROLL
  rdf:type owl:Class ;
  rdfs:comment "positive-displacement compressor using two inter-fitting, spiral-shaped scroll members."@en ;
  rdfs:isDefinedBy <http://pi.pauwel.be/voc/distributionelement> ;
  rdfs:label "Scroll Compressor"@en ;
  rdfs:label "spiral"@nb-no ;
  rdfs:seeAlso <http://bsdd.buildingsmart.org/#concept/details/1e5CFyUGv9suZ9ky8c_4Ir> ;
  rdfs:seeAlso ifc:IfcCompressorEnumType ;
  rdfs:subClassOf mep:Compressor ;
.
mep:Compressor-SEMIHERMETIC
  rdf:type owl:Class ;
  rdfs:comment "positive-displacement reciprocating compressor where the hermetic compressors use bolted construction amenable to field repair."@en ;
  rdfs:isDefinedBy <http://pi.pauwel.be/voc/distributionelement> ;
  rdfs:label "Semi Hermetic Compressor"@en ;
  rdfs:label "semilukket"@nb-no ;
  rdfs:seeAlso <http://bsdd.buildingsmart.org/#concept/details/0rQK7zwf97_vwAvPlWuuME> ;
  rdfs:seeAlso ifc:IfcCompressorEnumType ;
  rdfs:subClassOf mep:Compressor ;
.
mep:Compressor-SINGLESCREW
  rdf:type owl:Class ;
  rdfs:comment "positive-displacement rotary compressor using a single cylindrical main rotor that works with a pair of gate rotors."@en ;
  rdfs:isDefinedBy <http://pi.pauwel.be/voc/distributionelement> ;
  rdfs:label "Single Screw Compressor"@en ;
  rdfs:label "enkeltskrue"@nb-no ;
  rdfs:seeAlso <http://bsdd.buildingsmart.org/#concept/details/2U43NgKlnBqPnnBLsl6wU4> ;
  rdfs:seeAlso ifc:IfcCompressorEnumType ;
  rdfs:subClassOf mep:Compressor ;
.
mep:Compressor-SINGLESTAGE
  rdf:type owl:Class ;
  rdfs:comment "positive-displacement reciprocating compressor where vapor is compressed in a single stage."@en ;
  rdfs:isDefinedBy <http://pi.pauwel.be/voc/distributionelement> ;
  rdfs:label "Single Stage Compressor"@en ;
  rdfs:label "ettrinns"@nb-no ;
  rdfs:seeAlso <http://bsdd.buildingsmart.org/#concept/details/1sA1FIWkz8SRjvM$gcNai0> ;
  rdfs:seeAlso ifc:IfcCompressorEnumType ;
  rdfs:subClassOf mep:Compressor ;
.
mep:Compressor-TROCHOIDAL
  rdf:type owl:Class ;
  rdfs:comment "positive-displacement compressor using a rolling motion of one circle outside or inside the circumference of a basic circle and produce either epitrochoids or hypotrochoids."@en ;
  rdfs:isDefinedBy <http://pi.pauwel.be/voc/distributionelement> ;
  rdfs:label "Trochoidal Compressor"@en ;
  rdfs:label "trokoid"@nb-no ;
  rdfs:seeAlso <http://bsdd.buildingsmart.org/#concept/details/1L2jXYOSr0k980kt8JnyQv> ;
  rdfs:seeAlso ifc:IfcCompressorEnumType ;
  rdfs:subClassOf mep:Compressor ;
.
mep:Compressor-TWINSCREW
  rdf:type owl:Class ;
  rdfs:comment "positive-displacement rotary compressor using two mating helically grooved rotors, male (lobes) and female (flutes) in a stationary housing with inlet and outlet gas ports."@en ;
  rdfs:isDefinedBy <http://pi.pauwel.be/voc/distributionelement> ;
  rdfs:label "Twin Screw Compressor"@en ;
  rdfs:label "dobbelkompressor"@nb-no ;
  rdfs:seeAlso <http://bsdd.buildingsmart.org/#concept/details/3hihvfHSj9h8cGQM0xtKAu> ;
  rdfs:seeAlso ifc:IfcCompressorEnumType ;
  rdfs:subClassOf mep:Compressor ;
.
mep:Compressor-WELDEDSHELLHERMETIC
  rdf:type owl:Class ;
  rdfs:isDefinedBy <http://pi.pauwel.be/voc/distributionelement> ;
  rdfs:label "Welded Shell Hermetic Compressor"@en ;
  rdfs:seeAlso <http://bsdd.buildingsmart.org/#concept/details/3YKCxQG3X2xhA2b8$YRmuH> ;
  rdfs:seeAlso ifc:IfcCompressorEnumType ;
  rdfs:subClassOf mep:Compressor ;
.
mep:Condenser
  rdf:type owl:Class ;
  rdfs:comment "A device that is used to dissipate heat, typically by condensing a substance such as a refrigerant from its gaseous to its liquid state."@en ;
  rdfs:comment "heat exchanger that condenses refrigerant vapour by rejecting heat"@en ;
  rdfs:isDefinedBy <http://pi.pauwel.be/voc/distributionelement> ;
  rdfs:label "Condenser"@en ;
  rdfs:label "Condenseur"@fr-fr ;
  rdfs:label "Kondensator"@de-de ;
  rdfs:label "condensatore"@it-it ;
  rdfs:label "kondensator"@nb-no ;
  rdfs:seeAlso <http://bsdd.buildingsmart.org/#concept/details/2DpcsXxln2WvYyPFOAkV$n> ;
  rdfs:seeAlso ifc:IfcCondenser ;
  rdfs:subClassOf mep:EnergyConversionDevice ;
.
mep:Condenser-AIRCOOLED
  rdf:type owl:Class ;
  rdfs:comment "a condenser in which heat is transferred to an air-stream"@en ;
  rdfs:comment "a condenser in which heat is transferred to an air-stream"@en-gb ;
  rdfs:isDefinedBy <http://pi.pauwel.be/voc/distributionelement> ;
  rdfs:label "Air Cooled"@en ;
  rdfs:label "kondensator luftkjølt"@nb-no ;
  rdfs:seeAlso <http://bsdd.buildingsmart.org/#concept/details/3I1OxJC71BJOJi3xkrXKKM> ;
  rdfs:seeAlso ifc:IfcCondenserEnumType ;
  rdfs:subClassOf mep:Condenser ;
.
mep:Condenser-EVAPORATIVECOOLED
  rdf:type owl:Class ;
  rdfs:comment "a condenser that is cooled evaporatively."@en ;
  rdfs:isDefinedBy <http://pi.pauwel.be/voc/distributionelement> ;
  rdfs:label "Evaporative Cooled"@en ;
  rdfs:label "fordampningkjølt"@nb-no ;
  rdfs:seeAlso <http://bsdd.buildingsmart.org/#concept/details/1FUPWLndXE$hUQLc0y3Wj6> ;
  rdfs:seeAlso ifc:IfcCondenserEnumType ;
  rdfs:subClassOf mep:Condenser ;
.
mep:Condenser-WATERCOOLED
  rdf:type owl:Class ;
  rdfs:comment "water-cooled condenser with unspecified operation"@en ;
  rdfs:comment "water-cooled condenser with unspecified operation"@en-gb ;
  rdfs:isDefinedBy <http://pi.pauwel.be/voc/distributionelement> ;
  rdfs:label "Water Cooled"@en ;
  rdfs:seeAlso <http://bsdd.buildingsmart.org/#concept/details/1$_Cv8DcnEIhdevMYpgzOs> ;
  rdfs:seeAlso ifc:IfcCondenserEnumType ;
  rdfs:subClassOf mep:Condenser ;
.
mep:Condenser-WATERCOOLEDBRAZEDPLATE
  rdf:type owl:Class ;
  rdfs:comment "water-cooled condenser condenser with plates brazed together to form an assembly of separate channels."@en ;
  rdfs:isDefinedBy <http://pi.pauwel.be/voc/distributionelement> ;
  rdfs:label "Water Cooled Brazed Plate"@en ;
  rdfs:seeAlso <http://bsdd.buildingsmart.org/#concept/details/3DsQKabLb8PuG7s1BwpA5x> ;
  rdfs:seeAlso ifc:IfcCondenserEnumType ;
  rdfs:subClassOf mep:Condenser ;
.
mep:Condenser-WATERCOOLEDSHELLCOIL
  rdf:type owl:Class ;
  rdfs:comment "water-cooled condenser with cooling water circulated through one or more continuous or assembled coils contained within the shell."@en ;
  rdfs:isDefinedBy <http://pi.pauwel.be/voc/distributionelement> ;
  rdfs:label "Water Cooled Shell Coil"@en ;
  rdfs:seeAlso <http://bsdd.buildingsmart.org/#concept/details/2y2FRrDI58wPQ$P0QmPB4S> ;
  rdfs:seeAlso ifc:IfcCondenserEnumType ;
  rdfs:subClassOf mep:Condenser ;
.
mep:Condenser-WATERCOOLEDSHELLTUBE
  rdf:type owl:Class ;
  rdfs:isDefinedBy <http://pi.pauwel.be/voc/distributionelement> ;
  rdfs:label "Water Cooled Shell Tube"@en ;
  rdfs:seeAlso <http://bsdd.buildingsmart.org/#concept/details/1v95Mqhl19xxpoA6ogzO73> ;
  rdfs:seeAlso ifc:IfcCondenserEnumType ;
  rdfs:subClassOf mep:Condenser ;
.
mep:Condenser-WATERCOOLEDTUBEINTUBE
  rdf:type owl:Class ;
  rdfs:comment "water-cooled condenser consisting of one or more assemblies of two tubes, one within the other."@en ;
  rdfs:isDefinedBy <http://pi.pauwel.be/voc/distributionelement> ;
  rdfs:label "Water Cooled Tube In Tube"@en ;
  rdfs:label "vannkjøler - rør i rør"@nb-no ;
  rdfs:seeAlso <http://bsdd.buildingsmart.org/#concept/details/2qm75n0SHCbPRb1y1l8QGa> ;
  rdfs:seeAlso ifc:IfcCondenserEnumType ;
  rdfs:subClassOf mep:Condenser ;
.
mep:Controller
  rdf:type owl:Class ;
  rdfs:comment "A device that monitors inputs and controls outputs within a building automation system."@en ;
  rdfs:isDefinedBy <http://pi.pauwel.be/voc/distributionelement> ;
  rdfs:label "Controller"@en ;
  rdfs:label "Organe de contrôle"@fr-fr ;
  rdfs:label "Regler"@de-de ;
  rdfs:seeAlso <http://bsdd.buildingsmart.org/#concept/details/1yoko0qSqHuO00025QrE$V> ;
  rdfs:seeAlso ifc:IfcController ;
  rdfs:subClassOf mep:DistributionControlElement ;
.
mep:Controller-FLOATING
  rdf:type owl:Class ;
  rdfs:comment "output increases or decreases at a constant or accelerating rate."@en ;
  rdfs:isDefinedBy <http://pi.pauwel.be/voc/distributionelement> ;
  rdfs:label "Floating"@en ;
  rdfs:label "flottør"@nb-no ;
  rdfs:seeAlso <http://bsdd.buildingsmart.org/#concept/details/3v66KyDUH03vDK75zE5Ddn> ;
  rdfs:seeAlso ifc:IfcControllerEnumType ;
  rdfs:subClassOf mep:Controller ;
.
mep:Controller-MULTIPOSITION
  rdf:type owl:Class ;
  rdfs:comment "output is discrete value, can be one of three or more values."@en ;
  rdfs:isDefinedBy <http://pi.pauwel.be/voc/distributionelement> ;
  rdfs:label "Multi-Position"@en ;
  rdfs:label "flerposisjonskontroller"@nb-no ;
  rdfs:seeAlso <http://bsdd.buildingsmart.org/#concept/details/2a0hNKxwTAH8HS3TExjKQd> ;
  rdfs:seeAlso ifc:IfcControllerEnumType ;
  rdfs:subClassOf mep:Controller ;
.
mep:Controller-PROGRAMMABLE
  rdf:type owl:Class ;
  rdfs:comment "programmable logic controller containing interconnected operations and variables."@en ;
  rdfs:isDefinedBy <http://pi.pauwel.be/voc/distributionelement> ;
  rdfs:label "Programmable"@en ;
  rdfs:label "programerbar kontroller"@nb-no ;
  rdfs:seeAlso <http://bsdd.buildingsmart.org/#concept/details/1UXoUiKJr2XedXgGzf6I3D> ;
  rdfs:seeAlso ifc:IfcControllerEnumType ;
  rdfs:subClassOf mep:Controller ;
.
mep:Controller-PROPORTIONAL
  rdf:type owl:Class ;
  rdfs:comment "output is proportional to the control error and optionally time integral and derivative."@en ;
  rdfs:isDefinedBy <http://pi.pauwel.be/voc/distributionelement> ;
  rdfs:label "Proportional"@en ;
  rdfs:label "proporsjonal"@nb-no ;
  rdfs:seeAlso <http://bsdd.buildingsmart.org/#concept/details/3soSUmco55dRLnyEdLB2Pe> ;
  rdfs:seeAlso ifc:IfcControllerEnumType ;
  rdfs:subClassOf mep:Controller ;
.
mep:Controller-TWOPOSITION
  rdf:type owl:Class ;
  rdfs:isDefinedBy <http://pi.pauwel.be/voc/distributionelement> ;
  rdfs:label "Two-Position"@en ;
  rdfs:seeAlso <http://bsdd.buildingsmart.org/#concept/details/3eIN8kftz36v5YeB_hMmzI> ;
  rdfs:seeAlso ifc:IfcControllerEnumType ;
  rdfs:subClassOf mep:Controller ;
.
mep:CooledBeam
  rdf:type owl:Class ;
  rdfs:comment "A device typically used to cool air by circulating a fluid such as chilled water through exposed finned tubes above a space. Typically mounted overhead near or within a ceiling."@en ;
  rdfs:isDefinedBy <http://pi.pauwel.be/voc/distributionelement> ;
  rdfs:label "Chilled Beam"@en ;
  rdfs:label "Cooled Beam"@en ;
  rdfs:label "Kühlbalken"@de-de ;
  rdfs:label "Poutre froide type"@fr-fr ;
  rdfs:label "Poutre froide"@fr-fr ;
  rdfs:label "kjølekonvektor"@nb-no ;
  rdfs:seeAlso <http://bsdd.buildingsmart.org/#concept/details/1R134kf$f3g9C$U9ACWL3s> ;
  rdfs:seeAlso ifc:IfcCooledBeam ;
  rdfs:subClassOf mep:EnergyConversionDevice ;
.
mep:CooledBeam-ACTIVE
  rdf:type owl:Class ;
  rdfs:comment "an active or ventilated cooled beam provides cooling (and heating) but can also function as an air terminal in a ventilation system"@en ;
  rdfs:comment "an active or ventilated cooled beam provides cooling (and heating) but can also function as an air terminal in a ventilation system"@en-gb ;
  rdfs:isDefinedBy <http://pi.pauwel.be/voc/distributionelement> ;
  rdfs:label "Active"@en ;
  rdfs:label "kjølekonvektor - aktiv"@nb-no ;
  rdfs:seeAlso <http://bsdd.buildingsmart.org/#concept/details/366WDqf6H92RxKizKbtgeZ> ;
  rdfs:seeAlso ifc:IfcCooledBeamEnumType ;
  rdfs:subClassOf mep:CooledBeam ;
.
mep:CooledBeam-PASSIVE
  rdf:type owl:Class ;
  rdfs:isDefinedBy <http://pi.pauwel.be/voc/distributionelement> ;
  rdfs:label "Passive"@en ;
  rdfs:label "passiv"@nb-no ;
  rdfs:seeAlso <http://bsdd.buildingsmart.org/#concept/details/2xz0NcLlr5_O7fEPShW1WV> ;
  rdfs:seeAlso ifc:IfcCooledBeamEnumType ;
  rdfs:subClassOf mep:CooledBeam ;
.
mep:CoolingTower
  rdf:type owl:Class ;
  rdfs:comment "A device which rejects heat to ambient air by circulating a fluid such as water through it to reduce its temperature by partial evaporation."@en ;
  rdfs:isDefinedBy <http://pi.pauwel.be/voc/distributionelement> ;
  rdfs:label "Cooling Tower"@en ;
  rdfs:label "Kühlturm"@de-de ;
  rdfs:label "Tour de refroidissement"@fr-fr ;
  rdfs:label "kjøletårn"@nb-no ;
  rdfs:seeAlso <http://bsdd.buildingsmart.org/#concept/details/0ExTiEVwf5eBdOlVt_Lyd0> ;
  rdfs:seeAlso ifc:IfcCoolingTower ;
  rdfs:subClassOf mep:EnergyConversionDevice ;
.
mep:CoolingTower-MECHANICALFORCEDDRAFT
  rdf:type owl:Class ;
  rdfs:comment "air flow is produced by a mechanical device, typically one or more fans, located on the inlet air side of the cooling tower."@en ;
  rdfs:isDefinedBy <http://pi.pauwel.be/voc/distributionelement> ;
  rdfs:label "Mechanical Forced Draft"@en ;
  rdfs:label "mekanisk utkast"@nb-no ;
  rdfs:seeAlso <http://bsdd.buildingsmart.org/#concept/details/3dU1hLD$n4bwQx_$PVTTC6> ;
  rdfs:seeAlso ifc:IfcCoolingTowerEnumType ;
  rdfs:subClassOf mep:CoolingTower ;
.
mep:CoolingTower-MECHANICALINDUCEDDRAFT
  rdf:type owl:Class ;
  rdfs:comment "air flow is produced by a mechanical device, typically one or more fans, located on the air outlet side of the cooling tower."@en ;
  rdfs:isDefinedBy <http://pi.pauwel.be/voc/distributionelement> ;
  rdfs:label "Mechanical Induced Draft"@en ;
  rdfs:label "mekanisk indusert utkast"@nb-no ;
  rdfs:seeAlso <http://bsdd.buildingsmart.org/#concept/details/2aEmlXSRL6hO5XcfF8JxRk> ;
  rdfs:seeAlso ifc:IfcCoolingTowerEnumType ;
  rdfs:subClassOf mep:CoolingTower ;
.
mep:CoolingTower-NATURALDRAFT
  rdf:type owl:Class ;
  rdfs:comment "air flow is produced naturally."@en ;
  rdfs:isDefinedBy <http://pi.pauwel.be/voc/distributionelement> ;
  rdfs:label "Natural Draft"@en ;
  rdfs:label "naturlig trekk"@nb-no ;
  rdfs:seeAlso <http://bsdd.buildingsmart.org/#concept/details/3O4_SVPPzB3881fdAXOU7s> ;
  rdfs:seeAlso ifc:IfcCoolingTowerEnumType ;
  rdfs:subClassOf mep:CoolingTower ;
.
mep:Damper
  rdf:type owl:Class ;
  rdfs:comment "A flow controller in an HVAC duct distribution system and is used to control or modulate the flow of air."@en ;
  rdfs:comment "innretning som brukes til å redusere støt eller vibrasjoner med energiabsorberende metoder"@nb-no ;
  rdfs:isDefinedBy <http://pi.pauwel.be/voc/distributionelement> ;
  rdfs:label "Damper"@en ;
  rdfs:label "Détecteur d'incendie"@fr-fr ;
  rdfs:label "Regelklappe"@de-de ;
  rdfs:label "Spjæld"@da ;
  rdfs:label "serranda"@it-it ;
  rdfs:label "spjeld"@nb-no ;
  rdfs:seeAlso <http://bsdd.buildingsmart.org/#concept/details/2lAXa0qT0HuO00025QrE$V> ;
  rdfs:seeAlso ifc:IfcDamper ;
  rdfs:subClassOf mep:FlowController ;
.
mep:Damper-BACKDRAFTDAMPER
  rdf:type owl:Class ;
  rdfs:isDefinedBy <http://pi.pauwel.be/voc/distributionelement> ;
  rdfs:label "Back Draft Damper"@en ;
  rdfs:label "baktrekk demper"@nb-no ;
  rdfs:seeAlso <http://bsdd.buildingsmart.org/#concept/details/0g_pG9hAD1XgJ8pML2mm5H> ;
  rdfs:seeAlso ifc:IfcDamperEnumType ;
  rdfs:subClassOf mep:Damper ;
.
mep:Damper-BALANCINGDAMPER
  rdf:type owl:Class ;
  rdfs:isDefinedBy <http://pi.pauwel.be/voc/distributionelement> ;
  rdfs:label "Balancing Damper"@en ;
  rdfs:label "utjevningsspjeld"@nb-no ;
  rdfs:seeAlso <http://bsdd.buildingsmart.org/#concept/details/2p0wEtbSj4gxlyI6mhADq2> ;
  rdfs:seeAlso ifc:IfcDamperEnumType ;
  rdfs:subClassOf mep:Damper ;
.
mep:Damper-BLASTDAMPER
  rdf:type owl:Class ;
  rdfs:isDefinedBy <http://pi.pauwel.be/voc/distributionelement> ;
  rdfs:label "Blast Damper"@en ;
  rdfs:label "eksplosjon spjeld"@nb-no ;
  rdfs:seeAlso <http://bsdd.buildingsmart.org/#concept/details/369EqwVYL9pfnNqcXnoDHU> ;
  rdfs:seeAlso ifc:IfcDamperEnumType ;
  rdfs:subClassOf mep:Damper ;
.
mep:Damper-CONTROLDAMPER
  rdf:type owl:Class ;
  rdfs:isDefinedBy <http://pi.pauwel.be/voc/distributionelement> ;
  rdfs:label "Control Damper"@en ;
  rdfs:seeAlso <http://bsdd.buildingsmart.org/#concept/details/2rVf7QFRTEWOLI2fZJuW7H> ;
  rdfs:seeAlso ifc:IfcDamperEnumType ;
  rdfs:subClassOf mep:Damper ;
.
mep:Damper-FIREDAMPER
  rdf:type owl:Class ;
  rdfs:isDefinedBy <http://pi.pauwel.be/voc/distributionelement> ;
  rdfs:label "Fire Damper"@en ;
  rdfs:seeAlso <http://bsdd.buildingsmart.org/#concept/details/3mqiUJIz57JBFFnuqvB3qT> ;
  rdfs:seeAlso ifc:IfcDamperEnumType ;
  rdfs:subClassOf mep:Damper ;
.
mep:Damper-FIRESMOKEDAMPER
  rdf:type owl:Class ;
  rdfs:isDefinedBy <http://pi.pauwel.be/voc/distributionelement> ;
  rdfs:label "Fire Smoke Damper"@en ;
  rdfs:seeAlso <http://bsdd.buildingsmart.org/#concept/details/3fTPn78FL2kPB6iokOAbpY> ;
  rdfs:seeAlso ifc:IfcDamperEnumType ;
  rdfs:subClassOf mep:Damper ;
.
mep:Damper-FUMEHOODEXHAUST
  rdf:type owl:Class ;
  rdfs:isDefinedBy <http://pi.pauwel.be/voc/distributionelement> ;
  rdfs:label "Fume Hood Exhaust"@en ;
  rdfs:label "røykhette"@nb-no ;
  rdfs:seeAlso <http://bsdd.buildingsmart.org/#concept/details/1U6ESQrqDFCPr0rdPKWCka> ;
  rdfs:seeAlso ifc:IfcDamperEnumType ;
  rdfs:subClassOf mep:Damper ;
.
mep:Damper-GRAVITYDAMPER
  rdf:type owl:Class ;
  rdfs:isDefinedBy <http://pi.pauwel.be/voc/distributionelement> ;
  rdfs:label "Gravity Damper"@en ;
  rdfs:seeAlso <http://bsdd.buildingsmart.org/#concept/details/1A$dgK16XE_x2gK7uacSn3> ;
  rdfs:seeAlso ifc:IfcDamperEnumType ;
  rdfs:subClassOf mep:Damper ;
.
mep:Damper-GRAVITYRELIEFDAMPER
  rdf:type owl:Class ;
  rdfs:isDefinedBy <http://pi.pauwel.be/voc/distributionelement> ;
  rdfs:label "Gravity Relief Damper"@en ;
  rdfs:seeAlso <http://bsdd.buildingsmart.org/#concept/details/26urqKngv5ve948m7Tso_5> ;
  rdfs:seeAlso ifc:IfcDamperEnumType ;
  rdfs:subClassOf mep:Damper ;
.
mep:Damper-RELIEFDAMPER
  rdf:type owl:Class ;
  rdfs:isDefinedBy <http://pi.pauwel.be/voc/distributionelement> ;
  rdfs:label "Relief Damper"@en ;
  rdfs:label "relieff spjeld"@nb-no ;
  rdfs:seeAlso <http://bsdd.buildingsmart.org/#concept/details/0CQxb8jqP12etStsVhj0a2> ;
  rdfs:seeAlso ifc:IfcDamperEnumType ;
  rdfs:subClassOf mep:Damper ;
.
mep:Damper-SMOKEDAMPER
  rdf:type owl:Class ;
  rdfs:isDefinedBy <http://pi.pauwel.be/voc/distributionelement> ;
  rdfs:label "Smoke Damper"@en ;
  rdfs:label "røyspjeld"@nb-no ;
  rdfs:seeAlso <http://bsdd.buildingsmart.org/#concept/details/1vKdAZIn1BaBKbLSz3Ygwn> ;
  rdfs:seeAlso ifc:IfcDamperEnumType ;
  rdfs:subClassOf mep:Damper ;
.
mep:DistributionChamberElement
  rdf:type owl:Class ;
  rdfs:comment "A place at which distribution systems and their constituent elements may be inspected or through which they may travel."@en ;
  rdfs:isDefinedBy <http://pi.pauwel.be/voc/distributionelement> ;
  rdfs:label "Distribution Chamber Element"@en ;
  rdfs:label "Elément de chambre de distribution"@fr-fr ;
  rdfs:label "Schacht / Graben / Revisionsschacht"@de-de ;
  rdfs:label "distribusjonskammer element"@nb-no ;
  rdfs:seeAlso <http://bsdd.buildingsmart.org/#concept/details/1D7kC0qTCHuO00025QrE$V> ;
  rdfs:seeAlso ifc:IfcDistributionChamberElement ;
  rdfs:subClassOf mep:DistributionFlowElement ;
.
mep:DistributionChamberElement-FORMEDDUCT
  rdf:type owl:Class ;
  rdfs:isDefinedBy <http://pi.pauwel.be/voc/distributionelement> ;
  rdfs:label "Formed Duct"@en ;
  rdfs:seeAlso <http://bsdd.buildingsmart.org/#concept/details/02IcnFZFL5vOjShoJLi_XK> ;
  rdfs:seeAlso ifc:IfcDistributionChamberElementEnumType ;
  rdfs:subClassOf mep:DistributionChamberElement ;
.
mep:DistributionChamberElement-INSPECTIONCHAMBER
  rdf:type owl:Class ;
  rdfs:comment "chamber constructed on a drain, sewer or pipeline with a removable cover that permits visble inspection"@en ;
  rdfs:comment "chamber constructed on a drain, sewer or pipeline with a removable cover that permits visble inspection"@en-gb ;
  rdfs:isDefinedBy <http://pi.pauwel.be/voc/distributionelement> ;
  rdfs:label "Inspection Chamber"@en ;
  rdfs:label "inspeksjonskammer"@nb-no ;
  rdfs:seeAlso <http://bsdd.buildingsmart.org/#concept/details/0XN2ZdAhP8tPdjsk4V3170> ;
  rdfs:seeAlso ifc:IfcDistributionChamberElementEnumType ;
  rdfs:subClassOf mep:DistributionChamberElement ;
.
mep:DistributionChamberElement-INSPECTIONPIT
  rdf:type owl:Class ;
  rdfs:comment "recess or chamber formed to permit access for inspection of substructure and services"@en ;
  rdfs:comment "recess or chamber formed to permit access for inspection of substructure and services"@en-gb ;
  rdfs:isDefinedBy <http://pi.pauwel.be/voc/distributionelement> ;
  rdfs:label "Inspection Pit"@en ;
  rdfs:label "inspeksjonsbrønn"@nb-no ;
  rdfs:seeAlso <http://bsdd.buildingsmart.org/#concept/details/05cbWWHhL7kgrWsi2U6_yV> ;
  rdfs:seeAlso ifc:IfcDistributionChamberElementEnumType ;
  rdfs:subClassOf mep:DistributionChamberElement ;
.
mep:DistributionChamberElement-MANHOLE
  rdf:type owl:Class ;
  rdfs:isDefinedBy <http://pi.pauwel.be/voc/distributionelement> ;
  rdfs:label "Manhole"@en ;
  rdfs:label "kum"@nb-no ;
  rdfs:seeAlso <http://bsdd.buildingsmart.org/#concept/details/1bbvZoH6X72QXL2iztFvrY> ;
  rdfs:seeAlso ifc:IfcDistributionChamberElementEnumType ;
  rdfs:subClassOf mep:DistributionChamberElement ;
.
mep:DistributionChamberElement-METERCHAMBER
  rdf:type owl:Class ;
  rdfs:comment "chamber that houses a meter(s)"@en ;
  rdfs:comment "chamber that houses a meter(s)"@en-gb ;
  rdfs:isDefinedBy <http://pi.pauwel.be/voc/distributionelement> ;
  rdfs:label "Meter Chamber"@en ;
  rdfs:label "målekammer"@nb-no ;
  rdfs:seeAlso <http://bsdd.buildingsmart.org/#concept/details/2t4ttlLaz5zerB1pgSekJt> ;
  rdfs:seeAlso ifc:IfcDistributionChamberElementEnumType ;
  rdfs:subClassOf mep:DistributionChamberElement ;
.
mep:DistributionChamberElement-SUMP
  rdf:type owl:Class ;
  rdfs:isDefinedBy <http://pi.pauwel.be/voc/distributionelement> ;
  rdfs:label "Sump"@en ;
  rdfs:label "drenering"@nb-no ;
  rdfs:seeAlso <http://bsdd.buildingsmart.org/#concept/details/013MAut7T66e3F7FQ6GSpz> ;
  rdfs:seeAlso ifc:IfcDistributionChamberElementEnumType ;
  rdfs:subClassOf mep:DistributionChamberElement ;
.
mep:DistributionChamberElement-TRENCH
  rdf:type owl:Class ;
  rdfs:isDefinedBy <http://pi.pauwel.be/voc/distributionelement> ;
  rdfs:label "Trench"@en ;
  rdfs:label "grøft"@nb-no ;
  rdfs:seeAlso <http://bsdd.buildingsmart.org/#concept/details/2yGBCxZDXDlBMJTgQNqhCM> ;
  rdfs:seeAlso ifc:IfcDistributionChamberElementEnumType ;
  rdfs:subClassOf mep:DistributionChamberElement ;
.
mep:DistributionChamberElement-VALVECHAMBER
  rdf:type owl:Class ;
  rdfs:isDefinedBy <http://pi.pauwel.be/voc/distributionelement> ;
  rdfs:label "Valve Chamber"@en ;
  rdfs:seeAlso <http://bsdd.buildingsmart.org/#concept/details/1JHK2axxvBXQ7W3Ey18QZW> ;
  rdfs:seeAlso ifc:IfcDistributionChamberElementEnumType ;
  rdfs:subClassOf mep:DistributionChamberElement ;
.
mep:DistributionControlElement
  rdf:type owl:Class ;
  rdfs:comment "the distribution element ifcdistributioncontrolelement defines occurrence elements of a building automation control system that are used to impart control over elements of a distribution system. ifcdistributioncontrolelement defines elements of a building automation control system. these are typically used to control distribution system elements to maintain variables such as temperature, humidity, pressure, flow, power or lighting levels, through the modulation, staging or sequencing of mechanical or electrical devices. the three general functional categories of control elements are as follows: impart control over flow control elements (ifcflowcontroller) in a distribution system such as dampers, valves or relays, typically through the use of actuation (ifcactuator)., sensing elements (ifcsensor) that measure changes in the controlled variable such as temperature, humidity, pressure or flow., controllers (ifccontroller) typically classified according to the control action they seek to perform and generally responsible for making decisions about the elements under control.. since ifcdistributioncontrolelement and its subtypes typically relate to many different distribution flow elements (ifcdistributionflowelement), the objectified relationship ifcrelflowcontrolelements has been provided to relate control and flow elements as required. the key distinction between ifcdistributionflowelement and ifcdistributioncontrolelement is whether it is internal or external to the flow system, respectively. for example, the distinction between ifcflowmeter (subtype of ifcdistributionflowelement measuring a flow quantity) and ifcflowinstrument (subtype of ifcdistributioncontrolelement measuring a flow quality), is based on this principal. a physical device that connects within the flow system in which it measures (having inlet/outlet pipes for the measured substance) follows the ifcdistributionflowelement hierarchy (and therefore ifcflowmeter which measures the flow internally). otherwise, if it monitors/controls but does not connect inline within the flow system (it is external or is a component of another device), then it follows the ifcdistributioncontrolelement hierarchy (and therefore ifcflowinstrument which may display various attributes through connected sensors)."@en ;
  rdfs:isDefinedBy <http://pi.pauwel.be/voc/distributionelement> ;
  rdfs:label "Distribution Control Element"@en ;
  rdfs:label "Komponente der Gebäudeautomation (allgemein)"@de-de ;
  rdfs:label "distribusjon manøvreringsorgan"@nb-no ;
  rdfs:label "Élément de circuit de distribution"@fr-fr ;
  rdfs:seeAlso <http://bsdd.buildingsmart.org/#concept/details/3U4sRnv$D80uOqEQZrMx_Z> ;
  rdfs:seeAlso ifc:IfcDistributionControlElement ;
  rdfs:subClassOf mep:DistributionElement ;
.
mep:DistributionElement
  rdf:type owl:Class ;
  rdfs:comment """A generalization of all elements that participate in a distribution system. Typical examples :
building service elements within a heating systems, cooling system, ventilation system, plumbing system
or electrical elements within a communication network"""@en ;
  rdfs:isDefinedBy <http://pi.pauwel.be/voc/distributionelement> ;
  rdfs:label "Distribution Element"@en ;
  rdfs:label "Elément de distribution"@fr-fr ;
  rdfs:label "haustechnische Komponente (allgemein)"@de-de ;
  rdfs:seeAlso <http://bsdd.buildingsmart.org/#concept/details/1UHiGqJXTCL9Ds53EKce2Y> ;
  rdfs:seeAlso ifc:IfcDistributionElement ;
  rdfs:subClassOf contax:ConstructionComponent ;
.
mep:DistributionFlowElement
  rdf:type owl:Class ;
  rdfs:comment """A distribution element defined by occurrence elements of a distribution system that facilitate the distribution of energy or matter, such as air, water or power.
Examples are ducts, pipes, wires, fittings, and equipment."""@en ;
  rdfs:isDefinedBy <http://pi.pauwel.be/voc/distributionelement> ;
  rdfs:label "Distribution Flow Element"@en ;
  rdfs:label "Elément de distribution de fluide"@fr-fr ;
  rdfs:label "Komponente der TGA (allgemein)"@de-de ;
  rdfs:label "distribusjonsrørelement"@nb-no ;
  rdfs:seeAlso <http://bsdd.buildingsmart.org/#concept/details/2Ci$80qWWHuO00025QrE$V> ;
  rdfs:seeAlso ifc:IfcDistributionFlowElement ;
  rdfs:subClassOf mep:DistributionElement ;
.
mep:DuctFitting
  rdf:type owl:Class ;
  rdfs:comment "A junction or transition in a ducted flow distribution system or used to connect duct segments, resulting in changes in flow characteristics to the fluid such as direction and flow rate."@en ;
  rdfs:isDefinedBy <http://pi.pauwel.be/voc/distributionelement> ;
  rdfs:label "Duct Fitting"@en ;
  rdfs:label "Kanaalverbindingshulpstuk"@nl-nl ;
  rdfs:label "Kanalverbinder"@de-de ;
  rdfs:label "Raccord de gaine"@fr-fr ;
  rdfs:label "kanalfeste"@nb-no ;
  rdfs:seeAlso <http://bsdd.buildingsmart.org/#concept/details/3UarA0qTqHuO00025QrE$V> ;
  rdfs:seeAlso ifc:IfcDuctFitting ;
  rdfs:subClassOf mep:FlowFitting ;
.
mep:DuctFitting-BEND
  rdf:type owl:Class ;
  rdfs:comment "a fitting with typically two ports used to change the direction of flow between connected elements"@en ;
  rdfs:comment "a fitting with typically two ports used to change the direction of flow between connected elements"@en-gb ;
  rdfs:isDefinedBy <http://pi.pauwel.be/voc/distributionelement> ;
  rdfs:label "Bend"@en ;
  rdfs:label "bend"@nb-no ;
  rdfs:seeAlso <http://bsdd.buildingsmart.org/#concept/details/0TRO3rI8H6H9tkJsr0U5Zs> ;
  rdfs:seeAlso ifc:IfcDuctFittingEnumType ;
  rdfs:subClassOf mep:DuctFitting ;
.
mep:DuctFitting-CONNECTOR
  rdf:type owl:Class ;
  rdfs:isDefinedBy <http://pi.pauwel.be/voc/distributionelement> ;
  rdfs:label "Connector"@en ;
  rdfs:label "connecteur"@fr-fr ;
  rdfs:label "forbindelse"@nb-no ;
  rdfs:seeAlso <http://bsdd.buildingsmart.org/#concept/details/2uxftRh$fAkhgUKLmF1KRz> ;
  rdfs:seeAlso ifc:IfcDuctFittingEnumType ;
  rdfs:subClassOf mep:DuctFitting ;
.
mep:DuctFitting-ENTRY
  rdf:type owl:Class ;
  rdfs:comment "entry fitting, typically unconnected at one port and connected to a flow distribution system at the other (e.g., an outside air duct system intake opening)"@en ;
  rdfs:comment "entry fitting, typically unconnected at one port and connected to a flow distribution system at the other (e.g., an outside air duct system intake opening)"@en-gb ;
  rdfs:isDefinedBy <http://pi.pauwel.be/voc/distributionelement> ;
  rdfs:label "Entry"@en ;
  rdfs:label "inngang"@nb-no ;
  rdfs:seeAlso <http://bsdd.buildingsmart.org/#concept/details/05vd0J9Jv4yf_lzDUNR9nD> ;
  rdfs:seeAlso ifc:IfcDuctFittingEnumType ;
  rdfs:subClassOf mep:DuctFitting ;
.
mep:DuctFitting-EXIT
  rdf:type owl:Class ;
  rdfs:isDefinedBy <http://pi.pauwel.be/voc/distributionelement> ;
  rdfs:label "Exit"@en ;
  rdfs:label "utgang"@nb-no ;
  rdfs:seeAlso <http://bsdd.buildingsmart.org/#concept/details/0VmlPFMi57uO7GMaLeI9HP> ;
  rdfs:seeAlso ifc:IfcDuctFittingEnumType ;
  rdfs:subClassOf mep:DuctFitting ;
.
mep:DuctFitting-JUNCTION
  rdf:type owl:Class ;
  rdfs:comment "a fitting with typically more than two ports used to redistribute flow among the ports and/or to change the direction of flow between connected elements (e.g, tee, cross, wye, etc.)"@en ;
  rdfs:comment "a fitting with typically more than two ports used to redistribute flow among the ports and/or to change the direction of flow between connected elements (e.g, tee, cross, wye, etc.)."@en-gb ;
  rdfs:isDefinedBy <http://pi.pauwel.be/voc/distributionelement> ;
  rdfs:label "Junction"@en ;
  rdfs:label "grenrør"@nb-no ;
  rdfs:label "kryss"@nb-no ;
  rdfs:seeAlso <http://bsdd.buildingsmart.org/#concept/details/0UePnHIHn9vvttWhkbxrCv> ;
  rdfs:seeAlso ifc:IfcDuctFittingEnumType ;
  rdfs:subClassOf mep:DuctFitting ;
.
mep:DuctFitting-OBSTRUCTION
  rdf:type owl:Class ;
  rdfs:isDefinedBy <http://pi.pauwel.be/voc/distributionelement> ;
  rdfs:label "Obstruction"@en ;
  rdfs:label "hindring"@nb-no ;
  rdfs:seeAlso <http://bsdd.buildingsmart.org/#concept/details/0_eTgdHQn7MwoGtRPOoi4r> ;
  rdfs:seeAlso ifc:IfcDuctFittingEnumType ;
  rdfs:subClassOf mep:DuctFitting ;
.
mep:DuctFitting-TRANSITION
  rdf:type owl:Class ;
  rdfs:isDefinedBy <http://pi.pauwel.be/voc/distributionelement> ;
  rdfs:label "Transition"@en ;
  rdfs:label "overgang"@nb-no ;
  rdfs:seeAlso <http://bsdd.buildingsmart.org/#concept/details/1JknxHMCfDq9zypxDIsX5P> ;
  rdfs:seeAlso ifc:IfcDuctFittingEnumType ;
  rdfs:subClassOf mep:DuctFitting ;
.
mep:DuctSegment
  rdf:type owl:Class ;
  rdfs:comment "Used to typically join two sections of duct network."@en ;
  rdfs:isDefinedBy <http://pi.pauwel.be/voc/distributionelement> ;
  rdfs:label "Duct Segment"@en ;
  rdfs:label "Kanal"@de-de ;
  rdfs:label "Tronçon de gaine"@fr-fr ;
  rdfs:label "kanalsegment"@nb-no ;
  rdfs:seeAlso <http://bsdd.buildingsmart.org/#concept/details/0i3x_0qTuHuO00025QrE$V> ;
  rdfs:seeAlso ifc:IfcDuctSegment ;
  rdfs:subClassOf mep:FlowSegment ;
.
mep:DuctSegment-FLEXIBLESEGMENT
  rdf:type owl:Class ;
  rdfs:isDefinedBy <http://pi.pauwel.be/voc/distributionelement> ;
  rdfs:label "Flexible Duct Segment"@en ;
  rdfs:label "fleksibel delflate"@nb-no ;
  rdfs:label "fleksibel rørdel"@nb-no ;
  rdfs:seeAlso <http://bsdd.buildingsmart.org/#concept/details/2nqUfs2mn9YQ_jGNKRyiPP> ;
  rdfs:seeAlso ifc:IfcDuctSegmentEnumType ;
  rdfs:subClassOf mep:DuctSegment ;
.
mep:DuctSegment-RIGIDSEGMENT
  rdf:type owl:Class ;
  rdfs:comment "a rigid segment is a continuous linear segment of duct that cannot be deformed"@en ;
  rdfs:comment "a rigid segment is a continuous linear segment of duct that cannot be deformed"@en-gb ;
  rdfs:isDefinedBy <http://pi.pauwel.be/voc/distributionelement> ;
  rdfs:label "Rigid Duct Segment"@en ;
  rdfs:label "stiv delflate"@nb-no ;
  rdfs:seeAlso <http://bsdd.buildingsmart.org/#concept/details/0Wy45YhJ1Bee5B_Ev4IySE> ;
  rdfs:seeAlso ifc:IfcDuctSegmentEnumType ;
  rdfs:subClassOf mep:DuctSegment ;
.
mep:DuctSilencer
  rdf:type owl:Class ;
  rdfs:comment "A device that is typically installed inside a duct distribution system for the purpose of reducing the noise levels from air movement, fan noise, etc. in the adjacent space or downstream of the duct silencer device."@en ;
  rdfs:isDefinedBy <http://pi.pauwel.be/voc/distributionelement> ;
  rdfs:label "Duct Silencer"@en ;
  rdfs:label "Kanaalgeluiddemper"@nl-nl ;
  rdfs:label "Kanalschalldämpfer"@de-de ;
  rdfs:label "Silencieux circulaire"@fr-fr ;
  rdfs:seeAlso <http://bsdd.buildingsmart.org/#concept/details/2htluultzBmQOOYxoTJ2k5> ;
  rdfs:seeAlso ifc:IfcDuctSilencer ;
  rdfs:subClassOf mep:FlowTreatmentDevice ;
.
mep:DuctSilencer-FLATOVAL
  rdf:type owl:Class ;
  rdfs:isDefinedBy <http://pi.pauwel.be/voc/distributionelement> ;
  rdfs:label "Flat Oval Duct Silencer"@en ;
  rdfs:label "flatoval"@nb-no ;
  rdfs:seeAlso <http://bsdd.buildingsmart.org/#concept/details/0VN55_f5zDDwQXiRI$8Z_y> ;
  rdfs:seeAlso ifc:IfcDuctSilencerEnumType ;
  rdfs:subClassOf mep:DuctSilencer ;
.
mep:DuctSilencer-RECTANGULAR
  rdf:type owl:Class ;
  rdfs:isDefinedBy <http://pi.pauwel.be/voc/distributionelement> ;
  rdfs:label "Rectangular Duct Silencer"@en ;
  rdfs:label "rektangulær"@nb-no ;
  rdfs:seeAlso <http://bsdd.buildingsmart.org/#concept/details/3NtvXddFX5JRlghR5mPion> ;
  rdfs:seeAlso ifc:IfcDuctSilencerEnumType ;
  rdfs:subClassOf mep:DuctSilencer ;
.
mep:DuctSilencer-ROUND
  rdf:type owl:Class ;
  rdfs:isDefinedBy <http://pi.pauwel.be/voc/distributionelement> ;
  rdfs:label "Round Duct Silencer"@en ;
  rdfs:label "sirkulær"@nb-no ;
  rdfs:seeAlso <http://bsdd.buildingsmart.org/#concept/details/0Pab9zW$v0E8Xbyt9Joo2A> ;
  rdfs:seeAlso ifc:IfcDuctSilencerEnumType ;
  rdfs:subClassOf mep:DuctSilencer ;
.
mep:ElectricAppliance
  rdf:type owl:Class ;
  rdfs:comment """A device intended for consumer usage that is powered by electricity.
May be fixed in place or able to be moved from one space to another. Requires an electrical supply that may be supplied either by an electrical circuit or provided from a local battery source."""@en ;
  rdfs:isDefinedBy <http://pi.pauwel.be/voc/distributionelement> ;
  rdfs:label "Appareil électrique"@fr-fr ;
  rdfs:label "Electric Appliance"@en ;
  rdfs:label "Elektrisches Gerät"@de-de ;
  rdfs:label "elektrisk innretning"@nb-no ;
  rdfs:seeAlso <http://bsdd.buildingsmart.org/#concept/details/3YTFM$9GvByR7HJawXiG4V> ;
  rdfs:seeAlso ifc:IfcElectricAppliance ;
  rdfs:subClassOf mep:FlowTerminal ;
.
mep:ElectricAppliance-DISHWASHER
  rdf:type owl:Class ;
  rdfs:comment "an appliance that has the primary function of washing dishes"@en ;
  rdfs:comment "an appliance that has the primary function of washing dishes"@en-gb ;
  rdfs:comment "appliance for washing dishes"@en ;
  rdfs:comment "diskmaskin"@sv-se ;
  rdfs:isDefinedBy <http://pi.pauwel.be/voc/distributionelement> ;
  rdfs:label "Dishwasher"@en ;
  rdfs:label "Geschirrspülmaschine"@de-de ;
  rdfs:label "diskmaskin"@sv-se ;
  rdfs:label "machine à laver la vaisselle"@fr-fr ;
  rdfs:label "oppvaskmaskin"@nb-no ;
  rdfs:seeAlso <http://bsdd.buildingsmart.org/#concept/details/02NUQ13z56XvvUbtiIY3SW> ;
  rdfs:seeAlso ifc:IfcElectricApplianceEnumType ;
  rdfs:subClassOf mep:ElectricAppliance ;
.
mep:ElectricAppliance-ELECTRICCOOKER
  rdf:type owl:Class ;
  rdfs:comment "an electrical appliance that has the primary function of cooking food (including oven, hob, grill)"@en ;
  rdfs:comment "an electrical appliance that has the primary function of cooking food (including oven, hob, grill)"@en-gb ;
  rdfs:isDefinedBy <http://pi.pauwel.be/voc/distributionelement> ;
  rdfs:label "Electric Cooker"@en ;
  rdfs:label "kokeplate"@nb-no ;
  rdfs:seeAlso <http://bsdd.buildingsmart.org/#concept/details/1fQUOe4mvC$PVZhL6$zYMj> ;
  rdfs:seeAlso ifc:IfcElectricApplianceEnumType ;
  rdfs:subClassOf mep:ElectricAppliance ;
.
mep:ElectricAppliance-FREESTANDINGELECTRICHEATER
  rdf:type owl:Class ;
  rdfs:isDefinedBy <http://pi.pauwel.be/voc/distributionelement> ;
  rdfs:label "Free Standing Electric Heater"@en ;
  rdfs:seeAlso <http://bsdd.buildingsmart.org/#concept/details/2vmsBMt5f6vOIJtsLV43C5> ;
  rdfs:seeAlso ifc:IfcElectricApplianceEnumType ;
  rdfs:subClassOf mep:ElectricAppliance ;
.
mep:ElectricAppliance-FREESTANDINGFAN
  rdf:type owl:Class ;
  rdfs:isDefinedBy <http://pi.pauwel.be/voc/distributionelement> ;
  rdfs:label "Free Standing Fan"@en ;
  rdfs:seeAlso <http://bsdd.buildingsmart.org/#concept/details/1sbx$V$pfE3gA1HPGomlqC> ;
  rdfs:seeAlso ifc:IfcElectricApplianceEnumType ;
  rdfs:subClassOf mep:ElectricAppliance ;
.
mep:ElectricAppliance-FREESTANDINGWATERCOOLER
  rdf:type owl:Class ;
  rdfs:isDefinedBy <http://pi.pauwel.be/voc/distributionelement> ;
  rdfs:label "Free Standing Water Cooler"@en ;
  rdfs:seeAlso <http://bsdd.buildingsmart.org/#concept/details/2GNk4XczH2a9Bo486M2Dhf> ;
  rdfs:seeAlso ifc:IfcElectricApplianceEnumType ;
  rdfs:subClassOf mep:ElectricAppliance ;
.
mep:ElectricAppliance-FREESTANDINGWATERHEATER
  rdf:type owl:Class ;
  rdfs:comment "a small, local electrical appliance for heating water. a freestanding water heater is a 'plugged' appliance whose load may be removed from an electric circuit"@en ;
  rdfs:comment "a small, local electrical appliance for heating water. a freestanding water heater is a 'plugged' appliance whose load may be removed from an electric circuit"@en-gb ;
  rdfs:isDefinedBy <http://pi.pauwel.be/voc/distributionelement> ;
  rdfs:label "Free Standing Water Heater"@en ;
  rdfs:label "varmtvannsbereder"@nb-no ;
  rdfs:seeAlso <http://bsdd.buildingsmart.org/#concept/details/0hmcm_zGD2HuO7SHEfEIAX> ;
  rdfs:seeAlso ifc:IfcElectricApplianceEnumType ;
  rdfs:subClassOf mep:ElectricAppliance ;
.
mep:ElectricAppliance-FREEZER
  rdf:type owl:Class ;
  rdfs:comment "an electrical appliance that has the primary function of storing food at temperatures below the freezing point of water"@en ;
  rdfs:comment "an electrical appliance that has the primary function of storing food at temperatures below the freezing point of water"@en-gb ;
  rdfs:isDefinedBy <http://pi.pauwel.be/voc/distributionelement> ;
  rdfs:label "Freezer"@en ;
  rdfs:label "Vrieskast"@nl-nl ;
  rdfs:label "fryser"@nb-no ;
  rdfs:seeAlso <http://bsdd.buildingsmart.org/#concept/details/2lufsAWJmHu000025QrE$V> ;
  rdfs:seeAlso ifc:IfcElectricApplianceEnumType ;
  rdfs:subClassOf mep:ElectricAppliance ;
.
mep:ElectricAppliance-FRIDGE_FREEZER
  rdf:type owl:Class ;
  rdfs:isDefinedBy <http://pi.pauwel.be/voc/distributionelement> ;
  rdfs:label "Fridge Freezer"@en ;
  rdfs:seeAlso <http://bsdd.buildingsmart.org/#concept/details/2$l6h0fcP1u9I_bcu2_2t0> ;
  rdfs:seeAlso ifc:IfcElectricApplianceEnumType ;
  rdfs:subClassOf mep:ElectricAppliance ;
.
mep:ElectricAppliance-HANDDRYER
  rdf:type owl:Class ;
  rdfs:isDefinedBy <http://pi.pauwel.be/voc/distributionelement> ;
  rdfs:label "Hand Dryer"@en ;
  rdfs:seeAlso <http://bsdd.buildingsmart.org/#concept/details/0MdGYaJi90Ugvs9F4IBH45> ;
  rdfs:seeAlso ifc:IfcElectricApplianceEnumType ;
  rdfs:subClassOf mep:ElectricAppliance ;
.
mep:ElectricAppliance-KITCHENMACHINE
  rdf:type owl:Class ;
  rdfs:comment "a specialized appliance used in commercial kitchens such as a mixer"@en ;
  rdfs:comment "a specialized appliance used in commercial kitchens such as a mixer"@en-gb ;
  rdfs:isDefinedBy <http://pi.pauwel.be/voc/distributionelement> ;
  rdfs:label "Kitchen Machine"@en ;
  rdfs:label "kjøkkenmaskin"@nb-no ;
  rdfs:seeAlso <http://bsdd.buildingsmart.org/#concept/details/3jScF9EaLB6wWXD1wgq6DV> ;
  rdfs:seeAlso ifc:IfcElectricApplianceEnumType ;
  rdfs:subClassOf mep:ElectricAppliance ;
.
mep:ElectricAppliance-MICROWAVE
  rdf:type owl:Class ;
  rdfs:comment "an electrical appliance that has the primary function of cooking food using microwaves"@en ;
  rdfs:comment "an electrical appliance that has the primary function of cooking food using microwaves"@en-gb ;
  rdfs:isDefinedBy <http://pi.pauwel.be/voc/distributionelement> ;
  rdfs:label "MicroWave"@en ;
  rdfs:label "mikrobølge"@nb-no ;
  rdfs:seeAlso <http://bsdd.buildingsmart.org/#concept/details/3aYGRc49PF4AXOOV4IRJxc> ;
  rdfs:seeAlso ifc:IfcElectricApplianceEnumType ;
  rdfs:subClassOf mep:ElectricAppliance ;
.
mep:ElectricAppliance-PHOTOCOPIER
  rdf:type owl:Class ;
  rdfs:comment "a machine that has the primary function of reproduction of printed matter"@en ;
  rdfs:comment "a machine that has the primary function of reproduction of printed matter"@en-gb ;
  rdfs:isDefinedBy <http://pi.pauwel.be/voc/distributionelement> ;
  rdfs:label "Photocopier"@en ;
  rdfs:label "kopimaskin"@nb-no ;
  rdfs:seeAlso <http://bsdd.buildingsmart.org/#concept/details/3f7QlBmRH8ixz3XB$p1vFX> ;
  rdfs:seeAlso ifc:IfcElectricApplianceEnumType ;
  rdfs:subClassOf mep:ElectricAppliance ;
.
mep:ElectricAppliance-REFRIGERATOR
  rdf:type owl:Class ;
  rdfs:isDefinedBy <http://pi.pauwel.be/voc/distributionelement> ;
  rdfs:label "Koelkast"@nl-nl ;
  rdfs:label "Refrigerator"@en ;
  rdfs:label "kjøleskap"@nb-no ;
  rdfs:seeAlso <http://bsdd.buildingsmart.org/#concept/details/2lIWS0WJmHu000025QrE$V> ;
  rdfs:seeAlso ifc:IfcElectricApplianceEnumType ;
  rdfs:subClassOf mep:ElectricAppliance ;
.
mep:ElectricAppliance-TUMBLEDRYER
  rdf:type owl:Class ;
  rdfs:isDefinedBy <http://pi.pauwel.be/voc/distributionelement> ;
  rdfs:label "Tumble Dryer"@en ;
  rdfs:label "Wäschetrockner"@de-de ;
  rdfs:label "dryer"@en ;
  rdfs:label "machine séchante"@fr-fr ;
  rdfs:label "tørketrommel"@nb-no ;
  rdfs:seeAlso <http://bsdd.buildingsmart.org/#concept/details/3vHWUCoT0Hsm00051Mm008> ;
  rdfs:seeAlso ifc:IfcElectricApplianceEnumType ;
  rdfs:subClassOf mep:ElectricAppliance ;
.
mep:ElectricAppliance-VENDINGMACHINE
  rdf:type owl:Class ;
  rdfs:isDefinedBy <http://pi.pauwel.be/voc/distributionelement> ;
  rdfs:label "Vending Machine"@en ;
  rdfs:seeAlso <http://bsdd.buildingsmart.org/#concept/details/3a1GPgbGb4HhfJfWNNnwRG> ;
  rdfs:seeAlso ifc:IfcElectricApplianceEnumType ;
  rdfs:subClassOf mep:ElectricAppliance ;
.
mep:ElectricAppliance-WASHINGMACHINE
  rdf:type owl:Class ;
  rdfs:isDefinedBy <http://pi.pauwel.be/voc/distributionelement> ;
  rdfs:label "Washing Machine"@en ;
  rdfs:seeAlso <http://bsdd.buildingsmart.org/#concept/details/3nK_JH93v5JRpo7imsOJm6> ;
  rdfs:seeAlso ifc:IfcElectricApplianceEnumType ;
  rdfs:subClassOf mep:ElectricAppliance ;
.
mep:ElectricDistributionBoard
  rdf:type owl:Class ;
  rdfs:comment "A flow controller in which instances of electrical devices are brought together at a single place for a particular purpose. A distribution provides a housing for connected electrical distribution elements so that they can be viewed, operated or acted upon from a single place. Each connected item may have its own geometric representation and location."@en ;
  rdfs:isDefinedBy <http://pi.pauwel.be/voc/distributionelement> ;
  rdfs:label "Electric Distribution Board"@en ;
  rdfs:label "Elektrischer Verteilungsregler"@de-de ;
  rdfs:label "Tableau de distribution électrique"@fr-fr ;
  rdfs:seeAlso <http://bsdd.buildingsmart.org/#concept/details/1NTXNvjYPEHAEdF4$lUOA4> ;
  rdfs:seeAlso ifc:IfcElectricDistributionBoard ;
  rdfs:subClassOf mep:FlowController ;
.
mep:ElectricDistributionBoard-CONSUMERUNIT
  rdf:type owl:Class ;
  rdfs:isDefinedBy <http://pi.pauwel.be/voc/distributionelement> ;
  rdfs:label "Consumer Unit"@en ;
  rdfs:seeAlso <http://bsdd.buildingsmart.org/#concept/details/02vRNiXL17Ng6A0tyY3IZm> ;
  rdfs:seeAlso ifc:IfcElectricDistributionBoardEnumType ;
  rdfs:subClassOf mep:ElectricDistributionBoard ;
.
mep:ElectricDistributionBoard-DISTRIBUTIONBOARD
  rdf:type owl:Class ;
  rdfs:isDefinedBy <http://pi.pauwel.be/voc/distributionelement> ;
  rdfs:label "Distribution Board"@en ;
  rdfs:seeAlso <http://bsdd.buildingsmart.org/#concept/details/2t_kmsr_9FbOzG08gdq5sn> ;
  rdfs:seeAlso ifc:IfcElectricDistributionBoardEnumType ;
  rdfs:subClassOf mep:ElectricDistributionBoard ;
.
mep:ElectricDistributionBoard-MOTORCONTROLCENTRE
  rdf:type owl:Class ;
  rdfs:isDefinedBy <http://pi.pauwel.be/voc/distributionelement> ;
  rdfs:label "Motor Control Centre"@en ;
  rdfs:seeAlso <http://bsdd.buildingsmart.org/#concept/details/23gvwO2$16qPz5TGUDljzB> ;
  rdfs:seeAlso ifc:IfcElectricDistributionBoardEnumType ;
  rdfs:subClassOf mep:ElectricDistributionBoard ;
.
mep:ElectricDistributionBoard-SWITCHBOARD
  rdf:type owl:Class ;
  rdfs:isDefinedBy <http://pi.pauwel.be/voc/distributionelement> ;
  rdfs:label "Switch Board"@en ;
  rdfs:seeAlso <http://bsdd.buildingsmart.org/#concept/details/3XP0I3Joj7y8AYq9ASPean> ;
  rdfs:seeAlso ifc:IfcElectricDistributionBoardEnumType ;
  rdfs:subClassOf mep:ElectricDistributionBoard ;
.
mep:ElectricFlowStorageDevice
  rdf:type owl:Class ;
  rdfs:comment "A device in which electrical energy is stored and from which energy may be progressively released."@en ;
  rdfs:isDefinedBy <http://pi.pauwel.be/voc/distributionelement> ;
  rdfs:label "Electric Flow Storage Device"@en ;
  rdfs:label "Elektrisches Speichergerät"@de-de ;
  rdfs:label "strømlagringsenhet"@nb-no ;
  rdfs:seeAlso <http://bsdd.buildingsmart.org/#concept/details/1QtwhR5Zn328NFUBlGt0yh> ;
  rdfs:seeAlso ifc:IfcElectricFlowStorageDevice ;
  rdfs:subClassOf mep:FlowStorageDevice ;
.
mep:ElectricFlowStorageDevice-BATTERY
  rdf:type owl:Class ;
  rdfs:comment "a device for storing energy in chemical form so that it can be released as electrical energy"@en ;
  rdfs:comment "a device for storing energy in chemical form so that it can be released as electrical energy"@en-gb ;
  rdfs:isDefinedBy <http://pi.pauwel.be/voc/distributionelement> ;
  rdfs:label "Battery"@en ;
  rdfs:label "batteri"@nb-no ;
  rdfs:seeAlso <http://bsdd.buildingsmart.org/#concept/details/2SgW4DbB93yuwE75nOI9iX> ;
  rdfs:seeAlso ifc:IfcElectricFlowStorageDeviceEnumType ;
  rdfs:subClassOf mep:ElectricFlowStorageDevice ;
.
mep:ElectricFlowStorageDevice-CAPACITORBANK
  rdf:type owl:Class ;
  rdfs:comment "a device that stores electrical energy when an external power supply is present using the electrical property of capacitance"@en ;
  rdfs:comment "a device that stores electrical energy when an external power supply is present using the electrical property of capacitance"@en-gb ;
  rdfs:isDefinedBy <http://pi.pauwel.be/voc/distributionelement> ;
  rdfs:label "Capacitor Bank"@en ;
  rdfs:label "kapasitetsbank"@nb-no ;
  rdfs:seeAlso <http://bsdd.buildingsmart.org/#concept/details/3T$uPXx997$B5skfKbEgBk> ;
  rdfs:seeAlso ifc:IfcElectricFlowStorageDeviceEnumType ;
  rdfs:subClassOf mep:ElectricFlowStorageDevice ;
.
mep:ElectricFlowStorageDevice-HARMONICFILTER
  rdf:type owl:Class ;
  rdfs:isDefinedBy <http://pi.pauwel.be/voc/distributionelement> ;
  rdfs:label "Harmonic Filter"@en ;
  rdfs:seeAlso <http://bsdd.buildingsmart.org/#concept/details/3CCGbA$dfCHxGIK0Zz2C08> ;
  rdfs:seeAlso ifc:IfcElectricFlowStorageDeviceEnumType ;
  rdfs:subClassOf mep:ElectricFlowStorageDevice ;
.
mep:ElectricFlowStorageDevice-INDUCTORBANK
  rdf:type owl:Class ;
  rdfs:isDefinedBy <http://pi.pauwel.be/voc/distributionelement> ;
  rdfs:label "Inductor Bank"@en ;
  rdfs:seeAlso <http://bsdd.buildingsmart.org/#concept/details/0s_ACAnfD8YAPin0isHx0d> ;
  rdfs:seeAlso ifc:IfcElectricFlowStorageDeviceEnumType ;
  rdfs:subClassOf mep:ElectricFlowStorageDevice ;
.
mep:ElectricFlowStorageDevice-UPS
  rdf:type owl:Class ;
  rdfs:comment "a device that provides a time limited alternative source of power supply in the event of failure of the main supply"@en ;
  rdfs:comment "a device that provides a time limited alternative source of power supply in the event of failure of the main supply"@en-gb ;
  rdfs:comment "combination of convertors, switches and energy storage devices (for example batteries), constituting a power system for maintaining continuity of load power in case of input power failure."@en ;
  rdfs:isDefinedBy <http://pi.pauwel.be/voc/distributionelement> ;
  rdfs:label "UPS"@en ;
  rdfs:label "UPS"@nb-no ;
  rdfs:label "uninterruptible power supply"@en ;
  rdfs:label "uninterruptible power system"@en ;
  rdfs:seeAlso <http://bsdd.buildingsmart.org/#concept/details/1ru5tvtfLE7g$pBOrRs6g$> ;
  rdfs:seeAlso ifc:IfcElectricFlowStorageDeviceEnumType ;
  rdfs:subClassOf mep:ElectricFlowStorageDevice ;
.
mep:ElectricGenerator
  rdf:type owl:Class ;
  rdfs:comment "An engine that is a machine for converting mechanical energy into electrical energy."@en ;
  rdfs:isDefinedBy <http://pi.pauwel.be/voc/distributionelement> ;
  rdfs:label "Electric Generator"@en ;
  rdfs:label "Elektrogenerator"@de-de ;
  rdfs:label "elektrogenerator"@nb-no ;
  rdfs:label "générateur électrique"@fr-fr ;
  rdfs:seeAlso <http://bsdd.buildingsmart.org/#concept/details/1xmminhSL6bhcxZRNY$u6Z> ;
  rdfs:seeAlso ifc:IfcElectricGenerator ;
  rdfs:subClassOf mep:EnergyConversionDevice ;
.
mep:ElectricGenerator-CHP
  rdf:type owl:Class ;
  rdfs:comment "combined heat and power supply, used not only as a source of electric energy but also as a heating source for the building. it may therefore be not only part of an electrical system but also of a heating system"@en ;
  rdfs:comment "combined heat and power supply, used not only as a source of electric energy but also as a heating source for the building. it may therefore be not only part of an electrical system but also of a heating system"@en-gb ;
  rdfs:isDefinedBy <http://pi.pauwel.be/voc/distributionelement> ;
  rdfs:label "CHP"@en ;
  rdfs:label "kraftvarmeverk"@nb-no ;
  rdfs:seeAlso <http://bsdd.buildingsmart.org/#concept/details/2vNA8q44vBZRsy_n0gsv2T> ;
  rdfs:seeAlso ifc:IfcElectricGeneratorEnumType ;
  rdfs:subClassOf mep:ElectricGenerator ;
.
mep:ElectricGenerator-ENGINEGENERATOR
  rdf:type owl:Class ;
  rdfs:comment "electrical generator with a fuel-driven engine, for example a diesel-driven emergency power supply"@en ;
  rdfs:comment "electrical generator with a fuel-driven engine, for example a diesel-driven emergency power supply"@en-gb ;
  rdfs:isDefinedBy <http://pi.pauwel.be/voc/distributionelement> ;
  rdfs:label "Engine Generator"@en ;
  rdfs:label "motorgenerator"@nb-no ;
  rdfs:seeAlso <http://bsdd.buildingsmart.org/#concept/details/1cgIU0HJT6GuV3i$OWzcqr> ;
  rdfs:seeAlso ifc:IfcElectricGeneratorEnumType ;
  rdfs:subClassOf mep:ElectricGenerator ;
.
mep:ElectricGenerator-STANDALONE
  rdf:type owl:Class ;
  rdfs:comment "electrical generator which does not include its source of kinetic energy, that is, a motor, engine, or turbine are all modeled separately"@en ;
  rdfs:comment "electrical generator which does not include its source of kinetic energy, that is, a motor, engine, or turbine are all modeled separately"@en-gb ;
  rdfs:isDefinedBy <http://pi.pauwel.be/voc/distributionelement> ;
  rdfs:label "Standalone Generator"@en ;
  rdfs:label "frittstående"@nb-no ;
  rdfs:seeAlso <http://bsdd.buildingsmart.org/#concept/details/385E6cNGD9CAcjlAWZNrUW> ;
  rdfs:seeAlso ifc:IfcElectricGeneratorEnumType ;
  rdfs:subClassOf mep:ElectricGenerator ;
.
mep:ElectricMotor
  rdf:type owl:Class ;
  rdfs:comment "An engine that is a machine for converting electrical energy into mechanical energy."@en ;
  rdfs:isDefinedBy <http://pi.pauwel.be/voc/distributionelement> ;
  rdfs:label "Electric Motor"@en ;
  rdfs:label "Elektromotor"@de-de ;
  rdfs:label "Moteur électrique"@fr-fr ;
  rdfs:label "elektrisk motor"@nb-no ;
  rdfs:label "elektromotor"@nl-nl ;
  rdfs:seeAlso <http://bsdd.buildingsmart.org/#concept/details/3_kLW3eI10Xem4Z9zSCTzp> ;
  rdfs:seeAlso ifc:IfcElectricMotor ;
  rdfs:subClassOf mep:EnergyConversionDevice ;
.
mep:ElectricMotor-DC
  rdf:type owl:Class ;
  rdfs:comment "a motor using either generated or rectified Direct Current (DC) power"@en ;
  rdfs:comment "a motor using either generated or rectified Direct Current (DC) power"@en-gb ;
  rdfs:isDefinedBy <http://pi.pauwel.be/voc/distributionelement> ;
  rdfs:label "DC - motor"@nb-no ;
  rdfs:label "DC-motor"@en ;
  rdfs:seeAlso <http://bsdd.buildingsmart.org/#concept/details/3FK3hjao1DDw14M1qybLxa> ;
  rdfs:seeAlso ifc:IfcElectricMotorEnumType ;
  rdfs:subClassOf mep:ElectricMotor ;
.
mep:ElectricMotor-INDUCTION
  rdf:type owl:Class ;
  rdfs:comment "an alternating current motor in which the primary winding on one member (usually the stator) is connected to the power source and a secondary winding or a squirrel-cage secondary winding on the other member (usually the rotor) carries the induced current. there is no physical electrical connection to the secondary winding, its current is induced"@en ;
  rdfs:comment "an alternating current motor in which the primary winding on one member (usually the stator) is connected to the power source and a secondary winding or a squirrel-cage secondary winding on the other member (usually the rotor) carries the induced current. there is no physical electrical connection to the secondary winding, its current is induced"@en-gb ;
  rdfs:isDefinedBy <http://pi.pauwel.be/voc/distributionelement> ;
  rdfs:label "Induction Motor"@en ;
  rdfs:label "induksjon"@nb-no ;
  rdfs:seeAlso <http://bsdd.buildingsmart.org/#concept/details/3OYMbkndX6lxYQ5WInnHhX> ;
  rdfs:seeAlso ifc:IfcElectricMotorEnumType ;
  rdfs:subClassOf mep:ElectricMotor ;
.
mep:ElectricMotor-POLYPHASE
  rdf:type owl:Class ;
  rdfs:comment "a two or three-phase induction motor in which the windings, one for each phase, are evenly divided by the same number of electrical degrees"@en ;
  rdfs:comment "a two or three-phase induction motor in which the windings, one for each phase, are evenly divided by the same number of electrical degrees"@en-gb ;
  rdfs:isDefinedBy <http://pi.pauwel.be/voc/distributionelement> ;
  rdfs:label "Polyphase Motor"@en ;
  rdfs:label "flerfasmotor"@nb-no ;
  rdfs:seeAlso <http://bsdd.buildingsmart.org/#concept/details/1US3A1hwXBIA9FaVqUl3HY> ;
  rdfs:seeAlso ifc:IfcElectricMotorEnumType ;
  rdfs:subClassOf mep:ElectricMotor ;
.
mep:ElectricMotor-RELUCTANCESYNCHRONOUS
  rdf:type owl:Class ;
  rdfs:isDefinedBy <http://pi.pauwel.be/voc/distributionelement> ;
  rdfs:label "Reluctance Synchronous Motor"@en ;
  rdfs:seeAlso <http://bsdd.buildingsmart.org/#concept/details/2lD9V5iynEBB3XgItdjfos> ;
  rdfs:seeAlso ifc:IfcElectricMotorEnumType ;
  rdfs:subClassOf mep:ElectricMotor ;
.
mep:ElectricMotor-SYNCHRONOUS
  rdf:type owl:Class ;
  rdfs:comment "a motor that operates at a constant speed up to full load. the rotor speed is equal to the speed of the rotating magnetic field of the stator; there is no slip"@en ;
  rdfs:comment "a motor that operates at a constant speed up to full load. the rotor speed is equal to the speed of the rotating magnetic field of the stator; there is no slip"@en-gb ;
  rdfs:isDefinedBy <http://pi.pauwel.be/voc/distributionelement> ;
  rdfs:label "Synchronous Motor"@en ;
  rdfs:label "synkromotor"@nb-no ;
  rdfs:seeAlso <http://bsdd.buildingsmart.org/#concept/details/3aYFsz0Ij95vr3j85mOzlh> ;
  rdfs:seeAlso ifc:IfcElectricMotorEnumType ;
  rdfs:subClassOf mep:ElectricMotor ;
.
mep:ElectricTimeControl
  rdf:type owl:Class ;
  rdfs:comment "A device that applies control to the provision or flow of electrical energy over time."@en ;
  rdfs:isDefinedBy <http://pi.pauwel.be/voc/distributionelement> ;
  rdfs:label "Electric Time Control"@en ;
  rdfs:label "Elektrische Zeitsteuerung"@de-de ;
  rdfs:label "elektronisk tidskontroll"@nb-no ;
  rdfs:seeAlso <http://bsdd.buildingsmart.org/#concept/details/34zeeiRU160PRfc1BOv2UT> ;
  rdfs:seeAlso ifc:IfcElectricTimeControl ;
  rdfs:subClassOf mep:FlowController ;
.
mep:ElectricTimeControl-RELAY
  rdf:type owl:Class ;
  rdfs:comment "electromagnetically operated contactor for making or breaking a control circuit"@en ;
  rdfs:comment "electromagnetically operated contactor for making or breaking a control circuit"@en-gb ;
  rdfs:isDefinedBy <http://pi.pauwel.be/voc/distributionelement> ;
  rdfs:label "Relay"@en ;
  rdfs:label "relais"@fr-fr ;
  rdfs:label "relè"@nb-no ;
  rdfs:label "relé"@nb-no ;
  rdfs:seeAlso <http://bsdd.buildingsmart.org/#concept/details/1uMPSl_pL5eufzS8GVHHU$> ;
  rdfs:seeAlso ifc:IfcElectricTimeControlEnumType ;
  rdfs:subClassOf mep:ElectricTimeControl ;
.
mep:ElectricTimeControl-TIMECLOCK
  rdf:type owl:Class ;
  rdfs:isDefinedBy <http://pi.pauwel.be/voc/distributionelement> ;
  rdfs:label "Time Clock"@en ;
  rdfs:seeAlso <http://bsdd.buildingsmart.org/#concept/details/3_BiobHgL589mZt5gGZ6vc> ;
  rdfs:seeAlso ifc:IfcElectricTimeControlEnumType ;
  rdfs:subClassOf mep:ElectricTimeControl ;
.
mep:ElectricTimeControl-TIMEDELAY
  rdf:type owl:Class ;
  rdfs:isDefinedBy <http://pi.pauwel.be/voc/distributionelement> ;
  rdfs:label "Time Delay"@en ;
  rdfs:seeAlso <http://bsdd.buildingsmart.org/#concept/details/1frllCTITFVANbn$YJ11RW> ;
  rdfs:seeAlso ifc:IfcElectricTimeControlEnumType ;
  rdfs:subClassOf mep:ElectricTimeControl ;
.
mep:EnergyConversionDevice
  rdf:type owl:Class ;
  rdfs:comment "the distribution flow element ifcenergyconversiondevice defines the occurrence of a device used to perform energy conversion or heat transfer and typically participates in a flow distribution system. its type is defined by ifcenergyconversiondevicetype or its subtypes."@en ;
  rdfs:isDefinedBy <http://pi.pauwel.be/voc/distributionelement> ;
  rdfs:label "Energiewandler"@de-de ;
  rdfs:label "Energy Conversion Device"@en ;
  rdfs:label "aggregat frys"@nb-no ;
  rdfs:label "aggregat kjøl virksomhet"@nb-no ;
  rdfs:label "aggregate freezer"@en ;
  rdfs:label "aggregate refrigirator industry"@en ;
  rdfs:label "dispositif de conversion d'énergie"@fr-fr ;
  rdfs:label "kjøleaggregat"@nb-no ;
  rdfs:seeAlso <http://bsdd.buildingsmart.org/#concept/details/1VQ1GZZDD2pvhjZ8ZKtCoL> ;
  rdfs:seeAlso ifc:IfcEnergyConversionDevice ;
  rdfs:subClassOf mep:DistributionFlowElement ;
.
mep:Engine
  rdf:type owl:Class ;
  rdfs:comment "A device that converts fuel into mechanical energy through combustion."@en ;
  rdfs:isDefinedBy <http://pi.pauwel.be/voc/distributionelement> ;
  rdfs:label "Engine"@en ;
  rdfs:label "Moteur"@fr-fr ;
  rdfs:label "Motor"@de-de ;
  rdfs:label "motor"@nb-no ;
  rdfs:seeAlso <http://bsdd.buildingsmart.org/#concept/details/2Z1mXqriH13epQNHSH0Q6U> ;
  rdfs:seeAlso ifc:IfcEngine ;
  rdfs:subClassOf mep:EnergyConversionDevice ;
.
mep:Engine-EXTERNALCOMBUSTION
  rdf:type owl:Class ;
  rdfs:comment "combustion is external"@en ;
  rdfs:comment "combustion is external"@en-gb ;
  rdfs:isDefinedBy <http://pi.pauwel.be/voc/distributionelement> ;
  rdfs:label "External Combustion Engine"@en ;
  rdfs:label "utvendig forbrenning"@nb-no ;
  rdfs:seeAlso <http://bsdd.buildingsmart.org/#concept/details/2NLKuMKf91wviDc2F5qWzU> ;
  rdfs:seeAlso ifc:IfcEngineEnumType ;
  rdfs:subClassOf mep:Engine ;
.
mep:Engine-INTERNALCOMBUSTION
  rdf:type owl:Class ;
  rdfs:comment "combustion is internal"@en ;
  rdfs:comment "combustion is internal"@en-gb ;
  rdfs:isDefinedBy <http://pi.pauwel.be/voc/distributionelement> ;
  rdfs:label "Internal Combustion Engine"@en ;
  rdfs:label "forbrenningsmotor"@nb-no ;
  rdfs:seeAlso <http://bsdd.buildingsmart.org/#concept/details/2Tx86TGHX9mfF61hssJ$wH> ;
  rdfs:seeAlso ifc:IfcEngineEnumType ;
  rdfs:subClassOf mep:Engine ;
.
mep:EvaporativeCooler
  rdf:type owl:Class ;
  rdfs:comment "A device that cools air by saturating it with water vapor."@en ;
  rdfs:isDefinedBy <http://pi.pauwel.be/voc/distributionelement> ;
  rdfs:label "Evaporative Cooler"@en ;
  rdfs:label "Refroidisseur évaporatif"@fr-fr ;
  rdfs:label "Verdunstungskühler"@de-de ;
  rdfs:label "fordampningskjøler"@nb-no ;
  rdfs:label "verdampingskoeler"@nl-nl ;
  rdfs:seeAlso <http://bsdd.buildingsmart.org/#concept/details/3q9N4QJHXEvB$P7TiIBB3x> ;
  rdfs:seeAlso ifc:IfcEvaporativeCooler ;
  rdfs:subClassOf mep:EnergyConversionDevice ;
.
mep:EvaporativeCooler-DIRECTEVAPORATIVEAIRWASHER
  rdf:type owl:Class ;
  rdfs:isDefinedBy <http://pi.pauwel.be/voc/distributionelement> ;
  rdfs:label "Direct Evaporative Air Washer"@en ;
  rdfs:label "direkte luftfukter - luftvasker"@nb-no ;
  rdfs:seeAlso <http://bsdd.buildingsmart.org/#concept/details/1mfNeZzsr75wDjPDHJlb4H> ;
  rdfs:seeAlso ifc:IfcEvaporativeCoolerEnumType ;
  rdfs:subClassOf mep:EvaporativeCooler ;
.
mep:EvaporativeCooler-DIRECTEVAPORATIVEPACKAGEDROTARYAIRCOOLER
  rdf:type owl:Class ;
  rdfs:isDefinedBy <http://pi.pauwel.be/voc/distributionelement> ;
  rdfs:label "Direct Evaporative Packaged Rotary Air Cooler"@en ;
  rdfs:seeAlso <http://bsdd.buildingsmart.org/#concept/details/1cj7p5WhDB_xBonDIVd_4z> ;
  rdfs:seeAlso ifc:IfcEvaporativeCoolerEnumType ;
  rdfs:subClassOf mep:EvaporativeCooler ;
.
mep:EvaporativeCooler-DIRECTEVAPORATIVERANDOMMEDIAAIRCOOLER
  rdf:type owl:Class ;
  rdfs:isDefinedBy <http://pi.pauwel.be/voc/distributionelement> ;
  rdfs:label "Direct Evaporative Random Media Air Cooler"@en ;
  rdfs:seeAlso <http://bsdd.buildingsmart.org/#concept/details/0UORhKPhjCL85YKa2Bnb3r> ;
  rdfs:seeAlso ifc:IfcEvaporativeCoolerEnumType ;
  rdfs:subClassOf mep:EvaporativeCooler ;
.
mep:EvaporativeCooler-DIRECTEVAPORATIVERIGIDMEDIAAIRCOOLER
  rdf:type owl:Class ;
  rdfs:isDefinedBy <http://pi.pauwel.be/voc/distributionelement> ;
  rdfs:label "Direct Evaporative Rigid Media Air Cooler"@en ;
  rdfs:seeAlso <http://bsdd.buildingsmart.org/#concept/details/0MWgqKd0z5GPNm6aaAnj5C> ;
  rdfs:seeAlso ifc:IfcEvaporativeCoolerEnumType ;
  rdfs:subClassOf mep:EvaporativeCooler ;
.
mep:EvaporativeCooler-DIRECTEVAPORATIVESLINGERSPACKAGEDAIRCOOLER
  rdf:type owl:Class ;
  rdfs:isDefinedBy <http://pi.pauwel.be/voc/distributionelement> ;
  rdfs:label "Direct Evaporative Slingers Packaged Air Cooler"@en ;
  rdfs:seeAlso <http://bsdd.buildingsmart.org/#concept/details/16b3LdCezBDPr$dY5Jspfu> ;
  rdfs:seeAlso ifc:IfcEvaporativeCoolerEnumType ;
  rdfs:subClassOf mep:EvaporativeCooler ;
.
mep:EvaporativeCooler-INDIRECTDIRECTCOMBINATION
  rdf:type owl:Class ;
  rdfs:isDefinedBy <http://pi.pauwel.be/voc/distributionelement> ;
  rdfs:label "Indirect Direct Combination"@en ;
  rdfs:label "kombinasjonskjøler"@nb-no ;
  rdfs:seeAlso <http://bsdd.buildingsmart.org/#concept/details/0m3PNQ2HLCZxrflh7tIhW4> ;
  rdfs:seeAlso ifc:IfcEvaporativeCoolerEnumType ;
  rdfs:subClassOf mep:EvaporativeCooler ;
.
mep:EvaporativeCooler-INDIRECTEVAPORATIVECOOLINGTOWERORCOILCOOLER
  rdf:type owl:Class ;
  rdfs:isDefinedBy <http://pi.pauwel.be/voc/distributionelement> ;
  rdfs:label "Indirect Evaporative Cooling Tower Or Coil Cooler"@en ;
  rdfs:label "indirekte damp kjøletårn"@nb-no ;
  rdfs:seeAlso <http://bsdd.buildingsmart.org/#concept/details/2NrTpcYUv9zg$5$$fO_19L> ;
  rdfs:seeAlso ifc:IfcEvaporativeCoolerEnumType ;
  rdfs:subClassOf mep:EvaporativeCooler ;
.
mep:EvaporativeCooler-INDIRECTEVAPORATIVEPACKAGEAIRCOOLER
  rdf:type owl:Class ;
  rdfs:isDefinedBy <http://pi.pauwel.be/voc/distributionelement> ;
  rdfs:label "Indirect Evaporative Package Air Cooler"@en ;
  rdfs:label "indirekte dampkjøler"@nb-no ;
  rdfs:seeAlso <http://bsdd.buildingsmart.org/#concept/details/0jmwDswxz4_AQl2__GUqUv> ;
  rdfs:seeAlso ifc:IfcEvaporativeCoolerEnumType ;
  rdfs:subClassOf mep:EvaporativeCooler ;
.
mep:EvaporativeCooler-INDIRECTEVAPORATIVEWETCOIL
  rdf:type owl:Class ;
  rdfs:isDefinedBy <http://pi.pauwel.be/voc/distributionelement> ;
  rdfs:label "Indirect Evaporative Wet Coil"@en ;
  rdfs:label "indirekte damp coil"@nb-no ;
  rdfs:seeAlso <http://bsdd.buildingsmart.org/#concept/details/1LV$DC3_H2PQ4WPTuDrKrT> ;
  rdfs:seeAlso ifc:IfcEvaporativeCoolerEnumType ;
  rdfs:subClassOf mep:EvaporativeCooler ;
.
mep:Evaporator
  rdf:type owl:Class ;
  rdfs:comment "A liquid refrigerant is vaporized and absorbs heat from the surrounding fluid."@en ;
  rdfs:comment "In heat transfer systems, a evaporator is a device used to turn a liquid into its gaseous form"@en ;
  rdfs:isDefinedBy <http://pi.pauwel.be/voc/distributionelement> ;
  rdfs:label "Evaporateur"@fr-fr ;
  rdfs:label "Evaporator"@en ;
  rdfs:label "kjøleelement"@nb-no ;
  rdfs:label "luftfukter"@nb-no ;
  rdfs:label "verdamper"@nl-nl ;
  rdfs:label "verdampfer"@de-de ;
  rdfs:label "évaporateur"@fr-fr ;
  rdfs:seeAlso <http://bsdd.buildingsmart.org/#concept/details/1b85u16kXAuQVMX36yZmUh> ;
  rdfs:seeAlso ifc:IfcEvaporator ;
  rdfs:subClassOf mep:EnergyConversionDevice ;
.
mep:Evaporator-DIRECTEXPANSION
  rdf:type owl:Class ;
  rdfs:isDefinedBy <http://pi.pauwel.be/voc/distributionelement> ;
  rdfs:label "Direct Expansion"@en ;
  rdfs:label "direkte ekspansjon"@nb-no ;
  rdfs:seeAlso <http://bsdd.buildingsmart.org/#concept/details/09VTDOubL8rQM9Zzgh3ZOX> ;
  rdfs:seeAlso ifc:IfcEvaporatorEnumType ;
  rdfs:subClassOf mep:Evaporator ;
.
mep:Evaporator-DIRECTEXPANSIONBRAZEDPLATE
  rdf:type owl:Class ;
  rdfs:isDefinedBy <http://pi.pauwel.be/voc/distributionelement> ;
  rdfs:label "Direct Expansion Brazed Plate"@en ;
  rdfs:label "direkte ekspansjon loddeplate"@nb-no ;
  rdfs:seeAlso <http://bsdd.buildingsmart.org/#concept/details/1T3UjVbrn8GRRfXuXNLYnr> ;
  rdfs:seeAlso ifc:IfcEvaporatorEnumType ;
  rdfs:subClassOf mep:Evaporator ;
.
mep:Evaporator-DIRECTEXPANSIONSHELLANDTUBE
  rdf:type owl:Class ;
  rdfs:isDefinedBy <http://pi.pauwel.be/voc/distributionelement> ;
  rdfs:label "Direct Expansion Shell And Tube"@en ;
  rdfs:label "direkte ekspansjon rette rør"@nb-no ;
  rdfs:seeAlso <http://bsdd.buildingsmart.org/#concept/details/1u9oqdehL1dgBJ6OLyn3QA> ;
  rdfs:seeAlso ifc:IfcEvaporatorEnumType ;
  rdfs:subClassOf mep:Evaporator ;
.
mep:Evaporator-DIRECTEXPANSIONTUBEINTUBE
  rdf:type owl:Class ;
  rdfs:isDefinedBy <http://pi.pauwel.be/voc/distributionelement> ;
  rdfs:label "Direct Expansion Tube In Tube"@en ;
  rdfs:label "direkte ekspansjon rør-i-rør"@nb-no ;
  rdfs:seeAlso <http://bsdd.buildingsmart.org/#concept/details/3sib_FFsX9OPAtp2_avAxn> ;
  rdfs:seeAlso ifc:IfcEvaporatorEnumType ;
  rdfs:subClassOf mep:Evaporator ;
.
mep:Evaporator-FLOODEDSHELLANDTUBE
  rdf:type owl:Class ;
  rdfs:isDefinedBy <http://pi.pauwel.be/voc/distributionelement> ;
  rdfs:label "Flooded Shell And Tube"@en ;
  rdfs:seeAlso <http://bsdd.buildingsmart.org/#concept/details/0ccrsyQl54TBm8fRTQgQ74> ;
  rdfs:seeAlso ifc:IfcEvaporatorEnumType ;
  rdfs:subClassOf mep:Evaporator ;
.
mep:Evaporator-SHELLANDCOIL
  rdf:type owl:Class ;
  rdfs:isDefinedBy <http://pi.pauwel.be/voc/distributionelement> ;
  rdfs:label "Shell And Coil"@en ;
  rdfs:seeAlso <http://bsdd.buildingsmart.org/#concept/details/30V2jCzRrB$APJOlZf7jhx> ;
  rdfs:seeAlso ifc:IfcEvaporatorEnumType ;
  rdfs:subClassOf mep:Evaporator ;
.
mep:Fan
  rdf:type owl:Class ;
  rdfs:comment "A device which imparts mechanical work on a gas. A typical usage of a fan is to induce airflow in a building services air distribution system."@en ;
  rdfs:comment "A machine for the movement of air that has a rotating impeller, often for cooling."@en ;
  rdfs:comment "An artefact which delivers or exhausts volumes of air or gas at low differential pressure.       "@en ;
  rdfs:comment "funksjonsdel for bevegelse av luft med roterende element, ofte brukt til kjøling."@nb-no ;
  rdfs:isDefinedBy <http://pi.pauwel.be/voc/distributionelement> ;
  rdfs:label "Fan"@en ;
  rdfs:label "Ventilator"@de-de ;
  rdfs:label "ventilateur"@fr-fr ;
  rdfs:label "vifte"@nb-no ;
  rdfs:seeAlso <http://bsdd.buildingsmart.org/#concept/details/1ugSc0qUCHuO00025QrE$V> ;
  rdfs:seeAlso ifc:IfcFan ;
  rdfs:subClassOf mep:FlowMovingDevice ;
.
mep:Fan-CENTRIFUGALAIRFOIL
  rdf:type owl:Class ;
  rdfs:isDefinedBy <http://pi.pauwel.be/voc/distributionelement> ;
  rdfs:label "Centrifugal Air Foil"@en ;
  rdfs:seeAlso <http://bsdd.buildingsmart.org/#concept/details/2b2DdpoeD2DebGtqb8$WWB> ;
  rdfs:seeAlso ifc:IfcFanEnumType ;
  rdfs:subClassOf mep:Fan ;
.
mep:Fan-CENTRIFUGALBACKWARDINCLINEDCURVED
  rdf:type owl:Class ;
  rdfs:isDefinedBy <http://pi.pauwel.be/voc/distributionelement> ;
  rdfs:label "Centrifugal Backward Inclined Curved Fan"@en ;
  rdfs:seeAlso <http://bsdd.buildingsmart.org/#concept/details/2947TJClP4iRuoq1E3mkRW> ;
  rdfs:seeAlso ifc:IfcFanEnumType ;
  rdfs:subClassOf mep:Fan ;
.
mep:Fan-CENTRIFUGALFORWARDCURVED
  rdf:type owl:Class ;
  rdfs:isDefinedBy <http://pi.pauwel.be/voc/distributionelement> ;
  rdfs:label "Centrifugal Forward Curved Fan"@en ;
  rdfs:seeAlso <http://bsdd.buildingsmart.org/#concept/details/2BtF98qKP9pAJgsmJrKTcX> ;
  rdfs:seeAlso ifc:IfcFanEnumType ;
  rdfs:subClassOf mep:Fan ;
.
mep:Fan-CENTRIFUGALRADIAL
  rdf:type owl:Class ;
  rdfs:isDefinedBy <http://pi.pauwel.be/voc/distributionelement> ;
  rdfs:label "Centrifugal Radial Fan"@en ;
  rdfs:seeAlso <http://bsdd.buildingsmart.org/#concept/details/3ZTCLrBaz0NwkdZhJ1jzAB> ;
  rdfs:seeAlso ifc:IfcFanEnumType ;
  rdfs:subClassOf mep:Fan ;
.
mep:Fan-PROPELLORAXIAL
  rdf:type owl:Class ;
  rdfs:isDefinedBy <http://pi.pauwel.be/voc/distributionelement> ;
  rdfs:label "Propellor Axial Fan"@en ;
  rdfs:seeAlso <http://bsdd.buildingsmart.org/#concept/details/0B7IEewCf7DPbZs58QORZ_> ;
  rdfs:seeAlso ifc:IfcFanEnumType ;
  rdfs:subClassOf mep:Fan ;
.
mep:Fan-TUBEAXIAL
  rdf:type owl:Class ;
  rdfs:comment "air flows through the impeller axially with reduced tip clearance and operating at higher tip speeds"@en ;
  rdfs:isDefinedBy <http://pi.pauwel.be/voc/distributionelement> ;
  rdfs:label "Tube Axial Fan"@en ;
  rdfs:label "tube aksialvifte"@nb-no ;
  rdfs:seeAlso <http://bsdd.buildingsmart.org/#concept/details/0uYC2U15n0ggOtHNsP3kmN> ;
  rdfs:seeAlso ifc:IfcFanEnumType ;
  rdfs:subClassOf mep:Fan ;
.
mep:Fan-VANEAXIAL
  rdf:type owl:Class ;
  rdfs:comment "air flows through the impeller axially with guide vanes and reduced running blade tip clearance"@en ;
  rdfs:comment "air flows through the impeller axially with guide vanes and reduced running blade tip clearance"@en-gb ;
  rdfs:isDefinedBy <http://pi.pauwel.be/voc/distributionelement> ;
  rdfs:label "Vane Axial Fan"@en ;
  rdfs:label "lamellaksial vifte"@nb-no ;
  rdfs:seeAlso <http://bsdd.buildingsmart.org/#concept/details/2W_hdCD6D3DPaj$HRNjU0Z> ;
  rdfs:seeAlso ifc:IfcFanEnumType ;
  rdfs:subClassOf mep:Fan ;
.
mep:Filter
  rdf:type owl:Class ;
  rdfs:comment "An apparatus used to remove particulate or gaseous matter from fluids and gases"@en ;
  rdfs:isDefinedBy <http://pi.pauwel.be/voc/distributionelement> ;
  rdfs:label "Filter"@en ;
  rdfs:label "filtre"@fr-fr ;
  rdfs:seeAlso <http://bsdd.buildingsmart.org/#concept/details/07moCBVkH3OhoQDperZAGA> ;
  rdfs:seeAlso ifc:IfcFilter ;
  rdfs:subClassOf mep:FlowTreatmentDevice ;
.
mep:Filter-AIRPARTICLEFILTER
  rdf:type owl:Class ;
  rdfs:isDefinedBy <http://pi.pauwel.be/voc/distributionelement> ;
  rdfs:label "Air Particle Filter"@en ;
  rdfs:label "støvutskiller (filter)"@nb-no ;
  rdfs:seeAlso <http://bsdd.buildingsmart.org/#concept/details/2ha4cuVrn2CO6DtVG5m_2l> ;
  rdfs:seeAlso ifc:IfcFilterEnumType ;
  rdfs:subClassOf mep:Filter ;
.
mep:Filter-COMPRESSEDAIRFILTER
  rdf:type owl:Class ;
  rdfs:isDefinedBy <http://pi.pauwel.be/voc/distributionelement> ;
  rdfs:label "Compressed Air Filter"@en ;
  rdfs:seeAlso <http://bsdd.buildingsmart.org/#concept/details/3eXdymzEL2WwWgDskL3E7I> ;
  rdfs:seeAlso ifc:IfcFilterEnumType ;
  rdfs:subClassOf mep:Filter ;
.
mep:Filter-ODORFILTER
  rdf:type owl:Class ;
  rdfs:isDefinedBy <http://pi.pauwel.be/voc/distributionelement> ;
  rdfs:label "Odor Filter"@en ;
  rdfs:seeAlso <http://bsdd.buildingsmart.org/#concept/details/0Nh$mYaRT13xMPbS$8vqwW> ;
  rdfs:seeAlso ifc:IfcFilterEnumType ;
  rdfs:subClassOf mep:Filter ;
.
mep:Filter-OILFILTER
  rdf:type owl:Class ;
  rdfs:comment "a filter used to remove particulates from oil"@en ;
  rdfs:comment "a filter used to remove particulates from oil"@en-gb ;
  rdfs:isDefinedBy <http://pi.pauwel.be/voc/distributionelement> ;
  rdfs:label "Oil Filter"@en ;
  rdfs:label "oljefilter"@nb-no ;
  rdfs:seeAlso <http://bsdd.buildingsmart.org/#concept/details/0HemsvirL2luh4LogPKmfT> ;
  rdfs:seeAlso ifc:IfcFilterEnumType ;
  rdfs:subClassOf mep:Filter ;
.
mep:Filter-STRAINER
  rdf:type owl:Class ;
  rdfs:comment "A fitting for preventing that leaves enters the down-pipe"@en ;
  rdfs:comment "En innretning som hindrer løv og annet nedfall i å komme inn i nedløpsrøret"@nb-no ;
  rdfs:comment "device that prevents solid matter from entering a pipe, pump, valve or meter"@en ;
  rdfs:isDefinedBy <http://pi.pauwel.be/voc/distributionelement> ;
  rdfs:label "Siebe"@de-de ;
  rdfs:label "Strainer"@en ;
  rdfs:label "filtre"@fr-fr ;
  rdfs:label "løvrist"@nb-no ;
  rdfs:label "sil"@nb-no ;
  rdfs:seeAlso <http://bsdd.buildingsmart.org/#concept/details/30aQppcM58MR6pxe6iVccR> ;
  rdfs:seeAlso ifc:IfcFilterEnumType ;
  rdfs:subClassOf mep:Filter ;
.
mep:Filter-WATERFILTER
  rdf:type owl:Class ;
  rdfs:isDefinedBy <http://pi.pauwel.be/voc/distributionelement> ;
  rdfs:label "Water Filter"@en ;
  rdfs:label "vannfilter"@nb-no ;
  rdfs:seeAlso <http://bsdd.buildingsmart.org/#concept/details/3IqBAp0Tv5HxjI8BQo7oFW> ;
  rdfs:seeAlso ifc:IfcFilterEnumType ;
  rdfs:subClassOf mep:Filter ;
.
mep:FireSuppressionTerminal
  rdf:type owl:Class ;
  rdfs:comment """A suppression terminal has the purpose of delivering a fluid (gas or liquid) that will suppress a fire.
Provides for all forms of sprinkler, spreader and other form of terminal that is connected to a pipework system and intended to act in the role of suppressing a fire."""@en ;
  rdfs:isDefinedBy <http://pi.pauwel.be/voc/distributionelement> ;
  rdfs:label "Appareil terminal d'extinction d'incendie"@fr-fr ;
  rdfs:label "Feuerlöscheinrichtung"@de-de ;
  rdfs:label "Fire Suppression Terminal"@en ;
  rdfs:label "brannundertrykkelsessystem"@nb-no ;
  rdfs:seeAlso <http://bsdd.buildingsmart.org/#concept/details/1P1aiBVvPDjPVBP4TWbJw6> ;
  rdfs:seeAlso ifc:IfcFireSuppressionTerminal ;
  rdfs:subClassOf mep:FlowTerminal ;
.
mep:FireSuppressionTerminal-BREECHINGINLET
  rdf:type owl:Class ;
  rdfs:isDefinedBy <http://pi.pauwel.be/voc/distributionelement> ;
  rdfs:label "Breeching Inlet"@en ;
  rdfs:seeAlso <http://bsdd.buildingsmart.org/#concept/details/00IdsJ7iT7Nx$veMrXzcqM> ;
  rdfs:seeAlso ifc:IfcFireSuppressionTerminalEnumType ;
  rdfs:subClassOf mep:FireSuppressionTerminal ;
.
mep:FireSuppressionTerminal-FIREHYDRANT
  rdf:type owl:Class ;
  rdfs:isDefinedBy <http://pi.pauwel.be/voc/distributionelement> ;
  rdfs:label "Fire Hydrant"@en ;
  rdfs:seeAlso <http://bsdd.buildingsmart.org/#concept/details/1esoBNGDb2wOo3IcBnG9Zv> ;
  rdfs:seeAlso ifc:IfcFireSuppressionTerminalEnumType ;
  rdfs:subClassOf mep:FireSuppressionTerminal ;
.
mep:FireSuppressionTerminal-HOSEREEL
  rdf:type owl:Class ;
  rdfs:isDefinedBy <http://pi.pauwel.be/voc/distributionelement> ;
  rdfs:label "Hosereel"@en ;
  rdfs:seeAlso <http://bsdd.buildingsmart.org/#concept/details/3BjPDggX5A1uWncjNaSpTp> ;
  rdfs:seeAlso ifc:IfcFireSuppressionTerminalEnumType ;
  rdfs:subClassOf mep:FireSuppressionTerminal ;
.
mep:FireSuppressionTerminal-SPRINKLER
  rdf:type owl:Class ;
  rdfs:comment "nozzle with a thermally sensitive sealing device which opens to discharge water for fire fighting"@en ;
  rdfs:isDefinedBy <http://pi.pauwel.be/voc/distributionelement> ;
  rdfs:label "Sprinkler"@en ;
  rdfs:label "Sprinkler"@nl-nl ;
  rdfs:label "fire sprinkler"@en ;
  rdfs:label "sprinkler"@nb-no ;
  rdfs:seeAlso <http://bsdd.buildingsmart.org/#concept/details/09wWrp7P91aASjo0_dry01> ;
  rdfs:seeAlso ifc:IfcFireSuppressionTerminalEnumType ;
  rdfs:subClassOf mep:FireSuppressionTerminal ;
.
mep:FireSuppressionTerminal-SPRINKLERDEFLECTOR
  rdf:type owl:Class ;
  rdfs:isDefinedBy <http://pi.pauwel.be/voc/distributionelement> ;
  rdfs:label "Sprinkler Deflector"@en ;
  rdfs:seeAlso <http://bsdd.buildingsmart.org/#concept/details/2LU6yVzZT7U8X4VneBA$Bh> ;
  rdfs:seeAlso ifc:IfcFireSuppressionTerminalEnumType ;
  rdfs:subClassOf mep:FireSuppressionTerminal ;
.
mep:FlowController
  rdf:type owl:Class ;
  rdfs:comment "the distribution flow element ifcflowcontroller defines the occurrence of elements of a distribution system that are used to regulate flow through a distribution system. examples include dampers, valves, switches, and relays. its type is defined by ifcflowcontrollertype or subtypes."@en ;
  rdfs:isDefinedBy <http://pi.pauwel.be/voc/distributionelement> ;
  rdfs:label "Flow Controller"@en ;
  rdfs:label "Regler (allgemein)"@de-de ;
  rdfs:label "contrôleur de débit"@fr-fr ;
  rdfs:label "vannmengderegulator"@nb-no ;
  rdfs:seeAlso <http://bsdd.buildingsmart.org/#concept/details/1iDky6Xqz0NhbMNjWBjWCy> ;
  rdfs:seeAlso ifc:IfcFlowController ;
  rdfs:subClassOf mep:DistributionFlowElement ;
.
mep:FlowFitting
  rdf:type owl:Class ;
  rdfs:comment "Elkraftfordeling til driftstekniske installasjoner"@nb-no ;
  rdfs:comment "Elkraftfordeling til virksomhet"@nb-no ;
  rdfs:comment "the distribution flow element ifcflowfitting defines the occurrence of a junction or transition in a flow distribution system, such as an elbow or tee. its type is defined by ifcflowfittingtype or its subtypes."@en ;
  rdfs:isDefinedBy <http://pi.pauwel.be/voc/distributionelement> ;
  rdfs:label "Flow Fitting"@en ;
  rdfs:label "Verbinder / Formstück (allgemein)"@de-de ;
  rdfs:label "koblinger driftsteknisk"@nb-no ;
  rdfs:label "koblinger virksomhet"@nb-no ;
  rdfs:label "raccord d'installation fluides"@fr-fr ;
  rdfs:seeAlso <http://bsdd.buildingsmart.org/#concept/details/0QXNqIaY58ARlIeBKvxECI> ;
  rdfs:seeAlso ifc:IfcFlowFitting ;
  rdfs:subClassOf mep:DistributionFlowElement ;
.
mep:FlowInstrument
  rdf:type owl:Class ;
  rdfs:comment """An instrument reads and displays the flow value of a particular property of a system at a point, or displays the difference in the value of a property between two points.
Typically for the purpose of determining the value of the property at a point in time. Includes  forms of mechanical flow instrument (thermometers, pressure gauges etc.) and electrical flow instruments (ammeters, voltmeters etc.)"""@en ;
  rdfs:isDefinedBy <http://pi.pauwel.be/voc/distributionelement> ;
  rdfs:label "Flow Instrument"@en ;
  rdfs:label "Instrument d'installation fluides"@fr-fr ;
  rdfs:label "Messinstrument (allgemein)"@de-de ;
  rdfs:label "strømningsinstrument"@nb-no ;
  rdfs:seeAlso <http://bsdd.buildingsmart.org/#concept/details/11jUOktIH3ZBjsCen5K$76> ;
  rdfs:seeAlso ifc:IfcFlowInstrument ;
  rdfs:subClassOf mep:DistributionControlElement ;
.
mep:FlowInstrument-AMMETER
  rdf:type owl:Class ;
  rdfs:comment "a device that reads and displays the current flow in a circuit"@en ;
  rdfs:comment "a device that reads and displays the current flow in a circuit"@en-gb ;
  rdfs:isDefinedBy <http://pi.pauwel.be/voc/distributionelement> ;
  rdfs:label "AMMeter"@en ;
  rdfs:label "amperemeter"@nb-no ;
  rdfs:seeAlso <http://bsdd.buildingsmart.org/#concept/details/1ZnXtG18TFxghzaROUOOEo> ;
  rdfs:seeAlso ifc:IfcFlowInstrumentEnumType ;
  rdfs:subClassOf mep:FlowInstrument ;
.
mep:FlowInstrument-FREQUENCYMETER
  rdf:type owl:Class ;
  rdfs:comment "a device that reads and displays the electrical frequency of an alternating current circuit."@en ;
  rdfs:isDefinedBy <http://pi.pauwel.be/voc/distributionelement> ;
  rdfs:label "Frequency Meter"@en ;
  rdfs:label "frekvensmåler"@nb-no ;
  rdfs:seeAlso <http://bsdd.buildingsmart.org/#concept/details/01E8ZEHkn6nuRHiPM5blVG> ;
  rdfs:seeAlso ifc:IfcFlowInstrumentEnumType ;
  rdfs:subClassOf mep:FlowInstrument ;
.
mep:FlowInstrument-PHASEANGLEMETER
  rdf:type owl:Class ;
  rdfs:comment "a device that reads and displays the phase angle of a phase in a polyphase electrical circuit"@en ;
  rdfs:comment "a device that reads and displays the phase angle of a phase in a polyphase electrical circuit"@en-gb ;
  rdfs:isDefinedBy <http://pi.pauwel.be/voc/distributionelement> ;
  rdfs:label "Phase-Angle Meter"@en ;
  rdfs:label "fasevinkelmåler"@nb-no ;
  rdfs:seeAlso <http://bsdd.buildingsmart.org/#concept/details/3Gf7_xpUn18gOIu3amQEQH> ;
  rdfs:seeAlso ifc:IfcFlowInstrumentEnumType ;
  rdfs:subClassOf mep:FlowInstrument ;
.
mep:FlowInstrument-POWERFACTORMETER
  rdf:type owl:Class ;
  rdfs:isDefinedBy <http://pi.pauwel.be/voc/distributionelement> ;
  rdfs:label "Power Factor Meter"@en ;
  rdfs:seeAlso <http://bsdd.buildingsmart.org/#concept/details/1P$PbnF35AFwKgPqjZPzC0> ;
  rdfs:seeAlso ifc:IfcFlowInstrumentEnumType ;
  rdfs:subClassOf mep:FlowInstrument ;
.
mep:FlowInstrument-PRESSUREGAUGE
  rdf:type owl:Class ;
  rdfs:isDefinedBy <http://pi.pauwel.be/voc/distributionelement> ;
  rdfs:label "Pressure Gauge"@en ;
  rdfs:seeAlso <http://bsdd.buildingsmart.org/#concept/details/0OE6$aHKjCBBgczwu$WIy0> ;
  rdfs:seeAlso ifc:IfcFlowInstrumentEnumType ;
  rdfs:subClassOf mep:FlowInstrument ;
.
mep:FlowInstrument-THERMOMETER
  rdf:type owl:Class ;
  rdfs:comment "Måler og viser temperatur analogt"@nb-no ;
  rdfs:comment "a device that reads and displays a temperature value at a point"@en ;
  rdfs:comment "a device that reads and displays a temperature value at a point"@en-gb ;
  rdfs:isDefinedBy <http://pi.pauwel.be/voc/distributionelement> ;
  rdfs:label "Temperaturmeßgerät"@de-de ;
  rdfs:label "Thermometer"@en ;
  rdfs:label "Thermometer"@nl-nl ;
  rdfs:label "termometer"@nb-no ;
  rdfs:label "thermomètre"@fr-fr ;
  rdfs:seeAlso <http://bsdd.buildingsmart.org/#concept/details/3vHXe6oT0Hsm00051Mm008> ;
  rdfs:seeAlso ifc:IfcFlowInstrumentEnumType ;
  rdfs:subClassOf mep:FlowInstrument ;
.
mep:FlowInstrument-VOLTMETER_PEAK
  rdf:type owl:Class ;
  rdfs:comment "a device that reads and displays the peak voltage in an electrical circuit"@en ;
  rdfs:comment "a device that reads and displays the peak voltage in an electrical circuit"@en-gb ;
  rdfs:isDefinedBy <http://pi.pauwel.be/voc/distributionelement> ;
  rdfs:label "Peak Volt Meter"@en ;
  rdfs:label "toppverdi voltmeter"@nb-no ;
  rdfs:seeAlso <http://bsdd.buildingsmart.org/#concept/details/3HJn6Sn$TBNQmm9Dwrzknj> ;
  rdfs:seeAlso ifc:IfcFlowInstrumentEnumType ;
  rdfs:subClassOf mep:FlowInstrument ;
.
mep:FlowInstrument-VOLTMETER_RMS
  rdf:type owl:Class ;
  rdfs:comment "a device that reads and displays the RMS (mean) voltage in an electrical circuit"@en ;
  rdfs:comment "a device that reads and displays the RMS (mean) voltage in an electrical circuit"@en-gb ;
  rdfs:isDefinedBy <http://pi.pauwel.be/voc/distributionelement> ;
  rdfs:label "RMS Volt Meter"@en ;
  rdfs:label "rms voltmeter"@nb-no ;
  rdfs:seeAlso <http://bsdd.buildingsmart.org/#concept/details/2rsw3JDZn4yRFLbTU1Aq7v> ;
  rdfs:seeAlso ifc:IfcFlowInstrumentEnumType ;
  rdfs:subClassOf mep:FlowInstrument ;
.
mep:FlowMeter
  rdf:type owl:Class ;
  rdfs:comment "A device that is used to measure the flow rate in a system."@en ;
  rdfs:isDefinedBy <http://pi.pauwel.be/voc/distributionelement> ;
  rdfs:label "Appareil de mesure de débit"@fr-fr ;
  rdfs:label "Flow Meter"@en ;
  rdfs:label "Zähler (allgemein)"@de-de ;
  rdfs:label "flytmåler"@nb-no ;
  rdfs:label "vannmengdemåler"@nb-no ;
  rdfs:seeAlso <http://bsdd.buildingsmart.org/#concept/details/3lICO0qUSHuO00025QrE$V> ;
  rdfs:seeAlso ifc:IfcFlowMeter ;
  rdfs:subClassOf mep:FlowController ;
.
mep:FlowMeter-ENERGYMETER
  rdf:type owl:Class ;
  rdfs:comment "device that measures, indicates and sometimes records, the energy usage in a system"@en ;
  rdfs:comment "device that measures, indicates and sometimes records, the energy usage in a system"@en-gb ;
  rdfs:isDefinedBy <http://pi.pauwel.be/voc/distributionelement> ;
  rdfs:label "Energy Meter"@en ;
  rdfs:label "energimåler"@nb-no ;
  rdfs:seeAlso <http://bsdd.buildingsmart.org/#concept/details/0dqsT4P2DFmvAItnTOiex9> ;
  rdfs:seeAlso ifc:IfcFlowMeterEnumType ;
  rdfs:subClassOf mep:FlowMeter ;
.
mep:FlowMeter-GASMETER
  rdf:type owl:Class ;
  rdfs:comment "device that measures, indicates and sometimes records, the volume of gas that passes through it without interrupting the flow"@en ;
  rdfs:comment "device that measures, indicates and sometimes records, the volume of gas that passes through it without interrupting the flow"@en-gb ;
  rdfs:isDefinedBy <http://pi.pauwel.be/voc/distributionelement> ;
  rdfs:label "Gas Meter"@en ;
  rdfs:label "gassmåler"@nb-no ;
  rdfs:seeAlso <http://bsdd.buildingsmart.org/#concept/details/2d9Kt_TA9Dww_aaJ0$7nqk> ;
  rdfs:seeAlso ifc:IfcFlowMeterEnumType ;
  rdfs:subClassOf mep:FlowMeter ;
.
mep:FlowMeter-OILMETER
  rdf:type owl:Class ;
  rdfs:comment "not available"@en ;
  rdfs:isDefinedBy <http://pi.pauwel.be/voc/distributionelement> ;
  rdfs:label "Oil Meter"@en ;
  rdfs:label "oljemåler"@nb-no ;
  rdfs:seeAlso <http://bsdd.buildingsmart.org/#concept/details/2HD3O5A6XAmQiJv54wilAx> ;
  rdfs:seeAlso ifc:IfcFlowMeterEnumType ;
  rdfs:subClassOf mep:FlowMeter ;
.
mep:FlowMeter-WATERMETER
  rdf:type owl:Class ;
  rdfs:isDefinedBy <http://pi.pauwel.be/voc/distributionelement> ;
  rdfs:label "Water Meter"@en ;
  rdfs:seeAlso <http://bsdd.buildingsmart.org/#concept/details/2bpgnuN4XCdOPs0pKS1wP1> ;
  rdfs:seeAlso ifc:IfcFlowMeterEnumType ;
  rdfs:subClassOf mep:FlowMeter ;
.
mep:FlowMovingDevice
  rdf:type owl:Class ;
  rdfs:comment "the distribution flow element ifcflowmovingdevice defines the occurrence of an apparatus used to distribute, circulate or perform conveyance of fluids, including liquids and gases (such as a pump or fan), and typically participates in a flow distribution system. its type is defined by ifcflowmovingdevicetype or its subtypes."@en ;
  rdfs:isDefinedBy <http://pi.pauwel.be/voc/distributionelement> ;
  rdfs:label "Flow Moving Device"@en ;
  rdfs:label "Strömungsmaschine (allgemein)"@de-de ;
  rdfs:label "dispositif de circulation de fluide"@fr-fr ;
  rdfs:label "flow moving device type"@en ;
  rdfs:label "strømførende enhet"@nb-no ;
  rdfs:seeAlso <http://bsdd.buildingsmart.org/#concept/details/1z188Qjir3JArIaN1C$Jlp> ;
  rdfs:seeAlso ifc:IfcFlowMovingDevice ;
  rdfs:subClassOf mep:DistributionFlowElement ;
.
mep:FlowSegment
  rdf:type owl:Class ;
  rdfs:comment "the distribution flow element ifcflowsegment defines the occurrence of a segment of a flow distribution system. the ifcflowsegment defines a particular occurrence of a segment inserted in the spatial context of a project. the parameters defining the type of the segment and/or its shape are defined by the ifcflowsegmenttype, which is related by the inverse relationship isdefinedby pointing to ifcreldefinesbytype."@en ;
  rdfs:isDefinedBy <http://pi.pauwel.be/voc/distributionelement> ;
  rdfs:label "Flow Segment"@en ;
  rdfs:label "Verteiler (allgemein)"@de-de ;
  rdfs:label "strømførende segment"@nb-no ;
  rdfs:label "tronçon d'installation fluides"@fr-fr ;
  rdfs:seeAlso <http://bsdd.buildingsmart.org/#concept/details/3pgLxEkmTCmg6JWI8OZE4J> ;
  rdfs:seeAlso ifc:IfcFlowSegment ;
  rdfs:subClassOf mep:DistributionFlowElement ;
.
mep:FlowStorageDevice
  rdf:type owl:Class ;
  rdfs:comment "the distribution flow element ifcflowstoragedevice defines the occurrence of a device that participates in a distribution system and is used for temporary storage (such as a tank). its type is defined by ifcflowstoragedevicetype or its subtypes."@en ;
  rdfs:isDefinedBy <http://pi.pauwel.be/voc/distributionelement> ;
  rdfs:label "Flow Storage Device"@en ;
  rdfs:label "Speicher (allgemein)"@de-de ;
  rdfs:label "appareil de stockage de fluide"@fr-fr ;
  rdfs:label "strømlagrende enhet"@nb-no ;
  rdfs:seeAlso <http://bsdd.buildingsmart.org/#concept/details/32pa_OQBP6exzNXNT$7YTr> ;
  rdfs:seeAlso ifc:IfcFlowStorageDevice ;
  rdfs:subClassOf mep:DistributionFlowElement ;
.
mep:FlowTerminal
  rdf:type owl:Class ;
  rdfs:comment "the distribution flow element ifcflowterminal defines the occurrence of a permanently attached element that acts as a terminus or beginning of a distribution system (such as an air outlet, drain, water closet or sink). a terminal is typically a point at which a system interfaces with an external environment. its type is defined by ifcflowterminaltype or its subtypes."@en ;
  rdfs:isDefinedBy <http://pi.pauwel.be/voc/distributionelement> ;
  rdfs:label "Endgerät (allgemein)"@de-de ;
  rdfs:label "Flow Terminal"@en ;
  rdfs:label "elément terminal d'installation fluides"@fr-fr ;
  rdfs:label "strømterminal"@nb-no ;
  rdfs:seeAlso <http://bsdd.buildingsmart.org/#concept/details/2zsZIJsQfBq98RWGNFmix9> ;
  rdfs:seeAlso ifc:IfcFlowTerminal ;
  rdfs:subClassOf mep:DistributionFlowElement ;
.
mep:FlowTreatmentDevice
  rdf:type owl:Class ;
  rdfs:comment "the distribution flow element ifcflowtreatmentdevice defines the occurrence of a device typically used to remove unwanted matter from a fluid, either liquid or gas, and typically participates in a flow distribution system. its type is defined by ifcflowtreatmentdevicetype or its subtypes."@en ;
  rdfs:isDefinedBy <http://pi.pauwel.be/voc/distributionelement> ;
  rdfs:label "Filter"@de-de ;
  rdfs:label "Flow Treatment Device"@en ;
  rdfs:label "appareil de traitement de fluide"@fr-fr ;
  rdfs:label "strømbehandlingsenhet"@nb-no ;
  rdfs:seeAlso <http://bsdd.buildingsmart.org/#concept/details/358GrBQjP36vPq9aYtgYQa> ;
  rdfs:seeAlso ifc:IfcFlowTreatmentDevice ;
  rdfs:subClassOf mep:DistributionFlowElement ;
.
mep:HeatExchanger
  rdf:type owl:Class ;
  rdfs:comment "A device used to provide heat transfer between non-mixing media such as plate and shell and tube heat exchangers. Commonly used on water-side distribution systems to recover energy from a liquid to another liquid (typically water-based)."@en ;
  rdfs:comment "An artefact intended for transferring thermal energy from one fluid to another.        "@en ;
  rdfs:isDefinedBy <http://pi.pauwel.be/voc/distributionelement> ;
  rdfs:label "Echangeur de chaleur"@fr-fr ;
  rdfs:label "Heat Exchanger"@en ;
  rdfs:label "Varmeveksler"@da ;
  rdfs:label "Warmtewisselaar"@nl ;
  rdfs:label "Warmtewisselaar"@nl-nl ;
  rdfs:label "Wärmetauscher"@de-de ;
  rdfs:label "varmeveksler"@nb-no ;
  rdfs:seeAlso <http://bsdd.buildingsmart.org/#concept/details/3WpPiXIp5Bf89w8w0QL9_r> ;
  rdfs:seeAlso ifc:IfcHeatExchanger ;
  rdfs:subClassOf mep:EnergyConversionDevice ;
.
mep:HeatExchanger-PLATE
  rdf:type owl:Class ;
  rdfs:isDefinedBy <http://pi.pauwel.be/voc/distributionelement> ;
  rdfs:label "Plate Heat Exchanger"@en ;
  rdfs:label "platevarmeveksler"@nb-no ;
  rdfs:seeAlso <http://bsdd.buildingsmart.org/#concept/details/2pALi8Jfv7Se_pR4H3dTaH> ;
  rdfs:seeAlso ifc:IfcHeatExchangerEnumType ;
  rdfs:subClassOf mep:HeatExchanger ;
.
mep:HeatExchanger-SHELLANDTUBE
  rdf:type owl:Class ;
  rdfs:isDefinedBy <http://pi.pauwel.be/voc/distributionelement> ;
  rdfs:label "Shell And Tube Heat Exchanger"@en ;
  rdfs:label "varmeveksler med rette rør"@nb-no ;
  rdfs:seeAlso <http://bsdd.buildingsmart.org/#concept/details/1h3yHT$MPE0BoJuFFtf4$5> ;
  rdfs:seeAlso ifc:IfcHeatExchangerEnumType ;
  rdfs:subClassOf mep:HeatExchanger ;
.
mep:Humidifier
  rdf:type owl:Class ;
  rdfs:comment "A device that adds moisture into the air."@en ;
  rdfs:isDefinedBy <http://pi.pauwel.be/voc/distributionelement> ;
  rdfs:label "Befeuchter"@de-de ;
  rdfs:label "Befugter"@da ;
  rdfs:label "Humidifier"@en ;
  rdfs:label "humidificateur"@fr-fr ;
  rdfs:label "luftfukter"@nb-no ;
  rdfs:seeAlso <http://bsdd.buildingsmart.org/#concept/details/1FcXNG5qj2GQITbOwXrOIF> ;
  rdfs:seeAlso ifc:IfcHumidifier ;
  rdfs:subClassOf mep:EnergyConversionDevice ;
.
mep:Humidifier-ADIABATICAIRWASHER
  rdf:type owl:Class ;
  rdfs:isDefinedBy <http://pi.pauwel.be/voc/distributionelement> ;
  rdfs:label "Adiabatic Air Washer"@en ;
  rdfs:label "adiabatisk luftvasker"@nb-no ;
  rdfs:seeAlso <http://bsdd.buildingsmart.org/#concept/details/2MNV0vgOv328qlczPJ03OC> ;
  rdfs:seeAlso ifc:IfcHumidifierEnumType ;
  rdfs:subClassOf mep:Humidifier ;
.
mep:Humidifier-ADIABATICATOMIZING
  rdf:type owl:Class ;
  rdfs:comment "water vapor is added into the airstream through adiabatic evaporation using an atomizing element"@en ;
  rdfs:comment "water vapor is added into the airstream through adiabatic evaporation using an atomizing element"@en-gb ;
  rdfs:isDefinedBy <http://pi.pauwel.be/voc/distributionelement> ;
  rdfs:label "Adiabatic Atomizing"@en ;
  rdfs:label "adiabatisk forstøver"@nb-no ;
  rdfs:seeAlso <http://bsdd.buildingsmart.org/#concept/details/1K4HZEHEv1wQ19Vzk48Sgn> ;
  rdfs:seeAlso ifc:IfcHumidifierEnumType ;
  rdfs:subClassOf mep:Humidifier ;
.
mep:Humidifier-ADIABATICCOMPRESSEDAIRNOZZLE
  rdf:type owl:Class ;
  rdfs:comment "water vapor is added into the airstream through adiabatic evaporation using a compressed air nozzle"@en ;
  rdfs:comment "water vapor is added into the airstream through adiabatic evaporation using a compressed air nozzle"@en-gb ;
  rdfs:isDefinedBy <http://pi.pauwel.be/voc/distributionelement> ;
  rdfs:label "Adiabatic Compressed Air Nozzle"@en ;
  rdfs:label "adiabatisk trykkluftdyse"@nb-no ;
  rdfs:seeAlso <http://bsdd.buildingsmart.org/#concept/details/2HCfOW4In2BREPSqe5Ms$p> ;
  rdfs:seeAlso ifc:IfcHumidifierEnumType ;
  rdfs:subClassOf mep:Humidifier ;
.
mep:Humidifier-ADIABATICPAN
  rdf:type owl:Class ;
  rdfs:isDefinedBy <http://pi.pauwel.be/voc/distributionelement> ;
  rdfs:label "Adiabatic Pan"@en ;
  rdfs:label "adiabatisk kar"@nb-no ;
  rdfs:seeAlso <http://bsdd.buildingsmart.org/#concept/details/3d9dTNKyPFRRor9abHmtji> ;
  rdfs:seeAlso ifc:IfcHumidifierEnumType ;
  rdfs:subClassOf mep:Humidifier ;
.
mep:Humidifier-ADIABATICRIGIDMEDIA
  rdf:type owl:Class ;
  rdfs:comment "water vapor is added into the airstream through adiabatic evaporation using a rigid media"@en ;
  rdfs:comment "water vapor is added into the airstream through adiabatic evaporation using a rigid media"@en-gb ;
  rdfs:isDefinedBy <http://pi.pauwel.be/voc/distributionelement> ;
  rdfs:label "Adiabatic Rigid Media"@en ;
  rdfs:label "adiabatisk rigid medium"@nb-no ;
  rdfs:seeAlso <http://bsdd.buildingsmart.org/#concept/details/0RD4N$yNr7jQPEzfNuNDtm> ;
  rdfs:seeAlso ifc:IfcHumidifierEnumType ;
  rdfs:subClassOf mep:Humidifier ;
.
mep:Humidifier-ADIABATICULTRASONIC
  rdf:type owl:Class ;
  rdfs:comment "water vapor is added into the airstream through adiabatic evaporation using an ultrasonic element"@en ;
  rdfs:comment "water vapor is added into the airstream through adiabatic evaporation using an ultrasonic element"@en-gb ;
  rdfs:isDefinedBy <http://pi.pauwel.be/voc/distributionelement> ;
  rdfs:label "Adiabatic Ultra Sonic"@en ;
  rdfs:label "adiabatisk ultralyd"@nb-no ;
  rdfs:seeAlso <http://bsdd.buildingsmart.org/#concept/details/0LHdcNpKzA9fe_4pzr59WD> ;
  rdfs:seeAlso ifc:IfcHumidifierEnumType ;
  rdfs:subClassOf mep:Humidifier ;
.
mep:Humidifier-ADIABATICWETTEDELEMENT
  rdf:type owl:Class ;
  rdfs:isDefinedBy <http://pi.pauwel.be/voc/distributionelement> ;
  rdfs:label "Adiabatic Wetted Element"@en ;
  rdfs:label "adiabatisk våtelement"@nb-no ;
  rdfs:seeAlso <http://bsdd.buildingsmart.org/#concept/details/3K$6EMdYfCzPmmFTgegHDy> ;
  rdfs:seeAlso ifc:IfcHumidifierEnumType ;
  rdfs:subClassOf mep:Humidifier ;
.
mep:Humidifier-ASSISTEDBUTANE
  rdf:type owl:Class ;
  rdfs:comment "water vapor is added into the airstream through water heated evaporation using a butane heater"@en ;
  rdfs:comment "water vapor is added into the airstream through water heated evaporation using a butane heater"@en-gb ;
  rdfs:isDefinedBy <http://pi.pauwel.be/voc/distributionelement> ;
  rdfs:label "Assisted Butane"@en ;
  rdfs:label "assistert butan"@nb-no ;
  rdfs:seeAlso <http://bsdd.buildingsmart.org/#concept/details/2VKdEEkCn1ghIvaWPax9j3> ;
  rdfs:seeAlso ifc:IfcHumidifierEnumType ;
  rdfs:subClassOf mep:Humidifier ;
.
mep:Humidifier-ASSISTEDELECTRIC
  rdf:type owl:Class ;
  rdfs:comment "water vapor is added into the airstream through water heated evaporation using an electric heater"@en ;
  rdfs:comment "water vapor is added into the airstream through water heated evaporation using an electric heater"@en-gb ;
  rdfs:isDefinedBy <http://pi.pauwel.be/voc/distributionelement> ;
  rdfs:label "Assisted Electric"@en ;
  rdfs:label "assistert elektrisitet"@nb-no ;
  rdfs:seeAlso <http://bsdd.buildingsmart.org/#concept/details/157UtcquX8d8khI$Nxg6Dg> ;
  rdfs:seeAlso ifc:IfcHumidifierEnumType ;
  rdfs:subClassOf mep:Humidifier ;
.
mep:Humidifier-ASSISTEDNATURALGAS
  rdf:type owl:Class ;
  rdfs:isDefinedBy <http://pi.pauwel.be/voc/distributionelement> ;
  rdfs:label "Assisted Natural Gas"@en ;
  rdfs:label "assistert naturgass"@nb-no ;
  rdfs:seeAlso <http://bsdd.buildingsmart.org/#concept/details/2y1ecVVOv7Lfs9vbXts2uj> ;
  rdfs:seeAlso ifc:IfcHumidifierEnumType ;
  rdfs:subClassOf mep:Humidifier ;
.
mep:Humidifier-ASSISTEDPROPANE
  rdf:type owl:Class ;
  rdfs:comment "water vapor is added into the airstream through water heated evaporation using a propane heater"@en ;
  rdfs:comment "water vapor is added into the airstream through water heated evaporation using a propane heater"@en-gb ;
  rdfs:isDefinedBy <http://pi.pauwel.be/voc/distributionelement> ;
  rdfs:label "Assisted Propane"@en ;
  rdfs:label "assistert propan"@nb-no ;
  rdfs:seeAlso <http://bsdd.buildingsmart.org/#concept/details/1Byt2bBk58pg9rdsh_tvnd> ;
  rdfs:seeAlso ifc:IfcHumidifierEnumType ;
  rdfs:subClassOf mep:Humidifier ;
.
mep:Humidifier-ASSISTEDSTEAM
  rdf:type owl:Class ;
  rdfs:comment "water vapor is added into the airstream through water heated evaporation using a steam heater"@en ;
  rdfs:comment "water vapor is added into the airstream through water heated evaporation using a steam heater"@en-gb ;
  rdfs:isDefinedBy <http://pi.pauwel.be/voc/distributionelement> ;
  rdfs:label "Assisted Steam"@en ;
  rdfs:label "assistert damp"@nb-no ;
  rdfs:seeAlso <http://bsdd.buildingsmart.org/#concept/details/2INKwOIaXFgxGMKSsCa2Lm> ;
  rdfs:seeAlso ifc:IfcHumidifierEnumType ;
  rdfs:subClassOf mep:Humidifier ;
.
mep:Humidifier-STEAMINJECTION
  rdf:type owl:Class ;
  rdfs:comment "water vapor is added into the airstream through direct steam injection"@en ;
  rdfs:comment "water vapor is added into the airstream through direct steam injection"@en-gb ;
  rdfs:isDefinedBy <http://pi.pauwel.be/voc/distributionelement> ;
  rdfs:label "Steam Injection"@en ;
  rdfs:label "dampinjeksjon"@nb-no ;
  rdfs:seeAlso <http://bsdd.buildingsmart.org/#concept/details/05OOwwH2b5pwbQqrAayAR1> ;
  rdfs:seeAlso ifc:IfcHumidifierEnumType ;
  rdfs:subClassOf mep:Humidifier ;
.
mep:Interceptor
  rdf:type owl:Class ;
  rdfs:comment "A device designed and installed in order to separate and retain deleterious, hazardous or undesirable matter while permitting normal sewage or liquids to discharge into a collection system by gravity."@en ;
  rdfs:isDefinedBy <http://pi.pauwel.be/voc/distributionelement> ;
  rdfs:label "Abscheider"@de-de ;
  rdfs:label "Interceptor"@en ;
  rdfs:seeAlso <http://bsdd.buildingsmart.org/#concept/details/11vN9pRrz0KQUNzVQ5_2RM> ;
  rdfs:seeAlso ifc:IfcInterceptor ;
  rdfs:subClassOf mep:FlowTreatmentDevice ;
.
mep:Interceptor-CYCLONIC
  rdf:type owl:Class ;
  rdfs:comment "removes larger liquid drops or larger solid particles"@en ;
  rdfs:comment "removes larger liquid drops or larger solid particles"@en-gb ;
  rdfs:isDefinedBy <http://pi.pauwel.be/voc/distributionelement> ;
  rdfs:label "Cyclonic Interceptor"@en ;
  rdfs:label "syklonisk"@nb-no ;
  rdfs:seeAlso <http://bsdd.buildingsmart.org/#concept/details/2RxuKardj99Q$KLR33Cbq6> ;
  rdfs:seeAlso ifc:IfcInterceptorEnumType ;
  rdfs:subClassOf mep:Interceptor ;
.
mep:Interceptor-GREASE
  rdf:type owl:Class ;
  rdfs:comment "chamber, on the line of a drain or discharge pipe, that prevents grease passing into a drainage system"@en ;
  rdfs:comment "chamber, on the line of a drain or discharge pipe, that prevents grease passing into a drainage system"@en-gb ;
  rdfs:isDefinedBy <http://pi.pauwel.be/voc/distributionelement> ;
  rdfs:label "Grease Interceptor"@en ;
  rdfs:label "fett"@nb-no ;
  rdfs:seeAlso <http://bsdd.buildingsmart.org/#concept/details/3LXDZRMqX6hBYYip97WFpr> ;
  rdfs:seeAlso ifc:IfcInterceptorEnumType ;
  rdfs:subClassOf mep:Interceptor ;
.
mep:Interceptor-OIL
  rdf:type owl:Class ;
  rdfs:comment "one or more chambers arranged to prevent the ingress of oil to a drain or sewer that retains the oil for later removal"@en ;
  rdfs:comment "one or more chambers arranged to prevent the ingress of oil to a drain or sewer that retains the oil for later removal"@en-gb ;
  rdfs:isDefinedBy <http://pi.pauwel.be/voc/distributionelement> ;
  rdfs:label "Oil Interceptor"@en ;
  rdfs:label "olje"@nb-no ;
  rdfs:seeAlso <http://bsdd.buildingsmart.org/#concept/details/0efFn8L559X8O9PLL0mkNu> ;
  rdfs:seeAlso ifc:IfcInterceptorEnumType ;
  rdfs:subClassOf mep:Interceptor ;
.
mep:Interceptor-PETROL
  rdf:type owl:Class ;
  rdfs:isDefinedBy <http://pi.pauwel.be/voc/distributionelement> ;
  rdfs:label "Petrol Interceptor"@en ;
  rdfs:seeAlso <http://bsdd.buildingsmart.org/#concept/details/3AfygEMd1AwBWNHSyfyIiI> ;
  rdfs:seeAlso ifc:IfcInterceptorEnumType ;
  rdfs:subClassOf mep:Interceptor ;
.
mep:JunctionBox
  rdf:type owl:Class ;
  rdfs:comment "An enclosure within which cables are connected. Cables may be members of an electrical circuit (for electrical power systems) or be information carriers (in a telecommunications system). Typically intended to conceal a cable junction from sight, eliminate tampering or provide a safe place for electrical connection."@en ;
  rdfs:isDefinedBy <http://pi.pauwel.be/voc/distributionelement> ;
  rdfs:label "Boite de jonction"@fr-fr ;
  rdfs:label "Junction Box"@en ;
  rdfs:label "Verbindungsdose"@de-de ;
  rdfs:seeAlso <http://bsdd.buildingsmart.org/#concept/details/0kaRGER1f0o8KFilly53$b> ;
  rdfs:seeAlso ifc:IfcJunctionBox ;
  rdfs:subClassOf mep:FlowFitting ;
.
mep:JunctionBox-DATA
  rdf:type owl:Class ;
  rdfs:comment "contains cables, outlets, and/or switches for communications use"@en ;
  rdfs:comment "contains cables, outlets, and/or switches for communications use"@en-gb ;
  rdfs:isDefinedBy <http://pi.pauwel.be/voc/distributionelement> ;
  rdfs:label "Data"@en ;
  rdfs:label "data"@nb-no ;
  rdfs:seeAlso <http://bsdd.buildingsmart.org/#concept/details/1mq782MKb1ZxoRYPK9Umy2> ;
  rdfs:seeAlso ifc:IfcJunctionBoxEnumType ;
  rdfs:subClassOf mep:JunctionBox ;
.
mep:JunctionBox-POWER
  rdf:type owl:Class ;
  rdfs:isDefinedBy <http://pi.pauwel.be/voc/distributionelement> ;
  rdfs:label "Power"@en ;
  rdfs:label "strømtilførsel"@nb-no ;
  rdfs:seeAlso <http://bsdd.buildingsmart.org/#concept/details/2rfL__S75EcOfkEgBpZV_b> ;
  rdfs:seeAlso ifc:IfcJunctionBoxEnumType ;
  rdfs:subClassOf mep:JunctionBox ;
.
mep:Lamp
  rdf:type owl:Class ;
  rdfs:comment "An artificial light source such as a light bulb or tube."@en ;
  rdfs:isDefinedBy <http://pi.pauwel.be/voc/distributionelement> ;
  rdfs:label "Lamp"@en ;
  rdfs:label "Lampe"@de-de ;
  rdfs:label "Leuchtmittel"@de-de ;
  rdfs:label "lampe"@fr-fr ;
  rdfs:seeAlso <http://bsdd.buildingsmart.org/#concept/details/0ETiMxiX14xwxiqYleSsxj> ;
  rdfs:seeAlso ifc:IfcLamp ;
  rdfs:subClassOf mep:FlowTerminal ;
.
mep:Lamp-COMPACTFLUORESCENT
  rdf:type owl:Class ;
  rdfs:isDefinedBy <http://pi.pauwel.be/voc/distributionelement> ;
  rdfs:label "Compact Fluorescent"@en ;
  rdfs:seeAlso <http://bsdd.buildingsmart.org/#concept/details/3zxJlrQUXE3BF9p3XFK9sV> ;
  rdfs:seeAlso ifc:IfcLampEnumType ;
  rdfs:subClassOf mep:Lamp ;
.
mep:Lamp-FLUORESCENT
  rdf:type owl:Class ;
  rdfs:comment "a typically tubular discharge lamp in which most of the light is emitted by one or several layers of phosphors excited by ultraviolet radiation from the discharge."@en ;
  rdfs:comment "a typically tubular discharge lamp in which most of the light is emitted by one or several layers of phosphors excited by ultraviolet radiation from the discharge."@en-gb ;
  rdfs:isDefinedBy <http://pi.pauwel.be/voc/distributionelement> ;
  rdfs:label "Fluorescent"@en ;
  rdfs:label "fluoriserende lampe"@nb-no ;
  rdfs:seeAlso <http://bsdd.buildingsmart.org/#concept/details/0V1bibu4L13Bts98Ganx3k> ;
  rdfs:seeAlso ifc:IfcLampEnumType ;
  rdfs:subClassOf mep:Lamp ;
.
mep:Lamp-HALOGEN
  rdf:type owl:Class ;
  rdfs:comment "a gas-filled, high-intensity incandescent lamp containing a small amount of a halogen"@en ;
  rdfs:isDefinedBy <http://pi.pauwel.be/voc/distributionelement> ;
  rdfs:label "Halogen"@en ;
  rdfs:label "halogen"@nb-no ;
  rdfs:seeAlso <http://bsdd.buildingsmart.org/#concept/details/2EGers_2r5rBBnldpP0G_o> ;
  rdfs:seeAlso ifc:IfcLampEnumType ;
  rdfs:subClassOf mep:Lamp ;
.
mep:Lamp-HIGHPRESSUREMERCURY
  rdf:type owl:Class ;
  rdfs:comment "a discharge lamp in which most of the light is emitted by exciting mercury at high pressure"@en ;
  rdfs:comment "a discharge lamp in which most of the light is emitted by exciting mercury at high pressure"@en-gb ;
  rdfs:isDefinedBy <http://pi.pauwel.be/voc/distributionelement> ;
  rdfs:label "High Pressure Mercury"@en ;
  rdfs:label "høytrykk - bly lampe"@nb-no ;
  rdfs:seeAlso <http://bsdd.buildingsmart.org/#concept/details/2QODll5IXBLOrmpb298AP_> ;
  rdfs:seeAlso ifc:IfcLampEnumType ;
  rdfs:subClassOf mep:Lamp ;
.
mep:Lamp-HIGHPRESSURESODIUM
  rdf:type owl:Class ;
  rdfs:comment "a discharge lamp in which most of the light is emitted by exciting sodium at high pressure"@en ;
  rdfs:comment "a discharge lamp in which most of the light is emitted by exciting sodium at high pressure"@en-gb ;
  rdfs:isDefinedBy <http://pi.pauwel.be/voc/distributionelement> ;
  rdfs:label "High Pressure Sodium"@en ;
  rdfs:label "høytrykk - sodium"@nb-no ;
  rdfs:seeAlso <http://bsdd.buildingsmart.org/#concept/details/1vX9Auimj7BfAyryFJkgkm> ;
  rdfs:seeAlso ifc:IfcLampEnumType ;
  rdfs:subClassOf mep:Lamp ;
.
mep:Lamp-LED
  rdf:type owl:Class ;
  rdfs:comment "a light-emitting diode (LED) is a semiconductor device that emits visible light when an electric current passes through it."@en ;
  rdfs:isDefinedBy <http://pi.pauwel.be/voc/distributionelement> ;
  rdfs:label "LED"@en ;
  rdfs:label "LED"@nb-no ;
  rdfs:seeAlso <http://bsdd.buildingsmart.org/#concept/details/2mULGMKGf1cRYOSiyAofvb> ;
  rdfs:seeAlso ifc:IfcLampEnumType ;
  rdfs:subClassOf mep:Lamp ;
.
mep:Lamp-METALHALIDE
  rdf:type owl:Class ;
  rdfs:isDefinedBy <http://pi.pauwel.be/voc/distributionelement> ;
  rdfs:label "Metal Halide"@en ;
  rdfs:seeAlso <http://bsdd.buildingsmart.org/#concept/details/3esdl$BJXD9htEWoSEpsDg> ;
  rdfs:seeAlso ifc:IfcLampEnumType ;
  rdfs:subClassOf mep:Lamp ;
.
mep:Lamp-OLED
  rdf:type owl:Class ;
  rdfs:comment "a solid state lamp that uses light-emitting diodes as the source of light whose emissive electroluminescent layer is composed of a film of organic compounds"@en ;
  rdfs:comment "a solid state lamp that uses light-emitting diodes as the source of light whose emissive electroluminescent layer is composed of a film of organic compounds"@en-gb ;
  rdfs:isDefinedBy <http://pi.pauwel.be/voc/distributionelement> ;
  rdfs:label "OLED"@en ;
  rdfs:label "oled"@nb-no ;
  rdfs:seeAlso <http://bsdd.buildingsmart.org/#concept/details/2ga1cHzm5D$fItBN2Tozo9> ;
  rdfs:seeAlso ifc:IfcLampEnumType ;
  rdfs:subClassOf mep:Lamp ;
.
mep:Lamp-TUNGSTENFILAMENT
  rdf:type owl:Class ;
  rdfs:isDefinedBy <http://pi.pauwel.be/voc/distributionelement> ;
  rdfs:label "Tungsten Filament"@en ;
  rdfs:seeAlso <http://bsdd.buildingsmart.org/#concept/details/3n5ZYbHnnBuhtIMoheS78j> ;
  rdfs:seeAlso ifc:IfcLampEnumType ;
  rdfs:subClassOf mep:Lamp ;
.
mep:LightFixture
  rdf:type owl:Class ;
  rdfs:comment "A container that is designed for the purpose of housing one or more lamps and optionally devices that control, restrict or vary their emission."@en ;
  rdfs:isDefinedBy <http://pi.pauwel.be/voc/distributionelement> ;
  rdfs:label "Fixation de lampe"@fr-fr ;
  rdfs:label "Leuchte"@de-de ;
  rdfs:label "Light Fixture"@en ;
  rdfs:label "Verlichtingsarmatuur"@nl-nl ;
  rdfs:label "lysarmatur"@nb-no ;
  rdfs:seeAlso <http://bsdd.buildingsmart.org/#concept/details/1sxtfF6Gb1ieWm5Xy9aa5C> ;
  rdfs:seeAlso ifc:IfcLightFixture ;
  rdfs:subClassOf mep:FlowTerminal ;
.
mep:LightFixture-DIRECTIONSOURCE
  rdf:type owl:Class ;
  rdfs:comment "a light fixture that is considered to have a length or surface area from which it emits light in a direction. a light fixture containing one or more fluorescent lamps is an example of a direction source"@en ;
  rdfs:comment "a light fixture that is considered to have a length or surface area from which it emits light in a direction. a light fixture containing one or more fluorescent lamps is an example of a direction source"@en-gb ;
  rdfs:isDefinedBy <http://pi.pauwel.be/voc/distributionelement> ;
  rdfs:label "Direction Source"@en ;
  rdfs:label "kilderetning"@nb-no ;
  rdfs:seeAlso <http://bsdd.buildingsmart.org/#concept/details/0XEOjAoQb8nAOs58mf0C7S> ;
  rdfs:seeAlso ifc:IfcLightFixtureEnumType ;
  rdfs:subClassOf mep:LightFixture ;
.
mep:LightFixture-POINTSOURCE
  rdf:type owl:Class ;
  rdfs:isDefinedBy <http://pi.pauwel.be/voc/distributionelement> ;
  rdfs:label "Point Source"@en ;
  rdfs:seeAlso <http://bsdd.buildingsmart.org/#concept/details/1bOvnRIgnDhuRposkK0D7b> ;
  rdfs:seeAlso ifc:IfcLightFixtureEnumType ;
  rdfs:subClassOf mep:LightFixture ;
.
mep:LightFixture-SECURITYLIGHTING
  rdf:type owl:Class ;
  rdfs:comment "a light fixture having specific purpose of directing occupants in an emergency, such as an illuminated exit sign or emergency flood light"@en ;
  rdfs:comment "a light fixture having specific purpose of directing occupants in an emergency, such as an illuminated exit sign or emergency flood light"@en-gb ;
  rdfs:isDefinedBy <http://pi.pauwel.be/voc/distributionelement> ;
  rdfs:label "Security Lighting"@en ;
  rdfs:label "sikkerhetsbelysning"@nb-no ;
  rdfs:seeAlso <http://bsdd.buildingsmart.org/#concept/details/3r7SZninH9Uh6FH$yz54Pl> ;
  rdfs:seeAlso ifc:IfcLightFixtureEnumType ;
  rdfs:subClassOf mep:LightFixture ;
.
mep:MedicalDevice
  rdf:type owl:Class ;
  rdfs:comment "A device is attached to a medical piping system and operates upon medical gases to perform a specific function. Medical gases include medical air, medical vacuum, oxygen, carbon dioxide, nitrogen, and nitrous oxide."@en ;
  rdfs:isDefinedBy <http://pi.pauwel.be/voc/distributionelement> ;
  rdfs:label "Equipement médical"@fr-fr ;
  rdfs:label "Medical Device"@en ;
  rdfs:label "Medizinisches Gerät"@de-de ;
  rdfs:label "medisinsk utstyr"@nb-no ;
  rdfs:seeAlso <http://bsdd.buildingsmart.org/#concept/details/1AkDu7dZb8l8V$ZCIldlOl> ;
  rdfs:seeAlso ifc:IfcMedicalDevice ;
  rdfs:subClassOf mep:FlowTerminal ;
.
mep:MedicalDevice-AIRSTATION
  rdf:type owl:Class ;
  rdfs:comment "device that provides purified medical air, composed of an air compressor and air treatment line"@en ;
  rdfs:comment "device that provides purified medical air, composed of an air compressor and air treatment line"@en-gb ;
  rdfs:isDefinedBy <http://pi.pauwel.be/voc/distributionelement> ;
  rdfs:label "Air Station"@en ;
  rdfs:label "luftstasjon"@nb-no ;
  rdfs:seeAlso <http://bsdd.buildingsmart.org/#concept/details/3o0TKF$jb4JfwCg4jNP8QH> ;
  rdfs:seeAlso ifc:IfcMedicalDeviceEnumType ;
  rdfs:subClassOf mep:MedicalDevice ;
.
mep:MedicalDevice-FEEDAIRUNIT
  rdf:type owl:Class ;
  rdfs:isDefinedBy <http://pi.pauwel.be/voc/distributionelement> ;
  rdfs:label "Feed Air Unit"@en ;
  rdfs:seeAlso <http://bsdd.buildingsmart.org/#concept/details/0L4vXkvln2MRDKPQngnIZ1> ;
  rdfs:seeAlso ifc:IfcMedicalDeviceEnumType ;
  rdfs:subClassOf mep:MedicalDevice ;
.
mep:MedicalDevice-OXYGENGENERATOR
  rdf:type owl:Class ;
  rdfs:comment "device that generates oxygen from air"@en ;
  rdfs:comment "device that generates oxygen from air"@en-gb ;
  rdfs:isDefinedBy <http://pi.pauwel.be/voc/distributionelement> ;
  rdfs:label "Oxygen Generator"@en ;
  rdfs:label "oksygengenerator"@nb-no ;
  rdfs:seeAlso <http://bsdd.buildingsmart.org/#concept/details/2beptDYcnFLwdWqGq$GWRC> ;
  rdfs:seeAlso ifc:IfcMedicalDeviceEnumType ;
  rdfs:subClassOf mep:MedicalDevice ;
.
mep:MedicalDevice-OXYGENPLANT
  rdf:type owl:Class ;
  rdfs:comment "device that combines a feed air unit, oxygen generator, and backup oxygen cylinders"@en ;
  rdfs:isDefinedBy <http://pi.pauwel.be/voc/distributionelement> ;
  rdfs:label "Oxygen Plant"@en ;
  rdfs:label "oksygenanlegg"@nb-no ;
  rdfs:seeAlso <http://bsdd.buildingsmart.org/#concept/details/2Z$pgegmf8Bv9ktRxYuUY7> ;
  rdfs:seeAlso ifc:IfcMedicalDeviceEnumType ;
  rdfs:subClassOf mep:MedicalDevice ;
.
mep:MedicalDevice-VACUUMSTATION
  rdf:type owl:Class ;
  rdfs:comment "device that provides suction, composed of a vacuum pump and bacterial filtration line"@en ;
  rdfs:comment "device that provides suction, composed of a vacuum pump and bacterial filtration line"@en-gb ;
  rdfs:isDefinedBy <http://pi.pauwel.be/voc/distributionelement> ;
  rdfs:label "Vacuum Station"@en ;
  rdfs:label "vakuumstasjon"@nb-no ;
  rdfs:seeAlso <http://bsdd.buildingsmart.org/#concept/details/2qtw8iOMD6aQlRYJeE54Oe> ;
  rdfs:seeAlso ifc:IfcMedicalDeviceEnumType ;
  rdfs:subClassOf mep:MedicalDevice ;
.
mep:MotorConnection
  rdf:type owl:Class ;
  rdfs:comment "The means for connecting a motor as the driving device to the driven device."@en ;
  rdfs:isDefinedBy <http://pi.pauwel.be/voc/distributionelement> ;
  rdfs:label "Connection du moteur"@fr-fr ;
  rdfs:label "Motor Connection"@en ;
  rdfs:label "Motoranschluss"@de-de ;
  rdfs:label "Motorkoppeling"@nl-nl ;
  rdfs:label "motorkobling"@nb-no ;
  rdfs:seeAlso <http://bsdd.buildingsmart.org/#concept/details/1uD4xpI6rB28wdUvR8Y86u> ;
  rdfs:seeAlso ifc:IfcMotorConnection ;
  rdfs:subClassOf mep:EnergyConversionDevice ;
.
mep:MotorConnection-BELTDRIVE
  rdf:type owl:Class ;
  rdfs:comment "an indirect connection made through the medium of a shaped, flexible continuous loop"@en ;
  rdfs:comment "an indirect connection made through the medium of a shaped, flexible continuous loop"@en-gb ;
  rdfs:isDefinedBy <http://pi.pauwel.be/voc/distributionelement> ;
  rdfs:label "Belt Drive Motor Connection"@en ;
  rdfs:label "beltedrevet"@nb-no ;
  rdfs:label "drivbelte"@nb-no ;
  rdfs:seeAlso <http://bsdd.buildingsmart.org/#concept/details/337StHg8r5XxwkyT3aqNfr> ;
  rdfs:seeAlso ifc:IfcMotorConnectionEnumType ;
  rdfs:subClassOf mep:MotorConnection ;
.
mep:MotorConnection-COUPLING
  rdf:type owl:Class ;
  rdfs:comment "an indirect connection made through the medium of the viscosity of a fluid"@en ;
  rdfs:isDefinedBy <http://pi.pauwel.be/voc/distributionelement> ;
  rdfs:label "Coupling Motor Connection"@en ;
  rdfs:label "kopling"@nb-no ;
  rdfs:seeAlso <http://bsdd.buildingsmart.org/#concept/details/2ztf_P39HBTfamG9J37o0l> ;
  rdfs:seeAlso ifc:IfcMotorConnectionEnumType ;
  rdfs:subClassOf mep:MotorConnection ;
.
mep:MotorConnection-DIRECTDRIVE
  rdf:type owl:Class ;
  rdfs:comment "a direct, physical connection made between the motor and the driven device"@en ;
  rdfs:comment "a direct, physical connection made between the motor and the driven device"@en-gb ;
  rdfs:isDefinedBy <http://pi.pauwel.be/voc/distributionelement> ;
  rdfs:label "Direct Drive Motor Connection"@en ;
  rdfs:label "direktedrevet motor"@nb-no ;
  rdfs:seeAlso <http://bsdd.buildingsmart.org/#concept/details/26AgedTrrEsuQRrx2V_DY3> ;
  rdfs:seeAlso ifc:IfcMotorConnectionEnumType ;
  rdfs:subClassOf mep:MotorConnection ;
.
mep:Outlet
  rdf:type owl:Class ;
  rdfs:comment """A device installed at a point to receive one or more inserted plugs for electrical power or communications.
"""@en ;
  rdfs:isDefinedBy <http://pi.pauwel.be/voc/distributionelement> ;
  rdfs:label "Dose"@de-de ;
  rdfs:label "Outlet"@en ;
  rdfs:label "Steckdose"@de-de ;
  rdfs:label "prise"@fr-fr ;
  rdfs:label "uttak"@nb-no ;
  rdfs:seeAlso <http://bsdd.buildingsmart.org/#concept/details/28QPmBjcbAuOHAWzJovXA6> ;
  rdfs:seeAlso ifc:IfcOutlet ;
  rdfs:subClassOf mep:FlowTerminal ;
.
mep:Outlet-AUDIOVISUALOUTLET
  rdf:type owl:Class ;
  rdfs:comment "an outlet used for an audio or visual device"@en ;
  rdfs:comment "an outlet used for an audio or visual device"@en-gb ;
  rdfs:isDefinedBy <http://pi.pauwel.be/voc/distributionelement> ;
  rdfs:label "Audiovisual Outlet"@en ;
  rdfs:label "audiovisuelt utgang"@nb-no ;
  rdfs:seeAlso <http://bsdd.buildingsmart.org/#concept/details/0lKEDMjxLFNxLZF0uvQXvQ> ;
  rdfs:seeAlso ifc:IfcOutletEnumType ;
  rdfs:subClassOf mep:Outlet ;
.
mep:Outlet-COMMUNICATIONSOUTLET
  rdf:type owl:Class ;
  rdfs:comment "an outlet used for connecting communications equipment"@en ;
  rdfs:comment "an outlet used for connecting communications equipment"@en-gb ;
  rdfs:isDefinedBy <http://pi.pauwel.be/voc/distributionelement> ;
  rdfs:label "Communications Outlet"@en ;
  rdfs:label "kommunikasjonuttak"@nb-no ;
  rdfs:seeAlso <http://bsdd.buildingsmart.org/#concept/details/3LRis6YOnAhO_2qLThy$7d> ;
  rdfs:seeAlso ifc:IfcOutletEnumType ;
  rdfs:subClassOf mep:Outlet ;
.
mep:Outlet-DATAOUTLET
  rdf:type owl:Class ;
  rdfs:comment "an outlet used for connecting data communications equipment"@en ;
  rdfs:comment "an outlet used for connecting data communications equipment"@en-gb ;
  rdfs:isDefinedBy <http://pi.pauwel.be/voc/distributionelement> ;
  rdfs:label "Data Outlet"@en ;
  rdfs:label "datautgang"@nb-no ;
  rdfs:seeAlso <http://bsdd.buildingsmart.org/#concept/details/2nLbYVXBz2iPUzoVG9MSjL> ;
  rdfs:seeAlso ifc:IfcOutletEnumType ;
  rdfs:subClassOf mep:Outlet ;
.
mep:Outlet-POWEROUTLET
  rdf:type owl:Class ;
  rdfs:comment "an outlet used for connecting electrical devices requiring power"@en ;
  rdfs:comment "an outlet used for connecting electrical devices requiring power"@en-gb ;
  rdfs:isDefinedBy <http://pi.pauwel.be/voc/distributionelement> ;
  rdfs:label "Power Outlet"@en ;
  rdfs:label "strømuttak"@nb-no ;
  rdfs:seeAlso <http://bsdd.buildingsmart.org/#concept/details/1VO3tI1Bn2AO1KWd3ZVGi6> ;
  rdfs:seeAlso ifc:IfcOutletEnumType ;
  rdfs:subClassOf mep:Outlet ;
.
mep:Outlet-TELEPHONEOUTLET
  rdf:type owl:Class ;
  rdfs:comment "an outlet used for connecting telephone communications equipment"@en ;
  rdfs:comment "an outlet used for connecting telephone communications equipment"@en-gb ;
  rdfs:isDefinedBy <http://pi.pauwel.be/voc/distributionelement> ;
  rdfs:label "Telephone Outlet"@en ;
  rdfs:label "telekommunikasjonsuttak"@nb-no ;
  rdfs:seeAlso <http://bsdd.buildingsmart.org/#concept/details/3sQmISw8154AzAhVrfw8CI> ;
  rdfs:seeAlso ifc:IfcOutletEnumType ;
  rdfs:subClassOf mep:Outlet ;
.
mep:PipeFitting
  rdf:type owl:Class ;
  rdfs:comment "A junction or transition in a piping flow distribution system used to connect pipe segments, resulting in changes in flow characteristics to the fluid such as direction or flow rate. Includes elbows, junctions, manifolds, and plumbing boxes."@en ;
  rdfs:isDefinedBy <http://pi.pauwel.be/voc/distributionelement> ;
  rdfs:label "Pipe Fitting"@en ;
  rdfs:label "Rohrverbinder"@de-de ;
  rdfs:label "raccord de tuyauterie"@fr-fr ;
  rdfs:label "rørdel"@nb-no ;
  rdfs:seeAlso <http://bsdd.buildingsmart.org/#concept/details/36UVu0qV8HuO00025QrE$V> ;
  rdfs:seeAlso ifc:IfcPipeFitting ;
  rdfs:subClassOf mep:FlowFitting ;
.
mep:PipeFitting-BEND
  rdf:type owl:Class ;
  rdfs:comment "A fitting for joining the down-pipe in different angles pass blockings"@en ;
  rdfs:comment "Bend albue"@nb-no ;
  rdfs:comment "Bend, albue"@nb-no ;
  rdfs:comment "En innretning for å skjøte nedløpsrøret i ulike vinkler forbi hindringer"@nb-no ;
  rdfs:comment "a fitting with typically two ports used to change the direction of flow between connected elements"@en ;
  rdfs:comment "a fitting with typically two ports used to change the direction of flow between connected elements"@en-gb ;
  rdfs:isDefinedBy <http://pi.pauwel.be/voc/distributionelement> ;
  rdfs:label "Bend"@en ;
  rdfs:label "Krümmer"@de-de ;
  rdfs:label "bend brannslokking inertgass"@nb-no ;
  rdfs:label "bend brannslukking vann"@nb-no ;
  rdfs:label "bend bunnledning sanitær"@nb-no ;
  rdfs:label "bend gassinstallasjon virksomhet"@nb-no ;
  rdfs:label "bend gassinstallasjon"@nb-no ;
  rdfs:label "bend pipeline sanitation"@en ;
  rdfs:label "bend sanitær"@nb-no ;
  rdfs:label "bend"@nb-no ;
  rdfs:label "brannslokkingbend for tåke"@nb-no ;
  rdfs:label "brannslukkingbend for sprinkler"@nb-no ;
  rdfs:label "coude"@fr-fr ;
  rdfs:label "elbows"@en ;
  rdfs:label "rørbend"@nb-no ;
  rdfs:label "tee gas installation"@en ;
  rdfs:seeAlso <http://bsdd.buildingsmart.org/#concept/details/0_1uLp$45FjOqNjel4YBnY> ;
  rdfs:seeAlso <http://bsdd.buildingsmart.org/#concept/details/11IUzA0c9C9gGPcD6wjcm8> ;
  rdfs:seeAlso <http://bsdd.buildingsmart.org/#concept/details/2ScGOKl0TF58sYPFb6KHbc> ;
  rdfs:seeAlso <http://bsdd.buildingsmart.org/#concept/details/2VSwjMBw1DguPAi2T4j5Vo> ;
  rdfs:seeAlso <http://bsdd.buildingsmart.org/#concept/details/2Wxblu6ePDPQ1joWCcVscx> ;
  rdfs:seeAlso <http://bsdd.buildingsmart.org/#concept/details/3$QIJ5gKv4hPazehz8XSJr> ;
  rdfs:seeAlso <http://bsdd.buildingsmart.org/#concept/details/3qojuW1k5C89_5p3vK7la0> ;
  rdfs:seeAlso <http://bsdd.buildingsmart.org/#concept/details/3vHSO0oT0Hsm00051Mm008> ;
  rdfs:seeAlso ifc:IfcPipeFittingEnumType ;
  rdfs:subClassOf mep:PipeFitting ;
.
mep:PipeFitting-CONNECTOR
  rdf:type owl:Class ;
  rdfs:comment "device generally consisting of a plate, toothed-plate or ring which, when partly embedded in each or in one of the contact faces of two members and held together by a connecting bolt, is capable of transmitting a load from one member to another"@en ;
  rdfs:comment "innretning som vanligvis består av en plate, en fortannet plate eller en ring, og som, når den er delvis trengt inn i alle eller i en av kontaktflatene på to komponenter og holdt sammen med en bolt, er i stand til å overføre en last fra en komponent til e"@nb-no ;
  rdfs:isDefinedBy <http://pi.pauwel.be/voc/distributionelement> ;
  rdfs:label "Connector"@en ;
  rdfs:label "Dübel"@de-de ;
  rdfs:label "connecteur"@fr-fr ;
  rdfs:label "forbindelse"@nb-no ;
  rdfs:label "forbindelsesledd"@nb-no ;
  rdfs:label "forbinder"@nb-no ;
  rdfs:seeAlso <http://bsdd.buildingsmart.org/#concept/details/3tvMvSswv0Dw7HoTwOQYKj> ;
  rdfs:seeAlso ifc:IfcPipeFittingEnumType ;
  rdfs:subClassOf mep:PipeFitting ;
.
mep:PipeFitting-ENTRY
  rdf:type owl:Class ;
  rdfs:comment "entry fitting, typically unconnected at one port and connected to a flow distribution system at the other (e.g., a breeching inlet)"@en ;
  rdfs:comment "entry fitting, typically unconnected at one port and connected to a flow distribution system at the other (e.g., a breeching inlet)"@en-gb ;
  rdfs:comment "entry fitting, typically unconnected at one port and connected to a flow distribution system at the other (e.g., an outside air duct system intake opening)"@en ;
  rdfs:comment "entry fitting, typically unconnected at one port and connected to a flow distribution system at the other (e.g., an outside air duct system intake opening)"@en-gb ;
  rdfs:isDefinedBy <http://pi.pauwel.be/voc/distributionelement> ;
  rdfs:label "Entry"@en ;
  rdfs:label "inngang"@nb-no ;
  rdfs:seeAlso <http://bsdd.buildingsmart.org/#concept/details/3iMmwy9iv0SBFB7w4cNsVs> ;
  rdfs:seeAlso ifc:IfcPipeFittingEnumType ;
  rdfs:subClassOf mep:PipeFitting ;
.
mep:PipeFitting-EXIT
  rdf:type owl:Class ;
  rdfs:isDefinedBy <http://pi.pauwel.be/voc/distributionelement> ;
  rdfs:label "Exit"@en ;
  rdfs:label "utgang"@nb-no ;
  rdfs:seeAlso <http://bsdd.buildingsmart.org/#concept/details/1vLJsY3MX6I8Ss72zp5sN_> ;
  rdfs:seeAlso ifc:IfcPipeFittingEnumType ;
  rdfs:subClassOf mep:PipeFitting ;
.
mep:PipeFitting-JUNCTION
  rdf:type owl:Class ;
  rdfs:comment "a fitting with typically more than two ports used to redistribute flow among the ports and/or to change the direction of flow between connected elements (e.g, tee, cross, wye, etc.)"@en ;
  rdfs:comment "a fitting with typically more than two ports used to redistribute flow among the ports and/or to change the direction of flow between connected elements (e.g, tee, cross, wye, etc.)."@en-gb ;
  rdfs:isDefinedBy <http://pi.pauwel.be/voc/distributionelement> ;
  rdfs:label "Junction"@en ;
  rdfs:label "gren"@nb-no ;
  rdfs:label "grenrør"@nb-no ;
  rdfs:label "kryss"@nb-no ;
  rdfs:seeAlso <http://bsdd.buildingsmart.org/#concept/details/2OzMql95b8ouXEzC1oYarB> ;
  rdfs:seeAlso ifc:IfcPipeFittingEnumType ;
  rdfs:subClassOf mep:PipeFitting ;
.
mep:PipeFitting-OBSTRUCTION
  rdf:type owl:Class ;
  rdfs:isDefinedBy <http://pi.pauwel.be/voc/distributionelement> ;
  rdfs:label "Obstruction"@en ;
  rdfs:label "hindring"@nb-no ;
  rdfs:seeAlso <http://bsdd.buildingsmart.org/#concept/details/2gXay6NOz7NPfYIUbDxtmF> ;
  rdfs:seeAlso ifc:IfcPipeFittingEnumType ;
  rdfs:subClassOf mep:PipeFitting ;
.
mep:PipeFitting-TRANSITION
  rdf:type owl:Class ;
  rdfs:isDefinedBy <http://pi.pauwel.be/voc/distributionelement> ;
  rdfs:label "Transition"@en ;
  rdfs:label "overgang"@nb-no ;
  rdfs:seeAlso <http://bsdd.buildingsmart.org/#concept/details/0mLpncHvn8AguL5g1sYDP7> ;
  rdfs:seeAlso ifc:IfcPipeFittingEnumType ;
  rdfs:subClassOf mep:PipeFitting ;
.
mep:PipeSegment
  rdf:type owl:Class ;
  rdfs:comment "A segment is used to typically join two sections of a piping network."@en ;
  rdfs:isDefinedBy <http://pi.pauwel.be/voc/distributionelement> ;
  rdfs:label "Pipe Segment"@en ;
  rdfs:label "Rohr"@de-de ;
  rdfs:label "Tronçon de tuyauterie"@fr-fr ;
  rdfs:label "rørdel"@nb-no ;
  rdfs:seeAlso <http://bsdd.buildingsmart.org/#concept/details/27v4E0qV8HuO00025QrE$V> ;
  rdfs:seeAlso ifc:IfcPipeSegment ;
  rdfs:subClassOf mep:FlowSegment ;
.
mep:PipeSegment-CULVERT
  rdf:type owl:Class ;
  rdfs:isDefinedBy <http://pi.pauwel.be/voc/distributionelement> ;
  rdfs:label "Culvert"@en ;
  rdfs:label "kulvert"@nb-no ;
  rdfs:seeAlso <http://bsdd.buildingsmart.org/#concept/details/0kbHQAKHrDHfD6TQOe$Myu> ;
  rdfs:seeAlso ifc:IfcPipeSegmentEnumType ;
  rdfs:subClassOf mep:PipeSegment ;
.
mep:PipeSegment-FLEXIBLESEGMENT
  rdf:type owl:Class ;
  rdfs:isDefinedBy <http://pi.pauwel.be/voc/distributionelement> ;
  rdfs:label "Flexible Pipe Segment"@en ;
  rdfs:label "fleksibel delflate"@nb-no ;
  rdfs:label "fleksibel rørdel"@nb-no ;
  rdfs:seeAlso <http://bsdd.buildingsmart.org/#concept/details/0bMKZ$AyPEsOOwHPCXcOcT> ;
  rdfs:seeAlso ifc:IfcPipeSegmentEnumType ;
  rdfs:subClassOf mep:PipeSegment ;
.
mep:PipeSegment-GUTTER
  rdf:type owl:Class ;
  rdfs:comment "A gutter situated outside the building and supported by brackets"@en ;
  rdfs:comment "En renne som støttes av rennekroker og som er plassert på utsiden av bygningen for å lede bort regnvann."@nb-no ;
  rdfs:comment "Takrenne"@nb-no ;
  rdfs:isDefinedBy <http://pi.pauwel.be/voc/distributionelement> ;
  rdfs:label "Gutter"@en ;
  rdfs:label "eaves gutter"@en ;
  rdfs:label "renne"@nb-no ;
  rdfs:label "takrenne"@nb-no ;
  rdfs:seeAlso <http://bsdd.buildingsmart.org/#concept/details/2deKArJfvCcR42exJCfGfR> ;
  rdfs:seeAlso ifc:IfcPipeSegmentEnumType ;
  rdfs:subClassOf mep:PipeSegment ;
.
mep:PipeSegment-RIGIDSEGMENT
  rdf:type owl:Class ;
  rdfs:comment "a rigid segment is a continuous linear segment of pipe that cannot be deformed"@en ;
  rdfs:comment "a rigid segment is a continuous linear segment of pipe that cannot be deformed"@en-gb ;
  rdfs:isDefinedBy <http://pi.pauwel.be/voc/distributionelement> ;
  rdfs:label "Rigid Pipe Segment"@en ;
  rdfs:label "stiv delflate"@nb-no ;
  rdfs:seeAlso <http://bsdd.buildingsmart.org/#concept/details/0oZaW79IT5rfrDH337Wczh> ;
  rdfs:seeAlso ifc:IfcPipeSegmentEnumType ;
  rdfs:subClassOf mep:PipeSegment ;
.
mep:PipeSegment-SPOOL
  rdf:type owl:Class ;
  rdfs:comment "a type of rigid segment that is typically shorter and used for providing connectivity within a piping network"@en ;
  rdfs:comment "a type of rigid segment that is typically shorter and used for providing connectivity within a piping network"@en-gb ;
  rdfs:isDefinedBy <http://pi.pauwel.be/voc/distributionelement> ;
  rdfs:label "Spool"@en ;
  rdfs:seeAlso <http://bsdd.buildingsmart.org/#concept/details/1XnqgBB0b5Ehi3OXV3HNVt> ;
  rdfs:seeAlso ifc:IfcPipeSegmentEnumType ;
  rdfs:subClassOf mep:PipeSegment ;
.
mep:ProtectiveDevice
  rdf:type owl:Class ;
  rdfs:comment """A device breaks an electrical circuit when a stated electric current that passes through it is exceeded.
Provides protection against electrical current only (not as a general protective device)."""@en ;
  rdfs:isDefinedBy <http://pi.pauwel.be/voc/distributionelement> ;
  rdfs:label "Protective Device"@en ;
  rdfs:label "Sicherung"@de-de ;
  rdfs:label "beskyttende enhet"@nb-no ;
  rdfs:label "équipement de protection"@fr-fr ;
  rdfs:seeAlso <http://bsdd.buildingsmart.org/#concept/details/127XSeDXvD5haPLRkC8eyd> ;
  rdfs:seeAlso ifc:IfcProtectiveDevice ;
  rdfs:subClassOf mep:FlowController ;
.
mep:ProtectiveDevice-CIRCUITBREAKER
  rdf:type owl:Class ;
  rdfs:isDefinedBy <http://pi.pauwel.be/voc/distributionelement> ;
  rdfs:label "Circuit Breaker"@en ;
  rdfs:label "strømbryter"@nb-no ;
  rdfs:seeAlso <http://bsdd.buildingsmart.org/#concept/details/3EWAB3Ur5Cng3zn8b4wZEE> ;
  rdfs:seeAlso ifc:IfcProtectiveDeviceEnumType ;
  rdfs:subClassOf mep:ProtectiveDevice ;
.
mep:ProtectiveDevice-EARTHINGSWITCH
  rdf:type owl:Class ;
  rdfs:comment "a safety device used to open or close a circuit when there is no current. used to isolate a part of a circuit, a machine, a part of an overhead line or an underground line so that maintenance can be safely conducted"@en ;
  rdfs:comment "a safety device used to open or close a circuit when there is no current. used to isolate a part of a circuit, a machine, a part of an overhead line or an underground line so that maintenance can be safely conducted"@en-gb ;
  rdfs:isDefinedBy <http://pi.pauwel.be/voc/distributionelement> ;
  rdfs:label "Earthing Switch"@en ;
  rdfs:label "jordingsbryter"@nb-no ;
  rdfs:seeAlso <http://bsdd.buildingsmart.org/#concept/details/2q5Q9N9Az1Oh7iRLNISzdt> ;
  rdfs:seeAlso ifc:IfcProtectiveDeviceEnumType ;
  rdfs:subClassOf mep:ProtectiveDevice ;
.
mep:ProtectiveDevice-EARTHLEAKAGECIRCUITBREAKER
  rdf:type owl:Class ;
  rdfs:comment "a device that opens, closes, or isolates a circuit and has short circuit protection but no overload protection. it attempts to break the circuit when there is a leakage of current from phase to earth, by measuring voltage on the earth conductor"@en ;
  rdfs:comment "a device that opens, closes, or isolates a circuit and has short circuit protection but no overload protection. it attempts to break the circuit when there is a leakage of current from phase to earth, by measuring voltage on the earth conductor"@en-gb ;
  rdfs:isDefinedBy <http://pi.pauwel.be/voc/distributionelement> ;
  rdfs:label "Earth Leakage Circuit Breaker"@en ;
  rdfs:label "lekkstrømsikring"@nb-no ;
  rdfs:seeAlso <http://bsdd.buildingsmart.org/#concept/details/2h1MphDsfAOOGX2jycslmC> ;
  rdfs:seeAlso ifc:IfcProtectiveDeviceEnumType ;
  rdfs:subClassOf mep:ProtectiveDevice ;
.
mep:ProtectiveDevice-FUSEDISCONNECTOR
  rdf:type owl:Class ;
  rdfs:comment "a device that will electrically open the circuit after a period of prolonged, abnormal current flow"@en ;
  rdfs:isDefinedBy <http://pi.pauwel.be/voc/distributionelement> ;
  rdfs:label "Fuse Disconnector"@en ;
  rdfs:label "sikringskopling"@nb-no ;
  rdfs:seeAlso <http://bsdd.buildingsmart.org/#concept/details/2TfJqRtl5EbAjQ1_2wg3W9> ;
  rdfs:seeAlso ifc:IfcProtectiveDeviceEnumType ;
  rdfs:subClassOf mep:ProtectiveDevice ;
.
mep:ProtectiveDevice-RESIDUALCURRENTCIRCUITBREAKER
  rdf:type owl:Class ;
  rdfs:isDefinedBy <http://pi.pauwel.be/voc/distributionelement> ;
  rdfs:label "Residual Current Circuit Breaker"@en ;
  rdfs:seeAlso <http://bsdd.buildingsmart.org/#concept/details/2RbnT6FAn6fxAlZWiSgJ_I> ;
  rdfs:seeAlso ifc:IfcProtectiveDeviceEnumType ;
  rdfs:subClassOf mep:ProtectiveDevice ;
.
mep:ProtectiveDevice-RESIDUALCURRENTSWITCH
  rdf:type owl:Class ;
  rdfs:comment "a device that opens, closes or isolates a circuit and has no short circuit or overload protection. May also be identified as a 'ground fault switch'"@en ;
  rdfs:comment "a device that opens, closes or isolates a circuit and has no short circuit or overload protection. May also be identified as a 'ground fault switch'"@en-gb ;
  rdfs:isDefinedBy <http://pi.pauwel.be/voc/distributionelement> ;
  rdfs:label "Residual Current Switch"@en ;
  rdfs:label "reststrømsbryter"@nb-no ;
  rdfs:seeAlso <http://bsdd.buildingsmart.org/#concept/details/1P$J7BP319XvA_F1$sO9sN> ;
  rdfs:seeAlso ifc:IfcProtectiveDeviceEnumType ;
  rdfs:subClassOf mep:ProtectiveDevice ;
.
mep:ProtectiveDevice-VARISTOR
  rdf:type owl:Class ;
  rdfs:comment "a high voltage surge protection device"@en ;
  rdfs:comment "a high voltage surge protection device"@en-gb ;
  rdfs:isDefinedBy <http://pi.pauwel.be/voc/distributionelement> ;
  rdfs:label "Varistor"@en ;
  rdfs:label "varistor"@nb-no ;
  rdfs:seeAlso <http://bsdd.buildingsmart.org/#concept/details/3DtLJ1DjT4LOUFArBkjO_e> ;
  rdfs:seeAlso ifc:IfcProtectiveDeviceEnumType ;
  rdfs:subClassOf mep:ProtectiveDevice ;
.
mep:ProtectiveDeviceTrippingUnit
  rdf:type owl:Class ;
  rdfs:comment "A protective device breaks an electrical circuit at a separate breaking unit when a stated electric current that passes through the unit is exceeded."@en ;
  rdfs:isDefinedBy <http://pi.pauwel.be/voc/distributionelement> ;
  rdfs:label "Protective Device Tripping Unit"@en ;
  rdfs:label "Sicherungsschalter"@de-de ;
  rdfs:label "Unité de déclenchement d'équipement de protection"@fr-fr ;
  rdfs:label "beskyttende aktiveringsenhet"@nb-no ;
  rdfs:seeAlso <http://bsdd.buildingsmart.org/#concept/details/2XAj9nULf1_vBAY_PiQTNv> ;
  rdfs:seeAlso ifc:IfcProtectiveDeviceTrippingUnit ;
  rdfs:subClassOf mep:DistributionControlElement ;
.
mep:ProtectiveDeviceTrippingUnit-ELECTROMAGNETIC
  rdf:type owl:Class ;
  rdfs:comment "a tripping unit activated by electromagnetic action"@en ;
  rdfs:comment "a tripping unit activated by electromagnetic action"@en-gb ;
  rdfs:isDefinedBy <http://pi.pauwel.be/voc/distributionelement> ;
  rdfs:label "Electro-magnetic"@en ;
  rdfs:label "elektromagnetisk"@nb-no ;
  rdfs:seeAlso <http://bsdd.buildingsmart.org/#concept/details/1snzfjLSb6VxQ6A4KikKSh> ;
  rdfs:seeAlso ifc:IfcProtectiveDeviceTrippingUnitEnumType ;
  rdfs:subClassOf mep:ProtectiveDeviceTrippingUnit ;
.
mep:ProtectiveDeviceTrippingUnit-ELECTRONIC
  rdf:type owl:Class ;
  rdfs:comment "a tripping unit activated by electronic action"@en ;
  rdfs:comment "a tripping unit activated by electronic action"@en-gb ;
  rdfs:isDefinedBy <http://pi.pauwel.be/voc/distributionelement> ;
  rdfs:label "Electronic"@en ;
  rdfs:label "elektronisk"@nb-no ;
  rdfs:seeAlso <http://bsdd.buildingsmart.org/#concept/details/3LipcBG$z8SuRRCttfOFHZ> ;
  rdfs:seeAlso ifc:IfcProtectiveDeviceTrippingUnitEnumType ;
  rdfs:subClassOf mep:ProtectiveDeviceTrippingUnit ;
.
mep:ProtectiveDeviceTrippingUnit-RESIDUALCURRENT
  rdf:type owl:Class ;
  rdfs:comment "a tripping unit activated by residual current detection."@en ;
  rdfs:isDefinedBy <http://pi.pauwel.be/voc/distributionelement> ;
  rdfs:label "Residual Current"@en ;
  rdfs:label "jording"@nb-no ;
  rdfs:seeAlso <http://bsdd.buildingsmart.org/#concept/details/09h4iCV3XArhCUFOXrUJzB> ;
  rdfs:seeAlso ifc:IfcProtectiveDeviceTrippingUnitEnumType ;
  rdfs:subClassOf mep:ProtectiveDeviceTrippingUnit ;
.
mep:ProtectiveDeviceTrippingUnit-THERMAL
  rdf:type owl:Class ;
  rdfs:comment "a tripping unit activated by thermal action"@en ;
  rdfs:comment "a tripping unit activated by thermal action"@en-gb ;
  rdfs:isDefinedBy <http://pi.pauwel.be/voc/distributionelement> ;
  rdfs:label "Thermal"@en ;
  rdfs:label "termisk aktiveringsenhet"@nb-no ;
  rdfs:seeAlso <http://bsdd.buildingsmart.org/#concept/details/1xk5ZOrXj7hxv7ViGvtyU$> ;
  rdfs:seeAlso ifc:IfcProtectiveDeviceTrippingUnitEnumType ;
  rdfs:subClassOf mep:ProtectiveDeviceTrippingUnit ;
.
mep:Pump
  rdf:type owl:Class ;
  rdfs:comment "A device which imparts mechanical work on fluids to move them through a channel or pipe. "@en ;
  rdfs:comment "An equipment driven by a prime mover in which energy is either constantly or periodically added to an amount of pumped liquid in order to increase the pressure requiered for the process in which the pump is in operation.        "@en ;
  rdfs:isDefinedBy <http://pi.pauwel.be/voc/distributionelement> ;
  rdfs:label "Pump"@en ;
  rdfs:label "Pumpe"@da ;
  rdfs:label "Pumpe"@de-de ;
  rdfs:label "pomp"@nl-nl ;
  rdfs:label "pompe"@fr-fr ;
  rdfs:label "pump"@en ;
  rdfs:label "pumpe"@nb-no ;
  rdfs:seeAlso <http://bsdd.buildingsmart.org/#concept/details/1xPUW0qVuHuO00025QrE$V> ;
  rdfs:seeAlso ifc:IfcPump ;
  rdfs:subClassOf mep:FlowMovingDevice ;
.
mep:Pump-CIRCULATOR
  rdf:type owl:Class ;
  rdfs:comment "a circulator pump is a generic low-pressure, low-capacity pump. it may have a wet rotor and may be driven by a flexible-coupled motor"@en ;
  rdfs:comment "a circulator pump is a generic low-pressure, low-capacity pump. it may have a wet rotor and may be driven by a flexible-coupled motor"@en-gb ;
  rdfs:isDefinedBy <http://pi.pauwel.be/voc/distributionelement> ;
  rdfs:label "Circulator Pump"@en ;
  rdfs:label "sirkulasjonspumpe"@nb-no ;
  rdfs:seeAlso <http://bsdd.buildingsmart.org/#concept/details/3FNSRucOX3Mfl_kibtqQRr> ;
  rdfs:seeAlso ifc:IfcPumpEnumType ;
  rdfs:subClassOf mep:Pump ;
.
mep:Pump-ENDSUCTION
  rdf:type owl:Class ;
  rdfs:comment "an end suction pump, when mounted horizontally, has a single horizontal inlet on the impeller suction side and a vertical discharge. it may have a direct or close-coupled motor"@en ;
  rdfs:comment "an end suction pump, when mounted horizontally, has a single horizontal inlet on the impeller suction side and a vertical discharge. it may have a direct or close-coupled motor"@en-gb ;
  rdfs:isDefinedBy <http://pi.pauwel.be/voc/distributionelement> ;
  rdfs:label "End Suction Pump"@en ;
  rdfs:label "aksialt innløp"@nb-no ;
  rdfs:seeAlso <http://bsdd.buildingsmart.org/#concept/details/10iAdjK6fEqxsxJnj_WSZS> ;
  rdfs:seeAlso ifc:IfcPumpEnumType ;
  rdfs:subClassOf mep:Pump ;
.
mep:Pump-SPLITCASE
  rdf:type owl:Class ;
  rdfs:comment "a split case pump, when mounted horizontally, has an inlet and outlet on each side of the impeller. the impeller can be easily accessed by removing the front of the impeller casing. It may have a direct or close-coupled motor"@en ;
  rdfs:comment "a split case pump, when mounted horizontally, has an inlet and outlet on each side of the impeller. the impeller can be easily accessed by removing the front of the impeller casing. It may have a direct or close-coupled motor"@en-gb ;
  rdfs:isDefinedBy <http://pi.pauwel.be/voc/distributionelement> ;
  rdfs:label "Split Case Pump"@en ;
  rdfs:label "splitcase pumpe"@nb-no ;
  rdfs:seeAlso <http://bsdd.buildingsmart.org/#concept/details/3HSu1GQ8T9gQrSbYugJB2f> ;
  rdfs:seeAlso ifc:IfcPumpEnumType ;
  rdfs:subClassOf mep:Pump ;
.
mep:Pump-SUBMERSIBLEPUMP
  rdf:type owl:Class ;
  rdfs:isDefinedBy <http://pi.pauwel.be/voc/distributionelement> ;
  rdfs:label "Submersible Pump"@en ;
  rdfs:seeAlso <http://bsdd.buildingsmart.org/#concept/details/0rpKGArwf1S8H9bk1lkPiT> ;
  rdfs:seeAlso ifc:IfcPumpEnumType ;
  rdfs:subClassOf mep:Pump ;
.
mep:Pump-SUMPPUMP
  rdf:type owl:Class ;
  rdfs:comment "a pump designed to sit above a collection tank with a suction inlet extending into the tank"@en ;
  rdfs:comment "a pump designed to sit above a collection tank with a suction inlet extending into the tank"@en-gb ;
  rdfs:isDefinedBy <http://pi.pauwel.be/voc/distributionelement> ;
  rdfs:label "Sump Pump"@en ;
  rdfs:label "tørroppstilt pumpe"@nb-no ;
  rdfs:seeAlso <http://bsdd.buildingsmart.org/#concept/details/2WUDpiKfDE5u4DZMLBdExr> ;
  rdfs:seeAlso ifc:IfcPumpEnumType ;
  rdfs:subClassOf mep:Pump ;
.
mep:Pump-VERTICALINLINE
  rdf:type owl:Class ;
  rdfs:comment "a vertical Inline pump has the pump and motor close-coupled on the pump casing. the pump depends on the connected, horizontal piping for support, with the suction and discharge along the piping axis"@en ;
  rdfs:comment "a vertical Inline pump has the pump and motor close-coupled on the pump casing. the pump depends on the connected, horizontal piping for support, with the suction and discharge along the piping axis"@en-gb ;
  rdfs:isDefinedBy <http://pi.pauwel.be/voc/distributionelement> ;
  rdfs:label "Vertical Inline"@en ;
  rdfs:label "vertikallinje"@nb-no ;
  rdfs:seeAlso <http://bsdd.buildingsmart.org/#concept/details/0J3vLYrIDCfQEZZ8ZeRATw> ;
  rdfs:seeAlso <http://bsdd.buildingsmart.org/#concept/details/0VvmpeacrFf8rnDj2jyghe> ;
  rdfs:seeAlso ifc:IfcPumpEnumType ;
  rdfs:subClassOf mep:Pump ;
.
mep:Pump-VERTICALTURBINE
  rdf:type owl:Class ;
  rdfs:comment "a vertical turbine pump has a motor mounted vertically on the pump casing for either wet-pit sump mounting or dry-well mounting"@en ;
  rdfs:comment "a vertical turbine pump has a motor mounted vertically on the pump casing for either wet-pit sump mounting or dry-well mounting"@en-gb ;
  rdfs:isDefinedBy <http://pi.pauwel.be/voc/distributionelement> ;
  rdfs:label "Vertical Turbine"@en ;
  rdfs:label "vertikalpumpe"@nb-no ;
  rdfs:seeAlso <http://bsdd.buildingsmart.org/#concept/details/3Ld4kSekL8MOEqs2litt5v> ;
  rdfs:seeAlso ifc:IfcPumpEnumType ;
  rdfs:subClassOf mep:Pump ;
.
mep:SanitaryTerminal
  rdf:type owl:Class ;
  rdfs:comment "A fixed appliance or terminal usually supplied with water and used for drinking, cleaning or foul water disposal or that is an item of equipment directly used with such an appliance or terminal."@en ;
  rdfs:isDefinedBy <http://pi.pauwel.be/voc/distributionelement> ;
  rdfs:label "Equipement sanitaire"@fr-fr ;
  rdfs:label "Sanitair toestel"@nl-nl ;
  rdfs:label "Sanitary Terminal"@en ;
  rdfs:label "Sanitäreinrichtung"@de-de ;
  rdfs:label "sanitærstasjon"@nb-no ;
  rdfs:seeAlso <http://bsdd.buildingsmart.org/#concept/details/2JIcddz_X75xhHc1XUv7d2> ;
  rdfs:seeAlso ifc:IfcSanitaryTerminal ;
  rdfs:subClassOf mep:FlowTerminal ;
.
mep:SanitaryTerminal-BATH
  rdf:type owl:Class ;
  rdfs:comment "Badekar"@nb-no ;
  rdfs:comment "Badekar, generisk, modelleres av ARK i tidlig fase"@nb-no ;
  rdfs:comment "Sanitärobjekt, das der persönlichen Hygiene, vorzugsweise dem Baden und vollständigen Reinigen des menschlichen Körpers dient und mit das Wasser nach dem Gebrauch über ein Ablaufloch abgeleitet werden kann"@de-de ;
  rdfs:comment "badekar, generisk, arkitekttegnede modeller i tidlige designfaser"@dk-dk ;
  rdfs:comment "badkar, allmänt, arkitektens modeller under utformningens första steg"@sv-se ;
  rdfs:comment "baignoire, générique, modeles par l'architecte dans les premières étapes de la conception"@fr-fr ;
  rdfs:comment "sanitary appliance used for partial immersion and washing of the human body or parts of it, and for directing water to a waste outlet after use"@en ;
  rdfs:comment "sanitary appliance used for partial immersion and washing of the human body or parts of it, and for directing water to a waste outlet after use"@en-gb ;
  rdfs:comment "sanitærinnretning som brukes for delvis nedsenking og vasking av menneskekropp eller deler av den, og for å lede vann til et avløp etter bruk"@nb-no ;
  rdfs:comment "varhaisten arkkitehtisuunnitteluvaiheiden yleismalliset kylpyammeet"@fi-fi ;
  rdfs:isDefinedBy <http://pi.pauwel.be/voc/distributionelement> ;
  rdfs:label "Badewanne"@de-de ;
  rdfs:label "Bath"@en ;
  rdfs:label "bad"@dk-dk ;
  rdfs:label "bad"@nb-no ;
  rdfs:label "bad"@nl-nl ;
  rdfs:label "bad"@sv-se ;
  rdfs:label "badekar generisk"@nb-no ;
  rdfs:label "badekar"@nb-no ;
  rdfs:label "baignoire"@fr-fr ;
  rdfs:label "bath"@en-gb ;
  rdfs:label "bathtub"@en ;
  rdfs:label "kylpyamme"@fi-fi ;
  rdfs:label "wanna"@pl-pl ;
  rdfs:seeAlso <http://bsdd.buildingsmart.org/#concept/details/3obubztQ19OANL1cKUM33Z> ;
  rdfs:seeAlso ifc:IfcSanitaryTerminalEnumType ;
  rdfs:subClassOf mep:SanitaryTerminal ;
.
mep:SanitaryTerminal-BIDET
  rdf:type owl:Class ;
  rdfs:comment "Waste water appliance for washing the excretory organs while sitting astride the bowl"@en-gb ;
  rdfs:comment "waste water appliance for washing the excretory organs while sitting astride the bowl"@en ;
  rdfs:isDefinedBy <http://pi.pauwel.be/voc/distributionelement> ;
  rdfs:label "Bidet"@en ;
  rdfs:label "bidè"@nb-no ;
  rdfs:label "bidé"@nb-no ;
  rdfs:seeAlso <http://bsdd.buildingsmart.org/#concept/details/1OsGeXUlz249AKQbE4k_3S> ;
  rdfs:seeAlso ifc:IfcSanitaryTerminalEnumType ;
  rdfs:subClassOf mep:SanitaryTerminal ;
.
mep:SanitaryTerminal-CISTERN
  rdf:type owl:Class ;
  rdfs:comment "A water storage unit attached to a sanitary terminal that is fitted with a device, operated automatically or by the user, that discharges water to cleanse a water closet (toilet) pan, urinal or slop hopper"@en ;
  rdfs:comment "A water storage unit attached to a sanitary terminal that is fitted with a device, operated automatically or by the user, that discharges water to cleanse a water closet (toilet) pan, urinal or slop hopper"@en-gb ;
  rdfs:isDefinedBy <http://pi.pauwel.be/voc/distributionelement> ;
  rdfs:label "Cistern"@en ;
  rdfs:label "sisterne"@nb-no ;
  rdfs:seeAlso <http://bsdd.buildingsmart.org/#concept/details/2jTiagbH96wBuf5tVceOCR> ;
  rdfs:seeAlso ifc:IfcSanitaryTerminalEnumType ;
  rdfs:subClassOf mep:SanitaryTerminal ;
.
mep:SanitaryTerminal-SANITARYFOUNTAIN
  rdf:type owl:Class ;
  rdfs:isDefinedBy <http://pi.pauwel.be/voc/distributionelement> ;
  rdfs:label "Sanitary Fountain"@en ;
  rdfs:label "drikkefontene"@nb-no ;
  rdfs:seeAlso <http://bsdd.buildingsmart.org/#concept/details/3sjNvgHdPAH8fM1jgV3823> ;
  rdfs:seeAlso ifc:IfcSanitaryTerminalEnumType ;
  rdfs:subClassOf mep:SanitaryTerminal ;
.
mep:SanitaryTerminal-SHOWER
  rdf:type owl:Class ;
  rdfs:comment "Dusj beskyttet med kabinett"@nb-no ;
  rdfs:comment "Dusjhjørne"@nb-no ;
  rdfs:comment "Shower installed in its own cabinet"@en ;
  rdfs:isDefinedBy <http://pi.pauwel.be/voc/distributionelement> ;
  rdfs:label "Shower"@en ;
  rdfs:label "dusj"@nb-no ;
  rdfs:label "dusjhjørne"@nb-no ;
  rdfs:label "dusjkabinett"@nb-no ;
  rdfs:label "shower cabinet"@en ;
  rdfs:seeAlso <http://bsdd.buildingsmart.org/#concept/details/0epJRcLij1_O8OcMA6Y0WR> ;
  rdfs:seeAlso ifc:IfcSanitaryTerminalEnumType ;
  rdfs:subClassOf mep:SanitaryTerminal ;
.
mep:SanitaryTerminal-SINK
  rdf:type owl:Class ;
  rdfs:comment "Servant"@nb-no ;
  rdfs:comment "Servant, generisk, modelleres av ARK i tidlig fase"@nb-no ;
  rdfs:comment "Vanlig stor"@nb-no ;
  rdfs:comment "beholder for vann under kran til vasking av hender og ansikt"@nb-no ;
  rdfs:comment "container for water located below water dispenser, used for washing hands and face"@en ;
  rdfs:isDefinedBy <http://pi.pauwel.be/voc/distributionelement> ;
  rdfs:label "Sink"@en ;
  rdfs:label "kjøkken"@nb-no ;
  rdfs:label "servant generisk"@nb-no ;
  rdfs:label "servant"@nb-no ;
  rdfs:label "utslagsvask"@nb-no ;
  rdfs:label "vask"@nb-no ;
  rdfs:label "wash basin"@en ;
  rdfs:seeAlso <http://bsdd.buildingsmart.org/#concept/details/1SP1BV0Wj9lf1y$D1yvjLF> ;
  rdfs:seeAlso ifc:IfcSanitaryTerminalEnumType ;
  rdfs:subClassOf mep:SanitaryTerminal ;
.
mep:SanitaryTerminal-TOILETPAN
  rdf:type owl:Class ;
  rdfs:comment "soil appliance for the disposal of excrement"@en ;
  rdfs:comment "soil appliance for the disposal of excrement"@en-gb ;
  rdfs:isDefinedBy <http://pi.pauwel.be/voc/distributionelement> ;
  rdfs:label "Toilet Pan"@en ;
  rdfs:label "toalettskål"@nb-no ;
  rdfs:seeAlso <http://bsdd.buildingsmart.org/#concept/details/2DXU$3jIrFROZFEhM3vmoY> ;
  rdfs:seeAlso ifc:IfcSanitaryTerminalEnumType ;
  rdfs:subClassOf mep:SanitaryTerminal ;
.
mep:SanitaryTerminal-URINAL
  rdf:type owl:Class ;
  rdfs:comment "soil appliance that receives urine and directs it to a waste outlet"@en ;
  rdfs:comment "soil appliance that receives urine and directs it to a waste outlet"@en-gb ;
  rdfs:isDefinedBy <http://pi.pauwel.be/voc/distributionelement> ;
  rdfs:label "Urinal"@en ;
  rdfs:label "urinal"@nb-no ;
  rdfs:seeAlso <http://bsdd.buildingsmart.org/#concept/details/2B1zvMQAv9pPzzlnNtd5xA> ;
  rdfs:seeAlso ifc:IfcSanitaryTerminalEnumType ;
  rdfs:subClassOf mep:SanitaryTerminal ;
.
mep:SanitaryTerminal-WASHHANDBASIN
  rdf:type owl:Class ;
  rdfs:comment "waste water appliance for washing the upper parts of the body"@en ;
  rdfs:comment "waste water appliance for washing the upper parts of the body"@en-gb ;
  rdfs:isDefinedBy <http://pi.pauwel.be/voc/distributionelement> ;
  rdfs:label "Wash Hand Basin"@en ;
  rdfs:label "håndvask"@nb-no ;
  rdfs:seeAlso <http://bsdd.buildingsmart.org/#concept/details/2FTLxQE_19NPX9OHQSeAff> ;
  rdfs:seeAlso ifc:IfcSanitaryTerminalEnumType ;
  rdfs:subClassOf mep:SanitaryTerminal ;
.
mep:SanitaryTerminal-WCSEAT
  rdf:type owl:Class ;
  rdfs:comment "hinged seat that fits on the top of a water closet (WC) pan"@en ;
  rdfs:comment "hinged seat that fits on the top of a water closet (WC) pan"@en-gb ;
  rdfs:isDefinedBy <http://pi.pauwel.be/voc/distributionelement> ;
  rdfs:label "WC Seat"@en ;
  rdfs:label "toalettsete"@nb-no ;
  rdfs:seeAlso <http://bsdd.buildingsmart.org/#concept/details/12WSI21rv3UfKISz44T3B5> ;
  rdfs:seeAlso ifc:IfcSanitaryTerminalEnumType ;
  rdfs:subClassOf mep:SanitaryTerminal ;
.
mep:Sensor
  rdf:type owl:Class ;
  rdfs:comment "A device that measures a physical quantity and converts it into a signal which can be read by an observer or by an instrument."@en ;
  rdfs:isDefinedBy <http://pi.pauwel.be/voc/distributionelement> ;
  rdfs:label "Capteur"@fr-fr ;
  rdfs:label "Sensor"@de-de ;
  rdfs:label "Sensor"@en ;
  rdfs:label "sensor"@nb-no ;
  rdfs:label "sensor"@nl-nl ;
  rdfs:seeAlso <http://bsdd.buildingsmart.org/#concept/details/0fBybaDK56PuAX2mD3nQsg> ;
  rdfs:seeAlso ifc:IfcSensor ;
  rdfs:subClassOf mep:DistributionControlElement ;
.
mep:Sensor-CO2SENSOR
  rdf:type owl:Class ;
  rdfs:isDefinedBy <http://pi.pauwel.be/voc/distributionelement> ;
  rdfs:label "CO2Sensor"@en ;
  rdfs:seeAlso ifc:IfcSensorEnumType ;
  rdfs:subClassOf mep:Sensor ;
.
mep:Sensor-CONDUCTANCESENSOR
  rdf:type owl:Class ;
  rdfs:isDefinedBy <http://pi.pauwel.be/voc/distributionelement> ;
  rdfs:label "Conductance Sensor"@en ;
  rdfs:seeAlso <http://bsdd.buildingsmart.org/#concept/details/3B3V_G55z9nPyFZOVtZKu9> ;
  rdfs:seeAlso ifc:IfcSensorEnumType ;
  rdfs:subClassOf mep:Sensor ;
.
mep:Sensor-CONTACTSENSOR
  rdf:type owl:Class ;
  rdfs:isDefinedBy <http://pi.pauwel.be/voc/distributionelement> ;
  rdfs:label "Contact Sensor"@en ;
  rdfs:seeAlso <http://bsdd.buildingsmart.org/#concept/details/37ufVjEi1BZwCCYTaYZdgK> ;
  rdfs:seeAlso ifc:IfcSensorEnumType ;
  rdfs:subClassOf mep:Sensor ;
.
mep:Sensor-FIRESENSOR
  rdf:type owl:Class ;
  rdfs:isDefinedBy <http://pi.pauwel.be/voc/distributionelement> ;
  rdfs:label "Fire Sensor"@en ;
  rdfs:seeAlso <http://bsdd.buildingsmart.org/#concept/details/1uUUJfLpX03uy3ZC8j0YXd> ;
  rdfs:seeAlso ifc:IfcSensorEnumType ;
  rdfs:subClassOf mep:Sensor ;
.
mep:Sensor-FLOWSENSOR
  rdf:type owl:Class ;
  rdfs:isDefinedBy <http://pi.pauwel.be/voc/distributionelement> ;
  rdfs:label "Flow Sensor"@en ;
  rdfs:seeAlso <http://bsdd.buildingsmart.org/#concept/details/0uovCUrpn9leYila3fCeEN> ;
  rdfs:seeAlso ifc:IfcSensorEnumType ;
  rdfs:subClassOf mep:Sensor ;
.
mep:Sensor-FROSTSENSOR
  rdf:type owl:Class ;
  rdfs:isDefinedBy <http://pi.pauwel.be/voc/distributionelement> ;
  rdfs:label "Frost Sensor"@en ;
  rdfs:seeAlso ifc:IfcSensorEnumType ;
  rdfs:subClassOf mep:Sensor ;
.
mep:Sensor-GASSENSOR
  rdf:type owl:Class ;
  rdfs:isDefinedBy <http://pi.pauwel.be/voc/distributionelement> ;
  rdfs:label "Gas Sensor"@en ;
  rdfs:seeAlso <http://bsdd.buildingsmart.org/#concept/details/2EQoz$FyT5_wpwhtQt6Bt2> ;
  rdfs:seeAlso ifc:IfcSensorEnumType ;
  rdfs:subClassOf mep:Sensor ;
.
mep:Sensor-HEATSENSOR
  rdf:type owl:Class ;
  rdfs:isDefinedBy <http://pi.pauwel.be/voc/distributionelement> ;
  rdfs:label "Heat Sensor"@en ;
  rdfs:seeAlso <http://bsdd.buildingsmart.org/#concept/details/3Op4_nqmj6L96LAusX1Ytq> ;
  rdfs:seeAlso ifc:IfcSensorEnumType ;
  rdfs:subClassOf mep:Sensor ;
.
mep:Sensor-HUMIDITYSENSOR
  rdf:type owl:Class ;
  rdfs:isDefinedBy <http://pi.pauwel.be/voc/distributionelement> ;
  rdfs:label "Humidity Sensor"@en ;
  rdfs:seeAlso <http://bsdd.buildingsmart.org/#concept/details/3Pza_zqrDAwg4Pv44MusVg> ;
  rdfs:seeAlso ifc:IfcSensorEnumType ;
  rdfs:subClassOf mep:Sensor ;
.
mep:Sensor-IDENTIFIERSENSOR
  rdf:type owl:Class ;
  rdfs:isDefinedBy <http://pi.pauwel.be/voc/distributionelement> ;
  rdfs:label "Identifier Sensor"@en ;
  rdfs:seeAlso ifc:IfcSensorEnumType ;
  rdfs:subClassOf mep:Sensor ;
.
mep:Sensor-IONCONCENTRATIONSENSOR
  rdf:type owl:Class ;
  rdfs:isDefinedBy <http://pi.pauwel.be/voc/distributionelement> ;
  rdfs:label "Ion Concentration Sensor"@en ;
  rdfs:seeAlso <http://bsdd.buildingsmart.org/#concept/details/2MglfdfcTCuhCN57KBKgPd> ;
  rdfs:seeAlso ifc:IfcSensorEnumType ;
  rdfs:subClassOf mep:Sensor ;
.
mep:Sensor-LEVELSENSOR
  rdf:type owl:Class ;
  rdfs:isDefinedBy <http://pi.pauwel.be/voc/distributionelement> ;
  rdfs:label "Level Sensor"@en ;
  rdfs:seeAlso <http://bsdd.buildingsmart.org/#concept/details/2zHVmDmGT6zBRJIAqmQdkK> ;
  rdfs:seeAlso ifc:IfcSensorEnumType ;
  rdfs:subClassOf mep:Sensor ;
.
mep:Sensor-LIGHTSENSOR
  rdf:type owl:Class ;
  rdfs:isDefinedBy <http://pi.pauwel.be/voc/distributionelement> ;
  rdfs:label "Light Sensor"@en ;
  rdfs:seeAlso <http://bsdd.buildingsmart.org/#concept/details/3Y5B9ubBb0xxK9qw_nEkEk> ;
  rdfs:seeAlso ifc:IfcSensorEnumType ;
  rdfs:subClassOf mep:Sensor ;
.
mep:Sensor-MOISTURESENSOR
  rdf:type owl:Class ;
  rdfs:isDefinedBy <http://pi.pauwel.be/voc/distributionelement> ;
  rdfs:label "Moisture Sensor"@en ;
  rdfs:seeAlso <http://bsdd.buildingsmart.org/#concept/details/1LnA01HA5E7fPuuXLI2ZjZ> ;
  rdfs:seeAlso ifc:IfcSensorEnumType ;
  rdfs:subClassOf mep:Sensor ;
.
mep:Sensor-MOVEMENTSENSOR
  rdf:type owl:Class ;
  rdfs:isDefinedBy <http://pi.pauwel.be/voc/distributionelement> ;
  rdfs:label "Movement Sensor"@en ;
  rdfs:seeAlso <http://bsdd.buildingsmart.org/#concept/details/2$qvwDkgL0VRFBeuD9w9Si> ;
  rdfs:seeAlso ifc:IfcSensorEnumType ;
  rdfs:subClassOf mep:Sensor ;
.
mep:Sensor-PHSENSOR
  rdf:type owl:Class ;
  rdfs:isDefinedBy <http://pi.pauwel.be/voc/distributionelement> ;
  rdfs:label "PH-Sensor"@en ;
  rdfs:seeAlso <http://bsdd.buildingsmart.org/#concept/details/3lwBxJbnL9DAvFoYtIB3Li> ;
  rdfs:seeAlso ifc:IfcSensorEnumType ;
  rdfs:subClassOf mep:Sensor ;
.
mep:Sensor-PRESSURESENSOR
  rdf:type owl:Class ;
  rdfs:isDefinedBy <http://pi.pauwel.be/voc/distributionelement> ;
  rdfs:label "Pressure Sensor"@en ;
  rdfs:seeAlso <http://bsdd.buildingsmart.org/#concept/details/2RKICtIin2Rw5EFR0Z2J9j> ;
  rdfs:seeAlso ifc:IfcSensorEnumType ;
  rdfs:subClassOf mep:Sensor ;
.
mep:Sensor-RADIATIONSENSOR
  rdf:type owl:Class ;
  rdfs:isDefinedBy <http://pi.pauwel.be/voc/distributionelement> ;
  rdfs:label "Radiation Sensor"@en ;
  rdfs:seeAlso <http://bsdd.buildingsmart.org/#concept/details/3OXFVvFvPCePgxMcTylRzf> ;
  rdfs:seeAlso ifc:IfcSensorEnumType ;
  rdfs:subClassOf mep:Sensor ;
.
mep:Sensor-RADIOACTIVITYSENSOR
  rdf:type owl:Class ;
  rdfs:isDefinedBy <http://pi.pauwel.be/voc/distributionelement> ;
  rdfs:label "Radioactivity Sensor"@en ;
  rdfs:seeAlso <http://bsdd.buildingsmart.org/#concept/details/0wp1vLqNP9Lef8Pba4UI6P> ;
  rdfs:seeAlso ifc:IfcSensorEnumType ;
  rdfs:subClassOf mep:Sensor ;
.
mep:Sensor-SMOKESENSOR
  rdf:type owl:Class ;
  rdfs:isDefinedBy <http://pi.pauwel.be/voc/distributionelement> ;
  rdfs:label "Smoke Sensor"@en ;
  rdfs:seeAlso <http://bsdd.buildingsmart.org/#concept/details/05gekqn$D9nA81S2HC8u1E> ;
  rdfs:seeAlso ifc:IfcSensorEnumType ;
  rdfs:subClassOf mep:Sensor ;
.
mep:Sensor-SOUNDSENSOR
  rdf:type owl:Class ;
  rdfs:isDefinedBy <http://pi.pauwel.be/voc/distributionelement> ;
  rdfs:label "Sound Sensor"@en ;
  rdfs:seeAlso <http://bsdd.buildingsmart.org/#concept/details/0OvllOM7fDC8GX67w3ESF6> ;
  rdfs:seeAlso ifc:IfcSensorEnumType ;
  rdfs:subClassOf mep:Sensor ;
.
mep:Sensor-TEMPERATURESENSOR
  rdf:type owl:Class ;
  rdfs:isDefinedBy <http://pi.pauwel.be/voc/distributionelement> ;
  rdfs:label "Temperature Sensor"@en ;
  rdfs:seeAlso <http://bsdd.buildingsmart.org/#concept/details/2SmjV_2JXB4wdmD4Bzr$BP> ;
  rdfs:seeAlso ifc:IfcSensorEnumType ;
  rdfs:subClassOf mep:Sensor ;
.
mep:Sensor-WINDSENSOR
  rdf:type owl:Class ;
  rdfs:isDefinedBy <http://pi.pauwel.be/voc/distributionelement> ;
  rdfs:label "Wind Sensor"@en ;
  rdfs:seeAlso <http://bsdd.buildingsmart.org/#concept/details/1hMN0c8Rj5dw$7eow$VjWU> ;
  rdfs:seeAlso ifc:IfcSensorEnumType ;
  rdfs:subClassOf mep:Sensor ;
.
mep:SolarDevice
  rdf:type owl:Class ;
  rdfs:comment "A device converts solar radiation into other energy such as electric current or thermal energy."@en ;
  rdfs:isDefinedBy <http://pi.pauwel.be/voc/distributionelement> ;
  rdfs:label "Solar Device"@en ;
  rdfs:label "Solargerät"@de-de ;
  rdfs:label "capteur solaire"@fr-fr ;
  rdfs:label "solenergienhet"@nb-no ;
  rdfs:seeAlso <http://bsdd.buildingsmart.org/#concept/details/10kbcLuh91TeNXCNVtFC6g> ;
  rdfs:seeAlso ifc:IfcSolarDevice ;
  rdfs:subClassOf mep:EnergyConversionDevice ;
.
mep:SolarDevice-SOLARCOLLECTOR
  rdf:type owl:Class ;
  rdfs:isDefinedBy <http://pi.pauwel.be/voc/distributionelement> ;
  rdfs:label "Solar Collector"@en ;
  rdfs:seeAlso <http://bsdd.buildingsmart.org/#concept/details/0fo0nZHmT5twFp0u9haG2I> ;
  rdfs:seeAlso ifc:IfcSolarDeviceEnumType ;
  rdfs:subClassOf mep:SolarDevice ;
.
mep:SolarDevice-SOLARPANEL
  rdf:type owl:Class ;
  rdfs:comment "a device that converts solar radiation into electric current"@en ;
  rdfs:comment "a device that converts solar radiation into electric current"@en-gb ;
  rdfs:isDefinedBy <http://pi.pauwel.be/voc/distributionelement> ;
  rdfs:label "Solar Panel"@en ;
  rdfs:label "solpanel"@nb-no ;
  rdfs:seeAlso <http://bsdd.buildingsmart.org/#concept/details/2S$Xvvjqn1GAvVFoENZhtk> ;
  rdfs:seeAlso ifc:IfcSolarDeviceEnumType ;
  rdfs:subClassOf mep:SolarDevice ;
.
mep:SpaceHeater
  rdf:type owl:Class ;
  rdfs:comment "Heaters utilize a combination of radiation and/or natural convection using a heating source such as electricity, steam or hot water to heat a limited space or area. Examples of space heaters include radiators, convectors, baseboard and finned-tube heaters."@en ;
  rdfs:isDefinedBy <http://pi.pauwel.be/voc/distributionelement> ;
  rdfs:label "Heizkörper"@de-de ;
  rdfs:label "Space Heater"@en ;
  rdfs:label "heater"@en ;
  rdfs:label "kachel"@nl-nl ;
  rdfs:label "local heating device"@en ;
  rdfs:label "lokaal verwarmingstoestel"@nl-nl ;
  rdfs:label "radiateur"@fr-fr ;
  rdfs:label "ruimteverwarmingstoestel"@nl-nl ;
  rdfs:label "varmeenhet"@nb-no ;
  rdfs:seeAlso <http://bsdd.buildingsmart.org/#concept/details/39lbLJ2412vOKf6Cp8ojJd> ;
  rdfs:seeAlso ifc:IfcSpaceHeater ;
  rdfs:subClassOf mep:FlowTerminal ;
.
mep:SpaceHeater-CONVECTOR
  rdf:type owl:Class ;
  rdfs:comment "a heating appliance which emits heat almost entirely by convection. a convector comprises at least a heat emitter and a casing which provides an unheated convective chimney of defined height."@en ;
  rdfs:isDefinedBy <http://pi.pauwel.be/voc/distributionelement> ;
  rdfs:label "Convector"@en ;
  rdfs:label "Convector"@nl-nl ;
  rdfs:label "konvektor"@nb-no ;
  rdfs:label "varmekonvektor"@nb-no ;
  rdfs:seeAlso <http://bsdd.buildingsmart.org/#concept/details/0kMkKT22f00BAkHfSQ7c_B> ;
  rdfs:seeAlso ifc:IfcSpaceHeaterEnumType ;
  rdfs:subClassOf mep:SpaceHeater ;
.
mep:SpaceHeater-RADIATOR
  rdf:type owl:Class ;
  rdfs:comment "a heat appliance which emits heat by free convection and radiation"@en ;
  rdfs:isDefinedBy <http://pi.pauwel.be/voc/distributionelement> ;
  rdfs:label "Heizkörper"@de-de ;
  rdfs:label "Radiator"@de-de ;
  rdfs:label "Radiator"@en ;
  rdfs:label "radiateur"@fr-fr ;
  rdfs:label "radiator"@nb-no ;
  rdfs:label "varmelegeme"@nb-no ;
  rdfs:seeAlso <http://bsdd.buildingsmart.org/#concept/details/38a4eei5j5vQs7YtSb7quf> ;
  rdfs:seeAlso ifc:IfcSpaceHeaterEnumType ;
  rdfs:subClassOf mep:SpaceHeater ;
.
mep:StackTerminal
  rdf:type owl:Class ;
  rdfs:comment "A terminal placed at the top of a ventilating stack (such as to prevent ingress by birds or rainwater) or rainwater pipe (to act as a collector or hopper for discharge from guttering)."@en ;
  rdfs:isDefinedBy <http://pi.pauwel.be/voc/distributionelement> ;
  rdfs:label "Rohrabdeckung"@de-de ;
  rdfs:label "Stack Terminal"@en ;
  rdfs:label "system-terminal"@nb-no ;
  rdfs:seeAlso <http://bsdd.buildingsmart.org/#concept/details/0lNPT0EPbBWeJB7HGeHjgH> ;
  rdfs:seeAlso ifc:IfcStackTerminal ;
  rdfs:subClassOf mep:FlowTerminal ;
.
mep:StackTerminal-BIRDCAGE
  rdf:type owl:Class ;
  rdfs:comment "guard cage, typically wire mesh, at the top of the stack preventing access by birds"@en ;
  rdfs:comment "guard cage, typically wire mesh, at the top of the stack preventing access by birds"@en-gb ;
  rdfs:isDefinedBy <http://pi.pauwel.be/voc/distributionelement> ;
  rdfs:label "Birdcage"@en ;
  rdfs:label "ventilasjon gitter topp"@nb-no ;
  rdfs:seeAlso <http://bsdd.buildingsmart.org/#concept/details/2yx3o8h5157elNsihhcZZx> ;
  rdfs:seeAlso ifc:IfcStackTerminalEnumType ;
  rdfs:subClassOf mep:StackTerminal ;
.
mep:StackTerminal-COWL
  rdf:type owl:Class ;
  rdfs:comment "air terminal device intended to be installed above a natural ventilation exhaust duct with the aim, by creating negative pressure and depending on wind speed, of avoiding reverse flow and increasing flow rate"@en ;
  rdfs:isDefinedBy <http://pi.pauwel.be/voc/distributionelement> ;
  rdfs:label "cowl"@en ;
  rdfs:label "hette"@nb-no ;
  rdfs:label "vent cap"@en ;
  rdfs:label "vent turbine"@en ;
  rdfs:label "ventilasjonstopp"@nb-no ;
  rdfs:seeAlso <http://bsdd.buildingsmart.org/#concept/details/3XIKqh6OnDLvtnQcrmQvo4> ;
  rdfs:seeAlso ifc:IfcStackTerminalEnumType ;
  rdfs:subClassOf mep:StackTerminal ;
.
mep:StackTerminal-RAINWATERHOPPER
  rdf:type owl:Class ;
  rdfs:isDefinedBy <http://pi.pauwel.be/voc/distributionelement> ;
  rdfs:label "Rainwater Hopper"@en ;
  rdfs:seeAlso <http://bsdd.buildingsmart.org/#concept/details/0tlwEdOcDExuy98lwa6_38> ;
  rdfs:seeAlso ifc:IfcStackTerminalEnumType ;
  rdfs:subClassOf mep:StackTerminal ;
.
mep:SwitchingDevice
  rdf:type owl:Class ;
  rdfs:comment "A switch used in a cable distribution system (electrical circuit) to control or modulate the flow of electricity. Include those used for electrical power, communications, audio-visual, or other distribution system types as determined by the available ports."@en ;
  rdfs:isDefinedBy <http://pi.pauwel.be/voc/distributionelement> ;
  rdfs:label "Interrupteur"@fr-fr ;
  rdfs:label "Schalter"@de-de ;
  rdfs:label "Switching Device"@en ;
  rdfs:label "bryter"@nb-no ;
  rdfs:seeAlso <http://bsdd.buildingsmart.org/#concept/details/0JjKezzH55POBG1espn8W$> ;
  rdfs:seeAlso ifc:IfcSwitchingDevice ;
  rdfs:subClassOf mep:FlowController ;
.
mep:SwitchingDevice-CONTACTOR
  rdf:type owl:Class ;
  rdfs:comment "mechanical switching device having only one position of rest, operated otherwise than by hand, capable of making, carrying and breaking currents under normal circuit conditions including operating overload conditions"@en ;
  rdfs:isDefinedBy <http://pi.pauwel.be/voc/distributionelement> ;
  rdfs:label "Contactor"@en ;
  rdfs:label "Contactstop"@nl-nl ;
  rdfs:label "kontaktor"@nb-no ;
  rdfs:seeAlso <http://bsdd.buildingsmart.org/#concept/details/3rxqi3mzn8ovp5j4$AtKpj> ;
  rdfs:seeAlso ifc:IfcSwitchingDeviceEnumType ;
  rdfs:subClassOf mep:SwitchingDevice ;
.
mep:SwitchingDevice-DIMMERSWITCH
  rdf:type owl:Class ;
  rdfs:isDefinedBy <http://pi.pauwel.be/voc/distributionelement> ;
  rdfs:label "Dimmer Switch"@en ;
  rdfs:seeAlso <http://bsdd.buildingsmart.org/#concept/details/2Qsa6P6719HRwY$4OSoDq9> ;
  rdfs:seeAlso ifc:IfcSwitchingDeviceEnumType ;
  rdfs:subClassOf mep:SwitchingDevice ;
.
mep:SwitchingDevice-EMERGENCYSTOP
  rdf:type owl:Class ;
  rdfs:isDefinedBy <http://pi.pauwel.be/voc/distributionelement> ;
  rdfs:label "Emergency Stop"@en ;
  rdfs:seeAlso <http://bsdd.buildingsmart.org/#concept/details/1AkYCx5WrDfQSeajQs4GbK> ;
  rdfs:seeAlso ifc:IfcSwitchingDeviceEnumType ;
  rdfs:subClassOf mep:SwitchingDevice ;
.
mep:SwitchingDevice-KEYPAD
  rdf:type owl:Class ;
  rdfs:comment "а set of buttons or switches, each potentially applicable to a different device"@en ;
  rdfs:comment "а set of buttons or switches, each potentially applicable to a different device"@en-gb ;
  rdfs:isDefinedBy <http://pi.pauwel.be/voc/distributionelement> ;
  rdfs:label "Keypad"@en ;
  rdfs:label "tastatur"@nb-no ;
  rdfs:seeAlso <http://bsdd.buildingsmart.org/#concept/details/30Wun_rrP3hg09kZxKFSxo> ;
  rdfs:seeAlso ifc:IfcSwitchingDeviceEnumType ;
  rdfs:subClassOf mep:SwitchingDevice ;
.
mep:SwitchingDevice-MOMENTARYSWITCH
  rdf:type owl:Class ;
  rdfs:comment "а momentary switch has no position, and may trigger some action to occur"@en ;
  rdfs:comment "а momentary switch has no position, and may trigger some action to occur"@en-gb ;
  rdfs:isDefinedBy <http://pi.pauwel.be/voc/distributionelement> ;
  rdfs:label "Momentary Switch"@en ;
  rdfs:label "momentantbryter"@nb-no ;
  rdfs:seeAlso <http://bsdd.buildingsmart.org/#concept/details/1GXuot6Zv41wgJSbaoN8g7> ;
  rdfs:seeAlso ifc:IfcSwitchingDeviceEnumType ;
  rdfs:subClassOf mep:SwitchingDevice ;
.
mep:SwitchingDevice-SELECTORSWITCH
  rdf:type owl:Class ;
  rdfs:isDefinedBy <http://pi.pauwel.be/voc/distributionelement> ;
  rdfs:label "Selector Switch"@en ;
  rdfs:seeAlso <http://bsdd.buildingsmart.org/#concept/details/2WULe4Kq50n8t1M8n_T5Jc> ;
  rdfs:seeAlso ifc:IfcSwitchingDeviceEnumType ;
  rdfs:subClassOf mep:SwitchingDevice ;
.
mep:SwitchingDevice-STARTER
  rdf:type owl:Class ;
  rdfs:comment "а starter is a switch which in the closed position controls the application of power to an electrical device"@en ;
  rdfs:comment "а starter is a switch which in the closed position controls the application of power to an electrical device"@en-gb ;
  rdfs:isDefinedBy <http://pi.pauwel.be/voc/distributionelement> ;
  rdfs:label "Starter"@en ;
  rdfs:label "starter"@nb-no ;
  rdfs:seeAlso <http://bsdd.buildingsmart.org/#concept/details/2R7sKp3Zz8EvRVJenaoFA0> ;
  rdfs:seeAlso ifc:IfcSwitchingDeviceEnumType ;
  rdfs:subClassOf mep:SwitchingDevice ;
.
mep:SwitchingDevice-SWITCHDISCONNECTOR
  rdf:type owl:Class ;
  rdfs:isDefinedBy <http://pi.pauwel.be/voc/distributionelement> ;
  rdfs:label "Switch Disconnector"@en ;
  rdfs:seeAlso <http://bsdd.buildingsmart.org/#concept/details/2YJHtgvof1aQ6qN28MCYJh> ;
  rdfs:seeAlso ifc:IfcSwitchingDeviceEnumType ;
  rdfs:subClassOf mep:SwitchingDevice ;
.
mep:SwitchingDevice-TOGGLESWITCH
  rdf:type owl:Class ;
  rdfs:isDefinedBy <http://pi.pauwel.be/voc/distributionelement> ;
  rdfs:label "Toggle Switch"@en ;
  rdfs:seeAlso <http://bsdd.buildingsmart.org/#concept/details/2OMieHhU5ClBrIpriDbqmz> ;
  rdfs:seeAlso ifc:IfcSwitchingDeviceEnumType ;
  rdfs:subClassOf mep:SwitchingDevice ;
.
mep:Tank
  rdf:type owl:Class ;
  rdfs:comment "A vessel or container in which a fluid or gas is stored for later use."@en ;
  rdfs:isDefinedBy <http://pi.pauwel.be/voc/distributionelement> ;
  rdfs:label "Tank"@en ;
  rdfs:label "réservoir"@fr-fr ;
  rdfs:label "tank"@nb-no ;
  rdfs:seeAlso <http://bsdd.buildingsmart.org/#concept/details/2UJCW0qWyHuO00025QrE$V> ;
  rdfs:seeAlso ifc:IfcTank ;
  rdfs:subClassOf mep:FlowStorageDevice ;
.
mep:Tank-BASIN
  rdf:type owl:Class ;
  rdfs:comment "an arbitrary open tank type"@en ;
  rdfs:comment "an arbitrary open tank type"@en-gb ;
  rdfs:isDefinedBy <http://pi.pauwel.be/voc/distributionelement> ;
  rdfs:label "Basin"@en ;
  rdfs:label "servant"@nb-no ;
  rdfs:label "tank type basseng"@nb-no ;
  rdfs:seeAlso <http://bsdd.buildingsmart.org/#concept/details/2Kr7mfp3HFAfi67PdLwE0L> ;
  rdfs:seeAlso ifc:IfcTankEnumType ;
  rdfs:subClassOf mep:Tank ;
.
mep:Tank-BREAKPRESSURE
  rdf:type owl:Class ;
  rdfs:comment "an open container that breaks the hydraulic pressure in a distribution system, typically located between the fluid reservoir and the fluid supply points. a typical break pressure tank allows the flow to discharge into the atmosphere, thereby reducing its hydrostatic pressure to zero"@en ;
  rdfs:comment "an open container that breaks the hydraulic pressure in a distribution system, typically located between the fluid reservoir and the fluid supply points. a typical break pressure tank allows the flow to discharge into the atmosphere, thereby reducing its hydrostatic pressure to zero"@en-gb ;
  rdfs:isDefinedBy <http://pi.pauwel.be/voc/distributionelement> ;
  rdfs:label "Break Pressure Tank"@en ;
  rdfs:label "Bruddtrykk"@nb-no ;
  rdfs:seeAlso <http://bsdd.buildingsmart.org/#concept/details/1uUiVD63rEcPif0cejL9Vx> ;
  rdfs:seeAlso ifc:IfcTankEnumType ;
  rdfs:subClassOf mep:Tank ;
.
mep:Tank-EXPANSION
  rdf:type owl:Class ;
  rdfs:comment "a closed container used in a closed fluid distribution system to mitigate the effects of thermal expansion or water hammer. the tank is typically constructed with a diaphragm dividing the tank into two sections, with fluid on one side of the diaphragm and air on the other. one example application is when connected to the primary circuit of a hot water system to accommodate the increase in volume of the water when it is heated"@en ;
  rdfs:comment "a closed container used in a closed fluid distribution system to mitigate the effects of thermal expansion or water hammer. the tank is typically constructed with a diaphragm dividing the tank into two sections, with fluid on one side of the diaphragm and air on the other. one example application is when connected to the primary circuit of a hot water system to accommodate the increase in volume of the water when it is heated"@en-gb ;
  rdfs:isDefinedBy <http://pi.pauwel.be/voc/distributionelement> ;
  rdfs:label "Expansion Tank"@en ;
  rdfs:label "ekspansjon"@nb-no ;
  rdfs:seeAlso <http://bsdd.buildingsmart.org/#concept/details/1Lw1_wSbzFWe1SaTJeinCg> ;
  rdfs:seeAlso ifc:IfcTankEnumType ;
  rdfs:subClassOf mep:Tank ;
.
mep:Tank-FEEDANDEXPANSION
  rdf:type owl:Class ;
  rdfs:isDefinedBy <http://pi.pauwel.be/voc/distributionelement> ;
  rdfs:label "Feed And Expansion Tank"@en ;
  rdfs:label "mate og ekspansjonstank"@nb-no ;
  rdfs:seeAlso <http://bsdd.buildingsmart.org/#concept/details/371WHCLHb6vgWMDDSDFW4f> ;
  rdfs:seeAlso ifc:IfcTankEnumType ;
  rdfs:subClassOf mep:Tank ;
.
mep:Tank-PRESSUREVESSEL
  rdf:type owl:Class ;
  rdfs:isDefinedBy <http://pi.pauwel.be/voc/distributionelement> ;
  rdfs:label "Pressure Vessel"@en ;
  rdfs:label "trykktank"@nb-no ;
  rdfs:seeAlso <http://bsdd.buildingsmart.org/#concept/details/3pBTMtMgH5UOIRcXURYkQd> ;
  rdfs:seeAlso ifc:IfcTankEnumType ;
  rdfs:subClassOf mep:Tank ;
.
mep:Tank-STORAGE
  rdf:type owl:Class ;
  rdfs:isDefinedBy <http://pi.pauwel.be/voc/distributionelement> ;
  rdfs:label "Storage Tank"@en ;
  rdfs:label "lagringstank"@nb-no ;
  rdfs:seeAlso <http://bsdd.buildingsmart.org/#concept/details/36ZG4Tdk1CARQ9FrH0BlZe> ;
  rdfs:seeAlso ifc:IfcTankEnumType ;
  rdfs:subClassOf mep:Tank ;
.
mep:Tank-VESSEL
  rdf:type owl:Class ;
  rdfs:comment "an arbitrary closed tank type"@en ;
  rdfs:comment "an arbitrary closed tank type"@en-gb ;
  rdfs:isDefinedBy <http://pi.pauwel.be/voc/distributionelement> ;
  rdfs:label "Vessel"@en ;
  rdfs:label "beholder"@nb-no ;
  rdfs:seeAlso <http://bsdd.buildingsmart.org/#concept/details/2rdBMMRl56p9qdnIOKnbwO> ;
  rdfs:seeAlso ifc:IfcTankEnumType ;
  rdfs:subClassOf mep:Tank ;
.
mep:Transformer
  rdf:type owl:Class ;
  rdfs:comment "A artefact that transfers electric energy without change of frequency                "@en ;
  rdfs:comment "An inductive stationary device that transfers electrical energy from one circuit to another."@en ;
  rdfs:comment "Een statische energieomzetter die elektrische energie energie omzet zonder verandering van frequentie."@nl-nl ;
  rdfs:comment "Een toestel dat door elektromagnetische inductie één of meer veranderlijke stromen en spanningen omzet in één of meer verandelijke stromen en spanningen zonder dat voor de omzetting bewegende delen nodig zijn."@nl-nl ;
  rdfs:comment "Een transformator (veelal afgekort tot trafo (NL) of transfo (B)) is een statisch (d.w.z. zonder bewegende onderdelen) elektrisch apparaat, bestaande uit magnetisch gekoppelde spoelen. Stuurt men een veranderlijke stroom door een van de spoelen, de primaire spoel genoemd, dan wordt in de andere spoel(en), de secundaire, een spanning opgewekt."@nl-nl ;
  rdfs:comment "Elektrisch apparaat die elektrische wisselstroomenergie van een bepaald spanningsniveau en aantal fasen via magnetisch gekoppelde spoelen omzet in energie van een ander spanningsniveau, maar met dezelfde frequentie."@nl-nl ;
  rdfs:comment "Elektrisch apparaat waarmee spanning en stroom kunnen worden omgezet van hoge naar lage waarden. In de elektrotechniek een omzetter die elektrische wisselstroomenergie van een bepaald spanningsniveau en aantal fasen omzet in energie van een ander spanningsniveau, maar met dezelfde frequentie."@nl-nl ;
  rdfs:comment "static piece of apparatus with two or more windings which, by electromagnetic induction, transforms a system of alternating voltage and current into another system of voltage and current usually of different values and at the same frequency for the purpose of transmitting electrical power"@en ;
  rdfs:comment "static piece of apparatus with two or more windings which, by electromagnetic induction, transforms a system of alternating voltage and current into another system of voltage and current usually of different values and at the same frequency for the purpose of transmitting electrical power. (NEN-EN-IEC 61558-1)"@en ;
  rdfs:isDefinedBy <http://pi.pauwel.be/voc/distributionelement> ;
  rdfs:label "Transformer"@en ;
  rdfs:label "transformateur"@fr-fr ;
  rdfs:label "transformator"@de-de ;
  rdfs:label "transformator"@nb-no ;
  rdfs:label "transformator"@nl-nl ;
  rdfs:seeAlso <http://bsdd.buildingsmart.org/#concept/details/1d7Az5cjf79B356TXokPOF> ;
  rdfs:seeAlso ifc:IfcTransformer ;
  rdfs:subClassOf mep:EnergyConversionDevice ;
.
mep:Transformer-CURRENT
  rdf:type owl:Class ;
  rdfs:comment "a transformer that changes the current between circuits"@en ;
  rdfs:comment "a transformer that changes the current between circuits"@en-gb ;
  rdfs:isDefinedBy <http://pi.pauwel.be/voc/distributionelement> ;
  rdfs:label "Current Transformer"@en ;
  rdfs:label "strøm"@nb-no ;
  rdfs:seeAlso <http://bsdd.buildingsmart.org/#concept/details/0S1LeIGoj1CwsRLj4IxJSx> ;
  rdfs:seeAlso ifc:IfcTransformerEnumType ;
  rdfs:subClassOf mep:Transformer ;
.
mep:Transformer-FREQUENCY
  rdf:type owl:Class ;
  rdfs:comment "a transformer that changes the frequency between circuits"@en ;
  rdfs:comment "a transformer that changes the frequency between circuits"@en-gb ;
  rdfs:isDefinedBy <http://pi.pauwel.be/voc/distributionelement> ;
  rdfs:label "Frequency Transformer"@en ;
  rdfs:label "frekvens"@nb-no ;
  rdfs:seeAlso <http://bsdd.buildingsmart.org/#concept/details/1UAFNuQt5E0xPmuu4GQLrJ> ;
  rdfs:seeAlso ifc:IfcTransformerEnumType ;
  rdfs:subClassOf mep:Transformer ;
.
mep:Transformer-INVERTER
  rdf:type owl:Class ;
  rdfs:comment "device for the conversion of direct current (DC) to alternating current (AC)"@en ;
  rdfs:isDefinedBy <http://pi.pauwel.be/voc/distributionelement> ;
  rdfs:label "Inverter Transformer"@en ;
  rdfs:label "retter"@nb-no ;
  rdfs:seeAlso <http://bsdd.buildingsmart.org/#concept/details/1JVDHhnQb3Hv0o3sTOfXt3> ;
  rdfs:seeAlso ifc:IfcTransformerEnumType ;
  rdfs:subClassOf mep:Transformer ;
.
mep:Transformer-RECTIFIER
  rdf:type owl:Class ;
  rdfs:comment "electric energy converter that changes single-phase or polyphase alternating electric currents to unidirectional current"@en ;
  rdfs:isDefinedBy <http://pi.pauwel.be/voc/distributionelement> ;
  rdfs:label "Rectifier Transformer"@en ;
  rdfs:label "likeretter - transformator"@nb-no ;
  rdfs:label "likeretter"@nb-no ;
  rdfs:seeAlso <http://bsdd.buildingsmart.org/#concept/details/0J1BEZtan5FAXomnB0QhUR> ;
  rdfs:seeAlso ifc:IfcTransformerEnumType ;
  rdfs:subClassOf mep:Transformer ;
.
mep:Transformer-VOLTAGE
  rdf:type owl:Class ;
  rdfs:comment "a transformer that changes the voltage between circuits"@en ;
  rdfs:comment "a transformer that changes the voltage between circuits"@en-gb ;
  rdfs:isDefinedBy <http://pi.pauwel.be/voc/distributionelement> ;
  rdfs:label "Voltage Transformer"@en ;
  rdfs:label "spenning"@nb-no ;
  rdfs:seeAlso <http://bsdd.buildingsmart.org/#concept/details/1_4pUL3mX9fwVKh_9lcz1S> ;
  rdfs:seeAlso ifc:IfcTransformerEnumType ;
  rdfs:subClassOf mep:Transformer ;
.
mep:TubeBundle
  rdf:type owl:Class ;
  rdfs:comment "A device consisting of tubes and bundles of tubes used for heat transfer and contained typically within other energy conversion devices, such as a chiller or coil."@en ;
  rdfs:comment "An assembly of tubes constituting a part of a shell and tube heat exchanger. The tubes are in each end collected in a tube sheet.        "@en ;
  rdfs:isDefinedBy <http://pi.pauwel.be/voc/distributionelement> ;
  rdfs:label "Buizenregister"@nl-nl ;
  rdfs:label "Faisceau tubulaire"@fr-fr ;
  rdfs:label "Rohrbündel"@de-de ;
  rdfs:label "Tube Bundle"@en ;
  rdfs:label "rørbunt"@nb-no ;
  rdfs:seeAlso <http://bsdd.buildingsmart.org/#concept/details/2KKY0IUEj0J9jguEJqOHcm> ;
  rdfs:seeAlso ifc:IfcTubeBundle ;
  rdfs:subClassOf mep:EnergyConversionDevice ;
.
mep:TubeBundle-FINNED
  rdf:type owl:Class ;
  rdfs:isDefinedBy <http://pi.pauwel.be/voc/distributionelement> ;
  rdfs:label "Finned Tube Bundle"@en ;
  rdfs:label "ribberør"@nb-no ;
  rdfs:seeAlso <http://bsdd.buildingsmart.org/#concept/details/300_kyP4z8lfGEZ8$LKgLE> ;
  rdfs:seeAlso ifc:IfcTubeBundleEnumType ;
  rdfs:subClassOf mep:TubeBundle ;
.
mep:UnitaryControlElement
  rdf:type owl:Class ;
  rdfs:comment """A control element combines a number of control components into a single product, such as a thermostat or humidistat.
Provides a housing for an aggregation of control or electrical distribution elements that, in combination, perform a singular (unitary) purpose. Each item in the aggregation may have its own geometric representation and location."""@en ;
  rdfs:isDefinedBy <http://pi.pauwel.be/voc/distributionelement> ;
  rdfs:label "Einheitsregler"@de-de ;
  rdfs:label "Elément de contrôle unitaire"@fr-fr ;
  rdfs:label "Unitary Control Element"@en ;
  rdfs:label "enhetlig kontroll"@nb-no ;
  rdfs:seeAlso <http://bsdd.buildingsmart.org/#concept/details/1K4LPg0kL5k8UuFp4BB3Q9> ;
  rdfs:seeAlso ifc:IfcUnitaryControlElement ;
  rdfs:subClassOf mep:DistributionControlElement ;
.
mep:UnitaryControlElement-ALARMPANEL
  rdf:type owl:Class ;
  rdfs:isDefinedBy <http://pi.pauwel.be/voc/distributionelement> ;
  rdfs:label "Alarm Panel"@en ;
  rdfs:seeAlso <http://bsdd.buildingsmart.org/#concept/details/2E$a0foIL9GhqKHxJcRSkz> ;
  rdfs:seeAlso ifc:IfcUnitaryControlElementEnumType ;
  rdfs:subClassOf mep:UnitaryControlElement ;
.
mep:UnitaryControlElement-CONTROLPANEL
  rdf:type owl:Class ;
  rdfs:comment "a control element at which devices that control or monitor the operation of a site, building or part of a building are located"@en ;
  rdfs:comment "a control element at which devices that control or monitor the operation of a site, building or part of a building are located"@en-gb ;
  rdfs:isDefinedBy <http://pi.pauwel.be/voc/distributionelement> ;
  rdfs:label "Control Panel"@en ;
  rdfs:label "kontrollpanel"@nb-no ;
  rdfs:seeAlso <http://bsdd.buildingsmart.org/#concept/details/0szSYD3cD3$ucQuwpURDzs> ;
  rdfs:seeAlso ifc:IfcUnitaryControlElementEnumType ;
  rdfs:subClassOf mep:UnitaryControlElement ;
.
mep:UnitaryControlElement-GASDETECTIONPANEL
  rdf:type owl:Class ;
  rdfs:isDefinedBy <http://pi.pauwel.be/voc/distributionelement> ;
  rdfs:label "Gas Detection Panel"@en ;
  rdfs:seeAlso <http://bsdd.buildingsmart.org/#concept/details/26McOeRsjAPOMMV393Pkuv> ;
  rdfs:seeAlso ifc:IfcUnitaryControlElementEnumType ;
  rdfs:subClassOf mep:UnitaryControlElement ;
.
mep:UnitaryControlElement-HUMIDISTAT
  rdf:type owl:Class ;
  rdfs:comment "a control element that senses and regulates the humidity of a system or space so that the humidity is maintained near a desired setpoint."@en ;
  rdfs:isDefinedBy <http://pi.pauwel.be/voc/distributionelement> ;
  rdfs:label "Humidistat"@en ;
  rdfs:label "hygrostat"@nb-no ;
  rdfs:seeAlso <http://bsdd.buildingsmart.org/#concept/details/3duRJz_NHBsO8tukebn0Br> ;
  rdfs:seeAlso ifc:IfcUnitaryControlElementEnumType ;
  rdfs:subClassOf mep:UnitaryControlElement ;
.
mep:UnitaryControlElement-INDICATORPANEL
  rdf:type owl:Class ;
  rdfs:comment "а control element at which equipment operational status, condition, safety state or other required parameters are indicated"@en ;
  rdfs:isDefinedBy <http://pi.pauwel.be/voc/distributionelement> ;
  rdfs:label "Indicator Panel"@en ;
  rdfs:label "indikatorpanel"@nb-no ;
  rdfs:seeAlso <http://bsdd.buildingsmart.org/#concept/details/3wAtS33ID4zuEOa3x02EIn> ;
  rdfs:seeAlso ifc:IfcUnitaryControlElementEnumType ;
  rdfs:subClassOf mep:UnitaryControlElement ;
.
mep:UnitaryControlElement-MIMICPANEL
  rdf:type owl:Class ;
  rdfs:comment "а control element at which information that is available elsewhere is repeated or 'mimicked'"@en ;
  rdfs:comment "а control element at which information that is available elsewhere is repeated or 'mimicked'"@en-gb ;
  rdfs:isDefinedBy <http://pi.pauwel.be/voc/distributionelement> ;
  rdfs:label "Mimic Panel"@en ;
  rdfs:label "mimikkpanel"@nb-no ;
  rdfs:seeAlso <http://bsdd.buildingsmart.org/#concept/details/2gW6eFlD1A7Qnqh99Dspb0> ;
  rdfs:seeAlso ifc:IfcUnitaryControlElementEnumType ;
  rdfs:subClassOf mep:UnitaryControlElement ;
.
mep:UnitaryControlElement-THERMOSTAT
  rdf:type owl:Class ;
  rdfs:comment "Is the component of a control system which regulates the temperature of a system so that the system's temperature is maintained near a desired set point temperature"@en ;
  rdfs:comment "Temperaturstyrt bryter"@nb-no ;
  rdfs:isDefinedBy <http://pi.pauwel.be/voc/distributionelement> ;
  rdfs:label "Thermostat"@en ;
  rdfs:label "termostat"@nb-no ;
  rdfs:seeAlso <http://bsdd.buildingsmart.org/#concept/details/3MCWw0I6yHuO00025QrE$V> ;
  rdfs:seeAlso ifc:IfcUnitaryControlElementEnumType ;
  rdfs:subClassOf mep:UnitaryControlElement ;
.
mep:UnitaryControlElement-WEATHERSTATION
  rdf:type owl:Class ;
  rdfs:comment "a control element that senses multiple climate properties such as temperature, humidity, pressure, wind, and rain"@en ;
  rdfs:comment "a control element that senses multiple climate properties such as temperature, humidity, pressure, wind, and rain"@en-gb ;
  rdfs:isDefinedBy <http://pi.pauwel.be/voc/distributionelement> ;
  rdfs:label "Weather Station"@en ;
  rdfs:label "værstasjon"@nb-no ;
  rdfs:seeAlso <http://bsdd.buildingsmart.org/#concept/details/3d1EK0fY9CfwMNl1j5LmLc> ;
  rdfs:seeAlso ifc:IfcUnitaryControlElementEnumType ;
  rdfs:subClassOf mep:UnitaryControlElement ;
.
mep:UnitaryEquipment
  rdf:type owl:Class ;
  rdfs:comment "A combined of a number of components into a single product, such as air handlers, pre-packaged rooftop air-conditioning units, heat pumps, and split systems."@en ;
  rdfs:isDefinedBy <http://pi.pauwel.be/voc/distributionelement> ;
  rdfs:label "Einbaufertige Anlage"@de-de ;
  rdfs:label "Equipement unitaire"@fr-fr ;
  rdfs:label "Unitary Equipment"@en ;
  rdfs:label "enhetlig utstyr"@nb-no ;
  rdfs:seeAlso <http://bsdd.buildingsmart.org/#concept/details/0mUhAIpDb3mfYfYDW63M7U> ;
  rdfs:seeAlso ifc:IfcUnitaryEquipment ;
  rdfs:subClassOf mep:EnergyConversionDevice ;
.
mep:UnitaryEquipment-AIRCONDITIONINGUNIT
  rdf:type owl:Class ;
  rdfs:isDefinedBy <http://pi.pauwel.be/voc/distributionelement> ;
  rdfs:label "Air Conditioning Unit"@en ;
  rdfs:seeAlso <http://bsdd.buildingsmart.org/#concept/details/1PIU70CHzCMAt_h32UKgoE> ;
  rdfs:seeAlso ifc:IfcUnitaryEquipmentEnumType ;
  rdfs:subClassOf mep:UnitaryEquipment ;
.
mep:UnitaryEquipment-AIRHANDLER
  rdf:type owl:Class ;
  rdfs:isDefinedBy <http://pi.pauwel.be/voc/distributionelement> ;
  rdfs:label "Air Handler"@en ;
  rdfs:label "luftbehandling"@nb-no ;
  rdfs:seeAlso <http://bsdd.buildingsmart.org/#concept/details/1VnQL7ieb089ehb7syCaMo> ;
  rdfs:seeAlso ifc:IfcUnitaryEquipmentEnumType ;
  rdfs:subClassOf mep:UnitaryEquipment ;
.
mep:UnitaryEquipment-DEHUMIDIFIER
  rdf:type owl:Class ;
  rdfs:comment "a unitary packaged dehumidification unit. Note: units supporting multiple modes (dehumidification, cooling, and/or heating) should use AIRCONDITIONINGUNIT"@en ;
  rdfs:comment "a unitary packaged dehumidification unit. Note: units supporting multiple modes (dehumidification, cooling, and/or heating) should use AIRCONDITIONINGUNIT"@en-gb ;
  rdfs:isDefinedBy <http://pi.pauwel.be/voc/distributionelement> ;
  rdfs:label "Dehumidifier"@en ;
  rdfs:label "avfuktingsaggregat"@nb-no ;
  rdfs:seeAlso <http://bsdd.buildingsmart.org/#concept/details/1fDG4loZb609HKaHBIkk_l> ;
  rdfs:seeAlso ifc:IfcUnitaryEquipmentEnumType ;
  rdfs:subClassOf mep:UnitaryEquipment ;
.
mep:UnitaryEquipment-ROOFTOPUNIT
  rdf:type owl:Class ;
  rdfs:comment "unitary systems manufactured in various configurations providing single or multi-zone heating, cooling, and ventilation."@en ;
  rdfs:isDefinedBy <http://pi.pauwel.be/voc/distributionelement> ;
  rdfs:label "Rooftop Unit"@en ;
  rdfs:label "takenhet"@nb-no ;
  rdfs:seeAlso <http://bsdd.buildingsmart.org/#concept/details/0yMK$zpZz2Ahk9sfb3u4e7> ;
  rdfs:seeAlso ifc:IfcUnitaryEquipmentEnumType ;
  rdfs:subClassOf mep:UnitaryEquipment ;
.
mep:UnitaryEquipment-SPLITSYSTEM
  rdf:type owl:Class ;
  rdfs:isDefinedBy <http://pi.pauwel.be/voc/distributionelement> ;
  rdfs:label "Split System"@en ;
  rdfs:label "delt system"@nb-no ;
  rdfs:seeAlso <http://bsdd.buildingsmart.org/#concept/details/2iiBgNKl10ifd$UgILMf64> ;
  rdfs:seeAlso ifc:IfcUnitaryEquipmentEnumType ;
  rdfs:subClassOf mep:UnitaryEquipment ;
.
mep:Valve
  rdf:type owl:Class ;
  rdfs:comment "A flow control device used in a building services piping distribution system to control or modulate the flow of the fluid."@en ;
  rdfs:comment "An artefact used to control, i.e. permit, obstruct, regulate or divert a fluid stream.        "@en ;
  rdfs:comment "component isolating or controlling flow and pressure, e.g. isolating valve, control valve, pressure reducing valve, air valve, non-return valve, hydrant"@en ;
  rdfs:comment "komponent som isolerer eller kontrollerer vannføring og trykk, f.eks. stengeventil, kontrollventil, trykkreduksjonsventil, lufteventil, tilbakeslagsventil, brannventil/hydrant"@nb-no ;
  rdfs:isDefinedBy <http://pi.pauwel.be/voc/distributionelement> ;
  rdfs:label "Absperrarmatur; Ventil"@de-de ;
  rdfs:label "Afsluiter"@nl-nl ;
  rdfs:label "Armatur"@de-de ;
  rdfs:label "Valve"@en ;
  rdfs:label "Vanne"@fr-fr ;
  rdfs:label "Ventil"@da ;
  rdfs:label "Ventil"@de-de ;
  rdfs:label "appareil de robinetterie"@fr-fr ;
  rdfs:label "valve"@en ;
  rdfs:label "vanne; valve"@fr-fr ;
  rdfs:label "ventil"@nb-no ;
  rdfs:seeAlso <http://bsdd.buildingsmart.org/#concept/details/3s7E9HsSHBXejc$aKaBr8N> ;
  rdfs:seeAlso ifc:IfcValve ;
  rdfs:subClassOf mep:FlowController ;
.
mep:Valve-AIRRELEASE
  rdf:type owl:Class ;
  rdfs:isDefinedBy <http://pi.pauwel.be/voc/distributionelement> ;
  rdfs:label "Air Release"@en ;
  rdfs:seeAlso <http://bsdd.buildingsmart.org/#concept/details/3IEYICFuH8M9WXhUv2XVjI> ;
  rdfs:seeAlso ifc:IfcValveEnumType ;
  rdfs:subClassOf mep:Valve ;
.
mep:Valve-ANTIVACUUM
  rdf:type owl:Class ;
  rdfs:isDefinedBy <http://pi.pauwel.be/voc/distributionelement> ;
  rdfs:label "Antivacuum"@en ;
  rdfs:seeAlso <http://bsdd.buildingsmart.org/#concept/details/3akkmqwTrDKhcl5Sgc6MbM> ;
  rdfs:seeAlso ifc:IfcValveEnumType ;
  rdfs:subClassOf mep:Valve ;
.
mep:Valve-CHANGEOVER
  rdf:type owl:Class ;
  rdfs:isDefinedBy <http://pi.pauwel.be/voc/distributionelement> ;
  rdfs:label "Change Over"@en ;
  rdfs:seeAlso <http://bsdd.buildingsmart.org/#concept/details/0EkRKqfjHD0PwOY11Ixaxp> ;
  rdfs:seeAlso ifc:IfcValveEnumType ;
  rdfs:subClassOf mep:Valve ;
.
mep:Valve-CHECK
  rdf:type owl:Class ;
  rdfs:isDefinedBy <http://pi.pauwel.be/voc/distributionelement> ;
  rdfs:label "Check"@en ;
  rdfs:seeAlso <http://bsdd.buildingsmart.org/#concept/details/39bvtEU9T7Kwb0mdT3F1M9> ;
  rdfs:seeAlso ifc:IfcValveEnumType ;
  rdfs:subClassOf mep:Valve ;
.
mep:Valve-COMMISSIONING
  rdf:type owl:Class ;
  rdfs:isDefinedBy <http://pi.pauwel.be/voc/distributionelement> ;
  rdfs:label "Commissioning"@en ;
  rdfs:seeAlso <http://bsdd.buildingsmart.org/#concept/details/3YmvYjeBXElRSJyWt903HE> ;
  rdfs:seeAlso ifc:IfcValveEnumType ;
  rdfs:subClassOf mep:Valve ;
.
mep:Valve-DIVERTING
  rdf:type owl:Class ;
  rdfs:isDefinedBy <http://pi.pauwel.be/voc/distributionelement> ;
  rdfs:label "Diverting"@en ;
  rdfs:seeAlso <http://bsdd.buildingsmart.org/#concept/details/0OsZoKWAP7BBEErvuwAY_x> ;
  rdfs:seeAlso ifc:IfcValveEnumType ;
  rdfs:subClassOf mep:Valve ;
.
mep:Valve-DOUBLECHECK
  rdf:type owl:Class ;
  rdfs:isDefinedBy <http://pi.pauwel.be/voc/distributionelement> ;
  rdfs:label "DoubleCheck"@en ;
  rdfs:seeAlso <http://bsdd.buildingsmart.org/#concept/details/2$M2cKJh50r9iXgcDblZLB> ;
  rdfs:seeAlso ifc:IfcValveEnumType ;
  rdfs:subClassOf mep:Valve ;
.
mep:Valve-DOUBLEREGULATING
  rdf:type owl:Class ;
  rdfs:isDefinedBy <http://pi.pauwel.be/voc/distributionelement> ;
  rdfs:label "Double Regulating"@en ;
  rdfs:seeAlso <http://bsdd.buildingsmart.org/#concept/details/2Y8s3cCGf3WAkyIwDxHfmt> ;
  rdfs:seeAlso ifc:IfcValveEnumType ;
  rdfs:subClassOf mep:Valve ;
.
mep:Valve-DRAWOFFCOCK
  rdf:type owl:Class ;
  rdfs:isDefinedBy <http://pi.pauwel.be/voc/distributionelement> ;
  rdfs:label "Draw Off Cock"@en ;
  rdfs:seeAlso <http://bsdd.buildingsmart.org/#concept/details/1hIDIXF9r7MPfWQSquoEbq> ;
  rdfs:seeAlso ifc:IfcValveEnumType ;
  rdfs:subClassOf mep:Valve ;
.
mep:Valve-FAUCET
  rdf:type owl:Class ;
  rdfs:isDefinedBy <http://pi.pauwel.be/voc/distributionelement> ;
  rdfs:label "Faucet"@en ;
  rdfs:seeAlso <http://bsdd.buildingsmart.org/#concept/details/2j7S2gFkr9VAAkDsk9ttBg> ;
  rdfs:seeAlso ifc:IfcValveEnumType ;
  rdfs:subClassOf mep:Valve ;
.
mep:Valve-FLUSHING
  rdf:type owl:Class ;
  rdfs:isDefinedBy <http://pi.pauwel.be/voc/distributionelement> ;
  rdfs:label "Flushing"@en ;
  rdfs:seeAlso <http://bsdd.buildingsmart.org/#concept/details/3tbXQW_znFmQVfKs3YhQZ_> ;
  rdfs:seeAlso ifc:IfcValveEnumType ;
  rdfs:subClassOf mep:Valve ;
.
mep:Valve-GASCOCK
  rdf:type owl:Class ;
  rdfs:isDefinedBy <http://pi.pauwel.be/voc/distributionelement> ;
  rdfs:label "Gas Cock"@en ;
  rdfs:seeAlso <http://bsdd.buildingsmart.org/#concept/details/0WwwuPsrfCgv8h5yWR3dKz> ;
  rdfs:seeAlso ifc:IfcValveEnumType ;
  rdfs:subClassOf mep:Valve ;
.
mep:Valve-GASTAP
  rdf:type owl:Class ;
  rdfs:isDefinedBy <http://pi.pauwel.be/voc/distributionelement> ;
  rdfs:label "Gas Tap"@en ;
  rdfs:seeAlso <http://bsdd.buildingsmart.org/#concept/details/116lS7JG144hslqbHhbgkA> ;
  rdfs:seeAlso ifc:IfcValveEnumType ;
  rdfs:subClassOf mep:Valve ;
.
mep:Valve-ISOLATING
  rdf:type owl:Class ;
  rdfs:isDefinedBy <http://pi.pauwel.be/voc/distributionelement> ;
  rdfs:label "Isolating"@en ;
  rdfs:seeAlso <http://bsdd.buildingsmart.org/#concept/details/3fYepZO51AmflcVtRK9IVO> ;
  rdfs:seeAlso ifc:IfcValveEnumType ;
  rdfs:subClassOf mep:Valve ;
.
mep:Valve-MIXING
  rdf:type owl:Class ;
  rdfs:isDefinedBy <http://pi.pauwel.be/voc/distributionelement> ;
  rdfs:label "Mixing"@en ;
  rdfs:seeAlso <http://bsdd.buildingsmart.org/#concept/details/3cpFwtq7L1Owmcm7Yxvp05> ;
  rdfs:seeAlso ifc:IfcValveEnumType ;
  rdfs:subClassOf mep:Valve ;
.
mep:Valve-PRESSUREREDUCING
  rdf:type owl:Class ;
  rdfs:isDefinedBy <http://pi.pauwel.be/voc/distributionelement> ;
  rdfs:label "Pressure Reducing"@en ;
  rdfs:seeAlso <http://bsdd.buildingsmart.org/#concept/details/1P7aHESGb1JxvdNIDc1D9J> ;
  rdfs:seeAlso ifc:IfcValveEnumType ;
  rdfs:subClassOf mep:Valve ;
.
mep:Valve-PRESSURERELIEF
  rdf:type owl:Class ;
  rdfs:isDefinedBy <http://pi.pauwel.be/voc/distributionelement> ;
  rdfs:label "Pressure Relief"@en ;
  rdfs:seeAlso <http://bsdd.buildingsmart.org/#concept/details/0Si_BQgDr7f8BoS$bMsnAA> ;
  rdfs:seeAlso ifc:IfcValveEnumType ;
  rdfs:subClassOf mep:Valve ;
.
mep:Valve-REGULATING
  rdf:type owl:Class ;
  rdfs:isDefinedBy <http://pi.pauwel.be/voc/distributionelement> ;
  rdfs:label "Regulating"@en ;
  rdfs:seeAlso <http://bsdd.buildingsmart.org/#concept/details/2Y3yA_sy15NRRwfdI7LaxA> ;
  rdfs:seeAlso ifc:IfcValveEnumType ;
  rdfs:subClassOf mep:Valve ;
.
mep:Valve-SAFETYCUTOFF
  rdf:type owl:Class ;
  rdfs:isDefinedBy <http://pi.pauwel.be/voc/distributionelement> ;
  rdfs:label "Safety Cut Off"@en ;
  rdfs:seeAlso <http://bsdd.buildingsmart.org/#concept/details/2cRQlX33L53gdVBEMFha9_> ;
  rdfs:seeAlso ifc:IfcValveEnumType ;
  rdfs:subClassOf mep:Valve ;
.
mep:Valve-STEAMTRAP
  rdf:type owl:Class ;
  rdfs:isDefinedBy <http://pi.pauwel.be/voc/distributionelement> ;
  rdfs:label "Steam Trap"@en ;
  rdfs:seeAlso <http://bsdd.buildingsmart.org/#concept/details/1IXcpzdwj4SgIc_5uXMgrX> ;
  rdfs:seeAlso ifc:IfcValveEnumType ;
  rdfs:subClassOf mep:Valve ;
.
mep:Valve-STOPCOCK
  rdf:type owl:Class ;
  rdfs:isDefinedBy <http://pi.pauwel.be/voc/distributionelement> ;
  rdfs:label "Stop Cock"@en ;
  rdfs:seeAlso <http://bsdd.buildingsmart.org/#concept/details/0dmRan7HrB4v9gh4bkhOo3> ;
  rdfs:seeAlso ifc:IfcValveEnumType ;
  rdfs:subClassOf mep:Valve ;
.
mep:WasteTerminal
  rdf:type owl:Class ;
  rdfs:comment """A terminal for the purpose of collecting or intercepting waste from one or more sanitary terminals or other fluid waste generating equipment and discharging it into a single waste/drainage system.
Provides for all forms of trap and waste point that collects discharge from a sanitary terminal and discharges it into a waste/drainage subsystem or that collects waste from several terminals and passes it into a single waste/drainage subsystem. Includes the P and S traps from soil sanitary terminals, sinks, and basins as well as floor wastes and gully traps that provide collection points."""@en ;
  rdfs:isDefinedBy <http://pi.pauwel.be/voc/distributionelement> ;
  rdfs:label "Ablauf"@de-de ;
  rdfs:label "Abscheider"@de-de ;
  rdfs:label "Stockage des déchets"@fr-fr ;
  rdfs:label "Vuilwaterput"@nl-nl ;
  rdfs:label "Waste Terminal"@en ;
  rdfs:label "avfallsterminal"@nb-no ;
  rdfs:seeAlso <http://bsdd.buildingsmart.org/#concept/details/3IXcC8tvn4igBk64SckDjX> ;
  rdfs:seeAlso ifc:IfcWasteTerminal ;
  rdfs:subClassOf mep:FlowTerminal ;
.
mep:WasteTerminal-FLOORTRAP
  rdf:type owl:Class ;
  rdfs:isDefinedBy <http://pi.pauwel.be/voc/distributionelement> ;
  rdfs:label "Floor Trap"@en ;
  rdfs:seeAlso <http://bsdd.buildingsmart.org/#concept/details/33CCzm2CLBDfHv1gHVU8MC> ;
  rdfs:seeAlso ifc:IfcWasteTerminalEnumType ;
  rdfs:subClassOf mep:WasteTerminal ;
.
mep:WasteTerminal-FLOORWASTE
  rdf:type owl:Class ;
  rdfs:isDefinedBy <http://pi.pauwel.be/voc/distributionelement> ;
  rdfs:label "Floor Waste"@en ;
  rdfs:seeAlso <http://bsdd.buildingsmart.org/#concept/details/0Gg1lQtOn0jv4GqORpX2Y8> ;
  rdfs:seeAlso ifc:IfcWasteTerminalEnumType ;
  rdfs:subClassOf mep:WasteTerminal ;
.
mep:WasteTerminal-GULLYSUMP
  rdf:type owl:Class ;
  rdfs:isDefinedBy <http://pi.pauwel.be/voc/distributionelement> ;
  rdfs:label "Gully Sump"@en ;
  rdfs:seeAlso <http://bsdd.buildingsmart.org/#concept/details/0ZMLzB3o99aurJi3RGmMhG> ;
  rdfs:seeAlso ifc:IfcWasteTerminalEnumType ;
  rdfs:subClassOf mep:WasteTerminal ;
.
mep:WasteTerminal-GULLYTRAP
  rdf:type owl:Class ;
  rdfs:isDefinedBy <http://pi.pauwel.be/voc/distributionelement> ;
  rdfs:label "Gully Trap"@en ;
  rdfs:label "sluklås"@nb-no ;
  rdfs:seeAlso <http://bsdd.buildingsmart.org/#concept/details/1WBoKi2av2NxTXpoB2QfO5> ;
  rdfs:seeAlso ifc:IfcWasteTerminalEnumType ;
  rdfs:subClassOf mep:WasteTerminal ;
.
mep:WasteTerminal-ROOFDRAIN
  rdf:type owl:Class ;
  rdfs:comment "pipe fitting, set into the roof, that collects rainwater for discharge into the rainwater system."@en ;
  rdfs:isDefinedBy <http://pi.pauwel.be/voc/distributionelement> ;
  rdfs:label "Roof Drain"@en ;
  rdfs:label "taksluk"@nb-no ;
  rdfs:seeAlso <http://bsdd.buildingsmart.org/#concept/details/0Xkj0nlvX689aFUVxq3IMM> ;
  rdfs:seeAlso ifc:IfcWasteTerminalEnumType ;
  rdfs:subClassOf mep:WasteTerminal ;
.
mep:WasteTerminal-WASTEDISPOSALUNIT
  rdf:type owl:Class ;
  rdfs:comment "electrically operated device that reduces kitchen or other waste into fragments small enough to be flushed into a drainage system."@en ;
  rdfs:isDefinedBy <http://pi.pauwel.be/voc/distributionelement> ;
  rdfs:label "Waste Disposal Unit"@en ;
  rdfs:label "avfallsenhet"@nb-no ;
  rdfs:seeAlso <http://bsdd.buildingsmart.org/#concept/details/0khvv6MsL5DxzEnCFiP5mr> ;
  rdfs:seeAlso ifc:IfcWasteTerminalEnumType ;
  rdfs:subClassOf mep:WasteTerminal ;
.
mep:WasteTerminal-WASTETRAP
  rdf:type owl:Class ;
  rdfs:isDefinedBy <http://pi.pauwel.be/voc/distributionelement> ;
  rdfs:label "Waste Trap"@en ;
  rdfs:label "vannlås"@nb-no ;
  rdfs:seeAlso <http://bsdd.buildingsmart.org/#concept/details/1JPv81z_531vDlQ02VFI9a> ;
  rdfs:seeAlso ifc:IfcWasteTerminalEnumType ;
  rdfs:subClassOf mep:WasteTerminal ;
.
dcterms:contributor
  rdf:type owl:AnnotationProperty ;
.
dcterms:creator
  rdf:type owl:AnnotationProperty ;
.
dcterms:description
  rdf:type owl:AnnotationProperty ;
.
dcterms:issued
  rdf:type owl:AnnotationProperty ;
.
dcterms:license
  rdf:type owl:AnnotationProperty ;
.
dcterms:modified
  rdf:type owl:AnnotationProperty ;
.
dcterms:title
  rdf:type owl:AnnotationProperty ;
.
vann:preferredNamespacePrefix
  rdf:type owl:AnnotationProperty ;
.
vann:preferredNamespaceUri
  rdf:type owl:AnnotationProperty ;
.
voaf:Vocabulary
  rdf:type owl:Class ;
.
vs:term_status
  rdf:type owl:AnnotationProperty ;
.
foaf:Person
  rdf:type owl:Class ;
.
foaf:name
  rdf:type owl:DatatypeProperty ;
.
contax:ConstructionComponent
  rdf:type owl:Class ;
.
