# baseURI: http://pi.pauwel.be/voc/buildingelement
# prefix: beo

@prefix : <http://pi.pauwel.be/voc/buildingelement#> .
@prefix beo: <http://pi.pauwel.be/voc/buildingelement#> .
@prefix cc: <http://creativecommons.org/ns#> .
@prefix contax: <https://w3id.org/con-tax#> .
@prefix dbr: <http://dbpedia.org/resource/> .
@prefix dcterms: <http://purl.org/dc/terms/> .
@prefix foaf: <http://xmlns.com/foaf/0.1/> .
@prefix gr: <http://purl.org/goodrelations/v1#> .
@prefix ifc: <https://standards.buildingsmart.org/IFC/DEV/IFC4/ADD2/OWL#> .
@prefix owl: <http://www.w3.org/2002/07/owl#> .
@prefix rdf: <http://www.w3.org/1999/02/22-rdf-syntax-ns#> .
@prefix rdfs: <http://www.w3.org/2000/01/rdf-schema#> .
@prefix schema: <https://schema.org/> .
@prefix vann: <http://purl.org/vocab/vann/> .
@prefix vcard: <http://www.w3.org/2006/vcard/ns#> .
@prefix voaf: <http://purl.org/vocommons/voaf#> .
@prefix vs: <http://www.w3.org/2003/06/sw-vocab-status/ns#> .
@prefix xsd: <http://www.w3.org/2001/XMLSchema#> .

<http://pi.pauwel.be/voc/buildingelement>
  rdf:type voaf:Vocabulary ;
  rdf:type owl:Ontology ;
  cc:license <https://creativecommons.org/licenses/by/1.0/> ;
  dcterms:contributor [
      rdf:type vcard:Individual ;
      vcard:family-name "Bonduel" ;
      vcard:fn "Mathias Bonduel" ;
      vcard:given-name "Mathias" ;
      vcard:hasOrganizationName [
          rdf:type vcard:Organization ;
          owl:sameAs dbr:Katholieke_Universiteit_Leuven ;
          vcard:hasURL <https://www.kuleuven.be> ;
          vcard:organization-name "KU Leuven" ;
        ] ;
      vcard:hasURL <https://orcid.org/0000-0002-3313-924X> ;
      vcard:hasURL <https://www.kuleuven.be/wieiswie/nl/person/00110827> ;
      vcard:hasURL <https://www.researchgate.net/profile/Mathias_Bonduel> ;
    ] ;
  dcterms:creator [
      rdf:type foaf:Person ;
      foaf:name "Pieter Pauwels" ;
    ] ;
  dcterms:description "The Building Element Ontology (BEO) provides an ontology based on the IfcBuildingElement, IfcElementComponent and IfcTransportElement subtrees in the IFC specification, containing a taxonomy of classes that allow to define common building elements."@en ;
  dcterms:issued "2018-12-27"^^xsd:date ;
  dcterms:modified "2020-08-11"^^xsd:date ;
  dcterms:title "BEO: Building Element Ontology"@en ;
  vann:preferredNamespacePrefix "beo" ;
  vann:preferredNamespaceUri "http://pi.pauwel.be/voc/buildingelement#" ;
  rdfs:comment """- TODO: remove similar labels/comments with same language tag
- Version 0.3.0: changed ccc:ConstructionComponent into contax:ConstructionComponent and added contax:ConstructionSubComponent. Added rdfs:isDefinedBy
- Version 0.2.0: changed all subclasses of schema:Product and gr:SomeItems into a subclass of ccc:ConstructionComponent
- Version 0.1.1: small changes and corrections (completed onto metadata; changed labels containing a bSDD URL to URIs connected via rdfs:seeAlso; updated ifcOWL URI; replace erroneous language tags (remove @ifc-2x4); added gr:SomeItems class and make beo:ElementComponent and beo:TransportElement a subclass (similar to beo:BuildingElement); added missing language tags to strings)
- Version 0.1.0: initial version"""@en ;
  owl:versionInfo "0.3.0" ;
.
beo:Beam
  rdf:type owl:Class ;
  rdfs:comment "A horizontal, or nearly horizontal, structural member that is capable of withstanding load primarily by resisting bending. It represents such a member from an architectural point of view. It is not required to be load bearing."@en ;
  rdfs:isDefinedBy <http://pi.pauwel.be/voc/buildingelement> ;
  rdfs:label "Balk"@nl ;
  rdfs:label "Beam"@en ;
  rdfs:label "Bjælke"@da ;
  rdfs:label "balken"@de-de ;
  rdfs:label "biegeträger"@de-de ;
  rdfs:label "bjelke"@nb-no ;
  rdfs:label "poutre"@fr-fr ;
  rdfs:seeAlso <http://bsdd.buildingsmart.org/#concept/details/3zXEi0qSCHuO00025QrE$V> ;
  rdfs:seeAlso ifc:IfcBeam ;
  rdfs:subClassOf beo:BuildingElement ;
.
beo:Beam-BEAM
  rdf:type owl:Class ;
  rdfs:comment "A standard beam usually used horizontally."@en ;
  rdfs:isDefinedBy <http://pi.pauwel.be/voc/buildingelement> ;
  rdfs:label "Beam"@en ;
  rdfs:label "balk"@nl-nl ;
  rdfs:label "balken"@de-de ;
  rdfs:label "biegeträger"@de-de ;
  rdfs:label "bjelke"@nb-no ;
  rdfs:label "ligger"@nl-nl ;
  rdfs:label "poutre"@fr-fr ;
  rdfs:seeAlso <http://bsdd.buildingsmart.org/#concept/details/0KKIHMGYH7H8MAfgxbrxuV> ;
  rdfs:seeAlso ifc:IfcBeamEnumType ;
  rdfs:subClassOf beo:Beam ;
.
beo:Beam-HOLLOWCORE
  rdf:type owl:Class ;
  rdfs:comment "Platte mit rechteckigem Querschnitt, in der auf voller Länge in Längsrichtung kreisrunde oder ovale Hohlräume (Aussparungen) verlaufen"@de-de ;
  rdfs:comment "dalle de section rectangulaire comportant des vides longitudinaux sur toute leur longueur ou des vides de forme ovale"@fr-fr ;
  rdfs:comment "losa de sección rectangular con huecos circulares o óvales para toda su longitud"@es-es ;
  rdfs:comment "monolithic prestressed or reinforced elements with a constant overall depth divided into an upper and lower flange, linked by vertical webs, so constituting cores as longitudinal voids the cross section of which is constant and presents one vertical axis."@en ;
  rdfs:comment "prostokątna płyta z okrągłymi lub owalnymi przestrzeniami na całej długości"@pl-pl ;
  rdfs:comment "rectangular section slab with full-length longitudinal circular or oval shaped voids"@en-gb ;
  rdfs:comment "rektangulärt bjälklag med längsgående cirkelformade eller ovalformade tomrum längs med hela bjälklaget"@sv-se ;
  rdfs:comment "rektangulært element med hulrum i fuld længde i langsgående, cirkulær eller oval form"@dk-dk ;
  rdfs:comment "rektangulært element med langsgående sirkulære eller ovale hulrom i full lengde"@nb-no ;
  rdfs:comment "suorakaiteenmuotoinen laattaelementti, jossa on koko pituudeltaan pyöreitä tai ovaalinmuotoisia onteloita/tyhjätiloja"@fi-fi ;
  rdfs:comment "плоча с правоъгълно сечение и кухини по цялата дължина с надлъжна кръгла или овална форма "@bg-bg ;
  rdfs:isDefinedBy <http://pi.pauwel.be/voc/buildingelement> ;
  rdfs:label "Pre-cast Hollow Core Slab"@en ;
  rdfs:label "dalle alvéolée préfabriquée en béton"@fr-fr ;
  rdfs:label "förtillverkade betongprodukter - håldäcksplattor"@sv-se ;
  rdfs:label "hulldekke"@nb-no ;
  rdfs:label "hulldekkeelement"@nb-no ;
  rdfs:label "lastre alveolari precompresse"@it-it ;
  rdfs:label "losa alveolar prefabricada"@es-es ;
  rdfs:label "ontelolaatta"@fi-fi ;
  rdfs:label "pre-cast hollow core slab"@en-gb ;
  rdfs:label "prefabrikkert hulldekke"@nb-no ;
  rdfs:label "prefabrykowana płyta kanałowa stropowa"@pl-pl ;
  rdfs:label "præfabrikeret huldækelement"@dk-dk ;
  rdfs:label "werkseitig hergestellte Hohlplatte"@de-de ;
  rdfs:label "готови плочи с кухини"@bg-bg ;
  rdfs:seeAlso <http://bsdd.buildingsmart.org/#concept/details/2gzZKHqELB$gPVKajRAFXc> ;
  rdfs:seeAlso ifc:IfcBeamEnumType ;
  rdfs:subClassOf beo:Beam ;
.
beo:Beam-JOIST
  rdf:type owl:Class ;
  rdfs:isDefinedBy <http://pi.pauwel.be/voc/buildingelement> ;
  rdfs:label "Joiste"@en ;
  rdfs:label "tilpasset bjelke"@nb-no ;
  rdfs:seeAlso <http://bsdd.buildingsmart.org/#concept/details/1_zkjNhS95oA5oDSSTnEvO> ;
  rdfs:seeAlso ifc:IfcBeamEnumType ;
  rdfs:subClassOf beo:Beam ;
.
beo:Beam-LINTEL
  rdf:type owl:Class ;
  rdfs:isDefinedBy <http://pi.pauwel.be/voc/buildingelement> ;
  rdfs:label "Lintel"@en ;
  rdfs:label "overdekking"@nb-no ;
  rdfs:seeAlso <http://bsdd.buildingsmart.org/#concept/details/1PivEYC0575QGoaAFjN8c9> ;
  rdfs:seeAlso ifc:IfcBeamEnumType ;
  rdfs:subClassOf beo:Beam ;
.
beo:Beam-SPANDREL
  rdf:type owl:Class ;
  rdfs:isDefinedBy <http://pi.pauwel.be/voc/buildingelement> ;
  rdfs:label "Spandrel"@en ;
  rdfs:label "brystning"@nb-no ;
  rdfs:seeAlso <http://bsdd.buildingsmart.org/#concept/details/2$vr6UW$f3SwHilnemEZoH> ;
  rdfs:seeAlso ifc:IfcBeamEnumType ;
  rdfs:subClassOf beo:Beam ;
.
beo:Beam-T_BEAM
  rdf:type owl:Class ;
  rdfs:isDefinedBy <http://pi.pauwel.be/voc/buildingelement> ;
  rdfs:label "T_Beam"@en ;
  rdfs:label "t_bjelke"@nb-no ;
  rdfs:seeAlso <http://bsdd.buildingsmart.org/#concept/details/1o9Up6wBr339DlpjWIWE$l> ;
  rdfs:seeAlso ifc:IfcBeamEnumType ;
  rdfs:subClassOf beo:Beam ;
.
beo:BuildingElement
  rdf:type owl:Class ;
  rdfs:comment "Bauelement"@de-de ;
  rdfs:comment "Comprises all elements that are primarily part of the construction of a building, i.e., its structural and space separating system. Building elements are all physically existent and tangible things."@en ;
  rdfs:isDefinedBy <http://pi.pauwel.be/voc/buildingelement> ;
  rdfs:label "Bauteil"@de-de ;
  rdfs:label "Building Element"@en ;
  rdfs:label "Elément de construction"@fr-fr ;
  rdfs:seeAlso <http://bsdd.buildingsmart.org/#concept/details/2AFYKXkEn7RxYuvbduGfUV> ;
  rdfs:seeAlso ifc:IfcBuildingElement ;
  rdfs:subClassOf contax:ConstructionComponent ;
.
beo:BuildingElementPart
  rdf:type owl:Class ;
  rdfs:comment "ifcbuildingelementpart represents major components as subordinate parts of a building element. typical usage examples include precast concrete sandwich walls, where the layers may have different geometry representations. in this case the layered material representation does not sufficiently describe the element. each layer is represented by an own instance of the ifcbuildingelementpart with its own geometry description. the kind of building element part is further specified by a corresponding instance of ifcbuildingelementparttype, referred to by ifcreldefinesbytype."@en ;
  rdfs:isDefinedBy <http://pi.pauwel.be/voc/buildingelement> ;
  rdfs:label "Building Element Part"@en ;
  rdfs:label "Teil eines Bauelements"@de-de ;
  rdfs:label "partie d'élément de construction"@fr-fr ;
  rdfs:seeAlso <http://bsdd.buildingsmart.org/#concept/details/3v2S1DH0r50BHIhWE6QHMZ> ;
  rdfs:seeAlso ifc:IfcBuildingElementPart ;
  rdfs:subClassOf beo:ElementComponent ;
.
beo:BuildingElementPart-INSULATION
  rdf:type owl:Class ;
  rdfs:isDefinedBy <http://pi.pauwel.be/voc/buildingelement> ;
  rdfs:label "Insulation"@en ;
  rdfs:label "isolasjon"@nb-no ;
  rdfs:seeAlso <http://bsdd.buildingsmart.org/#concept/details/2CF$o8Mgv2_xbw_kioa_YW> ;
  rdfs:seeAlso ifc:IfcBuildingElementPartEnumType ;
  rdfs:subClassOf beo:BuildingElementPart ;
.
beo:BuildingElementPart-PRECASTPANEL
  rdf:type owl:Class ;
  rdfs:isDefinedBy <http://pi.pauwel.be/voc/buildingelement> ;
  rdfs:label "Precast Panel"@en ;
  rdfs:seeAlso <http://bsdd.buildingsmart.org/#concept/details/0pt2K5QIXB89suCXlsQZw$> ;
  rdfs:seeAlso ifc:IfcBuildingElementPartEnumType ;
  rdfs:subClassOf beo:BuildingElementPart ;
.
beo:Chimney
  rdf:type owl:Class ;
  rdfs:comment "A vertical structure of brick, masonry, or steel that carries exhaust gases or steam away from a fire, engine, etc."@en ;
  rdfs:comment "Typically vertical, or as near as vertical, parts of the construction of a building and part of the building fabric. Often constructed by pre-cast or insitu concrete, today seldom by bricks."@en ;
  rdfs:comment "konstruksjon bestående av én eller flere vegger som omslutter én eller flere røykkanaler"@nb-no ;
  rdfs:comment "structure consisting of a wall or walls enclosing  a flue or flues"@en ;
  rdfs:isDefinedBy <http://pi.pauwel.be/voc/buildingelement> ;
  rdfs:label "Abgasanlage"@de-de ;
  rdfs:label "Abgassanlage"@de-de ;
  rdfs:label "Chimney"@en ;
  rdfs:label "Schoorsteen"@nl ;
  rdfs:label "Schoorsteen"@nl-nl ;
  rdfs:label "Schornstein"@de-de ;
  rdfs:label "Skorsten"@da ;
  rdfs:label "cheminée"@fr-fr ;
  rdfs:label "conduit de fumée"@fr-fr ;
  rdfs:label "pipe"@nb-no ;
  rdfs:label "skorstein"@nb-no ;
  rdfs:seeAlso <http://bsdd.buildingsmart.org/#concept/details/0xE4A0qSaHuO00025QrE$V> ;
  rdfs:seeAlso ifc:IfcChimney ;
  rdfs:subClassOf beo:BuildingElement ;
.
beo:Column
  rdf:type owl:Class ;
  rdfs:comment "A vertical structural member which often is aligned with a structural grid intersection. It represents a vertical, or nearly vertical, structural member that transmits, through compression, the weight of the structure above to other structural elements below. It represents such a member from an architectural point of view. It is not required to be load bearing."@en ;
  rdfs:isDefinedBy <http://pi.pauwel.be/voc/buildingelement> ;
  rdfs:label "Column"@en ;
  rdfs:label "Kolom"@nl ;
  rdfs:label "Stütze / Pfeiler"@de-de ;
  rdfs:label "Søjle"@da ;
  rdfs:label "poteau"@fr-fr ;
  rdfs:seeAlso <http://bsdd.buildingsmart.org/#concept/details/1CDOE0qSeHuO00025QrE$V> ;
  rdfs:seeAlso ifc:IfcColumn ;
  rdfs:subClassOf beo:BuildingElement ;
.
beo:Column-COLUMN
  rdf:type owl:Class ;
  rdfs:comment "A vertical structural member which often is aligned with a structural grid intersection. It represents a vertical, or nearly vertical, structural member that transmits, through compression, the weight of the structure above to other structural elements below. It represents such a member from an architectural point of view. It is not required to be load bearing."@en ;
  rdfs:comment "Søyle"@nb-no ;
  rdfs:isDefinedBy <http://pi.pauwel.be/voc/buildingelement> ;
  rdfs:label "Column"@en ;
  rdfs:label "Druckstab"@de-de ;
  rdfs:label "Stütze"@de-de ;
  rdfs:label "poteau"@fr-fr ;
  rdfs:seeAlso <http://bsdd.buildingsmart.org/#concept/details/1k5QL8XejA8v7H3XePklst> ;
  rdfs:seeAlso ifc:IfcColumnEnumType ;
  rdfs:subClassOf beo:Column ;
.
beo:Column-PILASTER
  rdf:type owl:Class ;
  rdfs:comment "Pilaster"@nb-no ;
  rdfs:comment "vertikalt fremspring på vegg"@nb-no ;
  rdfs:isDefinedBy <http://pi.pauwel.be/voc/buildingelement> ;
  rdfs:label "Pilaster"@en ;
  rdfs:label "Pilaster"@nl-nl ;
  rdfs:seeAlso <http://bsdd.buildingsmart.org/#concept/details/08F4W56in3zeQ$ucplQrmF> ;
  rdfs:seeAlso <http://bsdd.buildingsmart.org/#concept/details/312dw0BS8Htm00025QrE$V> ;
  rdfs:seeAlso ifc:IfcColumnEnumType ;
  rdfs:subClassOf beo:Column ;
.
beo:Covering
  rdf:type owl:Class ;
  rdfs:comment "An element which covers some part of another element and is fully dependent on that other element."@en ;
  rdfs:isDefinedBy <http://pi.pauwel.be/voc/buildingelement> ;
  rdfs:label "Bekleidung / Belag"@de-de ;
  rdfs:label "Covering"@en ;
  rdfs:label "kledning / belegg"@nb-no ;
  rdfs:label "revêtement"@fr-fr ;
  rdfs:seeAlso <http://bsdd.buildingsmart.org/#concept/details/3uBPs0qSyHuO00025QrE$V> ;
  rdfs:seeAlso ifc:IfcCovering ;
  rdfs:subClassOf beo:BuildingElement ;
.
beo:Covering-CEILING
  rdf:type owl:Class ;
  rdfs:isDefinedBy <http://pi.pauwel.be/voc/buildingelement> ;
  rdfs:label "Ceiling"@en ;
  rdfs:label "tak"@nb-no ;
  rdfs:seeAlso <http://bsdd.buildingsmart.org/#concept/details/05pSAVKa99GQlGChUhmlv1> ;
  rdfs:seeAlso ifc:IfcCoveringEnumType ;
  rdfs:subClassOf beo:Covering ;
.
beo:Covering-CLADDING
  rdf:type owl:Class ;
  rdfs:isDefinedBy <http://pi.pauwel.be/voc/buildingelement> ;
  rdfs:label "Cladding"@en ;
  rdfs:label "kledning"@nb-no ;
  rdfs:seeAlso <http://bsdd.buildingsmart.org/#concept/details/0MKWgDXdn9OfqhAzFzvTUH> ;
  rdfs:seeAlso ifc:IfcCoveringEnumType ;
  rdfs:subClassOf beo:Covering ;
.
beo:Covering-FLOORING
  rdf:type owl:Class ;
  rdfs:isDefinedBy <http://pi.pauwel.be/voc/buildingelement> ;
  rdfs:label "Flooring"@en ;
  rdfs:label "gulv"@nb-no ;
  rdfs:seeAlso <http://bsdd.buildingsmart.org/#concept/details/1MZNPRnDz1jOV_XCmntitl> ;
  rdfs:seeAlso ifc:IfcCoveringEnumType ;
  rdfs:subClassOf beo:Covering ;
.
beo:Covering-INSULATION
  rdf:type owl:Class ;
  rdfs:isDefinedBy <http://pi.pauwel.be/voc/buildingelement> ;
  rdfs:label "Insulation"@en ;
  rdfs:label "isolasjon"@nb-no ;
  rdfs:seeAlso <http://bsdd.buildingsmart.org/#concept/details/0m_WyU8An7RAFjJPRPQn1j> ;
  rdfs:seeAlso ifc:IfcCoveringEnumType ;
  rdfs:subClassOf beo:Covering ;
.
beo:Covering-MEMBRANE
  rdf:type owl:Class ;
  rdfs:comment "vanntett og/eller damptett lag som er festet til sluket i gulvet, på gulvet eller på taket"@nb-no ;
  rdfs:comment """watertight and/or damp proof layer attached to the gully either in the floor or on the floor or
roof"""@en ;
  rdfs:isDefinedBy <http://pi.pauwel.be/voc/buildingelement> ;
  rdfs:label "Dichtungsbahn"@de-de ;
  rdfs:label "Membrane"@en ;
  rdfs:label "film d'étanchéité"@fr-fr ;
  rdfs:label "membran"@nb-no ;
  rdfs:seeAlso <http://bsdd.buildingsmart.org/#concept/details/3vHSkCoT0Hsm00051Mm008> ;
  rdfs:seeAlso ifc:IfcCoveringEnumType ;
  rdfs:subClassOf beo:Covering ;
.
beo:Covering-MOLDING
  rdf:type owl:Class ;
  rdfs:isDefinedBy <http://pi.pauwel.be/voc/buildingelement> ;
  rdfs:label "Gesims"@de-de ;
  rdfs:label "Matériau de la moulure"@fr-fr ;
  rdfs:label "Molding"@en ;
  rdfs:label "gerikt"@nb-no ;
  rdfs:label "taklist"@nb-no ;
  rdfs:seeAlso <http://bsdd.buildingsmart.org/#concept/details/0rO5hENaL0Sx5ncSZm5QWi> ;
  rdfs:seeAlso <http://bsdd.buildingsmart.org/#concept/details/39P8INeF1DvPcZnWFCA0jO> ;
  rdfs:seeAlso ifc:IfcCoveringEnumType ;
  rdfs:subClassOf beo:Covering ;
.
beo:Covering-ROOFING
  rdf:type owl:Class ;
  rdfs:isDefinedBy <http://pi.pauwel.be/voc/buildingelement> ;
  rdfs:label "Roofing"@en ;
  rdfs:label "takdekke"@nb-no ;
  rdfs:label "taktekking"@nb-no ;
  rdfs:seeAlso <http://bsdd.buildingsmart.org/#concept/details/1roIuYcU5AxfQM_Wf18q7t> ;
  rdfs:seeAlso ifc:IfcCoveringEnumType ;
  rdfs:subClassOf beo:Covering ;
.
beo:Covering-SKIRTINGBOARD
  rdf:type owl:Class ;
  rdfs:isDefinedBy <http://pi.pauwel.be/voc/buildingelement> ;
  rdfs:label "Matériau de la plinthe"@fr-fr ;
  rdfs:label "Skirting Board"@en ;
  rdfs:label "Sockelleiste"@de-de ;
  rdfs:label "skirtingboard"@en ;
  rdfs:label "幅木材"@ja-jp ;
  rdfs:seeAlso <http://bsdd.buildingsmart.org/#concept/details/0rhD2N_cvFRRnqQ6pRM9aE> ;
  rdfs:seeAlso ifc:IfcCoveringEnumType ;
  rdfs:subClassOf beo:Covering ;
.
beo:Covering-SLEEVING
  rdf:type owl:Class ;
  rdfs:isDefinedBy <http://pi.pauwel.be/voc/buildingelement> ;
  rdfs:label "Sleeving"@en ;
  rdfs:label "strømpe"@nb-no ;
  rdfs:seeAlso <http://bsdd.buildingsmart.org/#concept/details/2mox_rbmb43xWuIkQmJqW1> ;
  rdfs:seeAlso ifc:IfcCoveringEnumType ;
  rdfs:subClassOf beo:Covering ;
.
beo:Covering-WRAPPING
  rdf:type owl:Class ;
  rdfs:isDefinedBy <http://pi.pauwel.be/voc/buildingelement> ;
  rdfs:label "Wrapping"@en ;
  rdfs:label "innkledning"@nb-no ;
  rdfs:seeAlso <http://bsdd.buildingsmart.org/#concept/details/16XES3__TAdwQ57Ox4T_V8> ;
  rdfs:seeAlso ifc:IfcCoveringEnumType ;
  rdfs:subClassOf beo:Covering ;
.
beo:CurtainWall
  rdf:type owl:Class ;
  rdfs:comment "An exterior wall of a building which is an assembly of components, hung from the edge of the floor/roof structure rather than bearing on a floor. "@en ;
  rdfs:comment "Vertikale und horizontale Bauteile, die untereinander verbunden und mit dem Tragwerk des Gebäudes verankert sind sowie gefüllt sind, um eine raumabschließende, durchgehende Außenschicht zu bilden, die alleine oder gemeinsam mit der übrigen Baukonstruktion, alle normalen Funktionen einer Außenwand bietet, jedoch keine lastabtragenden Funktionen erfüllt"@de-de ;
  rdfs:comment "elementi strutturali verticali e orizzontali, collegati assieme e ancorati alla struttura di supporto dell'edificio e tamponati, a formare una pelle di chiusura continua che fornisce, da sola o in congiunzione con la costruzione, tutte le normali funzioni di un muro esterno, ma non assume nessuna delle caratteristiche portanti della struttura dell'edificio"@it-it ;
  rdfs:comment "elementos estructurales verticales y horizontales, conectados entre sí y anclados a la estructura portante del edificio y rellenados, para formar un conjunto de piel continua que proporciona, por sí mismo o conjuntamente con la construcción del edificio, todas las funciones normales de una pared externa, pero no se hace cargo de ninguna de las características portantes de la estructura del edificio"@es-es ;
  rdfs:comment "les éléments de structure verticaux et horizontaux reliés ensemble et ancrés sur la structure portante du bâtiment et remplis pour former un espace renfermant une peau continue qui fournit, par elle-même ou en combinaison avec la construction du bâtiment, toutes les fonctions normales d'un mur extérieur, mais n'emprunte aucune des caractéristiques de résistance à la charge de la structure du bâtiment"@fr-fr ;
  rdfs:comment "lodrette og vandrette bygningselementer, der er bundet sammen og forankret til bygningens bærende konstruktion og fyldt, så de danner en fortløbende inddækning, der i sig selv eller sammen med bygningskonstruktionen leverer alle en ydermurs normale funktioner, men som ikke påtager sig nogen af bygningskonstruktionens bærende egenskaber"@dk-dk ;
  rdfs:comment "pionowe i poziome elementy konstrukcyjne, połączone ze sobą i zakotwiczone w konstrukcji nośnej budynku i w zabudowie typu plomba, tworzące przestrzeń obejmującą ciągłą warstwę, która zapewnia, samodzielnie lub w połączeniu z konstrukcją budynku, wszystkie normalne funkcje ściany zewnętrznej, ale nie spełnia żadnej funkcji nośnej dla konstrukcji budynku"@pl-pl ;
  rdfs:comment "pysty- ja vaakasuuntaisia rakenneosia, toisiinsa liitettyinä ja rakennuksen kantavaan rakenteeseen kiinnitettynä, täydennettynä muodostamaan suojaavan yhtenäisen pintatilan, jolla on sellaisenaan tai yhdessä rakennuksen kanssa kaikki ulkoisen seinän normaalit toimintaominaisuudet, mutta jota ei käytetä kantavana rakenteena"@fi-fi ;
  rdfs:comment "utvendig, ikkebærende veggkonstruksjon forankret til bygningens hovedbærekonstruksjon. påhengsvegger bygges vanligvis av et rammeverk av metall, tre eller PVC med vertikale og horisontale komponenter som overfører påhengsveggens egenvekt og eventuelle vindkrefter til bygningens bærekonstruksjon"@nb-no ;
  rdfs:comment "vertical and horizontal structural members, connected together and anchored to the supporting structure of the building and infilled, to form a space enclosing continuous skin, which provides, by itself or in conjunction with the building construction, all the normal functions of an external wall, but does not take on any of the load bearing characteristics of the building structure"@en ;
  rdfs:comment "vertikala och horisontella byggnadsdelar som har sammanfogats och förankrats vid byggnadens stödkonstruktion och isolerats, för att skapa en inhägnad med kontinuerlig yta som, av sig själv eller tillsammans med byggnadskonstruktionen, erbjuder alla funktioner som en yttervägg vanligtvis har, men som inte har några av byggnadskonstruktionens bärande egenskaper"@sv-se ;
  rdfs:comment "вертикални и хоризонтални конструктивни елементи, свързани помежду си, закрепени към основната конструкция на сградата и запълнени, за да образуват непрекъсната ограждаща пространството обвивка, която осигурява, самостоятелно или съвместно с конструкцията на сградата, всички изисквани функции към една външна стена, но без да изпълнява никакви функции свързани с носимоспособността на сградната конструкция"@bg-bg ;
  rdfs:isDefinedBy <http://pi.pauwel.be/voc/buildingelement> ;
  rdfs:label "Curtain Wall"@en ;
  rdfs:label "Gordijngevel"@nl ;
  rdfs:label "Gordijngevel"@nl-nl ;
  rdfs:label "Mur rideau"@fr-fr ;
  rdfs:label "Vorhangfassade"@de-de ;
  rdfs:label "Vorhangfassadenbausatz"@de-de ;
  rdfs:label "julkisivujärjestelmä"@fi-fi ;
  rdfs:label "påhengsvegg"@nb-no ;
  rdfs:label "sats till utfackningsväggar"@sv-se ;
  rdfs:label "zestaw ściany osłonowej"@pl-pl ;
  rdfs:label "монтажни модули за окачени фасади"@bg-bg ;
  rdfs:seeAlso <http://bsdd.buildingsmart.org/#concept/details/1nBFK0qT0HuO00025QrE$V> ;
  rdfs:seeAlso ifc:IfcCurtainWall ;
  rdfs:subClassOf beo:BuildingElement ;
.
beo:DiscreteAccessory
  rdf:type owl:Class ;
  rdfs:comment "A representation of different kinds of accessories included in or added to elements."@en ;
  rdfs:isDefinedBy <http://pi.pauwel.be/voc/buildingelement> ;
  rdfs:label "Accessoire composé"@fr-fr ;
  rdfs:label "Discrete Accessory"@en ;
  rdfs:label "Zusatzgerät / Einbauteil"@de-de ;
  rdfs:seeAlso <http://bsdd.buildingsmart.org/#concept/details/0W7W20qT8HuO00025QrE$V> ;
  rdfs:seeAlso ifc:IfcDiscreteAccessory ;
  rdfs:subClassOf beo:ElementComponent ;
.
beo:DiscreteAccessory-ANCHORPLATE
  rdf:type owl:Class ;
  rdfs:isDefinedBy <http://pi.pauwel.be/voc/buildingelement> ;
  rdfs:label "Anchor Plate"@en ;
  rdfs:seeAlso <http://bsdd.buildingsmart.org/#concept/details/1XD5ysVrvF$haI5OgtznWi> ;
  rdfs:seeAlso ifc:IfcDiscreteAccessoryEnumType ;
  rdfs:subClassOf beo:DiscreteAccessory ;
.
beo:DiscreteAccessory-BRACKET
  rdf:type owl:Class ;
  rdfs:comment "An artefact which is projecting from the side of a wall or other structure intended to support some other artefacts.        "@en ;
  rdfs:comment "Brakkett for utstyr"@nb-no ;
  rdfs:comment "Innstøpningsbrakett"@nb-no ;
  rdfs:isDefinedBy <http://pi.pauwel.be/voc/buildingelement> ;
  rdfs:label "Bracket"@en ;
  rdfs:label "Console"@nl-nl ;
  rdfs:label "Winkellasche"@de-de ;
  rdfs:label "bracket for innerwall"@en ;
  rdfs:label "brakett innervegg"@nb-no ;
  rdfs:label "brakett"@nb-no ;
  rdfs:label "console"@en ;
  rdfs:label "crochet"@fr-fr ;
  rdfs:label "innervegg"@nb-no ;
  rdfs:label "innerveggbrakett"@nb-no ;
  rdfs:label "innstøpningsbrakett"@nb-no ;
  rdfs:seeAlso <http://bsdd.buildingsmart.org/#concept/details/3EGCgYGC9F3PmaQ821Ax2u> ;
  rdfs:seeAlso <http://bsdd.buildingsmart.org/#concept/details/3vHPwWoT0Hsm00051Mm008> ;
  rdfs:seeAlso <http://bsdd.buildingsmart.org/#concept/details/3vHcVCoT0Hsm00051Mm008> ;
  rdfs:seeAlso ifc:IfcDiscreteAccessoryEnumType ;
  rdfs:subClassOf beo:DiscreteAccessory ;
.
beo:DiscreteAccessory-SHOE
  rdf:type owl:Class ;
  rdfs:isDefinedBy <http://pi.pauwel.be/voc/buildingelement> ;
  rdfs:label "Shoe"@en ;
  rdfs:label "søylesko"@nb-no ;
  rdfs:seeAlso <http://bsdd.buildingsmart.org/#concept/details/1i44itooP5F9e53Jc$HR0o> ;
  rdfs:seeAlso ifc:IfcDiscreteAccessoryEnumType ;
  rdfs:subClassOf beo:DiscreteAccessory ;
.
beo:Door
  rdf:type owl:Class ;
  rdfs:comment "Bygningsdel som dekker en åpning i utvendig eller innvendig vegg, og som kan åpnes eller stenges for passasje."@nb-no ;
  rdfs:comment "En åpning i en barriære med et dørblad som kan lukke åpningen og en ramme som holder dørbladet."@nb-no ;
  rdfs:comment "a complete unit consisting of a door frame and a door leaf or leaves, supplied with the essential hardware and wheatherseal, as a product from a single source"@en ;
  rdfs:comment "construction for closing an opening intended primarily for access or egress or both. Typically consisting of a panel that swings on hinges or that slides or rotates"@en ;
  rdfs:isDefinedBy <http://pi.pauwel.be/voc/buildingelement> ;
  rdfs:label "Deur"@nl-nl ;
  rdfs:label "Door"@en ;
  rdfs:label "Dør"@da ;
  rdfs:label "Tür"@de-de ;
  rdfs:label "Türeinheit"@de-de ;
  rdfs:label "dør med karm"@nb-no ;
  rdfs:label "dør"@nb-no ;
  rdfs:label "porte"@fr-fr ;
  rdfs:seeAlso <http://bsdd.buildingsmart.org/#concept/details/3vHRQ8oT0Hsm00051Mm008> ;
  rdfs:seeAlso ifc:IfcDoor ;
  rdfs:subClassOf beo:BuildingElement ;
.
beo:Door-DOOR
  rdf:type owl:Class ;
  rdfs:comment "A standard door usually within a wall opening, as a door panel in a curtain wall, or as a \"free standing\" door."@en ;
  rdfs:comment "Bygningsdel som dekker en åpning i utvendig eller innvendig vegg, og som kan åpnes eller stenges for passasje."@nb-no ;
  rdfs:comment "En åpning i en barriære med et dørblad som kan lukke åpningen og en ramme som holder dørbladet."@nb-no ;
  rdfs:comment "a complete unit consisting of a door frame and a door leaf or leaves, supplied with the essential hardware and wheatherseal, as a product from a single source"@en ;
  rdfs:comment "construction for closing an opening intended primarily for access or egress or both. Typically consisting of a panel that swings on hinges or that slides or rotates"@en ;
  rdfs:isDefinedBy <http://pi.pauwel.be/voc/buildingelement> ;
  rdfs:label "Deur"@nl-nl ;
  rdfs:label "Door"@en ;
  rdfs:label "Tür"@de-de ;
  rdfs:label "Türeinheit"@de-de ;
  rdfs:label "bloc-porte"@fr-fr ;
  rdfs:label "deur"@nl-nl ;
  rdfs:label "dør med karm"@nb-no ;
  rdfs:label "dør"@nb-no ;
  rdfs:label "porte"@fr-fr ;
  rdfs:seeAlso <http://bsdd.buildingsmart.org/#concept/details/2reX7MzyDDPP8OCoYtmU7d> ;
  rdfs:seeAlso ifc:IfcDoorEnumType ;
  rdfs:subClassOf beo:Door ;
.
beo:Door-GATE
  rdf:type owl:Class ;
  rdfs:comment """Det engelske ordet 'gate' og det franske ordet 'portail' refererer til produkter utenfor bygninger, for eksempel i innhegninger, gjerder osv.
Det tyske ordet 'Tor' refererer til alle produkter for å stenge åpninger, som tillater passering av kjøretøyer."""@nb-no ;
  rdfs:comment "a movable barrier, usually on hinges, closing an opening in a fence, wall, or other enclosure"@en ;
  rdfs:comment "innretning for å lukke en åpning som er beregnet for passering av kjøretøyer og personer"@nb-no ;
  rdfs:isDefinedBy <http://pi.pauwel.be/voc/buildingelement> ;
  rdfs:label "Gate"@en ;
  rdfs:label "Hek"@nl-nl ;
  rdfs:label "Poort"@nl-nl ;
  rdfs:label "Tor"@de-de ;
  rdfs:label "fermeture"@fr-fr ;
  rdfs:label "port"@nb-no ;
  rdfs:seeAlso <http://bsdd.buildingsmart.org/#concept/details/3C6qVkdNfEGOKvZBfksYwB> ;
  rdfs:seeAlso ifc:IfcDoorEnumType ;
  rdfs:subClassOf beo:Door ;
.
beo:Door-TRAPDOOR
  rdf:type owl:Class ;
  rdfs:isDefinedBy <http://pi.pauwel.be/voc/buildingelement> ;
  rdfs:label "Roof Hatch"@en ;
  rdfs:label "Trap Door"@en ;
  rdfs:label "takluke"@nb-no ;
  rdfs:seeAlso <http://bsdd.buildingsmart.org/#concept/details/3_T7f4cxzB_ur2vAtd6pJe> ;
  rdfs:seeAlso ifc:IfcDoorEnumType ;
  rdfs:subClassOf beo:Door ;
.
beo:ElementComponent
  rdf:type owl:Class ;
  rdfs:comment "A representation for minor items included in, added to or connecting to or between elements, which usually are not of interest from the overall building structure viewpoint. However, these small parts may have vital and load carrying functions within the construction. These items do not provide any actual space boundaries. Typical examples include different kinds of fasteners and various accessories."@en ;
  rdfs:isDefinedBy <http://pi.pauwel.be/voc/buildingelement> ;
  rdfs:label "Composant d'élément"@fr-fr ;
  rdfs:label "Element Component"@en ;
  rdfs:label "Elementenbestandteil"@de-de ;
  rdfs:seeAlso <http://bsdd.buildingsmart.org/#concept/details/2pKpW0qSeHuO00025QrE$V> ;
  rdfs:seeAlso ifc:IfcElementComponent ;
  rdfs:subClassOf contax:ConstructionSubComponent ;
.
beo:Fastener
  rdf:type owl:Class ;
  rdfs:comment "Jointing component that is used to operate a door, window, shutter, gate or drawer ."@en ;
  rdfs:comment "Representations of fixing parts which are used as fasteners to connect or join elements with other elements. "@en ;
  rdfs:isDefinedBy <http://pi.pauwel.be/voc/buildingelement> ;
  rdfs:label "Befestigungsmittel"@de-de ;
  rdfs:label "Elément d'assemblage"@fr-fr ;
  rdfs:label "Fastener"@en ;
  rdfs:label "festeinnretning"@nb-no ;
  rdfs:seeAlso <http://bsdd.buildingsmart.org/#concept/details/2$v8e0qUGHuO00025QrE$V> ;
  rdfs:seeAlso ifc:IfcFastener ;
  rdfs:subClassOf beo:ElementComponent ;
.
beo:Fastener-GLUE
  rdf:type owl:Class ;
  rdfs:comment "bindemedel eller bindemedelslösning för hopfogning av fasta material"@sv-se ;
  rdfs:comment "binder or binder solution for joining solid materials"@en ;
  rdfs:isDefinedBy <http://pi.pauwel.be/voc/buildingelement> ;
  rdfs:label "Glue"@en ;
  rdfs:label "lim"@nb-no ;
  rdfs:label "lim"@sv-se ;
  rdfs:seeAlso <http://bsdd.buildingsmart.org/#concept/details/097NQ9z4T7eOn7nJCQC0yI> ;
  rdfs:seeAlso ifc:IfcFastenerEnumType ;
  rdfs:subClassOf beo:Fastener ;
.
beo:Fastener-MORTAR
  rdf:type owl:Class ;
  rdfs:isDefinedBy <http://pi.pauwel.be/voc/buildingelement> ;
  rdfs:label "Mortar"@en ;
  rdfs:label "mørtel"@nb-no ;
  rdfs:seeAlso <http://bsdd.buildingsmart.org/#concept/details/0dS2xSsC1BbvRjM1MIjNn5> ;
  rdfs:seeAlso ifc:IfcFastenerEnumType ;
  rdfs:subClassOf beo:Fastener ;
.
beo:Fastener-WELD
  rdf:type owl:Class ;
  rdfs:comment "a weld seam between parts of metallic material or other suitable materials"@en ;
  rdfs:comment "a weld seam between parts of metallic material or other suitable materials"@en-gb ;
  rdfs:isDefinedBy <http://pi.pauwel.be/voc/buildingelement> ;
  rdfs:label "Weld"@en ;
  rdfs:label "sveis"@nb-no ;
  rdfs:seeAlso <http://bsdd.buildingsmart.org/#concept/details/01DZw_Z2b4CwKEwBQ9ERPZ> ;
  rdfs:seeAlso ifc:IfcFastenerEnumType ;
  rdfs:subClassOf beo:Fastener ;
.
beo:Footing
  rdf:type owl:Class ;
  rdfs:comment "A part of the foundation of a structure that spreads and transmits the load to the soil. Also characterized as shallow foundation, where the loads are transferred to the ground near the surface."@en ;
  rdfs:comment "Flachgründung"@de-de ;
  rdfs:isDefinedBy <http://pi.pauwel.be/voc/buildingelement> ;
  rdfs:label "Footing"@en ;
  rdfs:label "Fundament"@de-de ;
  rdfs:label "Funderingsvoet"@nl-nl ;
  rdfs:label "fondation"@fr-fr ;
  rdfs:seeAlso <http://bsdd.buildingsmart.org/#concept/details/2vyAW0qUWHuO00025QrE$V> ;
  rdfs:seeAlso ifc:IfcFooting ;
  rdfs:subClassOf beo:BuildingElement ;
.
beo:Footing-CAISSON_FOUNDATION
  rdf:type owl:Class ;
  rdfs:isDefinedBy <http://pi.pauwel.be/voc/buildingelement> ;
  rdfs:label "Caisson Foundation"@en ;
  rdfs:label "senkekasse til fundament"@nb-no ;
  rdfs:seeAlso <http://bsdd.buildingsmart.org/#concept/details/0MGkpmTGDFC80qy7qA0W2w> ;
  rdfs:seeAlso ifc:IfcFootingEnumType ;
  rdfs:subClassOf beo:Footing ;
.
beo:Footing-FOOTING_BEAM
  rdf:type owl:Class ;
  rdfs:isDefinedBy <http://pi.pauwel.be/voc/buildingelement> ;
  rdfs:label "Footing Beam"@en ;
  rdfs:seeAlso <http://bsdd.buildingsmart.org/#concept/details/3hRbiifMvFOgC3tEfSPD8X> ;
  rdfs:seeAlso ifc:IfcFootingEnumType ;
  rdfs:subClassOf beo:Footing ;
.
beo:Footing-PAD_FOOTING
  rdf:type owl:Class ;
  rdfs:isDefinedBy <http://pi.pauwel.be/voc/buildingelement> ;
  rdfs:label "Pad Footing"@en ;
  rdfs:seeAlso <http://bsdd.buildingsmart.org/#concept/details/1XJ0TK6AbBfxMCQLLkdnDr> ;
  rdfs:seeAlso ifc:IfcFootingEnumType ;
  rdfs:subClassOf beo:Footing ;
.
beo:Footing-PILE_CAP
  rdf:type owl:Class ;
  rdfs:isDefinedBy <http://pi.pauwel.be/voc/buildingelement> ;
  rdfs:label "Pile Cap"@en ;
  rdfs:seeAlso <http://bsdd.buildingsmart.org/#concept/details/3$LxhKMZjFuBdi75OQXj0L> ;
  rdfs:seeAlso ifc:IfcFootingEnumType ;
  rdfs:subClassOf beo:Footing ;
.
beo:Footing-STRIP_FOOTING
  rdf:type owl:Class ;
  rdfs:isDefinedBy <http://pi.pauwel.be/voc/buildingelement> ;
  rdfs:label "Strip Footing"@en ;
  rdfs:label "platefundament"@nb-no ;
  rdfs:seeAlso <http://bsdd.buildingsmart.org/#concept/details/0mDEbMPpzB9B_vQTUHZLHe> ;
  rdfs:seeAlso ifc:IfcFootingEnumType ;
  rdfs:subClassOf beo:Footing ;
.
beo:MechanicalFastener
  rdf:type owl:Class ;
  rdfs:comment "A fastener connecting building elements mechanically. A single instance may represent one or many of actual mechanical fasteners, for example an array of bolts or a row of nails."@en ;
  rdfs:isDefinedBy <http://pi.pauwel.be/voc/buildingelement> ;
  rdfs:label "Mechanical Fastener"@en ;
  rdfs:label "MechanicalFastener"@en ;
  rdfs:label "Mechanisches Befestigungsmittel"@de-de ;
  rdfs:label "mekanisk festemiddel"@nb-no ;
  rdfs:seeAlso <http://bsdd.buildingsmart.org/#concept/details/2$KV20qV0HuO00025QrE$V> ;
  rdfs:seeAlso ifc:IfcMechanicalFastener ;
  rdfs:subClassOf beo:ElementComponent ;
.
beo:MechanicalFastener-ANCHORBOLT
  rdf:type owl:Class ;
  rdfs:isDefinedBy <http://pi.pauwel.be/voc/buildingelement> ;
  rdfs:label "Anchor Bolt"@en ;
  rdfs:label "mekanisk ankerbolt"@nb-no ;
  rdfs:seeAlso <http://bsdd.buildingsmart.org/#concept/details/3NJqge3HD7du28Nje_S1Yv> ;
  rdfs:seeAlso ifc:IfcMechanicalFastenerEnumType ;
  rdfs:subClassOf beo:MechanicalFastener ;
.
beo:MechanicalFastener-BOLT
  rdf:type owl:Class ;
  rdfs:comment "a threaded cylindrical rod that engages with a similarly threaded hole in a nut or any other part to form a fastener. the mechanical fastener often also includes one or more washers and one or more nuts."@en ;
  rdfs:isDefinedBy <http://pi.pauwel.be/voc/buildingelement> ;
  rdfs:label "Bolt"@en ;
  rdfs:label "mekanisk festemiddel - bolt"@nb-no ;
  rdfs:seeAlso <http://bsdd.buildingsmart.org/#concept/details/2yfVRHZ2X7heCLVLk0oVBK> ;
  rdfs:seeAlso ifc:IfcMechanicalFastenerEnumType ;
  rdfs:subClassOf beo:MechanicalFastener ;
.
beo:MechanicalFastener-DOWEL
  rdf:type owl:Class ;
  rdfs:comment "Dybel"@nb-no ;
  rdfs:comment "rod protruding from the toe of the sheet pile, used for fixing sheet piles to the bed-rock"@en ;
  rdfs:comment "stag som stikker ut fra foten av spuntnålen, og som brukes for å feste spunten til fjell"@nb-no ;
  rdfs:isDefinedBy <http://pi.pauwel.be/voc/buildingelement> ;
  rdfs:label "Dowel"@en ;
  rdfs:label "Felsdübel"@de-de ;
  rdfs:label "dowel"@en ;
  rdfs:label "dybel"@nb-no ;
  rdfs:label "goujon pour rocher"@fr-fr ;
  rdfs:label "rock dowel"@en ;
  rdfs:seeAlso <http://bsdd.buildingsmart.org/#concept/details/2jZSkKNyPBMwSeeMxlYWrc> ;
  rdfs:seeAlso <http://bsdd.buildingsmart.org/#concept/details/3vHOxEoT0Hsm00051Mm008> ;
  rdfs:seeAlso ifc:IfcMechanicalFastenerEnumType ;
  rdfs:subClassOf beo:MechanicalFastener ;
.
beo:MechanicalFastener-NAIL
  rdf:type owl:Class ;
  rdfs:isDefinedBy <http://pi.pauwel.be/voc/buildingelement> ;
  rdfs:label "Nail"@en ;
  rdfs:label "spiker"@nb-no ;
  rdfs:seeAlso <http://bsdd.buildingsmart.org/#concept/details/1WICu7sp12cQ$$2QCHf$DB> ;
  rdfs:seeAlso ifc:IfcMechanicalFastenerEnumType ;
  rdfs:subClassOf beo:MechanicalFastener ;
.
beo:MechanicalFastener-NAILPLATE
  rdf:type owl:Class ;
  rdfs:isDefinedBy <http://pi.pauwel.be/voc/buildingelement> ;
  rdfs:label "Nail Plate"@en ;
  rdfs:label "spikerplate"@nb-no ;
  rdfs:seeAlso <http://bsdd.buildingsmart.org/#concept/details/26FDcCBjH3BOLZTZb29fxk> ;
  rdfs:seeAlso ifc:IfcMechanicalFastenerEnumType ;
  rdfs:subClassOf beo:MechanicalFastener ;
.
beo:MechanicalFastener-RIVET
  rdf:type owl:Class ;
  rdfs:isDefinedBy <http://pi.pauwel.be/voc/buildingelement> ;
  rdfs:label "Rivet"@en ;
  rdfs:label "nagle"@nb-no ;
  rdfs:seeAlso <http://bsdd.buildingsmart.org/#concept/details/1zynxAt3H1eAVfmukRcO4R> ;
  rdfs:seeAlso ifc:IfcMechanicalFastenerEnumType ;
  rdfs:subClassOf beo:MechanicalFastener ;
.
beo:MechanicalFastener-SCREW
  rdf:type owl:Class ;
  rdfs:isDefinedBy <http://pi.pauwel.be/voc/buildingelement> ;
  rdfs:label "Screw"@en ;
  rdfs:label "skrue"@nb-no ;
  rdfs:seeAlso <http://bsdd.buildingsmart.org/#concept/details/2NLmoal3LAGxceh8SPCvI7> ;
  rdfs:seeAlso ifc:IfcMechanicalFastenerEnumType ;
  rdfs:subClassOf beo:MechanicalFastener ;
.
beo:MechanicalFastener-SHEARCONNECTOR
  rdf:type owl:Class ;
  rdfs:isDefinedBy <http://pi.pauwel.be/voc/buildingelement> ;
  rdfs:label "Shear Connector"@en ;
  rdfs:seeAlso <http://bsdd.buildingsmart.org/#concept/details/0sHCCoroj0pesEpqdsmtRT> ;
  rdfs:seeAlso ifc:IfcMechanicalFastenerEnumType ;
  rdfs:subClassOf beo:MechanicalFastener ;
.
beo:MechanicalFastener-STAPLE
  rdf:type owl:Class ;
  rdfs:isDefinedBy <http://pi.pauwel.be/voc/buildingelement> ;
  rdfs:label "Staple"@en ;
  rdfs:label "stift"@nb-no ;
  rdfs:seeAlso <http://bsdd.buildingsmart.org/#concept/details/3ugeBu3lP8WANu_d7DFAtv> ;
  rdfs:seeAlso ifc:IfcMechanicalFastenerEnumType ;
  rdfs:subClassOf beo:MechanicalFastener ;
.
beo:MechanicalFastener-STUDSHEARCONNECTOR
  rdf:type owl:Class ;
  rdfs:isDefinedBy <http://pi.pauwel.be/voc/buildingelement> ;
  rdfs:label "Stud Shear Connector"@en ;
  rdfs:seeAlso <http://bsdd.buildingsmart.org/#concept/details/2VmXuOwNvFIxXMT91lYI9q> ;
  rdfs:seeAlso ifc:IfcMechanicalFastenerEnumType ;
  rdfs:subClassOf beo:MechanicalFastener ;
.
beo:Member
  rdf:type owl:Class ;
  rdfs:comment "A structural member designed to carry loads between or beyond points of support. It is not required to be load bearing.  A linear architectural or structural element that cannot be expressed more specifically as either a beam or column."@en ;
  rdfs:isDefinedBy <http://pi.pauwel.be/voc/buildingelement> ;
  rdfs:label "Member"@en ;
  rdfs:label "Membre"@fr-fr ;
  rdfs:label "Stab / Stabträger"@de-de ;
  rdfs:label "konstruksjonsdel"@nb-no ;
  rdfs:seeAlso <http://bsdd.buildingsmart.org/#concept/details/11GXc0qV4HuO00025QrE$V> ;
  rdfs:seeAlso ifc:IfcMember ;
  rdfs:subClassOf beo:BuildingElement ;
.
beo:Member-BRACE
  rdf:type owl:Class ;
  rdfs:isDefinedBy <http://pi.pauwel.be/voc/buildingelement> ;
  rdfs:label "Brace"@en ;
  rdfs:label "avstiver"@nb-no ;
  rdfs:seeAlso <http://bsdd.buildingsmart.org/#concept/details/0ccYVvWMX5jwoOSredVplR> ;
  rdfs:seeAlso ifc:IfcMemberEnumType ;
  rdfs:subClassOf beo:Member ;
.
beo:Member-CHORD
  rdf:type owl:Class ;
  rdfs:isDefinedBy <http://pi.pauwel.be/voc/buildingelement> ;
  rdfs:label "Chord"@en ;
  rdfs:label "gurt"@nb-no ;
  rdfs:seeAlso <http://bsdd.buildingsmart.org/#concept/details/1_qCPXQ3j1VBh_PCDSM2PC> ;
  rdfs:seeAlso ifc:IfcMemberEnumType ;
  rdfs:subClassOf beo:Member ;
.
beo:Member-COLLAR
  rdf:type owl:Class ;
  rdfs:isDefinedBy <http://pi.pauwel.be/voc/buildingelement> ;
  rdfs:label "Collar"@en ;
  rdfs:label "krage"@nb-no ;
  rdfs:seeAlso <http://bsdd.buildingsmart.org/#concept/details/1r9F5o8Pv9mPKppdGc$YOw> ;
  rdfs:seeAlso ifc:IfcMemberEnumType ;
  rdfs:subClassOf beo:Member ;
.
beo:Member-MEMBER
  rdf:type owl:Class ;
  rdfs:comment "A structural member designed to carry loads between or beyond points of support. It is not required to be load bearing.  A linear architectural or structural element that cannot be expressed more specifically as either a beam or column."@en ;
  rdfs:isDefinedBy <http://pi.pauwel.be/voc/buildingelement> ;
  rdfs:label "Member"@en ;
  rdfs:label "Membre"@fr-fr ;
  rdfs:label "Stab / Stabträger"@de-de ;
  rdfs:label "konstruksjonsdel"@nb-no ;
  rdfs:seeAlso <http://bsdd.buildingsmart.org/#concept/details/11GXc0qV4HuO00025QrE$V> ;
  rdfs:seeAlso ifc:IfcMemberEnumType ;
  rdfs:subClassOf beo:Member ;
.
beo:Member-MULLION
  rdf:type owl:Class ;
  rdfs:isDefinedBy <http://pi.pauwel.be/voc/buildingelement> ;
  rdfs:label "Mullion"@en ;
  rdfs:label "midtstolpe"@nb-no ;
  rdfs:seeAlso <http://bsdd.buildingsmart.org/#concept/details/2H6TZXz1vEFOlOdhLv3CD7> ;
  rdfs:seeAlso ifc:IfcMemberEnumType ;
  rdfs:subClassOf beo:Member ;
.
beo:Member-PLATE
  rdf:type owl:Class ;
  rdfs:comment "A planar and often flat part with constant thickness. May carry loads between or beyond points of support, or provide stiffening. "@en ;
  rdfs:isDefinedBy <http://pi.pauwel.be/voc/buildingelement> ;
  rdfs:label "Plate"@en ;
  rdfs:label "Platte / Paneel"@de-de ;
  rdfs:label "plaque"@fr-fr ;
  rdfs:label "plate"@nb-no ;
  rdfs:label "platevarmeveksler"@nb-no ;
  rdfs:seeAlso <http://bsdd.buildingsmart.org/#concept/details/3zdC5dewn4ROXxRERahlnc> ;
  rdfs:seeAlso ifc:IfcMemberEnumType ;
  rdfs:subClassOf beo:Member ;
.
beo:Member-POST
  rdf:type owl:Class ;
  rdfs:comment "a linear member (usually used vertically) within a roof structure to support purlins"@en ;
  rdfs:comment "a linear member (usually used vertically) within a roof structure to support purlins"@en-gb ;
  rdfs:isDefinedBy <http://pi.pauwel.be/voc/buildingelement> ;
  rdfs:label "Post"@en ;
  rdfs:label "stolpe"@nb-no ;
  rdfs:seeAlso <http://bsdd.buildingsmart.org/#concept/details/3pLJTABEHCJeV4uMg1OJxY> ;
  rdfs:seeAlso ifc:IfcMemberEnumType ;
  rdfs:subClassOf beo:Member ;
.
beo:Member-PURLIN
  rdf:type owl:Class ;
  rdfs:isDefinedBy <http://pi.pauwel.be/voc/buildingelement> ;
  rdfs:label "Purlin"@en ;
  rdfs:label "takås"@nb-no ;
  rdfs:seeAlso <http://bsdd.buildingsmart.org/#concept/details/2ClC__ZBT6lgGn9bEtyKAq> ;
  rdfs:seeAlso ifc:IfcMemberEnumType ;
  rdfs:subClassOf beo:Member ;
.
beo:Member-RAFTER
  rdf:type owl:Class ;
  rdfs:comment "sperre"@nb-no ;
  rdfs:isDefinedBy <http://pi.pauwel.be/voc/buildingelement> ;
  rdfs:label "Rafter"@en ;
  rdfs:seeAlso <http://bsdd.buildingsmart.org/#concept/details/14MOjpDn1DYfI9uAgvn_Mm> ;
  rdfs:seeAlso ifc:IfcMemberEnumType ;
  rdfs:subClassOf beo:Member ;
.
beo:Member-STRINGER
  rdf:type owl:Class ;
  rdfs:isDefinedBy <http://pi.pauwel.be/voc/buildingelement> ;
  rdfs:label "Stringer"@en ;
  rdfs:label "vange"@nb-no ;
  rdfs:seeAlso <http://bsdd.buildingsmart.org/#concept/details/31phWfaoDEDwTkU1_cQp7G> ;
  rdfs:seeAlso ifc:IfcMemberEnumType ;
  rdfs:subClassOf beo:Member ;
.
beo:Member-STRUT
  rdf:type owl:Class ;
  rdfs:isDefinedBy <http://pi.pauwel.be/voc/buildingelement> ;
  rdfs:label "Strut"@en ;
  rdfs:label "trykkstav"@nb-no ;
  rdfs:seeAlso <http://bsdd.buildingsmart.org/#concept/details/0F1OouH1f9rPC$dWa4xYLb> ;
  rdfs:seeAlso ifc:IfcMemberEnumType ;
  rdfs:subClassOf beo:Member ;
.
beo:Member-STUD
  rdf:type owl:Class ;
  rdfs:isDefinedBy <http://pi.pauwel.be/voc/buildingelement> ;
  rdfs:label "Stud"@en ;
  rdfs:label "stender"@nb-no ;
  rdfs:seeAlso <http://bsdd.buildingsmart.org/#concept/details/14DS4URKP2au1B2s5ghLFp> ;
  rdfs:seeAlso ifc:IfcMemberEnumType ;
  rdfs:subClassOf beo:Member ;
.
beo:Pile
  rdf:type owl:Class ;
  rdfs:comment "A vertical structural member of timber, concrete, or steel, driven into the earth as a foundation or support for a structure for the transfer of actions. "@en ;
  rdfs:comment "En stråle av tømmer, betong eller stål, drevet ned i jorden som fundament eller støtte til en struktur."@nb-no ;
  rdfs:comment "slankt bærende element i grunnen for overføring av laster. I denne europeiske standarden er slankhetsforholdet ikke begrenset"@nb-no ;
  rdfs:isDefinedBy <http://pi.pauwel.be/voc/buildingelement> ;
  rdfs:label "Fundament / Tiefgründung"@de-de ;
  rdfs:label "Pfahl"@de-de ;
  rdfs:label "Pile"@en ;
  rdfs:label "pel"@nb-no ;
  rdfs:label "pele"@nb-no ;
  rdfs:label "pieu"@fr-fr ;
  rdfs:label "pæl"@nb-no ;
  rdfs:seeAlso <http://bsdd.buildingsmart.org/#concept/details/3vHXEAoT0Hsm00051Mm008> ;
  rdfs:seeAlso ifc:IfcPile ;
  rdfs:subClassOf beo:BuildingElement ;
.
beo:Pile-BORED
  rdf:type owl:Class ;
  rdfs:isDefinedBy <http://pi.pauwel.be/voc/buildingelement> ;
  rdfs:label "Bored Pile"@en ;
  rdfs:label "boret pel"@nb-no ;
  rdfs:seeAlso <http://bsdd.buildingsmart.org/#concept/details/1INEbwMtrBy9rKhAuvXYmq> ;
  rdfs:seeAlso ifc:IfcPileEnumType ;
  rdfs:subClassOf beo:Pile ;
.
beo:Pile-COHESION
  rdf:type owl:Class ;
  rdfs:isDefinedBy <http://pi.pauwel.be/voc/buildingelement> ;
  rdfs:label "Cohesion Pile"@en ;
  rdfs:label "kohesjon pel"@nb-no ;
  rdfs:seeAlso <http://bsdd.buildingsmart.org/#concept/details/3xzAjG3Uv5qeCDRxYCXd4d> ;
  rdfs:seeAlso ifc:IfcPileEnumType ;
  rdfs:subClassOf beo:Pile ;
.
beo:Pile-DRIVEN
  rdf:type owl:Class ;
  rdfs:isDefinedBy <http://pi.pauwel.be/voc/buildingelement> ;
  rdfs:label "Driven Pile"@en ;
  rdfs:label "rammet pel"@nb-no ;
  rdfs:seeAlso <http://bsdd.buildingsmart.org/#concept/details/2Qg5YD6TD299EHtweCaOOy> ;
  rdfs:seeAlso ifc:IfcPileEnumType ;
  rdfs:subClassOf beo:Pile ;
.
beo:Pile-FRICTION
  rdf:type owl:Class ;
  rdfs:isDefinedBy <http://pi.pauwel.be/voc/buildingelement> ;
  rdfs:label "Friction Pile"@en ;
  rdfs:label "friksjonspele"@nb-no ;
  rdfs:seeAlso <http://bsdd.buildingsmart.org/#concept/details/3LgOubO_D3EhcElUZP9dMe> ;
  rdfs:seeAlso ifc:IfcPileEnumType ;
  rdfs:subClassOf beo:Pile ;
.
beo:Pile-JETGROUTING
  rdf:type owl:Class ;
  rdfs:isDefinedBy <http://pi.pauwel.be/voc/buildingelement> ;
  rdfs:label "Jet Grouting Pile"@en ;
  rdfs:seeAlso <http://bsdd.buildingsmart.org/#concept/details/1tI0jqBjHEmADWyrGGYig6> ;
  rdfs:seeAlso ifc:IfcPileEnumType ;
  rdfs:subClassOf beo:Pile ;
.
beo:Pile-SUPPORT
  rdf:type owl:Class ;
  rdfs:isDefinedBy <http://pi.pauwel.be/voc/buildingelement> ;
  rdfs:label "Support"@en ;
  rdfs:label "støtte"@nb-no ;
  rdfs:seeAlso <http://bsdd.buildingsmart.org/#concept/details/3qZud6iazFjOZ3wK3WoQch> ;
  rdfs:seeAlso ifc:IfcPileEnumType ;
  rdfs:subClassOf beo:Pile ;
.
beo:Plate
  rdf:type owl:Class ;
  rdfs:comment "A planar and often flat part with constant thickness. May carry loads between or beyond points of support, or provide stiffening. "@en ;
  rdfs:isDefinedBy <http://pi.pauwel.be/voc/buildingelement> ;
  rdfs:label "Plate"@en ;
  rdfs:label "Platte / Paneel"@de-de ;
  rdfs:label "plaque"@fr-fr ;
  rdfs:label "plate"@nb-no ;
  rdfs:seeAlso <http://bsdd.buildingsmart.org/#concept/details/3z14Y0qVCHuO00025QrE$V> ;
  rdfs:seeAlso ifc:IfcPlate ;
  rdfs:subClassOf beo:BuildingElement ;
.
beo:Plate-CURTAIN_PANEL
  rdf:type owl:Class ;
  rdfs:comment "a planar element within a curtain wall, often consisting of a frame with fixed glazing"@en ;
  rdfs:comment "a planar element within a curtain wall, often consisting of a frame with fixed glazing"@en-gb ;
  rdfs:isDefinedBy <http://pi.pauwel.be/voc/buildingelement> ;
  rdfs:label "Curtain Panel"@en ;
  rdfs:label "skjermpanel"@nb-no ;
  rdfs:seeAlso <http://bsdd.buildingsmart.org/#concept/details/2N7mbvPFL0QRlf$nLuQE0U> ;
  rdfs:seeAlso ifc:IfcPlateEnumType ;
  rdfs:subClassOf beo:Plate ;
.
beo:Plate-SHEET
  rdf:type owl:Class ;
  rdfs:isDefinedBy <http://pi.pauwel.be/voc/buildingelement> ;
  rdfs:label "Sheet"@en ;
  rdfs:seeAlso <http://bsdd.buildingsmart.org/#concept/details/2C4D8j05v51eRokWOWtlju> ;
  rdfs:seeAlso ifc:IfcPlateEnumType ;
  rdfs:subClassOf beo:Plate ;
.
beo:Railing
  rdf:type owl:Class ;
  rdfs:comment "A frame assembly adjacent to human circulation spaces and at some space boundaries where it is used in line of walls or to compliment walls. Designed to aid humans, either as an optional physical support, or to prevent injury by falling."@en ;
  rdfs:isDefinedBy <http://pi.pauwel.be/voc/buildingelement> ;
  rdfs:label "Garde corps"@fr-fr ;
  rdfs:label "Geländer"@de-de ;
  rdfs:label "Gelænder"@da ;
  rdfs:label "Hekwerk"@nl-nl ;
  rdfs:label "Leuning"@nl ;
  rdfs:label "Railing"@en ;
  rdfs:label "Reling"@nl-nl ;
  rdfs:label "garde-corps"@fr-fr ;
  rdfs:label "rekkverk"@nb-no ;
  rdfs:seeAlso <http://bsdd.buildingsmart.org/#concept/details/02irk0qVyHuO00025QrE$V> ;
  rdfs:seeAlso ifc:IfcRailing ;
  rdfs:subClassOf beo:BuildingElement ;
.
beo:Railing-BALUSTRADE
  rdf:type owl:Class ;
  rdfs:comment "A balustrade is a separation construction alongside the edges of floors, roofs, stairs and ramps, protecting against falling into the deep."@en ;
  rdfs:isDefinedBy <http://pi.pauwel.be/voc/buildingelement> ;
  rdfs:label "Balustrade"@en ;
  rdfs:label "Geländer"@de-de ;
  rdfs:label "Hekwerk"@nl-nl ;
  rdfs:label "balustrader"@nb-no ;
  rdfs:label "rekkverk"@nb-no ;
  rdfs:seeAlso <http://bsdd.buildingsmart.org/#concept/details/0ZHKicPyL9l8uyCir_Dsef> ;
  rdfs:seeAlso <http://bsdd.buildingsmart.org/#concept/details/30Ez0HE6XAHQh6wJkRK6T$> ;
  rdfs:seeAlso ifc:IfcRailingEnumType ;
  rdfs:subClassOf beo:Railing ;
.
beo:Railing-GUARDRAIL
  rdf:type owl:Class ;
  rdfs:comment "A frame assembly adjacent to human circulation spaces and at some space boundaries where it is used in line of walls or to compliment walls. Designed to aid humans, either as an optional physical support, or to prevent injury by falling."@en ;
  rdfs:isDefinedBy <http://pi.pauwel.be/voc/buildingelement> ;
  rdfs:label "Garde corps"@fr-fr ;
  rdfs:label "Geländer"@de-de ;
  rdfs:label "Guardrail"@en ;
  rdfs:label "garde-corps"@fr-fr ;
  rdfs:label "rekkverk"@nb-no ;
  rdfs:seeAlso <http://bsdd.buildingsmart.org/#concept/details/2804vLstn5DfaH_vxv53w3> ;
  rdfs:seeAlso ifc:IfcRailingEnumType ;
  rdfs:subClassOf beo:Railing ;
.
beo:Railing-HANDRAIL
  rdf:type owl:Class ;
  rdfs:comment "Håndlister, typisk i korridorer"@nb-no ;
  rdfs:isDefinedBy <http://pi.pauwel.be/voc/buildingelement> ;
  rdfs:label "Handlauf"@de-de ;
  rdfs:label "Handrail"@en ;
  rdfs:label "håndlist"@nb-no ;
  rdfs:label "main courante"@fr-fr ;
  rdfs:seeAlso <http://bsdd.buildingsmart.org/#concept/details/3vHRZWoT0Hsm00051Mm008> ;
  rdfs:seeAlso ifc:IfcRailingEnumType ;
  rdfs:subClassOf beo:Railing ;
.
beo:Ramp
  rdf:type owl:Class ;
  rdfs:comment "A vertical passageway which provides a human circulation link between one floor level and another floor level at a different elevation. Normally does not include steps."@en ;
  rdfs:comment "Rampe"@nb-no ;
  rdfs:isDefinedBy <http://pi.pauwel.be/voc/buildingelement> ;
  rdfs:label "Helling"@nl ;
  rdfs:label "Ramp"@en ;
  rdfs:label "Rampe"@da ;
  rdfs:label "Rampe"@de-de ;
  rdfs:label "Rampe"@fr-fr ;
  rdfs:label "helling"@nl-nl ;
  rdfs:label "hellingbaan"@nl-nl ;
  rdfs:label "rampe"@nb-no ;
  rdfs:label "skråplan"@nb-no ;
  rdfs:seeAlso <http://bsdd.buildingsmart.org/#concept/details/0kpjo0qVyHuO00025QrE$V> ;
  rdfs:seeAlso ifc:IfcRamp ;
  rdfs:subClassOf beo:BuildingElement ;
.
beo:Ramp-HALF_TURN_RAMP
  rdf:type owl:Class ;
  rdfs:isDefinedBy <http://pi.pauwel.be/voc/buildingelement> ;
  rdfs:label "Half Turn Ramp"@en ;
  rdfs:label "halv omdreining rampe"@nb-no ;
  rdfs:seeAlso <http://bsdd.buildingsmart.org/#concept/details/1hJB5FgjL4_v2TrvOBjmzz> ;
  rdfs:seeAlso ifc:IfcRampEnumType ;
  rdfs:subClassOf beo:Ramp ;
.
beo:Ramp-QUARTER_TURN_RAMP
  rdf:type owl:Class ;
  rdfs:isDefinedBy <http://pi.pauwel.be/voc/buildingelement> ;
  rdfs:label "Quarter Turn Ramp"@en ;
  rdfs:label "rampe med en sving"@nb-no ;
  rdfs:seeAlso <http://bsdd.buildingsmart.org/#concept/details/1FZ7G8CAP2UxmW6fnuOOfQ> ;
  rdfs:seeAlso ifc:IfcRampEnumType ;
  rdfs:subClassOf beo:Ramp ;
.
beo:Ramp-SPIRAL_RAMP
  rdf:type owl:Class ;
  rdfs:isDefinedBy <http://pi.pauwel.be/voc/buildingelement> ;
  rdfs:label "Spiral Ramp"@en ;
  rdfs:seeAlso <http://bsdd.buildingsmart.org/#concept/details/2__YGgu4XCN9NmT3LhvE6V> ;
  rdfs:seeAlso ifc:IfcRampEnumType ;
  rdfs:subClassOf beo:Ramp ;
.
beo:Ramp-STRAIGHT_RUN_RAMP
  rdf:type owl:Class ;
  rdfs:isDefinedBy <http://pi.pauwel.be/voc/buildingelement> ;
  rdfs:label "Straight Run Ramp"@en ;
  rdfs:seeAlso <http://bsdd.buildingsmart.org/#concept/details/1SYNqJ72H64g7EG2vm8VJu> ;
  rdfs:seeAlso ifc:IfcRampEnumType ;
  rdfs:subClassOf beo:Ramp ;
.
beo:Ramp-TWO_QUARTER_TURN_RAMP
  rdf:type owl:Class ;
  rdfs:isDefinedBy <http://pi.pauwel.be/voc/buildingelement> ;
  rdfs:label "Two Quarter Turn Ramp"@en ;
  rdfs:label "rampe med to svinger"@nb-no ;
  rdfs:seeAlso <http://bsdd.buildingsmart.org/#concept/details/2wUjACPhnDyAgFiGarLaek> ;
  rdfs:seeAlso ifc:IfcRampEnumType ;
  rdfs:subClassOf beo:Ramp ;
.
beo:Ramp-TWO_STRAIGHT_RUN_RAMP
  rdf:type owl:Class ;
  rdfs:isDefinedBy <http://pi.pauwel.be/voc/buildingelement> ;
  rdfs:label "Two Straight Run Ramp"@en ;
  rdfs:seeAlso <http://bsdd.buildingsmart.org/#concept/details/2skPwOQSH1Ex7UR3SpDGbT> ;
  rdfs:seeAlso ifc:IfcRampEnumType ;
  rdfs:subClassOf beo:Ramp ;
.
beo:RampFlight
  rdf:type owl:Class ;
  rdfs:comment "A single inclined segment, or several inclined segments that are connected by a horizontal segment, referred to as a landing. "@en ;
  rdfs:isDefinedBy <http://pi.pauwel.be/voc/buildingelement> ;
  rdfs:label "Ramp Flight"@en ;
  rdfs:label "Rampenlauf"@de-de ;
  rdfs:label "Volée"@fr-fr ;
  rdfs:label "rampe"@nb-no ;
  rdfs:seeAlso <http://bsdd.buildingsmart.org/#concept/details/1kbSG0qVyHuO00025QrE$V> ;
  rdfs:seeAlso ifc:IfcRampFlight ;
  rdfs:subClassOf beo:BuildingElement ;
.
beo:RampFlight-SPIRAL
  rdf:type owl:Class ;
  rdfs:isDefinedBy <http://pi.pauwel.be/voc/buildingelement> ;
  rdfs:label "Spiral"@en ;
  rdfs:label "spiral"@nb-no ;
  rdfs:label "vindel"@nb-no ;
  rdfs:seeAlso <http://bsdd.buildingsmart.org/#concept/details/0CDsSbmyb4GA$0xajhCLYB> ;
  rdfs:seeAlso ifc:IfcRampFlightEnumType ;
  rdfs:subClassOf beo:RampFlight ;
.
beo:RampFlight-STRAIGHT
  rdf:type owl:Class ;
  rdfs:isDefinedBy <http://pi.pauwel.be/voc/buildingelement> ;
  rdfs:label "Straight"@en ;
  rdfs:label "rett"@nb-no ;
  rdfs:seeAlso <http://bsdd.buildingsmart.org/#concept/details/0fyv31IoL8mwvU9TcZR2FC> ;
  rdfs:seeAlso ifc:IfcRampFlightEnumType ;
  rdfs:subClassOf beo:RampFlight ;
.
beo:ReinforcingBar
  rdf:type owl:Class ;
  rdfs:comment "a reinforcing bar is usually made of steel with manufactured deformations in the surface, and used in concrete and masonry construction to provide additional strength. a single instance of this class may represent one or many of actual rebars, for example a row of rebars."@en ;
  rdfs:isDefinedBy <http://pi.pauwel.be/voc/buildingelement> ;
  rdfs:label "Bewehrungsstab"@de-de ;
  rdfs:label "Reinforcing Bar"@en ;
  rdfs:label "armeringsstang"@nb-no ;
  rdfs:label "barre d'armature"@fr-fr ;
  rdfs:seeAlso <http://bsdd.buildingsmart.org/#concept/details/1zlbN6A$z4r8Er6nWNbSMZ> ;
  rdfs:seeAlso ifc:IfcReinforcingBar ;
  rdfs:subClassOf beo:ReinforcingElement ;
.
beo:ReinforcingBar-ANCHORING
  rdf:type owl:Class ;
  rdfs:isDefinedBy <http://pi.pauwel.be/voc/buildingelement> ;
  rdfs:label "Anchoring"@en ;
  rdfs:seeAlso <http://bsdd.buildingsmart.org/#concept/details/3X1mNZzk542ez6g92TTVdH> ;
  rdfs:seeAlso ifc:IfcReinforcingBarEnumType ;
  rdfs:subClassOf beo:ReinforcingBar ;
.
beo:ReinforcingBar-EDGE
  rdf:type owl:Class ;
  rdfs:isDefinedBy <http://pi.pauwel.be/voc/buildingelement> ;
  rdfs:label "Edge"@en ;
  rdfs:seeAlso <http://bsdd.buildingsmart.org/#concept/details/0tRGNh1sv19OvGghikeGYQ> ;
  rdfs:seeAlso ifc:IfcReinforcingBarEnumType ;
  rdfs:subClassOf beo:ReinforcingBar ;
.
beo:ReinforcingBar-LIGATURE
  rdf:type owl:Class ;
  rdfs:isDefinedBy <http://pi.pauwel.be/voc/buildingelement> ;
  rdfs:label "Ligature"@en ;
  rdfs:seeAlso <http://bsdd.buildingsmart.org/#concept/details/09DzOB3qT10AwjdzYLo1LA> ;
  rdfs:seeAlso ifc:IfcReinforcingBarEnumType ;
  rdfs:subClassOf beo:ReinforcingBar ;
.
beo:ReinforcingBar-MAIN
  rdf:type owl:Class ;
  rdfs:isDefinedBy <http://pi.pauwel.be/voc/buildingelement> ;
  rdfs:label "Main"@en ;
  rdfs:seeAlso <http://bsdd.buildingsmart.org/#concept/details/0ZDnwDkMT9fhTxjjLnIpAX> ;
  rdfs:seeAlso ifc:IfcReinforcingBarEnumType ;
  rdfs:subClassOf beo:ReinforcingBar ;
.
beo:ReinforcingBar-PUNCHING
  rdf:type owl:Class ;
  rdfs:isDefinedBy <http://pi.pauwel.be/voc/buildingelement> ;
  rdfs:label "Punching"@en ;
  rdfs:seeAlso <http://bsdd.buildingsmart.org/#concept/details/1RO$_IvNP7eQABna$VzMm_> ;
  rdfs:seeAlso ifc:IfcReinforcingBarEnumType ;
  rdfs:subClassOf beo:ReinforcingBar ;
.
beo:ReinforcingBar-RING
  rdf:type owl:Class ;
  rdfs:isDefinedBy <http://pi.pauwel.be/voc/buildingelement> ;
  rdfs:label "Ring"@en ;
  rdfs:seeAlso <http://bsdd.buildingsmart.org/#concept/details/2zA8DFnW5B8hiBjIlXcktx> ;
  rdfs:seeAlso ifc:IfcReinforcingBarEnumType ;
  rdfs:subClassOf beo:ReinforcingBar ;
.
beo:ReinforcingBar-SHEAR
  rdf:type owl:Class ;
  rdfs:isDefinedBy <http://pi.pauwel.be/voc/buildingelement> ;
  rdfs:label "Shear"@en ;
  rdfs:label "skive"@nb-no ;
  rdfs:seeAlso <http://bsdd.buildingsmart.org/#concept/details/220Wv8D4n11hjTIo_DzfBR> ;
  rdfs:seeAlso ifc:IfcReinforcingBarEnumType ;
  rdfs:subClassOf beo:ReinforcingBar ;
.
beo:ReinforcingBar-STUD
  rdf:type owl:Class ;
  rdfs:isDefinedBy <http://pi.pauwel.be/voc/buildingelement> ;
  rdfs:label "Stud"@en ;
  rdfs:label "stender"@nb-no ;
  rdfs:seeAlso <http://bsdd.buildingsmart.org/#concept/details/3cWXnrQEvAfRCh9LjK26$R> ;
  rdfs:seeAlso ifc:IfcReinforcingBarEnumType ;
  rdfs:subClassOf beo:ReinforcingBar ;
.
beo:ReinforcingElement
  rdf:type owl:Class ;
  rdfs:comment "a reinforcing element represents bars, wires, strands, meshes, tendons, and other components embedded in concrete in such a manner that the reinforcement and the concrete act together in resisting forces."@en ;
  rdfs:isDefinedBy <http://pi.pauwel.be/voc/buildingelement> ;
  rdfs:label "Bewehrung"@de-de ;
  rdfs:label "Reinforcing Element"@en ;
  rdfs:label "elément d'armature"@fr-fr ;
  rdfs:seeAlso <http://bsdd.buildingsmart.org/#concept/details/1aiY$$Wf98m8a5cp3Hzgdu> ;
  rdfs:seeAlso ifc:IfcReinforcingElement ;
  rdfs:subClassOf beo:ElementComponent ;
.
beo:ReinforcingMesh
  rdf:type owl:Class ;
  rdfs:comment "a reinforcing mesh is a series of longitudinal and transverse wires or bars of various gauges, arranged at right angles to each other and welded at all points of intersection; usually used for concrete slab reinforcement. it is also known as welded wire fabric. in scope are plane meshes as well as bent meshes."@en ;
  rdfs:isDefinedBy <http://pi.pauwel.be/voc/buildingelement> ;
  rdfs:label "Bewehrungsmatte"@de-de ;
  rdfs:label "Reinforcing Mesh"@en ;
  rdfs:label "treillis"@fr-fr ;
  rdfs:seeAlso <http://bsdd.buildingsmart.org/#concept/details/3R4n2h6wn67Q4clocrGT7J> ;
  rdfs:seeAlso ifc:IfcReinforcingMesh ;
  rdfs:subClassOf beo:ReinforcingElement ;
.
beo:Roof
  rdf:type owl:Class ;
  rdfs:comment "A covering of the top part of a building. Protects the building against the effects of weather."@en ;
  rdfs:isDefinedBy <http://pi.pauwel.be/voc/buildingelement> ;
  rdfs:label "Dach"@de-de ;
  rdfs:label "Dak"@nl ;
  rdfs:label "Roof"@en ;
  rdfs:label "Tag"@da ;
  rdfs:label "toiture"@fr-fr ;
  rdfs:seeAlso <http://bsdd.buildingsmart.org/#concept/details/2Iyg00qW4HuO00025QrE$V> ;
  rdfs:seeAlso ifc:IfcRoof ;
  rdfs:subClassOf beo:BuildingElement ;
.
beo:Roof-BARREL_ROOF
  rdf:type owl:Class ;
  rdfs:isDefinedBy <http://pi.pauwel.be/voc/buildingelement> ;
  rdfs:label "Barrel Roof"@en ;
  rdfs:seeAlso <http://bsdd.buildingsmart.org/#concept/details/172RLdein1b8WIbTtDLVbc> ;
  rdfs:seeAlso ifc:IfcRoofEnumType ;
  rdfs:subClassOf beo:Roof ;
.
beo:Roof-BUTTERFLY_ROOF
  rdf:type owl:Class ;
  rdfs:isDefinedBy <http://pi.pauwel.be/voc/buildingelement> ;
  rdfs:label "Butterfly Roof"@en ;
  rdfs:seeAlso <http://bsdd.buildingsmart.org/#concept/details/2W6yLK2r968h2TWfGC2xWu> ;
  rdfs:seeAlso ifc:IfcRoofEnumType ;
  rdfs:subClassOf beo:Roof ;
.
beo:Roof-DOME_ROOF
  rdf:type owl:Class ;
  rdfs:isDefinedBy <http://pi.pauwel.be/voc/buildingelement> ;
  rdfs:label "Dome Roof"@en ;
  rdfs:label "kuppeltak"@nb-no ;
  rdfs:seeAlso <http://bsdd.buildingsmart.org/#concept/details/3UcE2aJPP4ewOoRn29unfZ> ;
  rdfs:seeAlso ifc:IfcRoofEnumType ;
  rdfs:subClassOf beo:Roof ;
.
beo:Roof-FLAT_ROOF
  rdf:type owl:Class ;
  rdfs:isDefinedBy <http://pi.pauwel.be/voc/buildingelement> ;
  rdfs:label "Flat Roof"@en ;
  rdfs:label "flatt tak"@nb-no ;
  rdfs:seeAlso <http://bsdd.buildingsmart.org/#concept/details/3IeKrtrMz2SQN7qpJt82e5> ;
  rdfs:seeAlso ifc:IfcRoofEnumType ;
  rdfs:subClassOf beo:Roof ;
.
beo:Roof-FREEFORM
  rdf:type owl:Class ;
  rdfs:isDefinedBy <http://pi.pauwel.be/voc/buildingelement> ;
  rdfs:label "Free Form Roof"@en ;
  rdfs:label "friform tak"@nb-no ;
  rdfs:seeAlso <http://bsdd.buildingsmart.org/#concept/details/2KVHvK7iXAEfKlD5hGIFEc> ;
  rdfs:seeAlso ifc:IfcRoofEnumType ;
  rdfs:subClassOf beo:Roof ;
.
beo:Roof-GABLE_ROOF
  rdf:type owl:Class ;
  rdfs:isDefinedBy <http://pi.pauwel.be/voc/buildingelement> ;
  rdfs:label "Gable Roof"@en ;
  rdfs:label "gavl"@nb-no ;
  rdfs:seeAlso <http://bsdd.buildingsmart.org/#concept/details/0gHJNRNhz6LOTHVbnW$nEj> ;
  rdfs:seeAlso ifc:IfcRoofEnumType ;
  rdfs:subClassOf beo:Roof ;
.
beo:Roof-GAMBREL_ROOF
  rdf:type owl:Class ;
  rdfs:isDefinedBy <http://pi.pauwel.be/voc/buildingelement> ;
  rdfs:label "Gambrel Roof"@en ;
  rdfs:label "gambrel tak"@nb-no ;
  rdfs:seeAlso <http://bsdd.buildingsmart.org/#concept/details/2BnDhKP1HF3vXxnwqccewa> ;
  rdfs:seeAlso ifc:IfcRoofEnumType ;
  rdfs:subClassOf beo:Roof ;
.
beo:Roof-HIPPED_GABLE_ROOF
  rdf:type owl:Class ;
  rdfs:isDefinedBy <http://pi.pauwel.be/voc/buildingelement> ;
  rdfs:label "Hipped Gable Roof"@en ;
  rdfs:label "valm/saltak"@nb-no ;
  rdfs:seeAlso <http://bsdd.buildingsmart.org/#concept/details/3Su_2ncLX1Oes0r3fNr4uE> ;
  rdfs:seeAlso ifc:IfcRoofEnumType ;
  rdfs:subClassOf beo:Roof ;
.
beo:Roof-HIP_ROOF
  rdf:type owl:Class ;
  rdfs:isDefinedBy <http://pi.pauwel.be/voc/buildingelement> ;
  rdfs:label "Hip Roof"@en ;
  rdfs:label "valmtak"@nb-no ;
  rdfs:seeAlso <http://bsdd.buildingsmart.org/#concept/details/0waejMcyT3zwP6nRClvfSx> ;
  rdfs:seeAlso ifc:IfcRoofEnumType ;
  rdfs:subClassOf beo:Roof ;
.
beo:Roof-MANSARD_ROOF
  rdf:type owl:Class ;
  rdfs:isDefinedBy <http://pi.pauwel.be/voc/buildingelement> ;
  rdfs:label "Mansard Roof"@en ;
  rdfs:label "mansardtak"@nb-no ;
  rdfs:seeAlso <http://bsdd.buildingsmart.org/#concept/details/1hB_MPg3j35vRsm_vutjD2> ;
  rdfs:seeAlso ifc:IfcRoofEnumType ;
  rdfs:subClassOf beo:Roof ;
.
beo:Roof-PAVILION_ROOF
  rdf:type owl:Class ;
  rdfs:isDefinedBy <http://pi.pauwel.be/voc/buildingelement> ;
  rdfs:label "Pavilion Roof"@en ;
  rdfs:label "paviljongtak"@nb-no ;
  rdfs:seeAlso <http://bsdd.buildingsmart.org/#concept/details/11Ltv09Eb7lRJW184fZ9gF> ;
  rdfs:seeAlso ifc:IfcRoofEnumType ;
  rdfs:subClassOf beo:Roof ;
.
beo:Roof-RAINBOW_ROOF
  rdf:type owl:Class ;
  rdfs:isDefinedBy <http://pi.pauwel.be/voc/buildingelement> ;
  rdfs:label "Rainbow Roof"@en ;
  rdfs:label "buetak"@nb-no ;
  rdfs:seeAlso <http://bsdd.buildingsmart.org/#concept/details/1MnaPoqUb0L8PGqS6yHzbq> ;
  rdfs:seeAlso ifc:IfcRoofEnumType ;
  rdfs:subClassOf beo:Roof ;
.
beo:Roof-SHED_ROOF
  rdf:type owl:Class ;
  rdfs:isDefinedBy <http://pi.pauwel.be/voc/buildingelement> ;
  rdfs:label "Shed Roof"@en ;
  rdfs:label "pulttak"@nb-no ;
  rdfs:seeAlso <http://bsdd.buildingsmart.org/#concept/details/3GsCyHvinDMPWmecHluOEq> ;
  rdfs:seeAlso ifc:IfcRoofEnumType ;
  rdfs:subClassOf beo:Roof ;
.
beo:ShadingDevice
  rdf:type owl:Class ;
  rdfs:comment """Purpose built devices to protect from the sunlight, from natural light, or screening them from view. Shading devices can form part of the facade or can be mounted inside the building, they can be fixed or operable.
"""@en ;
  rdfs:isDefinedBy <http://pi.pauwel.be/voc/buildingelement> ;
  rdfs:label "Afskærmningsanordning"@da ;
  rdfs:label "Shading Device"@en ;
  rdfs:label "Sonnenschutz festeingebaut"@de-de ;
  rdfs:label "Zonnewering"@nl ;
  rdfs:label "protection solaire"@fr-fr ;
  rdfs:label "skjermingstype"@nb-no ;
  rdfs:seeAlso <http://bsdd.buildingsmart.org/#concept/details/11vQg0qWSHuO00025QrE$V> ;
  rdfs:seeAlso ifc:IfcShadingDevice ;
  rdfs:subClassOf beo:BuildingElement ;
.
beo:ShadingDevice-AWNING
  rdf:type owl:Class ;
  rdfs:comment "a rooflike shelter of canvas or other material extending over a doorway, from the top of a window, over a deck, etc., in order to provide protection, as from the sun"@en ;
  rdfs:comment "product made of fabric/material, located externally, above, in front of, or within an opening and extending in a horizontal and/or sloping and/or vertical plane"@en ;
  rdfs:comment "produkt laget av stoff/materiale som plasseres utvendig over, foran eller i en åpning, og som stikker ut i et horisontalt og/eller skrånende og/eller vertikalt plan"@nb-no ;
  rdfs:isDefinedBy <http://pi.pauwel.be/voc/buildingelement> ;
  rdfs:label "Awning"@en ;
  rdfs:label "Zonwering"@nl-nl ;
  rdfs:label "markise"@nb-no ;
  rdfs:label "solskjerming"@nb-no ;
  rdfs:seeAlso <http://bsdd.buildingsmart.org/#concept/details/3NoPxSKmL7yQEzPT8cmssT> ;
  rdfs:subClassOf beo:ShadingDevice ;
.
beo:ShadingDevice-JALOUSIE
  rdf:type owl:Class ;
  rdfs:comment "Solavskjerming, Persienner"@nb-no ;
  rdfs:comment "product consisting of horizontal slats which can be tilted. it may be retracted by raising and stacking the slats."@en ;
  rdfs:isDefinedBy <http://pi.pauwel.be/voc/buildingelement> ;
  rdfs:label "Jalousie"@de-de ;
  rdfs:label "Jalousie"@en ;
  rdfs:label "blinds"@en ;
  rdfs:label "lamell"@nb-no ;
  rdfs:label "persienne"@nb-no ;
  rdfs:label "persienner"@nb-no ;
  rdfs:label "sjalusi"@nb-no ;
  rdfs:label "stores vénetiens"@fr-fr ;
  rdfs:label "sun shading device"@en ;
  rdfs:label "venetian blind"@en ;
  rdfs:seeAlso <http://bsdd.buildingsmart.org/#concept/details/1$w9Dw6W9DJvD2GfuZFMSR> ;
  rdfs:seeAlso <http://bsdd.buildingsmart.org/#concept/details/3vHLsWoT0Hsm00051Mm008> ;
  rdfs:seeAlso ifc:IfcShadingDeviceEnumType ;
  rdfs:subClassOf beo:ShadingDevice ;
.
beo:ShadingDevice-SHUTTER
  rdf:type owl:Class ;
  rdfs:comment "An artefact which is a part of an assembly that can be moved from a position where it permits contact, to a position where it becomes a part of the enclosure or partition shielding the fixed contacts.                "@en ;
  rdfs:comment "Movable component installed in an opening or duct to form a barrier for security purposes; used to control the passage of heat or light or to delay the spread of fire, smoke or gases."@en ;
  rdfs:comment "Solavskjerming, Solgardin"@nb-no ;
  rdfs:comment "Sun-shading device"@en ;
  rdfs:comment "product installed either internally or externally to provide additional covering and/or protection to an opening"@en ;
  rdfs:isDefinedBy <http://pi.pauwel.be/voc/buildingelement> ;
  rdfs:label "Abschluß"@de-de ;
  rdfs:label "Shutter"@en ;
  rdfs:label "fermeture"@fr-fr ;
  rdfs:label "markise"@nb-no ;
  rdfs:label "skodde"@nb-no ;
  rdfs:label "solgardin"@nb-no ;
  rdfs:seeAlso <http://bsdd.buildingsmart.org/#concept/details/0w_lVI8P10c9rjT$RsNEVr> ;
  rdfs:seeAlso <http://bsdd.buildingsmart.org/#concept/details/27f2fkTV50YwB1IZgMURLa> ;
  rdfs:seeAlso <http://bsdd.buildingsmart.org/#concept/details/3vHUzKoT0Hsm00051Mm008> ;
  rdfs:seeAlso ifc:IfcShadingDeviceEnumType ;
  rdfs:subClassOf beo:ShadingDevice ;
.
beo:Slab
  rdf:type owl:Class ;
  rdfs:comment """A component of the construction that normally encloses a space vertically. May provide the lower support (floor) or upper construction (roof slab) in any space in a building.
Only the core or constructional part of this construction is considered to be a slab. The upper finish (flooring, roofing) and the lower finish (ceiling, suspended ceiling) are considered to be coverings. """@en ;
  rdfs:isDefinedBy <http://pi.pauwel.be/voc/buildingelement> ;
  rdfs:label "Decke / Dachfläche / Bodenplatte"@de-de ;
  rdfs:label "Dæk"@da ;
  rdfs:label "Plaat"@nl ;
  rdfs:label "Slab"@en ;
  rdfs:label "dalle"@fr-fr ;
  rdfs:label "dekke"@nb-no ;
  rdfs:seeAlso <http://bsdd.buildingsmart.org/#concept/details/3pXDk0qWSHuO00025QrE$V> ;
  rdfs:seeAlso ifc:IfcSlab ;
  rdfs:subClassOf beo:BuildingElement ;
.
beo:Slab-BASESLAB
  rdf:type owl:Class ;
  rdfs:isDefinedBy <http://pi.pauwel.be/voc/buildingelement> ;
  rdfs:label "Base Slab"@en ;
  rdfs:label "støpt fundament"@nb-no ;
  rdfs:seeAlso <http://bsdd.buildingsmart.org/#concept/details/1hBroEIeL9neS3mSSGZiyC> ;
  rdfs:seeAlso ifc:IfcSlabEnumType ;
  rdfs:subClassOf beo:Slab ;
.
beo:Slab-FLOOR
  rdf:type owl:Class ;
  rdfs:isDefinedBy <http://pi.pauwel.be/voc/buildingelement> ;
  rdfs:label "Floor"@en ;
  rdfs:label "dekke"@nb-no ;
  rdfs:label "gulv"@nb-no ;
  rdfs:seeAlso <http://bsdd.buildingsmart.org/#concept/details/0jBALpJIv7vvlWkbd9HdCx> ;
  rdfs:seeAlso ifc:IfcSlabEnumType ;
  rdfs:subClassOf beo:Slab ;
.
beo:Slab-LANDING
  rdf:type owl:Class ;
  rdfs:isDefinedBy <http://pi.pauwel.be/voc/buildingelement> ;
  rdfs:label "Landing"@en ;
  rdfs:label "repo"@nb-no ;
  rdfs:seeAlso <http://bsdd.buildingsmart.org/#concept/details/3tQbZvvrfA8OUjU1kc2rUZ> ;
  rdfs:seeAlso ifc:IfcSlabEnumType ;
  rdfs:subClassOf beo:Slab ;
.
beo:Slab-ROOF
  rdf:type owl:Class ;
  rdfs:comment "A covering of the top part of a building. Protects the building against the effects of weather."@en ;
  rdfs:isDefinedBy <http://pi.pauwel.be/voc/buildingelement> ;
  rdfs:label "Dach"@de-de ;
  rdfs:label "Roof"@en ;
  rdfs:label "flatt tak"@nb-no ;
  rdfs:label "toiture"@fr-fr ;
  rdfs:seeAlso <http://bsdd.buildingsmart.org/#concept/details/3Hvwx39_rCaRS49F4qRGBb> ;
  rdfs:seeAlso ifc:IfcSlabEnumType ;
  rdfs:subClassOf beo:Slab ;
.
beo:Stair
  rdf:type owl:Class ;
  rdfs:comment "A vertical passageway allowing occupants to walk (step) from one floor level to another floor level at a different elevation. May include a landing as an intermediate floor slab."@en ;
  rdfs:isDefinedBy <http://pi.pauwel.be/voc/buildingelement> ;
  rdfs:label "Stair"@en ;
  rdfs:label "Trap"@nl ;
  rdfs:label "Trap"@nl-nl ;
  rdfs:label "Trappe"@da ;
  rdfs:label "Trapslag"@nl-nl ;
  rdfs:label "Treppe"@de-de ;
  rdfs:label "escalier"@fr-fr ;
  rdfs:label "trapp"@nb-no ;
  rdfs:seeAlso <http://bsdd.buildingsmart.org/#concept/details/3DhWM0qWmHuO00025QrE$V> ;
  rdfs:seeAlso ifc:IfcStair ;
  rdfs:subClassOf beo:BuildingElement ;
.
beo:Stair-CURVED_RUN_STAIR
  rdf:type owl:Class ;
  rdfs:comment "a stair extending from one level to another without turns or winders. the stair is consisting of one curved flight."@en ;
  rdfs:isDefinedBy <http://pi.pauwel.be/voc/buildingelement> ;
  rdfs:label "Curved Run Stair"@en ;
  rdfs:seeAlso <http://bsdd.buildingsmart.org/#concept/details/1lkxIX8Gj23Bi50H2qpZB9> ;
  rdfs:seeAlso ifc:IfcStairEnumType ;
  rdfs:subClassOf beo:Stair ;
.
beo:Stair-DOUBLE_RETURN_STAIR
  rdf:type owl:Class ;
  rdfs:comment "a stair having one straight flight to a wide quarterspace landing, and two side flights from that landing into opposite directions. the stair is making a 90° turn. the direction of traffic is determined by the walking line."@en ;
  rdfs:isDefinedBy <http://pi.pauwel.be/voc/buildingelement> ;
  rdfs:label "Double Return Stair"@en ;
  rdfs:seeAlso <http://bsdd.buildingsmart.org/#concept/details/3NNCQTceL7Uf8ZhJf40gs9> ;
  rdfs:seeAlso ifc:IfcStairEnumType ;
  rdfs:subClassOf beo:Stair ;
.
beo:Stair-HALF_TURN_STAIR
  rdf:type owl:Class ;
  rdfs:comment "a stair making a 180° turn, consisting of two straight flights connected by a halfspace landing. the orientation of the turn is determined by the walking line."@en ;
  rdfs:isDefinedBy <http://pi.pauwel.be/voc/buildingelement> ;
  rdfs:label "Half Turn Stair"@en ;
  rdfs:seeAlso <http://bsdd.buildingsmart.org/#concept/details/3YmaH1onP90PM6kEWHUjFv> ;
  rdfs:seeAlso ifc:IfcStairEnumType ;
  rdfs:subClassOf beo:Stair ;
.
beo:Stair-HALF_WINDING_STAIR
  rdf:type owl:Class ;
  rdfs:isDefinedBy <http://pi.pauwel.be/voc/buildingelement> ;
  rdfs:label "Half Winding Stair"@en ;
  rdfs:seeAlso <http://bsdd.buildingsmart.org/#concept/details/0Vw081Hfz1AQne1V5CsfUA> ;
  rdfs:seeAlso ifc:IfcStairEnumType ;
  rdfs:subClassOf beo:Stair ;
.
beo:Stair-QUARTER_TURN_STAIR
  rdf:type owl:Class ;
  rdfs:comment "a stair making a 90° turn, consisting of two straight flights connected by a quarterspace landing. the direction of the turn is determined by the walking line."@en ;
  rdfs:isDefinedBy <http://pi.pauwel.be/voc/buildingelement> ;
  rdfs:label "Quarter Turn Stair"@en ;
  rdfs:seeAlso <http://bsdd.buildingsmart.org/#concept/details/1IEbbDJDHAFQb9SZweXH3x> ;
  rdfs:seeAlso ifc:IfcStairEnumType ;
  rdfs:subClassOf beo:Stair ;
.
beo:Stair-QUARTER_WINDING_STAIR
  rdf:type owl:Class ;
  rdfs:isDefinedBy <http://pi.pauwel.be/voc/buildingelement> ;
  rdfs:label "Quarter Winding Stair"@en ;
  rdfs:seeAlso <http://bsdd.buildingsmart.org/#concept/details/3PzSNWl5T1EgMXH$Tn6uuQ> ;
  rdfs:seeAlso ifc:IfcStairEnumType ;
  rdfs:subClassOf beo:Stair ;
.
beo:Stair-SPIRAL_STAIR
  rdf:type owl:Class ;
  rdfs:isDefinedBy <http://pi.pauwel.be/voc/buildingelement> ;
  rdfs:label "Spiral Stair"@en ;
  rdfs:seeAlso <http://bsdd.buildingsmart.org/#concept/details/0UwQe$TXP47AhE5k0mZzCe> ;
  rdfs:seeAlso ifc:IfcStairEnumType ;
  rdfs:subClassOf beo:Stair ;
.
beo:Stair-STRAIGHT_RUN_STAIR
  rdf:type owl:Class ;
  rdfs:isDefinedBy <http://pi.pauwel.be/voc/buildingelement> ;
  rdfs:label "Straight Run Stair"@en ;
  rdfs:seeAlso <http://bsdd.buildingsmart.org/#concept/details/3p4WSJmK96Oe6HXE$jmWWy> ;
  rdfs:seeAlso ifc:IfcStairEnumType ;
  rdfs:subClassOf beo:Stair ;
.
beo:Stair-THREE_QUARTER_TURN_STAIR
  rdf:type owl:Class ;
  rdfs:isDefinedBy <http://pi.pauwel.be/voc/buildingelement> ;
  rdfs:label "Three Quarter Turn Stair"@en ;
  rdfs:seeAlso <http://bsdd.buildingsmart.org/#concept/details/2jTG3NRNHCyhbsMbwK38v5> ;
  rdfs:seeAlso ifc:IfcStairEnumType ;
  rdfs:subClassOf beo:Stair ;
.
beo:Stair-THREE_QUARTER_WINDING_STAIR
  rdf:type owl:Class ;
  rdfs:isDefinedBy <http://pi.pauwel.be/voc/buildingelement> ;
  rdfs:label "Three Quarter Winding Stair"@en ;
  rdfs:seeAlso <http://bsdd.buildingsmart.org/#concept/details/0rPjGYk_LFnOayZFsJg3tr> ;
  rdfs:seeAlso ifc:IfcStairEnumType ;
  rdfs:subClassOf beo:Stair ;
.
beo:Stair-TWO_CURVED_RUN_STAIR
  rdf:type owl:Class ;
  rdfs:isDefinedBy <http://pi.pauwel.be/voc/buildingelement> ;
  rdfs:label "Two Curved Run Stair"@en ;
  rdfs:seeAlso <http://bsdd.buildingsmart.org/#concept/details/0cSo1dkGL8NunRzp$sQsTc> ;
  rdfs:seeAlso ifc:IfcStairEnumType ;
  rdfs:subClassOf beo:Stair ;
.
beo:Stair-TWO_QUARTER_TURN_STAIR
  rdf:type owl:Class ;
  rdfs:comment "a stair making a 180° turn, consisting of three straight flights connected by two quarterspace landings. the direction of the turns is determined by the walking line"@en ;
  rdfs:isDefinedBy <http://pi.pauwel.be/voc/buildingelement> ;
  rdfs:label "Two Quarter Turn Stair"@en ;
  rdfs:seeAlso <http://bsdd.buildingsmart.org/#concept/details/0mW4DtraD3SA57fcejW4cS> ;
  rdfs:seeAlso ifc:IfcStairEnumType ;
  rdfs:subClassOf beo:Stair ;
.
beo:Stair-TWO_QUARTER_WINDING_STAIR
  rdf:type owl:Class ;
  rdfs:isDefinedBy <http://pi.pauwel.be/voc/buildingelement> ;
  rdfs:label "Two Quarter Winding Stair"@en ;
  rdfs:seeAlso <http://bsdd.buildingsmart.org/#concept/details/3SSlfuJ_nA49lzIOhda6Xr> ;
  rdfs:seeAlso ifc:IfcStairEnumType ;
  rdfs:subClassOf beo:Stair ;
.
beo:Stair-TWO_STRAIGHT_RUN_STAIR
  rdf:type owl:Class ;
  rdfs:comment "a straight stair consisting of two straight flights without turns but with one landing."@en ;
  rdfs:isDefinedBy <http://pi.pauwel.be/voc/buildingelement> ;
  rdfs:label "Two Straight Run Stair"@en ;
  rdfs:seeAlso <http://bsdd.buildingsmart.org/#concept/details/3VuqGJNz160B87TSrFhrM4> ;
  rdfs:seeAlso ifc:IfcStairEnumType ;
  rdfs:subClassOf beo:Stair ;
.
beo:StairFlight
  rdf:type owl:Class ;
  rdfs:comment "An assembly of building components in a single \"run\" of stair steps (not interrupted by a landing)."@en ;
  rdfs:isDefinedBy <http://pi.pauwel.be/voc/buildingelement> ;
  rdfs:label "Stair Flight"@en ;
  rdfs:label "Volée d'escalier"@fr-fr ;
  rdfs:label "trap"@nl-nl ;
  rdfs:label "trapp"@nb-no ;
  rdfs:label "trapslag"@nl-nl ;
  rdfs:label "treppenlauf"@de-de ;
  rdfs:seeAlso <http://bsdd.buildingsmart.org/#concept/details/0pceq0qWqHuO00025QrE$V> ;
  rdfs:seeAlso ifc:IfcStairFlight ;
  rdfs:subClassOf beo:BuildingElement ;
.
beo:StairFlight-CURVED
  rdf:type owl:Class ;
  rdfs:isDefinedBy <http://pi.pauwel.be/voc/buildingelement> ;
  rdfs:label "Curved"@en ;
  rdfs:label "trapp - kurvet"@nb-no ;
  rdfs:seeAlso <http://bsdd.buildingsmart.org/#concept/details/2DeCDqEVHDjwFaGVpyNC89> ;
  rdfs:seeAlso ifc:IfcStairFlightEnumType ;
  rdfs:subClassOf beo:StairFlight ;
.
beo:StairFlight-FREEFORM
  rdf:type owl:Class ;
  rdfs:isDefinedBy <http://pi.pauwel.be/voc/buildingelement> ;
  rdfs:label "Freeform"@en ;
  rdfs:label "friform tak"@nb-no ;
  rdfs:label "friform"@nb-no ;
  rdfs:seeAlso <http://bsdd.buildingsmart.org/#concept/details/0uFuIDRO1EZPmcL8pEkVU$> ;
  rdfs:seeAlso ifc:IfcStairFlightEnumType ;
  rdfs:subClassOf beo:StairFlight ;
.
beo:StairFlight-SPIRAL
  rdf:type owl:Class ;
  rdfs:isDefinedBy <http://pi.pauwel.be/voc/buildingelement> ;
  rdfs:label "Spiral"@en ;
  rdfs:label "scroll"@en ;
  rdfs:label "spiral"@nb-no ;
  rdfs:label "vindel"@nb-no ;
  rdfs:seeAlso <http://bsdd.buildingsmart.org/#concept/details/1zj3DVJij6IBVuIqOLbi46> ;
  rdfs:seeAlso ifc:IfcStairFlightEnumType ;
  rdfs:subClassOf beo:StairFlight ;
.
beo:StairFlight-STRAIGHT
  rdf:type owl:Class ;
  rdfs:isDefinedBy <http://pi.pauwel.be/voc/buildingelement> ;
  rdfs:label "Straight"@en ;
  rdfs:label "rett"@nb-no ;
  rdfs:seeAlso <http://bsdd.buildingsmart.org/#concept/details/247CeErMz16BZyRhwbAOdR> ;
  rdfs:seeAlso ifc:IfcStairFlightEnumType ;
  rdfs:subClassOf beo:StairFlight ;
.
beo:StairFlight-WINDER
  rdf:type owl:Class ;
  rdfs:isDefinedBy <http://pi.pauwel.be/voc/buildingelement> ;
  rdfs:label "Winder"@en ;
  rdfs:label "svingtrapp"@nb-no ;
  rdfs:seeAlso <http://bsdd.buildingsmart.org/#concept/details/3XVLP1SZf8YQfshhp0Vjph> ;
  rdfs:seeAlso ifc:IfcStairFlightEnumType ;
  rdfs:subClassOf beo:StairFlight ;
.
beo:Tendon
  rdf:type owl:Class ;
  rdfs:comment "a tendon is a steel element such as a wire, cable, bar, rod or strand used to impart prestress to concrete when the element is tensioned."@en ;
  rdfs:isDefinedBy <http://pi.pauwel.be/voc/buildingelement> ;
  rdfs:label "Spannglied"@de-de ;
  rdfs:label "Tendon"@en ;
  rdfs:label "cable"@fr-fr ;
  rdfs:seeAlso <http://bsdd.buildingsmart.org/#concept/details/0GEDRkhJ9DdQ2MRE_CaSCF> ;
  rdfs:seeAlso ifc:IfcTendon ;
  rdfs:subClassOf beo:ReinforcingElement ;
.
beo:Tendon-BAR
  rdf:type owl:Class ;
  rdfs:isDefinedBy <http://pi.pauwel.be/voc/buildingelement> ;
  rdfs:label "Bar"@en ;
  rdfs:seeAlso <http://bsdd.buildingsmart.org/#concept/details/3seMZXSSH4YfQCPjOcaoZG> ;
  rdfs:seeAlso ifc:IfcTendonEnumType ;
  rdfs:subClassOf beo:Tendon ;
.
beo:Tendon-COATED
  rdf:type owl:Class ;
  rdfs:isDefinedBy <http://pi.pauwel.be/voc/buildingelement> ;
  rdfs:label "Coated"@en ;
  rdfs:seeAlso <http://bsdd.buildingsmart.org/#concept/details/1WLzEVaRD77A5KPd3$v9DB> ;
  rdfs:seeAlso ifc:IfcTendonEnumType ;
  rdfs:subClassOf beo:Tendon ;
.
beo:Tendon-STRAND
  rdf:type owl:Class ;
  rdfs:isDefinedBy <http://pi.pauwel.be/voc/buildingelement> ;
  rdfs:label "Strand"@en ;
  rdfs:seeAlso <http://bsdd.buildingsmart.org/#concept/details/1d4UrJXi92ivdu3FflJ62n> ;
  rdfs:seeAlso ifc:IfcTendonEnumType ;
  rdfs:subClassOf beo:Tendon ;
.
beo:Tendon-WIRE
  rdf:type owl:Class ;
  rdfs:isDefinedBy <http://pi.pauwel.be/voc/buildingelement> ;
  rdfs:label "Wire"@en ;
  rdfs:seeAlso <http://bsdd.buildingsmart.org/#concept/details/1NCnQvMs9AaRqwexu7DofF> ;
  rdfs:seeAlso ifc:IfcTendonEnumType ;
  rdfs:subClassOf beo:Tendon ;
.
beo:TendonAnchor
  rdf:type owl:Class ;
  rdfs:comment "a tendon anchor is the end connection for tendons in prestressed or posttensioned concrete."@en ;
  rdfs:isDefinedBy <http://pi.pauwel.be/voc/buildingelement> ;
  rdfs:label "Spanngliedanker"@de-de ;
  rdfs:label "Tendon Anchor"@en ;
  rdfs:label "ancrage"@fr-fr ;
  rdfs:seeAlso <http://bsdd.buildingsmart.org/#concept/details/0Z116ntsH6xBFYGYsNg38f> ;
  rdfs:seeAlso ifc:IfcTendonAnchor ;
  rdfs:subClassOf beo:ReinforcingElement ;
.
beo:TendonAnchor-COUPLER
  rdf:type owl:Class ;
  rdfs:isDefinedBy <http://pi.pauwel.be/voc/buildingelement> ;
  rdfs:label "Coupler"@en ;
  rdfs:seeAlso <http://bsdd.buildingsmart.org/#concept/details/2yrjArQAnBL9EdTqIc7Uv7> ;
  rdfs:seeAlso ifc:IfcTendonAnchorEnumType ;
  rdfs:subClassOf beo:TendonAnchor ;
.
beo:TendonAnchor-FIXED_END
  rdf:type owl:Class ;
  rdfs:isDefinedBy <http://pi.pauwel.be/voc/buildingelement> ;
  rdfs:label "Fixed End"@en ;
  rdfs:seeAlso <http://bsdd.buildingsmart.org/#concept/details/133YYoKAv8mBxccTJtzWju> ;
  rdfs:seeAlso ifc:IfcTendonAnchorEnumType ;
  rdfs:subClassOf beo:TendonAnchor ;
.
beo:TendonAnchor-TENSIONING_END
  rdf:type owl:Class ;
  rdfs:isDefinedBy <http://pi.pauwel.be/voc/buildingelement> ;
  rdfs:label "Tensioning End"@en ;
  rdfs:seeAlso <http://bsdd.buildingsmart.org/#concept/details/2Bp8P7qwn1Hg1BaRHyCQP4> ;
  rdfs:seeAlso ifc:IfcTendonAnchorEnumType ;
  rdfs:subClassOf beo:TendonAnchor ;
.
beo:TransportElement
  rdf:type owl:Class ;
  rdfs:comment "A generalization of all transport related objects that move people, animals or goods within a building or building complex. Include elevator (lift), escalator, moving walkway, etc."@en ;
  rdfs:comment """An element type defined by commonly shared information for occurrences of transport elements. The set of shared information may include:
common properties within shared property sets
common material information
common shape representations
It is used to define a transport element specification (i.e. the specific product information that is common to all occurrences of that beam type). """@en ;
  rdfs:isDefinedBy <http://pi.pauwel.be/voc/buildingelement> ;
  rdfs:label "Beförderungsgerät"@de-de ;
  rdfs:label "Equipement de transport"@fr-fr ;
  rdfs:label "Transport Element"@en ;
  rdfs:label "transportelement"@nb-no ;
  rdfs:seeAlso <http://bsdd.buildingsmart.org/#concept/details/3ZSVc0qX4HuO00025QrE$V> ;
  rdfs:seeAlso ifc:IfcTransportElement ;
  rdfs:subClassOf contax:ConstructionComponent ;
.
beo:TransportElement-CRANEWAY
  rdf:type owl:Class ;
  rdfs:comment "An artefact for raising, shifting and lowering heavy weights by means of a projecting swinging arm or with hoisting mechanism supported on an overhead track.        "@en ;
  rdfs:comment "a crane way system, normally including the crane rails, fasteners and the crane. it is primarily used to move heavy goods in a factory or other industry buildings"@en ;
  rdfs:comment "a crane way system, normally including the crane rails, fasteners and the crane. it is primarily used to move heavy goods in a factory or other industry buildings"@en-gb ;
  rdfs:isDefinedBy <http://pi.pauwel.be/voc/buildingelement> ;
  rdfs:label "Craneway"@en ;
  rdfs:label "kran"@nb-no ;
  rdfs:label "kranbane"@nb-no ;
  rdfs:seeAlso <http://bsdd.buildingsmart.org/#concept/details/087V4aTMPA09OItHDUip4G> ;
  rdfs:seeAlso ifc:IfcTransportElementEnumType ;
  rdfs:subClassOf beo:TransportElement ;
.
beo:TransportElement-ELEVATOR
  rdf:type owl:Class ;
  rdfs:comment "a permanent lifting equipment serving defined landing levels, comprising a car, whose dimensions and means of construction clearly permit the access of persons; running at least partially between rigid vertical guides or guides whose inclination to the ve"@en ;
  rdfs:comment "permanent løfteutstyr som betjener definerte etasjenivåer, og som består av en stol hvis dimensjoner og konstruksjonsmåte klart gir adgang for personer, og som minst delvis beveger seg mellom stive, vertikale føringsskinner eller føringer hvor hellingen f"@nb-no ;
  rdfs:isDefinedBy <http://pi.pauwel.be/voc/buildingelement> ;
  rdfs:label "Aufzug"@de-de ;
  rdfs:label "Elevator"@en ;
  rdfs:label "ascenseur"@fr-fr ;
  rdfs:label "heis"@nb-no ;
  rdfs:label "lift"@en ;
  rdfs:seeAlso <http://bsdd.buildingsmart.org/#concept/details/2qanav0WDASA8V5to62fCx> ;
  rdfs:seeAlso <http://bsdd.buildingsmart.org/#concept/details/3vHX1_oT0Hsm00051Mm008> ;
  rdfs:seeAlso ifc:IfcTransportElementEnumType ;
  rdfs:subClassOf beo:TransportElement ;
.
beo:TransportElement-ESCALATOR
  rdf:type owl:Class ;
  rdfs:comment "power-driven, inclined, continuous moving stairway used for raising or lowering persons in which the user carrying surface (e.g. steps) remains horizontal"@en ;
  rdfs:isDefinedBy <http://pi.pauwel.be/voc/buildingelement> ;
  rdfs:label "Escalator"@en ;
  rdfs:label "Fahrtreppe"@de-de ;
  rdfs:label "Roltrap"@nl-nl ;
  rdfs:label "escalier roulant"@fr-fr ;
  rdfs:label "rulletrapp"@nb-no ;
  rdfs:seeAlso <http://bsdd.buildingsmart.org/#concept/details/377eo0WJOHu000025QrE$V> ;
  rdfs:seeAlso <http://bsdd.buildingsmart.org/#concept/details/3vHZncoT0Hsm00051Mm008> ;
  rdfs:seeAlso ifc:IfcTransportElementEnumType ;
  rdfs:subClassOf beo:TransportElement ;
.
beo:TransportElement-LIFTINGGEAR
  rdf:type owl:Class ;
  rdfs:comment "a device used for lifting or lowering heavy goods. It may be manually operated or electrically or pneumatically driven"@en ;
  rdfs:comment "a device used for lifting or lowering heavy goods. It may be manually operated or electrically or pneumatically driven"@en-gb ;
  rdfs:isDefinedBy <http://pi.pauwel.be/voc/buildingelement> ;
  rdfs:label "Lifting Gear"@en ;
  rdfs:label "løfteinretning"@nb-no ;
  rdfs:seeAlso <http://bsdd.buildingsmart.org/#concept/details/3qsVNaK3r6Uw2tccQdpTmo> ;
  rdfs:seeAlso ifc:IfcTransportElementEnumType ;
  rdfs:subClassOf beo:TransportElement ;
.
beo:TransportElement-MOVINGWALKWAY
  rdf:type owl:Class ;
  rdfs:isDefinedBy <http://pi.pauwel.be/voc/buildingelement> ;
  rdfs:label "Moving Walkway"@en ;
  rdfs:label "rullebånd"@nb-no ;
  rdfs:seeAlso <http://bsdd.buildingsmart.org/#concept/details/0Fn7lcsC5As81fnfma0hsy> ;
  rdfs:seeAlso ifc:IfcTransportElementEnumType ;
  rdfs:subClassOf beo:TransportElement ;
.
beo:VibrationIsolator
  rdf:type owl:Class ;
  rdfs:comment "A device used to minimize the effects of vibration transmissibility in a building."@en ;
  rdfs:isDefinedBy <http://pi.pauwel.be/voc/buildingelement> ;
  rdfs:label "Schwingungsisolator"@de-de ;
  rdfs:label "Vibration Isolator"@en ;
  rdfs:label "isolateur de vibrations"@fr-fr ;
  rdfs:label "isolation anti-vibratoire"@fr-fr ;
  rdfs:label "trillingsisolator"@nl-nl ;
  rdfs:label "vibrasjonsisolator"@nb-no ;
  rdfs:seeAlso <http://bsdd.buildingsmart.org/#concept/details/0Oy60xvFT7TO70hyDzhWWZ> ;
  rdfs:seeAlso ifc:IfcVibrationIsolator ;
  rdfs:subClassOf beo:ElementComponent ;
.
beo:VibrationIsolator-COMPRESSION
  rdf:type owl:Class ;
  rdfs:comment "compression type vibration isolator"@en ;
  rdfs:comment "compression type vibration isolator"@en-gb ;
  rdfs:isDefinedBy <http://pi.pauwel.be/voc/buildingelement> ;
  rdfs:label "Compression-based vibration isolator"@en ;
  rdfs:label "kompresjon"@nb-no ;
  rdfs:seeAlso <http://bsdd.buildingsmart.org/#concept/details/0EwSGR8PX1z9zHS_KHBRcA> ;
  rdfs:seeAlso ifc:IfcVibrationIsolatorEnumType ;
  rdfs:subClassOf beo:VibrationIsolator ;
.
beo:VibrationIsolator-SPRING
  rdf:type owl:Class ;
  rdfs:comment "spring type vibration isolator"@en ;
  rdfs:comment "spring type vibration isolator"@en-gb ;
  rdfs:isDefinedBy <http://pi.pauwel.be/voc/buildingelement> ;
  rdfs:label "Spring"@en ;
  rdfs:label "fjær"@nb-no ;
  rdfs:seeAlso <http://bsdd.buildingsmart.org/#concept/details/3cKim0GJf3mxz7EqVVfQ8u> ;
  rdfs:seeAlso ifc:IfcVibrationIsolatorEnumType ;
  rdfs:subClassOf beo:VibrationIsolator ;
.
beo:Wall
  rdf:type owl:Class ;
  rdfs:comment "A vertical construction that bounds or subdivides spaces. Usually vertical, or nearly vertical, planar elements, often designed to bear structural loads. However not required to be load bearing."@en ;
  rdfs:isDefinedBy <http://pi.pauwel.be/voc/buildingelement> ;
  rdfs:label "Muur"@nl ;
  rdfs:label "Væg"@da ;
  rdfs:label "Wall"@en ;
  rdfs:label "Wand"@de-de ;
  rdfs:label "mur"@fr-fr ;
  rdfs:label "vegg"@nb-no ;
  rdfs:label "wall"@en ;
  rdfs:seeAlso <http://bsdd.buildingsmart.org/#concept/details/2Xuqs0qXKHuO00025QrE$V> ;
  rdfs:seeAlso ifc:IfcWall ;
  rdfs:subClassOf beo:BuildingElement ;
.
beo:Wall-ELEMENTEDWALL
  rdf:type owl:Class ;
  rdfs:comment "a stud wall framed with studs and faced with sheetings, sidings, wallboard, or plasterwork"@en ;
  rdfs:comment "a stud wall framed with studs and faced with sheetings, sidings, wallboard, or plasterwork"@en-gb ;
  rdfs:isDefinedBy <http://pi.pauwel.be/voc/buildingelement> ;
  rdfs:label "Elemented Wall"@en ;
  rdfs:label "elementvegg"@nb-no ;
  rdfs:label "systemvegg"@nb-no ;
  rdfs:seeAlso <http://bsdd.buildingsmart.org/#concept/details/0sVBQjaqvEcAVsdRJorFkQ> ;
  rdfs:seeAlso ifc:IfcWallEnumType ;
  rdfs:subClassOf beo:Wall ;
.
beo:Wall-MOVABLE
  rdf:type owl:Class ;
  rdfs:isDefinedBy <http://pi.pauwel.be/voc/buildingelement> ;
  rdfs:label "Flyttbar"@nb-no ;
  rdfs:label "Movable Wall"@en ;
  rdfs:seeAlso <http://bsdd.buildingsmart.org/#concept/details/2nSQnTH_18RB$MO5daYxD0> ;
  rdfs:seeAlso ifc:IfcWallEnumType ;
  rdfs:subClassOf beo:Wall ;
.
beo:Wall-PARAPET
  rdf:type owl:Class ;
  rdfs:comment """Parapet/brystning
Opphøyet kant som stikker opp over tak"""@nb-no ;
  rdfs:isDefinedBy <http://pi.pauwel.be/voc/buildingelement> ;
  rdfs:label "Balustrade"@nl-nl ;
  rdfs:label "Borstwering"@nl-nl ;
  rdfs:label "Parapet Wall"@en ;
  rdfs:label "balustrade"@en ;
  rdfs:label "parapet"@en ;
  rdfs:label "parapet"@nb-no ;
  rdfs:seeAlso <http://bsdd.buildingsmart.org/#concept/details/1uS$40WJmHu000025QrE$V> ;
  rdfs:seeAlso <http://bsdd.buildingsmart.org/#concept/details/2BlEUUV2L2BBUdnPO3PtnQ> ;
  rdfs:seeAlso ifc:IfcWallEnumType ;
  rdfs:subClassOf beo:Wall ;
.
beo:Wall-PARTITIONING
  rdf:type owl:Class ;
  rdfs:isDefinedBy <http://pi.pauwel.be/voc/buildingelement> ;
  rdfs:label "Partitioning Wall"@en ;
  rdfs:label "skillevegg"@nb-no ;
  rdfs:seeAlso <http://bsdd.buildingsmart.org/#concept/details/3DBpG2jff4GAXiQp8trskt> ;
  rdfs:seeAlso ifc:IfcWallEnumType ;
  rdfs:subClassOf beo:Wall ;
.
beo:Wall-PLUMBINGWALL
  rdf:type owl:Class ;
  rdfs:isDefinedBy <http://pi.pauwel.be/voc/buildingelement> ;
  rdfs:label "Plumbing Wall"@en ;
  rdfs:label "rør i vegg"@nb-no ;
  rdfs:seeAlso <http://bsdd.buildingsmart.org/#concept/details/1YFt0DFB99uxbJnz4oFiew> ;
  rdfs:seeAlso ifc:IfcWallEnumType ;
  rdfs:subClassOf beo:Wall ;
.
beo:Wall-POLYGONAL
  rdf:type owl:Class ;
  rdfs:comment "a polygonal wall, extruded vertically, where the wall thickness varies along the wall path"@en ;
  rdfs:comment "a polygonal wall, extruded vertically, where the wall thickness varies along the wall path"@en-gb ;
  rdfs:isDefinedBy <http://pi.pauwel.be/voc/buildingelement> ;
  rdfs:label "Polygonal Wall"@en ;
  rdfs:label "mangekantet"@nb-no ;
  rdfs:seeAlso <http://bsdd.buildingsmart.org/#concept/details/0cJEMJHYj6Hh7Q1xNPsiIf> ;
  rdfs:seeAlso ifc:IfcWallEnumType ;
  rdfs:subClassOf beo:Wall ;
.
beo:Wall-SHEAR
  rdf:type owl:Class ;
  rdfs:isDefinedBy <http://pi.pauwel.be/voc/buildingelement> ;
  rdfs:label "Shear Wall"@en ;
  rdfs:label "skive"@nb-no ;
  rdfs:seeAlso <http://bsdd.buildingsmart.org/#concept/details/0MAk1miOTAJQpI0VGyMnjS> ;
  rdfs:seeAlso ifc:IfcWallEnumType ;
  rdfs:subClassOf beo:Wall ;
.
beo:Wall-SOLIDWALL
  rdf:type owl:Class ;
  rdfs:isDefinedBy <http://pi.pauwel.be/voc/buildingelement> ;
  rdfs:label "Solid Wall"@en ;
  rdfs:label "massiv vegg"@nb-no ;
  rdfs:seeAlso <http://bsdd.buildingsmart.org/#concept/details/2J1xt_ADz7heqvTyh5YGEM> ;
  rdfs:seeAlso ifc:IfcWallEnumType ;
  rdfs:subClassOf beo:Wall ;
.
beo:Wall-STANDARD
  rdf:type owl:Class ;
  rdfs:isDefinedBy <http://pi.pauwel.be/voc/buildingelement> ;
  rdfs:label "Standard Wall"@en ;
  rdfs:seeAlso <http://bsdd.buildingsmart.org/#concept/details/2HWHt8Yiz4m9UzhlqVFLeO> ;
  rdfs:seeAlso ifc:IfcWallEnumType ;
  rdfs:subClassOf beo:Wall ;
.
beo:WallElementedCase
  rdf:type owl:Class ;
  rdfs:comment "A wall with certain constraints for the provision of its components."@en ;
  rdfs:isDefinedBy <http://pi.pauwel.be/voc/buildingelement> ;
  rdfs:label "Elemented Wall Case"@en ;
  rdfs:label "Mur composite"@fr-fr ;
  rdfs:label "Wand elementiert"@de-de ;
  rdfs:seeAlso <http://bsdd.buildingsmart.org/#concept/details/2dG9W0qXKHuO00025QrE$V> ;
  rdfs:seeAlso ifc:IfcWallElementedCase ;
  rdfs:subClassOf beo:Wall ;
.
beo:Window
  rdf:type owl:Class ;
  rdfs:comment "Abertura destinada a iluminar e ventilar os ambientes internos, além de facilitar a visão do exterior."@pt-br ;
  rdfs:comment "Bauteil zum Schließen einer Öffnung in einer Wand oder Satteldach, das Licht durchlassen und Belüftung ermöglichen kann"@de-de ;
  rdfs:comment "building component for closing an opening in a wall or pitched roof that will admit light and may provide ventilation"@en ;
  rdfs:comment "building component for closing an opening in a wall or pitched roof that will admit light and may provide ventilation"@en-gb ;
  rdfs:comment "byggelement som används för att stänga en öppning i en vägg eller ett sadeltak som kan släppa in ljus och bidra med ventilation"@sv-se ;
  rdfs:comment "componente costruttivo atto a chiudere un'apertura in un muro o in un tetto a spiovente che ammetta la luce e possa fornire ventilazione"@it-it ;
  rdfs:comment "componente de construcción para cerrar una abertura en una pared o techo a dos aguas que deja pasar la luz y puede proporcionar ventilación"@es-es ;
  rdfs:comment "construction for closing a vertical or near-vertical opening in a wall or pitched roof which will admit light and may provide ventilation. Often a pane of glass framed and mounted to permit opening and closing"@en ;
  rdfs:comment "construction for closing a vertical or near-vertical opening in a wall or pitched roof which will admit light and may provide ventilation. Often a pane of glass framed and mounted to permit opening and closing"@en-gb ;
  rdfs:comment "ein konstruksjon som står i ei opning som i ein vegg eller tak og som normalt er dekt av glas, med det føremålet å sleppa inn lys og luft. | konstruksjon for *lukking av ein vertikal eller nesten vertikal opning i ein vegg eller eit skråtak som skal sleppa igjennom lys kan gje ventilasjon. Ofte ei glasrute *innrammet og montert for å gjera muleg opning og lukking"@nn-no ;
  rdfs:comment "element budynku służący do zamykania i otwierania, osadzony w ścianie lub w dachu dwuspadowym, przepuszczający światło i mogący zapewniać wentylację"@pl-pl ;
  rdfs:comment "en konstruksjon som står i en åpning som i en vegg eller tak og som normalt er dekket av glass, med det formål å slippe inn lys og luft."@nb-no ;
  rdfs:comment "konstruksjon for lukking av en vertikal eller nesten vertikal åpning i en vegg eller et skråtak som skal slippe igjennom lys kan gi ventilasjon. Ofte en glassrute innrammet og montert for å muliggjøre åpning og lukking"@nb-no ;
  rdfs:comment "konstruktion til lukning af en lodret eller næsten lodret åbning i en mur eller skråt tag, der lader lys trænge igennem og kan muliggøre ventilation. Ofte en rude i en karm og monteret, så den kan åbnes og lukkes"@dk-dk ;
  rdfs:comment "seinä- tai kattoaukon sulkeva, valoa läpipäästävä rakenneosa varustettuna mahdollisin ilmanvaihto-ominaisuuksin"@fi-fi ;
  rdfs:comment "une construction destinée à fermer une ouverture verticale ou quasi-verticale dans un mur ou un toit en pente qui laissera passer la lumière et pourra fournir une ventilation. souvent constituée d'un panneau vitré monté sur un châssis permettant son ouverture et sa fermeture."@fr-fr ;
  rdfs:comment "строителен компонент за затваряне на отвор в стена или скатен покрив, който служи за осветяване и евентуално за проветряване"@bg-bg ;
  rdfs:isDefinedBy <http://pi.pauwel.be/voc/buildingelement> ;
  rdfs:label "Fenster"@de-de ;
  rdfs:label "Raam"@nl ;
  rdfs:label "Raam"@nl-nl ;
  rdfs:label "Vindue"@da ;
  rdfs:label "Window"@en ;
  rdfs:label "fenêtre"@fr-fr ;
  rdfs:label "finestra"@it-it ;
  rdfs:label "fönster"@sv-se ;
  rdfs:label "ikkuna"@fi-fi ;
  rdfs:label "janela"@pt-br ;
  rdfs:label "okna"@pl-pl ;
  rdfs:label "ventana"@es-es ;
  rdfs:label "vindauge"@nn-no ;
  rdfs:label "vindu"@nb-no ;
  rdfs:label "vindue"@dk-dk ;
  rdfs:label "window"@en-gb ;
  rdfs:label "windowset"@en ;
  rdfs:label "прозорец"@bg-bg ;
  rdfs:label "نافذة"@ar-sa ;
  rdfs:label "窓"@ja-jp ;
  rdfs:seeAlso <http://bsdd.buildingsmart.org/#concept/details/3vHUaooT0Hsm00051Mm008> ;
  rdfs:seeAlso ifc:IfcWindow ;
  rdfs:subClassOf beo:BuildingElement ;
.
beo:Window-LIGHTDOME
  rdf:type owl:Class ;
  rdfs:comment "a special window that lies horizonally in a roof slab opening"@en ;
  rdfs:isDefinedBy <http://pi.pauwel.be/voc/buildingelement> ;
  rdfs:label "Light dome"@en ;
  rdfs:label "lyskuppel"@nb-no ;
  rdfs:seeAlso <http://bsdd.buildingsmart.org/#concept/details/3aXmro5wX3FeEqYU7Y7w5X> ;
  rdfs:seeAlso ifc:IfcWindowEnumType ;
  rdfs:subClassOf beo:Window ;
.
beo:Window-SKYLIGHT
  rdf:type owl:Class ;
  rdfs:comment "Overlys"@nb-no ;
  rdfs:comment "construction for closing an opening in a flat roof or low pitched roof, intended primarily for lighting and consisting of a frame and glazing"@en ;
  rdfs:isDefinedBy <http://pi.pauwel.be/voc/buildingelement> ;
  rdfs:label "Daklicht"@nl-nl ;
  rdfs:label "Skylight"@en ;
  rdfs:label "overlys"@nb-no ;
  rdfs:seeAlso <http://bsdd.buildingsmart.org/#concept/details/1irgDncIrAVQwjja3JEbnb> ;
  rdfs:seeAlso ifc:IfcWindowEnumType ;
  rdfs:subClassOf beo:Window ;
.
beo:Window-WINDOW
  rdf:type owl:Class ;
  rdfs:comment """A building element that is predominately used to provide natural light and fresh air. It includes vertical opening but also horizontal opening such as skylights or light domes. It includes constructions with swinging, pivoting, sliding, or revolving panels and fixed panels. A window consists of a lining and one or several panels.
NOTE  Definition according to ISO 6707-1
Construction for closing a vertical or near vertical opening in a wall or pitched roof that will admit light and may admit fresh air."""@en ;
  rdfs:comment "Abertura destinada a iluminar e ventilar os ambientes internos, além de facilitar a visão do exterior."@pt-br ;
  rdfs:comment "Bauteil zum Schließen einer Öffnung in einer Wand oder Satteldach, das Licht durchlassen und Belüftung ermöglichen kann"@de-de ;
  rdfs:comment "Een raam is een constructie met een scheidingsfunctie en een lichttoetredingsfunctie."@nl-nl ;
  rdfs:comment "building component for closing an opening in a wall or pitched roof that will admit light and may provide ventilation"@en ;
  rdfs:comment "building component for closing an opening in a wall or pitched roof that will admit light and may provide ventilation"@en-gb ;
  rdfs:comment "byggelement som används för att stänga en öppning i en vägg eller ett sadeltak som kan släppa in ljus och bidra med ventilation"@sv-se ;
  rdfs:comment "componente costruttivo atto a chiudere un'apertura in un muro o in un tetto a spiovente che ammetta la luce e possa fornire ventilazione"@it-it ;
  rdfs:comment "componente de construcción para cerrar una abertura en una pared o techo a dos aguas que deja pasar la luz y puede proporcionar ventilación"@es-es ;
  rdfs:comment "construction for closing a vertical or near-vertical opening in a wall or pitched roof which will admit light and may provide ventilation. Often a pane of glass framed and mounted to permit opening and closing"@en ;
  rdfs:comment "construction for closing a vertical or near-vertical opening in a wall or pitched roof which will admit light and may provide ventilation. Often a pane of glass framed and mounted to permit opening and closing"@en-gb ;
  rdfs:comment "ein konstruksjon som står i ei opning som i ein vegg eller tak og som normalt er dekt av glas, med det føremålet å sleppa inn lys og luft. | konstruksjon for *lukking av ein vertikal eller nesten vertikal opning i ein vegg eller eit skråtak som skal sleppa igjennom lys kan gje ventilasjon. Ofte ei glasrute *innrammet og montert for å gjera muleg opning og lukking"@nn-no ;
  rdfs:comment "element budynku służący do zamykania i otwierania, osadzony w ścianie lub w dachu dwuspadowym, przepuszczający światło i mogący zapewniać wentylację"@pl-pl ;
  rdfs:comment "en konstruksjon som står i en åpning som i en vegg eller tak og som normalt er dekket av glass, med det formål å slippe inn lys og luft."@nb-no ;
  rdfs:comment "konstruksjon for lukking av en vertikal eller nesten vertikal åpning i en vegg eller et skråtak som skal slippe igjennom lys kan gi ventilasjon. Ofte en glassrute innrammet og montert for å muliggjøre åpning og lukking"@nb-no ;
  rdfs:comment "konstruktion til lukning af en lodret eller næsten lodret åbning i en mur eller skråt tag, der lader lys trænge igennem og kan muliggøre ventilation. Ofte en rude i en karm og monteret, så den kan åbnes og lukkes"@dk-dk ;
  rdfs:comment "objekt för tillträde till utrymme för enbart ljus"@sv-se ;
  rdfs:comment "seinä- tai kattoaukon sulkeva, valoa läpipäästävä rakenneosa varustettuna mahdollisin ilmanvaihto-ominaisuuksin"@fi-fi ;
  rdfs:comment "space access object for light entry only"@en ;
  rdfs:comment "une construction destinée à fermer une ouverture verticale ou quasi-verticale dans un mur ou un toit en pente qui laissera passer la lumière et pourra fournir une ventilation. souvent constituée d'un panneau vitré monté sur un châssis permettant son ouverture et sa fermeture."@fr-fr ;
  rdfs:comment "строителен компонент за затваряне на отвор в стена или скатен покрив, който служи за осветяване и евентуално за проветряване"@bg-bg ;
  rdfs:isDefinedBy <http://pi.pauwel.be/voc/buildingelement> ;
  rdfs:label "Fenster"@de-de ;
  rdfs:label "Raam"@nl-nl ;
  rdfs:label "Window"@en ;
  rdfs:label "fenster"@de-ch ;
  rdfs:label "fenêtre"@fr-fr ;
  rdfs:label "finestra"@it-it ;
  rdfs:label "fönster"@sv-se ;
  rdfs:label "ikkuna"@fi-fi ;
  rdfs:label "janela"@pt-br ;
  rdfs:label "okna"@pl-pl ;
  rdfs:label "ventana"@es-es ;
  rdfs:label "vindauge"@nn-no ;
  rdfs:label "vindu"@nb-no ;
  rdfs:label "vindue"@dk-dk ;
  rdfs:label "window"@en-gb ;
  rdfs:label "прозорец"@bg-bg ;
  rdfs:label "نافذة"@ar-sa ;
  rdfs:label "窓"@ja-jp ;
  rdfs:seeAlso <http://bsdd.buildingsmart.org/#concept/details/3QkFVA4cD3YvP3Y3zVGFc3> ;
  rdfs:seeAlso ifc:IfcWindowEnumType ;
  rdfs:subClassOf beo:Window ;
.
<http://purl.org/dc/elements/1.1/Language>
  rdf:type owl:AnnotationProperty ;
.
<http://purl.org/dc/elements/1.1/description>
  rdf:type owl:AnnotationProperty ;
.
<http://purl.org/dc/elements/1.1/modified>
  rdf:type owl:AnnotationProperty ;
.
<http://purl.org/dc/elements/1.1/title>
  rdf:type owl:AnnotationProperty ;
.
dcterms:contributor
  rdf:type owl:AnnotationProperty ;
.
dcterms:creator
  rdf:type owl:AnnotationProperty ;
.
dcterms:description
  rdf:type owl:AnnotationProperty ;
.
dcterms:issued
  rdf:type owl:AnnotationProperty ;
.
dcterms:license
  rdf:type owl:AnnotationProperty ;
.
dcterms:modified
  rdf:type owl:AnnotationProperty ;
.
dcterms:title
  rdf:type owl:AnnotationProperty ;
.
vann:preferredNamespacePrefix
  rdf:type owl:AnnotationProperty ;
.
vann:preferredNamespaceUri
  rdf:type owl:AnnotationProperty ;
.
voaf:Vocabulary
  rdf:type owl:Class ;
.
vs:term_status
  rdf:type owl:AnnotationProperty ;
.
foaf:Person
  rdf:type owl:Class ;
.
foaf:name
  rdf:type owl:DatatypeProperty ;
.
contax:ConstructionComponent
  rdf:type owl:Class ;
.
